@prefix :      <https://www.linkedbuildingdata.net/IFC4-PSD/Pset_ProtectiveDeviceTrippingUnitTimeAdjustment#> .
@prefix IFC4-PSD: <https://www.linkedbuildingdata.net/IFC4-PSD#> .
@prefix rdf:   <http://www.w3.org/1999/02/22-rdf-syntax-ns#> .
@prefix owl:   <http://www.w3.org/2002/07/owl#> .
@prefix rdfs:  <http://www.w3.org/2000/01/rdf-schema#> .
@prefix IFC4:  <http://lbd.arch.rwth-aachen.de/ifcOWL/IFC4#> .

:pf083ee00d1fb11e1800000215ad4efdf
        a                         IFC4-PSD:PropertyDef ;
        rdfs:comment              "The tripping current in [x In] at which the time delay is specified. A value for this property should only be asserted for time delay of L-function, and for I2t of the S and G function." ;
        rdfs:label                "CurrentForTimeDelay" ;
        IFC4-PSD:definition       "The tripping current in [x In] at which the time delay is specified. A value for this property should only be asserted for time delay of L-function, and for I2t of the S and G function." ;
        IFC4-PSD:definitionAlias  "시간 연장 [x]의 트립 전류는 L 함수의 지연 시간 및 S와 G 함수 I2t를 지정합니다."@ko-KR , ""@en , "時延[x]ののトリップ電流は、L関数の遅延時間、およびSとG関数のI2tを指定。"@ja-JP ;
        IFC4-PSD:ifdguid          "f083ee00d1fb11e1800000215ad4efdf" ;
        IFC4-PSD:name             "CurrentForTimeDelay" ;
        IFC4-PSD:nameAlias        "Current For Time Delay"@en , "시간연장 전류"@ko-KR , "時延電流"@ja-JP ;
        IFC4-PSD:propertyType     [ a                  IFC4-PSD:TypePropertySingleValue ;
                                    IFC4-PSD:dataType  IFC4:IfcTimeMeasure
                                  ] .

:Pset_ProtectiveDeviceTrippingUnitTimeAdjustment
        a                             IFC4-PSD:PropertySetDef ;
        rdfs:comment                  "A set of time adjustment values that may be applied to an electronic or thermal tripping unit type." ;
        rdfs:label                    "Pset_ProtectiveDeviceTrippingUnitTimeAdjustment" ;
        IFC4-PSD:applicableClass      IFC4:IfcProtectiveDeviceTrippingUnit ;
        IFC4-PSD:applicableTypeValue  "IfcProtectiveDeviceTrippingUnit" ;
        IFC4-PSD:definition           "A set of time adjustment values that may be applied to an electronic or thermal tripping unit type." ;
        IFC4-PSD:definitionAlias      "電磁式または熱動式トリップユニット型に適用することができる時間調整（時延）のセット。"@ja-JP , ""@en ;
        IFC4-PSD:ifcVersion           [ a                 IFC4-PSD:IfcVersion ;
                                        IFC4-PSD:version  "IFC4"
                                      ] ;
        IFC4-PSD:name                 "Pset_ProtectiveDeviceTrippingUnitTimeAdjustment" ;
        IFC4-PSD:propertyDef          :pd813d380d1fb11e1800000215ad4efdf , :pf548a200d1fb11e1800000215ad4efdf , :pe9f57680d1fb11e1800000215ad4efdf , :pe530c280d1fb11e1800000215ad4efdf , :pcfbb9880d1fb11e1800000215ad4efdf , :pdfd37800d1fb11e1800000215ad4efdf , :pf083ee00d1fb11e1800000215ad4efdf .

:AdjustmentValues  a        rdf:Property ;
        rdfs:seeAlso        :pe530c280d1fb11e1800000215ad4efdf ;
        rdfs:subPropertyOf  IFC4-PSD:AdjustmentValues .

:pf548a200d1fb11e1800000215ad4efdf
        a                         IFC4-PSD:PropertyDef ;
        rdfs:comment              "The applicability of the time adjustment related to the tripping function." ;
        rdfs:label                "I2TApplicability" ;
        IFC4-PSD:definition       "The applicability of the time adjustment related to the tripping function." ;
        IFC4-PSD:definitionAlias  ""@en , "트립 기능 시간 연장을 요구할 때 적용하는 함수입니다."@ko-KR , "トリップ機能の時延を求める時に適用する関数。"@ja-JP ;
        IFC4-PSD:ifdguid          "f548a200d1fb11e1800000215ad4efdf" ;
        IFC4-PSD:name             "I2TApplicability" ;
        IFC4-PSD:nameAlias        "I2Tの適用"@ja-JP , "I2 TApplicability"@en , "12 T적용"@ko-KR ;
        IFC4-PSD:propertyType     [ a                  IFC4-PSD:TypePropertyEnumeratedValue ;
                                    IFC4-PSD:enumItem  "RANGE" , "LIST"
                                  ] .

:pcfbb9880d1fb11e1800000215ad4efdf
        a                         IFC4-PSD:PropertyDef ;
        rdfs:comment              "The type of adjustment value that is applied through the property set. This determines the properties that should be asserted (see below)." ;
        rdfs:label                "AdjustmentValueType" ;
        IFC4-PSD:definition       "The type of adjustment value that is applied through the property set. This determines the properties that should be asserted (see below)." ;
        IFC4-PSD:definitionAlias  "조정 값 유형을 설정합니다."@ko-KR , "調整値のタイプを設定。"@ja-JP , ""@en ;
        IFC4-PSD:ifdguid          "cfbb9880d1fb11e1800000215ad4efdf" ;
        IFC4-PSD:name             "AdjustmentValueType" ;
        IFC4-PSD:nameAlias        "조정 형식"@ko-KR , "調整値の型"@ja-JP , "Adjustment Value Type"@en ;
        IFC4-PSD:propertyType     [ a                  IFC4-PSD:TypePropertyEnumeratedValue ;
                                    IFC4-PSD:enumItem  "RANGE" , "LIST"
                                  ] .

:CurrentForTimeDelay  a     rdf:Property ;
        rdfs:seeAlso        :pf083ee00d1fb11e1800000215ad4efdf ;
        rdfs:subPropertyOf  IFC4-PSD:CurrentForTimeDelay .

:AdjustmentRangeStepValue
        a                   rdf:Property ;
        rdfs:seeAlso        :pdfd37800d1fb11e1800000215ad4efdf ;
        rdfs:subPropertyOf  IFC4-PSD:AdjustmentRangeStepValue .

:AdjustmentDesignation
        a                   rdf:Property ;
        rdfs:seeAlso        :pe9f57680d1fb11e1800000215ad4efdf ;
        rdfs:subPropertyOf  IFC4-PSD:AdjustmentDesignation .

:pe530c280d1fb11e1800000215ad4efdf
        a                         IFC4-PSD:PropertyDef ;
        rdfs:comment              "A list of time adjustment values that may be applied to a tripping unit for an AdjustmentValueType = LIST. A minimum of 1 and a maximum of 16 adjustment values may be specified. Note that this property should not have a value for an  AdjustmentValueType = RANGE." ;
        rdfs:label                "AdjustmentValues" ;
        IFC4-PSD:definition       "A list of time adjustment values that may be applied to a tripping unit for an AdjustmentValueType = LIST. A minimum of 1 and a maximum of 16 adjustment values may be specified. Note that this property should not have a value for an  AdjustmentValueType = RANGE." ;
        IFC4-PSD:definitionAlias  "시간 조정 값을 1에서 16로 설정. 범위는없는 것을주의."@ko-KR , ""@en , "時間調整値を１から16で設定。範囲では、ない事を注意。"@ja-JP ;
        IFC4-PSD:ifdguid          "e530c280d1fb11e1800000215ad4efdf" ;
        IFC4-PSD:name             "AdjustmentValues" ;
        IFC4-PSD:nameAlias        "Adjustment Values"@en , "조정 값"@ko-KR , "調整値"@ja-JP ;
        IFC4-PSD:propertyType     [ a                  IFC4-PSD:TypePropertyListValue ;
                                    IFC4-PSD:dataType  IFC4:IfcTimeMeasure
                                  ] .

<https://www.linkedbuildingdata.net/IFC4-PSD/Pset_ProtectiveDeviceTrippingUnitTimeAdjustment>
        a                owl:Ontology ;
        owl:imports      <http://lbd.arch.rwth-aachen.de/ifcOWL/IFC4-PSD> ;
        owl:versionInfo  "Created with BIM-Bots PSD Repository" .

:AdjustmentValueType  a     rdf:Property ;
        rdfs:seeAlso        :pcfbb9880d1fb11e1800000215ad4efdf ;
        rdfs:subPropertyOf  IFC4-PSD:AdjustmentValueType .

:pdfd37800d1fb11e1800000215ad4efdf
        a                         IFC4-PSD:PropertyDef ;
        rdfs:comment              "Step value of time adjustment for an AdjustmentValueType = RANGE. Note that this property should not have a value for an  AdjustmentValueType = LIST." ;
        rdfs:label                "AdjustmentRangeStepValue" ;
        IFC4-PSD:definition       "Step value of time adjustment for an AdjustmentValueType = RANGE. Note that this property should not have a value for an  AdjustmentValueType = LIST." ;
        IFC4-PSD:definitionAlias  "時間調整の範囲をステップ値を設定。一覧表ではもっていない事を注意。"@ja-JP , "시간 조정 범위를 단계 값을 설정합니다. 목록은 갖고 있지 않은 것을주의."@ko-KR , ""@en ;
        IFC4-PSD:ifdguid          "dfd37800d1fb11e1800000215ad4efdf" ;
        IFC4-PSD:name             "AdjustmentRangeStepValue" ;
        IFC4-PSD:nameAlias        "조정범위 단계값"@ko-KR , "Adjustment Range Step Value"@en , "調整範囲のステップ値"@ja-JP ;
        IFC4-PSD:propertyType     [ a                  IFC4-PSD:TypePropertySingleValue ;
                                    IFC4-PSD:dataType  IFC4:IfcTimeMeasure
                                  ] .

:I2TApplicability  a        rdf:Property ;
        rdfs:seeAlso        :pf548a200d1fb11e1800000215ad4efdf ;
        rdfs:subPropertyOf  IFC4-PSD:I2TApplicability .

:AdjustmentRange  a         rdf:Property ;
        rdfs:seeAlso        :pd813d380d1fb11e1800000215ad4efdf ;
        rdfs:subPropertyOf  IFC4-PSD:AdjustmentRange .

:pd813d380d1fb11e1800000215ad4efdf
        a                         IFC4-PSD:PropertyDef ;
        rdfs:comment              "Upper and lower time adjustment limits for an AdjustmentValueType = RANGE. Note that this property should not have a value for an  AdjustmentValueType = LIST." ;
        rdfs:label                "AdjustmentRange" ;
        IFC4-PSD:definition       "Upper and lower time adjustment limits for an AdjustmentValueType = RANGE. Note that this property should not have a value for an  AdjustmentValueType = LIST." ;
        IFC4-PSD:definitionAlias  ""@en , "시간 조정 범위의 상한 치와 하한 치를 설정합니다. 목록은 갖고 있지 않은 것을주의."@ko-KR , "時間調整の範囲の上限値と下限値を設定。一覧表ではもっていない事を注意。"@ja-JP ;
        IFC4-PSD:ifdguid          "d813d380d1fb11e1800000215ad4efdf" ;
        IFC4-PSD:name             "AdjustmentRange" ;
        IFC4-PSD:nameAlias        "Adjustment Range"@en , "조정 범위"@ko-KR , "調整範囲"@ja-JP ;
        IFC4-PSD:propertyType     [ a                  IFC4-PSD:TypePropertyBoundedValue ;
                                    IFC4-PSD:dataType  IFC4:IfcTimeMeasure
                                  ] .

:pe9f57680d1fb11e1800000215ad4efdf
        a                         IFC4-PSD:PropertyDef ;
        rdfs:comment              "The desgnation on the device for the adjustment." ;
        rdfs:label                "AdjustmentDesignation" ;
        IFC4-PSD:definition       "The desgnation on the device for the adjustment." ;
        IFC4-PSD:definitionAlias  ""@en , "조정하는 장치를 지정합니다."@ko-KR , "調整する装置の指定。"@ja-JP ;
        IFC4-PSD:ifdguid          "e9f57680d1fb11e1800000215ad4efdf" ;
        IFC4-PSD:name             "AdjustmentDesignation" ;
        IFC4-PSD:nameAlias        "Adjustment Designation"@en , "調整の指定"@ja-JP , "조정지정"@ko-KR ;
        IFC4-PSD:propertyType     [ a                  IFC4-PSD:TypePropertySingleValue ;
                                    IFC4-PSD:dataType  IFC4:IfcLabel
                                  ] .
