@prefix :      <https://www.linkedbuildingdata.net/IFC4-PSD/Pset_ConcreteElementGeneral#> .
@prefix IFC4-PSD: <https://www.linkedbuildingdata.net/IFC4-PSD#> .
@prefix owl:   <http://www.w3.org/2002/07/owl#> .
@prefix rdf:   <http://www.w3.org/1999/02/22-rdf-syntax-ns#> .
@prefix rdfs:  <http://www.w3.org/2000/01/rdf-schema#> .
@prefix IFC4:  <http://lbd.arch.rwth-aachen.de/ifcOWL/IFC4#> .

:pb88ca2252c4b4014bcf289bbbd596398
        a                         IFC4-PSD:PropertyDef ;
        rdfs:comment              "Classification of the reinforcement strength in accordance with the concrete design code which is applied in the project. The reinforcing strength class often combines strength and ductility." ;
        rdfs:label                "ReinforcementStrengthClass" ;
        IFC4-PSD:definition       "Classification of the reinforcement strength in accordance with the concrete design code which is applied in the project. The reinforcing strength class often combines strength and ductility." ;
        IFC4-PSD:definitionAlias  ""@en ;
        IFC4-PSD:ifdguid          "b88ca2252c4b4014bcf289bbbd596398" ;
        IFC4-PSD:name             "ReinforcementStrengthClass" ;
        IFC4-PSD:nameAlias        "Reinforcement Strength Class"@en ;
        IFC4-PSD:propertyType     [ a                  IFC4-PSD:TypePropertySingleValue ;
                                    IFC4-PSD:dataType  IFC4:IfcLabel
                                  ] .

:DimensionalAccuracyClass
        a                   rdf:Property ;
        rdfs:seeAlso        :pa4b95080d1cb11e1800000215ad4efdf ;
        rdfs:subPropertyOf  IFC4-PSD:DimensionalAccuracyClass .

:ConcreteCoverAtMainBars
        a                   rdf:Property ;
        rdfs:seeAlso        :pb8fd4d80d1cb11e1800000215ad4efdf ;
        rdfs:subPropertyOf  IFC4-PSD:ConcreteCoverAtMainBars .

<https://www.linkedbuildingdata.net/IFC4-PSD/Pset_ConcreteElementGeneral>
        a                owl:Ontology ;
        owl:imports      <http://lbd.arch.rwth-aachen.de/ifcOWL/IFC4-PSD> ;
        owl:versionInfo  "Created with BIM-Bots PSD Repository" .

:p0764b8e36a7c4275859f1534ea3eec09
        a                         IFC4-PSD:PropertyDef ;
        rdfs:comment              "The protective concrete cover at the reinforcing bars according to local building regulations." ;
        rdfs:label                "ConcreteCover" ;
        IFC4-PSD:definition       "The protective concrete cover at the reinforcing bars according to local building regulations." ;
        IFC4-PSD:definitionAlias  "Abstand zwischen der Betonoberfläche und der Außenkante einer vom Beton umhüllten Bewehrung."@de-DE , ""@en ;
        IFC4-PSD:ifdguid          "0764b8e36a7c4275859f1534ea3eec09" ;
        IFC4-PSD:name             "ConcreteCover" ;
        IFC4-PSD:nameAlias        "Concrete Cover"@en , "Betonüberdeckung"@de-DE ;
        IFC4-PSD:propertyType     [ a                  IFC4-PSD:TypePropertySingleValue ;
                                    IFC4-PSD:dataType  IFC4:IfcPositiveLengthMeasure
                                  ] .

:p96390dc443fd41d88cb6aca86dce4993
        a                         IFC4-PSD:PropertyDef ;
        rdfs:comment              "Classification of the concrete strength in accordance with the concrete design code which is applied in the project." ;
        rdfs:label                "StrengthClass" ;
        IFC4-PSD:definition       "Classification of the concrete strength in accordance with the concrete design code which is applied in the project." ;
        IFC4-PSD:definitionAlias  ""@en , "Klassifikation der Betonfestigkeit gemäß der aktuellen, im Projekt angewandten, Norm."@de-DE ;
        IFC4-PSD:ifdguid          "96390dc443fd41d88cb6aca86dce4993" ;
        IFC4-PSD:name             "StrengthClass" ;
        IFC4-PSD:nameAlias        "Strength Class"@en , "Betonfestigkeitsklasse"@de-DE ;
        IFC4-PSD:propertyType     [ a                  IFC4-PSD:TypePropertySingleValue ;
                                    IFC4-PSD:dataType  IFC4:IfcLabel
                                  ] .

:ReinforcementVolumeRatio
        a                   rdf:Property ;
        rdfs:seeAlso        :pa1c0e785c9bc41878ddbc67fd0ff3d26 ;
        rdfs:subPropertyOf  IFC4-PSD:ReinforcementVolumeRatio .

:p9bee0bf72ad34a66bef57b71b7ca175b
        a                         IFC4-PSD:PropertyDef ;
        rdfs:comment              "Classification of exposure to environmental conditions, usually specified in accordance with the concrete design code which is applied in the project." ;
        rdfs:label                "ExposureClass" ;
        IFC4-PSD:definition       "Classification of exposure to environmental conditions, usually specified in accordance with the concrete design code which is applied in the project." ;
        IFC4-PSD:definitionAlias  ""@en , "Klassifikation der Widerstandsfähigkeit gegenüber chemischen und physikalischen Einwirkungen gemäß der aktuellen, im Projekt angewandten, Norm."@de-DE ;
        IFC4-PSD:ifdguid          "9bee0bf72ad34a66bef57b71b7ca175b" ;
        IFC4-PSD:name             "ExposureClass" ;
        IFC4-PSD:nameAlias        "Exposure Class"@en , "Expositionsklasse"@de-DE ;
        IFC4-PSD:propertyType     [ a                  IFC4-PSD:TypePropertySingleValue ;
                                    IFC4-PSD:dataType  IFC4:IfcLabel
                                  ] .

:Pset_ConcreteElementGeneral
        a                             IFC4-PSD:PropertySetDef ;
        rdfs:comment                  "General properties common to different types of concrete elements, including reinforced concrete elements. The property set can be used by a number of subtypes of IfcBuildingElement, indicated that such element is designed or constructed using a concrete construction method." ;
        rdfs:label                    "Pset_ConcreteElementGeneral" ;
        IFC4-PSD:applicableClass      IFC4:IfcMember , IFC4:IfcWall , IFC4:IfcChimney , IFC4:IfcRampFlight , IFC4:IfcRailing , IFC4:IfcCivilElement , IFC4:IfcPlate , IFC4:IfcRamp , IFC4:IfcRoof , IFC4:IfcColumn , IFC4:IfcStair , IFC4:IfcStairFlight , IFC4:IfcSlab , IFC4:IfcBuildingElementProxy , IFC4:IfcPile , IFC4:IfcBeam , IFC4:IfcFooting ;
        IFC4-PSD:applicableTypeValue  "IfcBeam,IfcBuildingElementProxy,IfcChimney,IfcColumn,IfcFooting,IfcMember,IfcPile,IfcPlate,IfcRailing,IfcRamp,IfcRampFlight,IfcRoof,IfcSlab,IfcStair,IfcStairFlight,IfcWall,IfcCivilElement" ;
        IFC4-PSD:definition           "General properties common to different types of concrete elements, including reinforced concrete elements. The property set can be used by a number of subtypes of IfcBuildingElement, indicated that such element is designed or constructed using a concrete construction method." ;
        IFC4-PSD:definitionAlias      "コンクリート要素の異なるタイプに対する共通の一般的な属性。 Pset は IfcBuildingElement の多くのサブタイプによって使うことができる。"@ja-JP , ""@en , "Generelle Eigenschaften die allen Betonbauteilen, einschließlich Stahlbetonbauteilen, gemeinsam sind. Dieser Eigenschaftssatz kann den verschiedenen Bauelementklassen (Subtypen von IfcBuildingElement) zugeordnet werden."@de ;
        IFC4-PSD:ifcVersion           [ a                 IFC4-PSD:IfcVersion ;
                                        IFC4-PSD:version  "IFC4"
                                      ] ;
        IFC4-PSD:name                 "Pset_ConcreteElementGeneral" ;
        IFC4-PSD:propertyDef          :pb88ca2252c4b4014bcf289bbbd596398 , :pb8fd4d80d1cb11e1800000215ad4efdf , :p0764b8e36a7c4275859f1534ea3eec09 , :pabe05e80d1cb11e1800000215ad4efdf , :pbef32e80d1cb11e1800000215ad4efdf , :p9bee0bf72ad34a66bef57b71b7ca175b , :pa4b95080d1cb11e1800000215ad4efdf , :p84899180d1cb11e1800000215ad4efdf , :p64af56b30b4540c2b43d74b49a28b9db , :p036938642cbf49e2a90d346134ac7475 , :p96390dc443fd41d88cb6aca86dce4993 , :pa1c0e785c9bc41878ddbc67fd0ff3d26 .

:pa4b95080d1cb11e1800000215ad4efdf
        a                         IFC4-PSD:PropertyDef ;
        rdfs:comment              "Classification designation of the dimensional accuracy requirement according to local standards." ;
        rdfs:label                "DimensionalAccuracyClass" ;
        IFC4-PSD:definition       "Classification designation of the dimensional accuracy requirement according to local standards." ;
        IFC4-PSD:definitionAlias  "국가 표준이 요구하는 치수 정밀도의 분류 지정"@ko-KR , "国の基準が求める寸法精度の分類指定。"@ja-JP , ""@en ;
        IFC4-PSD:ifdguid          "a4b95080d1cb11e1800000215ad4efdf" ;
        IFC4-PSD:name             "DimensionalAccuracyClass" ;
        IFC4-PSD:nameAlias        "Dimensional Accuracy Class"@en , "寸法精度クラス"@ja-JP , "치수 정밀도 클래스"@ko-KR ;
        IFC4-PSD:propertyType     [ a                  IFC4-PSD:TypePropertySingleValue ;
                                    IFC4-PSD:dataType  IFC4:IfcLabel
                                  ] .

:ReinforcementAreaRatio
        a                   rdf:Property ;
        rdfs:seeAlso        :p036938642cbf49e2a90d346134ac7475 ;
        rdfs:subPropertyOf  IFC4-PSD:ReinforcementAreaRatio .

:pabe05e80d1cb11e1800000215ad4efdf
        a                         IFC4-PSD:PropertyDef ;
        rdfs:comment              "Classification designation of the on-site construction tolerances according to local standards." ;
        rdfs:label                "ConstructionToleranceClass" ;
        IFC4-PSD:definition       "Classification designation of the on-site construction tolerances according to local standards." ;
        IFC4-PSD:definitionAlias  "国の基準が求める現場での製造許容の分類指定。"@ja-JP , "국가 표준이 요구하는 현장에서 제조 허용 범주 지정"@ko-KR , ""@en ;
        IFC4-PSD:ifdguid          "abe05e80d1cb11e1800000215ad4efdf" ;
        IFC4-PSD:name             "ConstructionToleranceClass" ;
        IFC4-PSD:nameAlias        "製造許容クラス"@ja-JP , "제조 허용 클래스"@ko-KR , "Construction Tolerance Class"@en ;
        IFC4-PSD:propertyType     [ a                  IFC4-PSD:TypePropertySingleValue ;
                                    IFC4-PSD:dataType  IFC4:IfcLabel
                                  ] .

:p036938642cbf49e2a90d346134ac7475
        a                         IFC4-PSD:PropertyDef ;
        rdfs:comment              "The required ratio of the effective area of the reinforcement to the effective area of the concrete At any section of a reinforced concrete structural element." ;
        rdfs:label                "ReinforcementAreaRatio" ;
        IFC4-PSD:definition       "The required ratio of the effective area of the reinforcement to the effective area of the concrete At any section of a reinforced concrete structural element." ;
        IFC4-PSD:definitionAlias  ""@en , "Das geforderte Verhältnis der effektiven flächenbezogenen Masse der Bewehrung im Verhältnis zur effektiven Fläche des Betons für dieses Element."@de-DE ;
        IFC4-PSD:ifdguid          "036938642cbf49e2a90d346134ac7475" ;
        IFC4-PSD:name             "ReinforcementAreaRatio" ;
        IFC4-PSD:nameAlias        "Reinforcement Area Ratio"@en , "Bewehrungsgrad Fläche"@de-DE ;
        IFC4-PSD:propertyType     [ a                  IFC4-PSD:TypePropertySingleValue ;
                                    IFC4-PSD:dataType  IFC4:IfcAreaDensityMeasure
                                  ] .

:p64af56b30b4540c2b43d74b49a28b9db
        a                         IFC4-PSD:PropertyDef ;
        rdfs:comment              "Designator for whether the concrete element is constructed on site or prefabricated. Allowed values are: 'In-Situ' vs 'Precast'." ;
        rdfs:label                "ConstructionMethod" ;
        IFC4-PSD:definition       "Designator for whether the concrete element is constructed on site or prefabricated. Allowed values are: 'In-Situ' vs 'Precast'." ;
        IFC4-PSD:definitionAlias  "Angabe, ob dieses Betonbauteil als Ortbeton (\"In-Situ\") oder als Fertigteil (\"Precast\") ausgeführt werden soll."@de-DE , ""@en ;
        IFC4-PSD:ifdguid          "64af56b30b4540c2b43d74b49a28b9db" ;
        IFC4-PSD:name             "ConstructionMethod" ;
        IFC4-PSD:nameAlias        "Construction Method"@en , "Ausführung"@de-DE ;
        IFC4-PSD:propertyType     [ a                  IFC4-PSD:TypePropertySingleValue ;
                                    IFC4-PSD:dataType  IFC4:IfcLabel
                                  ] .

:ConcreteCoverAtLinks
        a                   rdf:Property ;
        rdfs:seeAlso        :pbef32e80d1cb11e1800000215ad4efdf ;
        rdfs:subPropertyOf  IFC4-PSD:ConcreteCoverAtLinks .

:pb8fd4d80d1cb11e1800000215ad4efdf
        a                         IFC4-PSD:PropertyDef ;
        rdfs:comment              "The protective concrete cover at the main reinforcing bars according to local building regulations." ;
        rdfs:label                "ConcreteCoverAtMainBars" ;
        IFC4-PSD:definition       "The protective concrete cover at the main reinforcing bars according to local building regulations." ;
        IFC4-PSD:definitionAlias  "国の建築基準に従い、主鉄筋をコンクリートの被りで保護する。"@ja-JP , ""@en , "Abstand zwischen der Betonoberfläche und der Außenkante den vom Beton umhüllten Bewehrungshauptstäben."@de-DE , "국가의 건축 기준에 따라 주로 철근을 콘크리트 입고로 보호"@ko-KR ;
        IFC4-PSD:ifdguid          "b8fd4d80d1cb11e1800000215ad4efdf" ;
        IFC4-PSD:name             "ConcreteCoverAtMainBars" ;
        IFC4-PSD:nameAlias        "주근 콘크리트 입고"@ko-KR , "Concrete Cover At Main Bars"@en , "Betonüberdeckung Hauptstäbe"@de-DE , "主筋のコンクリート被り"@ja-JP ;
        IFC4-PSD:propertyType     [ a                  IFC4-PSD:TypePropertySingleValue ;
                                    IFC4-PSD:dataType  IFC4:IfcPositiveLengthMeasure
                                  ] .

:ExposureClass  a           rdf:Property ;
        rdfs:seeAlso        :p9bee0bf72ad34a66bef57b71b7ca175b ;
        rdfs:subPropertyOf  IFC4-PSD:ExposureClass .

:ReinforcementStrengthClass
        a                   rdf:Property ;
        rdfs:seeAlso        :pb88ca2252c4b4014bcf289bbbd596398 ;
        rdfs:subPropertyOf  IFC4-PSD:ReinforcementStrengthClass .

:StrengthClass  a           rdf:Property ;
        rdfs:seeAlso        :p96390dc443fd41d88cb6aca86dce4993 ;
        rdfs:subPropertyOf  IFC4-PSD:StrengthClass .

:ConcreteCover  a           rdf:Property ;
        rdfs:seeAlso        :p0764b8e36a7c4275859f1534ea3eec09 ;
        rdfs:subPropertyOf  IFC4-PSD:ConcreteCover .

:pa1c0e785c9bc41878ddbc67fd0ff3d26
        a                         IFC4-PSD:PropertyDef ;
        rdfs:comment              "The required ratio of the effective mass of the reinforcement to the effective volume of the concrete of a reinforced concrete structural element." ;
        rdfs:label                "ReinforcementVolumeRatio" ;
        IFC4-PSD:definition       "The required ratio of the effective mass of the reinforcement to the effective volume of the concrete of a reinforced concrete structural element." ;
        IFC4-PSD:definitionAlias  ""@en , "Das geforderte Verhältnis der effektiven Masse der Bewehrung im Verhältnis zur effektiven Masse des Betons für dieses Element."@de-DE ;
        IFC4-PSD:ifdguid          "a1c0e785c9bc41878ddbc67fd0ff3d26" ;
        IFC4-PSD:name             "ReinforcementVolumeRatio" ;
        IFC4-PSD:nameAlias        "Bewehrungsgrad Volumen"@de-DE , "Reinforcement Volume Ratio"@en ;
        IFC4-PSD:propertyType     [ a                  IFC4-PSD:TypePropertySingleValue ;
                                    IFC4-PSD:dataType  IFC4:IfcMassDensityMeasure
                                  ] .

:pbef32e80d1cb11e1800000215ad4efdf
        a                         IFC4-PSD:PropertyDef ;
        rdfs:comment              "The protective concrete cover at the reinforcement links according to local building regulations." ;
        rdfs:label                "ConcreteCoverAtLinks" ;
        IFC4-PSD:definition       "The protective concrete cover at the reinforcement links according to local building regulations." ;
        IFC4-PSD:definitionAlias  ""@en , "Abstand zwischen der Betonoberfläche und der Außenkante der vom Beton umhüllten Bewehrungsverbindungsstäben."@de-DE , "国の建築基準に従い、補強筋をコンクリートの被りで保護する。"@ja-JP , "국가의 건축 기준에 따라 보강근 콘크리트의 입고로 보호"@ko-KR ;
        IFC4-PSD:ifdguid          "bef32e80d1cb11e1800000215ad4efdf" ;
        IFC4-PSD:name             "ConcreteCoverAtLinks" ;
        IFC4-PSD:nameAlias        "補強筋のコンクリート被り"@ja-JP , "Concrete Cover At Links"@en , "Betonüberdeckung Verbindungsstäbe"@de-DE , "보강근 콘크리트 입고"@ko-KR ;
        IFC4-PSD:propertyType     [ a                  IFC4-PSD:TypePropertySingleValue ;
                                    IFC4-PSD:dataType  IFC4:IfcPositiveLengthMeasure
                                  ] .

:StructuralClass  a         rdf:Property ;
        rdfs:seeAlso        :p84899180d1cb11e1800000215ad4efdf ;
        rdfs:subPropertyOf  IFC4-PSD:StructuralClass .

:p84899180d1cb11e1800000215ad4efdf
        a                         IFC4-PSD:PropertyDef ;
        rdfs:comment              "The structural class defined for the concrete structure (e.g. '1')." ;
        rdfs:label                "StructuralClass" ;
        IFC4-PSD:definition       "The structural class defined for the concrete structure (e.g. '1')." ;
        IFC4-PSD:definitionAlias  "구조 클래스는 콘크리트 구조를 정의했다 (예를 들어 \"1\")"@ko-KR , "構造クラスはコンクリート構造を定義した。（例えば「１」）"@ja-JP , ""@en ;
        IFC4-PSD:ifdguid          "84899180d1cb11e1800000215ad4efdf" ;
        IFC4-PSD:name             "StructuralClass" ;
        IFC4-PSD:nameAlias        "構造クラス"@ja-JP , "Structural Class"@en , "구조 클래스"@ko-KR ;
        IFC4-PSD:propertyType     [ a                  IFC4-PSD:TypePropertySingleValue ;
                                    IFC4-PSD:dataType  IFC4:IfcLabel
                                  ] .

:ConstructionToleranceClass
        a                   rdf:Property ;
        rdfs:seeAlso        :pabe05e80d1cb11e1800000215ad4efdf ;
        rdfs:subPropertyOf  IFC4-PSD:ConstructionToleranceClass .

:ConstructionMethod  a      rdf:Property ;
        rdfs:seeAlso        :p64af56b30b4540c2b43d74b49a28b9db ;
        rdfs:subPropertyOf  IFC4-PSD:ConstructionMethod .
