@prefix :      <https://www.linkedbuildingdata.net/IFC4-PSD/Pset_SensorPHistory#> .
@prefix IFC4-PSD: <https://www.linkedbuildingdata.net/IFC4-PSD#> .
@prefix rdf:   <http://www.w3.org/1999/02/22-rdf-syntax-ns#> .
@prefix owl:   <http://www.w3.org/2002/07/owl#> .
@prefix rdfs:  <http://www.w3.org/2000/01/rdf-schema#> .
@prefix IFC4:  <http://lbd.arch.rwth-aachen.de/ifcOWL/IFC4#> .

:Value  a                   rdf:Property ;
        rdfs:seeAlso        :pd569ac00d20411e1800000215ad4efdf ;
        rdfs:subPropertyOf  IFC4-PSD:Value .

<https://www.linkedbuildingdata.net/IFC4-PSD/Pset_SensorPHistory>
        a                owl:Ontology ;
        owl:imports      <http://lbd.arch.rwth-aachen.de/ifcOWL/IFC4-PSD> ;
        owl:versionInfo  "Created with BIM-Bots PSD Repository" .

:Pset_SensorPHistory  a               IFC4-PSD:PropertySetDef ;
        rdfs:comment                  "Properties for history of controller values.  HISTORY: Added in IFC4." ;
        rdfs:label                    "Pset_SensorPHistory" ;
        IFC4-PSD:applicableClass      IFC4:IfcSensor ;
        IFC4-PSD:applicableTypeValue  "IfcSensor" ;
        IFC4-PSD:definition           "Properties for history of controller values.  HISTORY: Added in IFC4." ;
        IFC4-PSD:definitionAlias      ""@en ;
        IFC4-PSD:ifcVersion           [ a                 IFC4-PSD:IfcVersion ;
                                        IFC4-PSD:version  "IFC4"
                                      ] ;
        IFC4-PSD:name                 "Pset_SensorPHistory" ;
        IFC4-PSD:propertyDef          :pd569ac00d20411e1800000215ad4efdf , :pdbf82380d20411e1800000215ad4efdf , :pd8fd3300d20411e1800000215ad4efdf , :pdef31400d20411e1800000215ad4efdf .

:pd8fd3300d20411e1800000215ad4efdf
        a                         IFC4-PSD:PropertyDef ;
        rdfs:comment              "Indicates sensed direction for sensors capturing magnitude and direction measured from True North (0 degrees) in a clockwise direction." ;
        rdfs:label                "Direction" ;
        IFC4-PSD:definition       "Indicates sensed direction for sensors capturing magnitude and direction measured from True North (0 degrees) in a clockwise direction." ;
        IFC4-PSD:definitionAlias  ""@en ;
        IFC4-PSD:ifdguid          "d8fd3300d20411e1800000215ad4efdf" ;
        IFC4-PSD:name             "Direction" ;
        IFC4-PSD:nameAlias        "Direction"@en ;
        IFC4-PSD:propertyType     [ a                 IFC4-PSD:TypePropertyReferenceValue ;
                                    IFC4-PSD:reftype  IFC4:IfcTimeSeries
                                  ] .

:pd569ac00d20411e1800000215ad4efdf
        a                         IFC4-PSD:PropertyDef ;
        rdfs:comment              "Indicates sensed values over time which may be recorded continuously or only when changed beyond a particular deadband.  The range of possible values is defined by the SetPoint property of the corresponding sensor type property set." ;
        rdfs:label                "Value" ;
        IFC4-PSD:definition       "Indicates sensed values over time which may be recorded continuously or only when changed beyond a particular deadband.  The range of possible values is defined by the SetPoint property of the corresponding sensor type property set." ;
        IFC4-PSD:definitionAlias  ""@en ;
        IFC4-PSD:ifdguid          "d569ac00d20411e1800000215ad4efdf" ;
        IFC4-PSD:name             "Value" ;
        IFC4-PSD:nameAlias        "Value"@en ;
        IFC4-PSD:propertyType     [ a                 IFC4-PSD:TypePropertyReferenceValue ;
                                    IFC4-PSD:reftype  IFC4:IfcTimeSeries
                                  ] .

:Quality  a                 rdf:Property ;
        rdfs:seeAlso        :pdbf82380d20411e1800000215ad4efdf ;
        rdfs:subPropertyOf  IFC4-PSD:Quality .

:Status  a                  rdf:Property ;
        rdfs:seeAlso        :pdef31400d20411e1800000215ad4efdf ;
        rdfs:subPropertyOf  IFC4-PSD:Status .

:pdbf82380d20411e1800000215ad4efdf
        a                         IFC4-PSD:PropertyDef ;
        rdfs:comment              "Indicates the quality of measurement or failure condition, which may be further qualified by the Status.  True: measured values are considered reliable; False: measured values are considered not reliable (i.e. a fault has been detected); Unknown: reliability of values is uncertain." ;
        rdfs:label                "Quality" ;
        IFC4-PSD:definition       "Indicates the quality of measurement or failure condition, which may be further qualified by the Status.  True: measured values are considered reliable; False: measured values are considered not reliable (i.e. a fault has been detected); Unknown: reliability of values is uncertain." ;
        IFC4-PSD:definitionAlias  ""@en ;
        IFC4-PSD:ifdguid          "dbf82380d20411e1800000215ad4efdf" ;
        IFC4-PSD:name             "Quality" ;
        IFC4-PSD:nameAlias        "Quality"@en ;
        IFC4-PSD:propertyType     [ a                 IFC4-PSD:TypePropertyReferenceValue ;
                                    IFC4-PSD:reftype  IFC4:IfcTimeSeries
                                  ] .

:Direction  a               rdf:Property ;
        rdfs:seeAlso        :pd8fd3300d20411e1800000215ad4efdf ;
        rdfs:subPropertyOf  IFC4-PSD:Direction .

:pdef31400d20411e1800000215ad4efdf
        a                         IFC4-PSD:PropertyDef ;
        rdfs:comment              "Indicates an error code or identifier, whose meaning is specific to the particular automation system.  Example values include: 'ConfigurationError', 'NotConnected', 'DeviceFailure', 'SensorFailure', 'LastKnown, 'CommunicationsFailure', 'OutOfService'." ;
        rdfs:label                "Status" ;
        IFC4-PSD:definition       "Indicates an error code or identifier, whose meaning is specific to the particular automation system.  Example values include: 'ConfigurationError', 'NotConnected', 'DeviceFailure', 'SensorFailure', 'LastKnown, 'CommunicationsFailure', 'OutOfService'." ;
        IFC4-PSD:definitionAlias  ""@en ;
        IFC4-PSD:ifdguid          "def31400d20411e1800000215ad4efdf" ;
        IFC4-PSD:name             "Status" ;
        IFC4-PSD:nameAlias        "Status"@en ;
        IFC4-PSD:propertyType     [ a                 IFC4-PSD:TypePropertyReferenceValue ;
                                    IFC4-PSD:reftype  IFC4:IfcTimeSeries
                                  ] .
