@prefix :      <https://www.linkedbuildingdata.net/IFC4-PSD/Pset_DistributionChamberElementTypeManhole#> .
@prefix IFC4-PSD: <https://www.linkedbuildingdata.net/IFC4-PSD#> .
@prefix rdf:   <http://www.w3.org/1999/02/22-rdf-syntax-ns#> .
@prefix owl:   <http://www.w3.org/2002/07/owl#> .
@prefix rdfs:  <http://www.w3.org/2000/01/rdf-schema#> .
@prefix IFC4:  <http://lbd.arch.rwth-aachen.de/ifcOWL/IFC4#> .

:WallMaterial  a            rdf:Property ;
        rdfs:seeAlso        :p01206e00d1d411e1800000215ad4efdf ;
        rdfs:subPropertyOf  IFC4-PSD:WallMaterial .

:IsShallow  a               rdf:Property ;
        rdfs:seeAlso        :p13021100d1d411e1800000215ad4efdf ;
        rdfs:subPropertyOf  IFC4-PSD:IsShallow .

:p0da4c680d1d411e1800000215ad4efdf
        a                         IFC4-PSD:PropertyDef ;
        rdfs:comment              "The thickness of the chamber base construction\nNOTE: It is assumed that chamber base will be constructed at a single thickness." ;
        rdfs:label                "BaseThickness" ;
        IFC4-PSD:definition       "The thickness of the chamber base construction\nNOTE: It is assumed that chamber base will be constructed at a single thickness." ;
        IFC4-PSD:definitionAlias  "ダクトスペース床面の厚さ。\n注：ダクトスペースの床は単層と仮定する"@ja-JP , "덕트 공간 바닥의 두께 참고 : 덕트 공간의 바닥은 단층 가정"@ko-KR , ""@en ;
        IFC4-PSD:ifdguid          "0da4c680d1d411e1800000215ad4efdf" ;
        IFC4-PSD:name             "BaseThickness" ;
        IFC4-PSD:nameAlias        "Base Thickness"@en , "바닥의 두께"@ko-KR , "床の厚さ"@ja-JP ;
        IFC4-PSD:propertyType     [ a                  IFC4-PSD:TypePropertySingleValue ;
                                    IFC4-PSD:dataType  IFC4:IfcPositiveLengthMeasure
                                  ] .

:p185f5b80d1d411e1800000215ad4efdf
        a                         IFC4-PSD:PropertyDef ;
        rdfs:comment              "Indicates whether the chamber has steps (TRUE) or not (FALSE)." ;
        rdfs:label                "HasSteps" ;
        IFC4-PSD:definition       "Indicates whether the chamber has steps (TRUE) or not (FALSE)." ;
        IFC4-PSD:definitionAlias  "덕트 공간은 계단 표시 여부 (TRUE 또는 FALSE)"@ko-KR , ""@en , "ダクトスペースは階段付けかどうか（TRUE或いはFALSE）。"@ja-JP ;
        IFC4-PSD:ifdguid          "185f5b80d1d411e1800000215ad4efdf" ;
        IFC4-PSD:name             "HasSteps" ;
        IFC4-PSD:nameAlias        "Has Steps"@en , "계단 지정"@ko-KR , "階段付け"@ja-JP ;
        IFC4-PSD:propertyType     [ a                  IFC4-PSD:TypePropertySingleValue ;
                                    IFC4-PSD:dataType  IFC4:IfcBoolean
                                  ] .

:pfc5bba00d1d311e1800000215ad4efdf
        a                         IFC4-PSD:PropertyDef ;
        rdfs:comment              "Level of the highest internal part of the cross section as measured from ground level." ;
        rdfs:label                "SoffitLevel" ;
        IFC4-PSD:definition       "Level of the highest internal part of the cross section as measured from ground level." ;
        IFC4-PSD:definitionAlias  "단면의 가장 높은 부분의 깊이 (지상에서)"@ko-KR , ""@en , "断面の最も高い部分の深さ（地面から）。"@ja-JP ;
        IFC4-PSD:ifdguid          "fc5bba00d1d311e1800000215ad4efdf" ;
        IFC4-PSD:name             "SoffitLevel" ;
        IFC4-PSD:nameAlias        "Soffit Level"@en , "최소깊이"@ko-KR , "最小深さ"@ja-JP ;
        IFC4-PSD:propertyType     [ a                  IFC4-PSD:TypePropertySingleValue ;
                                    IFC4-PSD:dataType  IFC4:IfcLengthMeasure
                                  ] .

:InvertLevel  a             rdf:Property ;
        rdfs:seeAlso        :pf7970600d1d311e1800000215ad4efdf ;
        rdfs:subPropertyOf  IFC4-PSD:InvertLevel .

:p13021100d1d411e1800000215ad4efdf
        a                         IFC4-PSD:PropertyDef ;
        rdfs:comment              "Indicates whether the chamber has been designed as being shallow (TRUE) or deep (FALSE)." ;
        rdfs:label                "IsShallow" ;
        IFC4-PSD:definition       "Indicates whether the chamber has been designed as being shallow (TRUE) or deep (FALSE)." ;
        IFC4-PSD:definitionAlias  "덕트 공간이 얕은 여부 (TRUE 또는 FALSE)"@ko-KR , "ダクトスペースは浅いかどうか（TRUE或いはFALSE）。"@ja-JP , ""@en ;
        IFC4-PSD:ifdguid          "13021100d1d411e1800000215ad4efdf" ;
        IFC4-PSD:name             "IsShallow" ;
        IFC4-PSD:nameAlias        "Is Shallow"@en , "덕트공간"@ko-KR , "浅いか"@ja-JP ;
        IFC4-PSD:propertyType     [ a                  IFC4-PSD:TypePropertySingleValue ;
                                    IFC4-PSD:dataType  IFC4:IfcBoolean
                                  ] .

:p1dbca600d1d411e1800000215ad4efdf
        a                         IFC4-PSD:PropertyDef ;
        rdfs:comment              "Indicates whether the chamber has a backdrop or tumbling bay (TRUE) or not (FALSE)." ;
        rdfs:label                "WithBackdrop" ;
        IFC4-PSD:definition       "Indicates whether the chamber has a backdrop or tumbling bay (TRUE) or not (FALSE)." ;
        IFC4-PSD:definitionAlias  "ダクトスペースはバックドロップ或いは堰付けかどうか（TRUE或いはFALSE）。"@ja-JP , "덕트 공간 백드롭 혹은 보 표시 여부 (TRUE 또는 FALSE)"@ko-KR , ""@en ;
        IFC4-PSD:ifdguid          "1dbca600d1d411e1800000215ad4efdf" ;
        IFC4-PSD:name             "WithBackdrop" ;
        IFC4-PSD:nameAlias        "With Backdrop"@en , "バックドロップ付け"@ja-JP , "백 드롭 지정"@ko-KR ;
        IFC4-PSD:propertyType     [ a                  IFC4-PSD:TypePropertySingleValue ;
                                    IFC4-PSD:dataType  IFC4:IfcBoolean
                                  ] .

:p01206e00d1d411e1800000215ad4efdf
        a                         IFC4-PSD:PropertyDef ;
        rdfs:comment              "The material from which the wall of the chamber is constructed.\nNOTE: It is assumed that chamber walls will be constructed of a single material." ;
        rdfs:label                "WallMaterial" ;
        IFC4-PSD:definition       "The material from which the wall of the chamber is constructed.\nNOTE: It is assumed that chamber walls will be constructed of a single material." ;
        IFC4-PSD:definitionAlias  "덕트 공간 벽의 재질 참고 : 덕트 공간의 벽은 단층 가정"@ko-KR , "ダクトスペース壁の材質。\n注：ダクトスペースの壁は単層と仮定する"@ja-JP , ""@en ;
        IFC4-PSD:ifdguid          "01206e00d1d411e1800000215ad4efdf" ;
        IFC4-PSD:name             "WallMaterial" ;
        IFC4-PSD:nameAlias        "壁の材質"@ja-JP , "Wall Material"@en , "벽의 재질"@ko-KR ;
        IFC4-PSD:propertyType     [ a                 IFC4-PSD:TypePropertyReferenceValue ;
                                    IFC4-PSD:reftype  IFC4:IfcMaterialDefinition
                                  ] .

:p26ad7780d1d411e1800000215ad4efdf
        a                         IFC4-PSD:PropertyDef ;
        rdfs:comment              "The length of the chamber access cover or, where the plan shape of the cover is circular, the radius." ;
        rdfs:label                "AccessLengthOrRadius" ;
        IFC4-PSD:definition       "The length of the chamber access cover or, where the plan shape of the cover is circular, the radius." ;
        IFC4-PSD:definitionAlias  "사용 (체크) 덮개 길이, 혹은 원형 커버 반경"@ko-KR , ""@en , "アクセス（点検）カバーの長さ、或いは円形カバーの半径。"@ja-JP ;
        IFC4-PSD:ifdguid          "26ad7780d1d411e1800000215ad4efdf" ;
        IFC4-PSD:name             "AccessLengthOrRadius" ;
        IFC4-PSD:nameAlias        "Access Length Or Radius"@en , "사용(체크)덮개 길이 혹은 반경"@ko-KR , "アクセス（点検）カバーの長さ或いは半径"@ja-JP ;
        IFC4-PSD:propertyType     [ a                  IFC4-PSD:TypePropertySingleValue ;
                                    IFC4-PSD:dataType  IFC4:IfcPositiveLengthMeasure
                                  ] .

:HasSteps  a                rdf:Property ;
        rdfs:seeAlso        :p185f5b80d1d411e1800000215ad4efdf ;
        rdfs:subPropertyOf  IFC4-PSD:HasSteps .

:pf7970600d1d311e1800000215ad4efdf
        a                         IFC4-PSD:PropertyDef ;
        rdfs:comment              "Level of the lowest part of the cross section as measured from ground level." ;
        rdfs:label                "InvertLevel" ;
        IFC4-PSD:definition       "Level of the lowest part of the cross section as measured from ground level." ;
        IFC4-PSD:definitionAlias  "단면의 가장 낮은 부분의 깊이 (지상에서)"@ko-KR , "断面の最も低い部分の深さ（地面から）。"@ja-JP , ""@en ;
        IFC4-PSD:ifdguid          "f7970600d1d311e1800000215ad4efdf" ;
        IFC4-PSD:name             "InvertLevel" ;
        IFC4-PSD:nameAlias        "Invert Level"@en , "最大深さ"@ja-JP , "최대 깊이"@ko-KR ;
        IFC4-PSD:propertyType     [ a                  IFC4-PSD:TypePropertySingleValue ;
                                    IFC4-PSD:dataType  IFC4:IfcLengthMeasure
                                  ] .

:WithBackdrop  a            rdf:Property ;
        rdfs:seeAlso        :p1dbca600d1d411e1800000215ad4efdf ;
        rdfs:subPropertyOf  IFC4-PSD:WithBackdrop .

:AccessCoverMaterial  a     rdf:Property ;
        rdfs:seeAlso        :p23b28700d1d411e1800000215ad4efdf ;
        rdfs:subPropertyOf  IFC4-PSD:AccessCoverMaterial .

:p2ca35880d1d411e1800000215ad4efdf
        a                         IFC4-PSD:PropertyDef ;
        rdfs:comment              "The width of the chamber access cover where the plan shape of the cover is not circular." ;
        rdfs:label                "AccessWidth" ;
        IFC4-PSD:definition       "The width of the chamber access cover where the plan shape of the cover is not circular." ;
        IFC4-PSD:definitionAlias  ""@en , "アクセス（点検）カバーの幅。"@ja-JP , "사용 (체크) 커버 폭"@ko-KR ;
        IFC4-PSD:ifdguid          "2ca35880d1d411e1800000215ad4efdf" ;
        IFC4-PSD:name             "AccessWidth" ;
        IFC4-PSD:nameAlias        "사용 (체크)커버 폭"@ko-KR , "Access Width"@en , "アクセス（点検）カバーの幅"@ja-JP ;
        IFC4-PSD:propertyType     [ a                  IFC4-PSD:TypePropertySingleValue ;
                                    IFC4-PSD:dataType  IFC4:IfcPositiveLengthMeasure
                                  ] .

:p04b3f500d1d411e1800000215ad4efdf
        a                         IFC4-PSD:PropertyDef ;
        rdfs:comment              "The thickness of the chamber wall construction\nNOTE: It is assumed that chamber walls will be constructed at a single thickness." ;
        rdfs:label                "WallThickness" ;
        IFC4-PSD:definition       "The thickness of the chamber wall construction\nNOTE: It is assumed that chamber walls will be constructed at a single thickness." ;
        IFC4-PSD:definitionAlias  "ダクトスペース壁の厚さ。\n注：ダクトスペースの壁は単層と仮定する"@ja-JP , "덕트 공간 벽 두께 참고 : 덕트 공간의 벽은 단층 가정"@ko-KR , ""@en ;
        IFC4-PSD:ifdguid          "04b3f500d1d411e1800000215ad4efdf" ;
        IFC4-PSD:name             "WallThickness" ;
        IFC4-PSD:nameAlias        "벽 두께"@ko-KR , "Wall Thickness"@en , "壁厚さ"@ja-JP ;
        IFC4-PSD:propertyType     [ a                  IFC4-PSD:TypePropertySingleValue ;
                                    IFC4-PSD:dataType  IFC4:IfcPositiveLengthMeasure
                                  ] .

:AccessCoverLoadRating
        a                   rdf:Property ;
        rdfs:seeAlso        :p32993980d1d411e1800000215ad4efdf ;
        rdfs:subPropertyOf  IFC4-PSD:AccessCoverLoadRating .

:p32993980d1d411e1800000215ad4efdf
        a                         IFC4-PSD:PropertyDef ;
        rdfs:comment              "The load rating of the access cover (which may be a value or an alphanumerically defined class rating)." ;
        rdfs:label                "AccessCoverLoadRating" ;
        IFC4-PSD:definition       "The load rating of the access cover (which may be a value or an alphanumerically defined class rating)." ;
        IFC4-PSD:definitionAlias  ""@en , "사용 (체크) 커버 하중 (숫자 혹은 알파벳에서 정의됨)"@ko-KR , "アクセス（点検）カバーの耐荷重（数字或いはアルファベットで定義する）。"@ja-JP ;
        IFC4-PSD:ifdguid          "32993980d1d411e1800000215ad4efdf" ;
        IFC4-PSD:name             "AccessCoverLoadRating" ;
        IFC4-PSD:nameAlias        "アクセス（点検）カバーの耐荷重"@ja-JP , "Access Cover Load Rating"@en , "사용 (체크)커버 하중"@ko-KR ;
        IFC4-PSD:propertyType     [ a                  IFC4-PSD:TypePropertySingleValue ;
                                    IFC4-PSD:dataType  IFC4:IfcText
                                  ] .

:AccessLengthOrRadius
        a                   rdf:Property ;
        rdfs:seeAlso        :p26ad7780d1d411e1800000215ad4efdf ;
        rdfs:subPropertyOf  IFC4-PSD:AccessLengthOrRadius .

:BaseMaterial  a            rdf:Property ;
        rdfs:seeAlso        :p0a113f80d1d411e1800000215ad4efdf ;
        rdfs:subPropertyOf  IFC4-PSD:BaseMaterial .

:AccessWidth  a             rdf:Property ;
        rdfs:seeAlso        :p2ca35880d1d411e1800000215ad4efdf ;
        rdfs:subPropertyOf  IFC4-PSD:AccessWidth .

:SoffitLevel  a             rdf:Property ;
        rdfs:seeAlso        :pfc5bba00d1d311e1800000215ad4efdf ;
        rdfs:subPropertyOf  IFC4-PSD:SoffitLevel .

:BaseThickness  a           rdf:Property ;
        rdfs:seeAlso        :p0da4c680d1d411e1800000215ad4efdf ;
        rdfs:subPropertyOf  IFC4-PSD:BaseThickness .

:p0a113f80d1d411e1800000215ad4efdf
        a                         IFC4-PSD:PropertyDef ;
        rdfs:comment              "The material from which the base of the chamber is constructed.\nNOTE: It is assumed that chamber base will be constructed of a single material." ;
        rdfs:label                "BaseMaterial" ;
        IFC4-PSD:definition       "The material from which the base of the chamber is constructed.\nNOTE: It is assumed that chamber base will be constructed of a single material." ;
        IFC4-PSD:definitionAlias  "덕트 공간 바닥의 재질 참고 : 덕트 공간의 바닥은 단층 가정"@ko-KR , ""@en , "ダクトスペース床面の材質。\n注：ダクトスペースの床は単層と仮定する"@ja-JP ;
        IFC4-PSD:ifdguid          "0a113f80d1d411e1800000215ad4efdf" ;
        IFC4-PSD:name             "BaseMaterial" ;
        IFC4-PSD:nameAlias        "바닥의 재질"@ko-KR , "床の材質"@ja-JP , "Base Material"@en ;
        IFC4-PSD:propertyType     [ a                 IFC4-PSD:TypePropertyReferenceValue ;
                                    IFC4-PSD:reftype  IFC4:IfcMaterialDefinition
                                  ] .

<https://www.linkedbuildingdata.net/IFC4-PSD/Pset_DistributionChamberElementTypeManhole>
        a                owl:Ontology ;
        owl:imports      <http://lbd.arch.rwth-aachen.de/ifcOWL/IFC4-PSD> ;
        owl:versionInfo  "Created with BIM-Bots PSD Repository" .

:p23b28700d1d411e1800000215ad4efdf
        a                         IFC4-PSD:PropertyDef ;
        rdfs:comment              "The material from which the access cover to the chamber is constructed.\nNOTE: It is assumed that chamber walls will be constructed of a single material." ;
        rdfs:label                "AccessCoverMaterial" ;
        IFC4-PSD:definition       "The material from which the access cover to the chamber is constructed.\nNOTE: It is assumed that chamber walls will be constructed of a single material." ;
        IFC4-PSD:definitionAlias  "액세스 (체크) 커버의 재질 주 : 챔퍼 공간의 벽은 단층 가정"@ko-KR , ""@en , "アクセス（点検）カバーの材質。\n注：バイブスペースの壁は単層と仮定する"@ja-JP ;
        IFC4-PSD:ifdguid          "23b28700d1d411e1800000215ad4efdf" ;
        IFC4-PSD:name             "AccessCoverMaterial" ;
        IFC4-PSD:nameAlias        "사용(체크)커버의 재질"@ko-KR , "アクセス（点検）カバーの材質"@ja-JP , "Access Cover Material"@en ;
        IFC4-PSD:propertyType     [ a                 IFC4-PSD:TypePropertyReferenceValue ;
                                    IFC4-PSD:reftype  IFC4:IfcMaterialDefinition
                                  ] .

:WallThickness  a           rdf:Property ;
        rdfs:seeAlso        :p04b3f500d1d411e1800000215ad4efdf ;
        rdfs:subPropertyOf  IFC4-PSD:WallThickness .

:Pset_DistributionChamberElementTypeManhole
        a                             IFC4-PSD:PropertySetDef ;
        rdfs:comment                  "Chamber constructed on a drain, sewer or pipeline and with a removable cover, that permits the entry of a person." ;
        rdfs:label                    "Pset_DistributionChamberElementTypeManhole" ;
        IFC4-PSD:applicableClass      <http://lbd.arch.rwth-aachen.de/ifcOWL/IFC4#IfcDistributionChamberElement/MANHOLE> ;
        IFC4-PSD:applicableTypeValue  "IfcDistributionChamberElement/MANHOLE" ;
        IFC4-PSD:definition           "Chamber constructed on a drain, sewer or pipeline and with a removable cover, that permits the entry of a person." ;
        IFC4-PSD:definitionAlias      "排水、下水管の上にある・点検用可移動カバー付けパイプスペース。"@ja-JP , ""@en ;
        IFC4-PSD:ifcVersion           [ a                 IFC4-PSD:IfcVersion ;
                                        IFC4-PSD:version  "IFC4"
                                      ] ;
        IFC4-PSD:name                 "Pset_DistributionChamberElementTypeManhole" ;
        IFC4-PSD:propertyDef          :p01206e00d1d411e1800000215ad4efdf , :p0a113f80d1d411e1800000215ad4efdf , :p1dbca600d1d411e1800000215ad4efdf , :p23b28700d1d411e1800000215ad4efdf , :p32993980d1d411e1800000215ad4efdf , :p0da4c680d1d411e1800000215ad4efdf , :pfc5bba00d1d311e1800000215ad4efdf , :p26ad7780d1d411e1800000215ad4efdf , :p04b3f500d1d411e1800000215ad4efdf , :p13021100d1d411e1800000215ad4efdf , :p185f5b80d1d411e1800000215ad4efdf , :pf7970600d1d311e1800000215ad4efdf , :p2ca35880d1d411e1800000215ad4efdf .
