@prefix :      <https://www.linkedbuildingdata.net/IFC4-PSD/Pset_MaterialCombustion#> .
@prefix IFC4-PSD: <https://www.linkedbuildingdata.net/IFC4-PSD#> .
@prefix rdf:   <http://www.w3.org/1999/02/22-rdf-syntax-ns#> .
@prefix owl:   <http://www.w3.org/2002/07/owl#> .
@prefix rdfs:  <http://www.w3.org/2000/01/rdf-schema#> .
@prefix IFC4:  <http://lbd.arch.rwth-aachen.de/ifcOWL/IFC4#> .

:N20Content  a              rdf:Property ;
        rdfs:seeAlso        :pbc550100d1ec11e1800000215ad4efdf ;
        rdfs:subPropertyOf  IFC4-PSD:N20Content .

:SpecificHeatCapacity
        a                   rdf:Property ;
        rdfs:seeAlso        :pb6f7b680d1ec11e1800000215ad4efdf ;
        rdfs:subPropertyOf  IFC4-PSD:SpecificHeatCapacity .

:pb6f7b680d1ec11e1800000215ad4efdf
        a                         IFC4-PSD:PropertyDef ;
        rdfs:comment              "Specific heat of the products of combustion: heat energy absorbed per temperature unit." ;
        rdfs:label                "SpecificHeatCapacity" ;
        IFC4-PSD:definition       "Specific heat of the products of combustion: heat energy absorbed per temperature unit." ;
        IFC4-PSD:definitionAlias  ""@en ;
        IFC4-PSD:ifdguid          "b6f7b680d1ec11e1800000215ad4efdf" ;
        IFC4-PSD:name             "SpecificHeatCapacity" ;
        IFC4-PSD:nameAlias        "Specific Heat Capacity"@en ;
        IFC4-PSD:propertyType     [ a                  IFC4-PSD:TypePropertySingleValue ;
                                    IFC4-PSD:dataType  IFC4:IfcSpecificHeatCapacityMeasure
                                  ] .

<https://www.linkedbuildingdata.net/IFC4-PSD/Pset_MaterialCombustion>
        a                owl:Ontology ;
        owl:imports      <http://lbd.arch.rwth-aachen.de/ifcOWL/IFC4-PSD> ;
        owl:versionInfo  "Created with BIM-Bots PSD Repository" .

:Pset_MaterialCombustion
        a                             IFC4-PSD:PropertySetDef ;
        rdfs:comment                  "A set of extended material properties of products of combustion generated by elements typically used within the context of building services and flow distribution systems." ;
        rdfs:label                    "Pset_MaterialCombustion" ;
        IFC4-PSD:applicableClass      IFC4:IfcMaterial ;
        IFC4-PSD:applicableTypeValue  "IfcMaterial" ;
        IFC4-PSD:definition           "A set of extended material properties of products of combustion generated by elements typically used within the context of building services and flow distribution systems." ;
        IFC4-PSD:definitionAlias      ""@en ;
        IFC4-PSD:ifcVersion           [ a                 IFC4-PSD:IfcVersion ;
                                        IFC4-PSD:version  "IFC4"
                                      ] ;
        IFC4-PSD:name                 "Pset_MaterialCombustion" ;
        IFC4-PSD:propertyDef          :pc1b24b80d1ec11e1800000215ad4efdf , :pbc550100d1ec11e1800000215ad4efdf , :pb6f7b680d1ec11e1800000215ad4efdf , :pc7a82c80d1ec11e1800000215ad4efdf .

:pbc550100d1ec11e1800000215ad4efdf
        a                         IFC4-PSD:PropertyDef ;
        rdfs:comment              "Nitrous oxide (N2O) content of the products of combustion. This is measured in weight of N2O per unit weight and is therefore unitless." ;
        rdfs:label                "N20Content" ;
        IFC4-PSD:definition       "Nitrous oxide (N2O) content of the products of combustion. This is measured in weight of N2O per unit weight and is therefore unitless." ;
        IFC4-PSD:definitionAlias  ""@en ;
        IFC4-PSD:ifdguid          "bc550100d1ec11e1800000215ad4efdf" ;
        IFC4-PSD:name             "N20Content" ;
        IFC4-PSD:nameAlias        "N20 Content"@en ;
        IFC4-PSD:propertyType     [ a                  IFC4-PSD:TypePropertySingleValue ;
                                    IFC4-PSD:dataType  IFC4:IfcPositiveRatioMeasure
                                  ] .

:pc1b24b80d1ec11e1800000215ad4efdf
        a                         IFC4-PSD:PropertyDef ;
        rdfs:comment              "Carbon monoxide (CO) content of the products of combustion. This is measured in weight of CO per unit weight and is therefore unitless." ;
        rdfs:label                "COContent" ;
        IFC4-PSD:definition       "Carbon monoxide (CO) content of the products of combustion. This is measured in weight of CO per unit weight and is therefore unitless." ;
        IFC4-PSD:definitionAlias  ""@en ;
        IFC4-PSD:ifdguid          "c1b24b80d1ec11e1800000215ad4efdf" ;
        IFC4-PSD:name             "COContent" ;
        IFC4-PSD:nameAlias        "COContent"@en ;
        IFC4-PSD:propertyType     [ a                  IFC4-PSD:TypePropertySingleValue ;
                                    IFC4-PSD:dataType  IFC4:IfcPositiveRatioMeasure
                                  ] .

:pc7a82c80d1ec11e1800000215ad4efdf
        a                         IFC4-PSD:PropertyDef ;
        rdfs:comment              "Carbon dioxide (CO2) content of the products of combustion. This is measured in weight of CO2 per unit weight and is therefore unitless." ;
        rdfs:label                "CO2Content" ;
        IFC4-PSD:definition       "Carbon dioxide (CO2) content of the products of combustion. This is measured in weight of CO2 per unit weight and is therefore unitless." ;
        IFC4-PSD:definitionAlias  ""@en ;
        IFC4-PSD:ifdguid          "c7a82c80d1ec11e1800000215ad4efdf" ;
        IFC4-PSD:name             "CO2Content" ;
        IFC4-PSD:nameAlias        "CO2 Content"@en ;
        IFC4-PSD:propertyType     [ a                  IFC4-PSD:TypePropertySingleValue ;
                                    IFC4-PSD:dataType  IFC4:IfcPositiveRatioMeasure
                                  ] .

:CO2Content  a              rdf:Property ;
        rdfs:seeAlso        :pc7a82c80d1ec11e1800000215ad4efdf ;
        rdfs:subPropertyOf  IFC4-PSD:CO2Content .

:COContent  a               rdf:Property ;
        rdfs:seeAlso        :pc1b24b80d1ec11e1800000215ad4efdf ;
        rdfs:subPropertyOf  IFC4-PSD:COContent .
