@prefix :      <https://www.linkedbuildingdata.net/IFC4-PSD/Pset_ProtectiveDeviceTrippingUnitTypeElectroMagnetic#> .
@prefix IFC4-PSD: <https://www.linkedbuildingdata.net/IFC4-PSD#> .
@prefix rdf:   <http://www.w3.org/1999/02/22-rdf-syntax-ns#> .
@prefix owl:   <http://www.w3.org/2002/07/owl#> .
@prefix rdfs:  <http://www.w3.org/2000/01/rdf-schema#> .
@prefix IFC4:  <http://lbd.arch.rwth-aachen.de/ifcOWL/IFC4#> .

:p799b2500d1fc11e1800000215ad4efdf
        a                         IFC4-PSD:PropertyDef ;
        rdfs:comment              "The upper electromagnetic testing current limit in [x In], indicating that for currents larger than I5, the tripping time shall be shorter than or equal to the associated tripping time, T5, i.e. the device shall trip instantaneous." ;
        rdfs:label                "I5" ;
        IFC4-PSD:definition       "The upper electromagnetic testing current limit in [x In], indicating that for currents larger than I5, the tripping time shall be shorter than or equal to the associated tripping time, T5, i.e. the device shall trip instantaneous." ;
        IFC4-PSD:definitionAlias  "電磁の高試験電流限界値を [x In], 電流は I4 よりも低い値を示す。トリップ時間は関連する T5 と瞬時に遮断する定格使用電流の時間よりも長い。"@ja-JP , ""@en , "전자의 높은 시험 전류 한계를 [x In] 전류는 I4보다 낮은 값을 나타낸다. 트립 시간은 관련 T5 즉석에서 차단하는 정격 사용 전류의 시간보다 길다."@ko-KR ;
        IFC4-PSD:ifdguid          "799b2500d1fc11e1800000215ad4efdf" ;
        IFC4-PSD:name             "I5" ;
        IFC4-PSD:nameAlias        "I5"@ja-JP , "I5"@ko-KR , "I5"@en ;
        IFC4-PSD:propertyType     [ a                  IFC4-PSD:TypePropertySingleValue ;
                                    IFC4-PSD:dataType  IFC4:IfcReal
                                  ] .

:Pset_ProtectiveDeviceTrippingUnitTypeElectroMagnetic
        a                             IFC4-PSD:PropertySetDef ;
        rdfs:comment                  "Information on tripping units that are electrically or magnetically tripped." ;
        rdfs:label                    "Pset_ProtectiveDeviceTrippingUnitTypeElectroMagnetic" ;
        IFC4-PSD:applicableClass      <http://lbd.arch.rwth-aachen.de/ifcOWL/IFC4#IfcProtectiveDeviceTrippingUnit/ELECTROMAGNETIC> ;
        IFC4-PSD:applicableTypeValue  "IfcProtectiveDeviceTrippingUnit/ELECTROMAGNETIC" ;
        IFC4-PSD:definition           "Information on tripping units that are electrically or magnetically tripped." ;
        IFC4-PSD:definitionAlias      ""@en , "電気と磁気により遮断するトリップ装置の情報。"@ja-JP ;
        IFC4-PSD:ifcVersion           [ a                 IFC4-PSD:IfcVersion ;
                                        IFC4-PSD:version  "IFC4"
                                      ] ;
        IFC4-PSD:name                 "Pset_ProtectiveDeviceTrippingUnitTypeElectroMagnetic" ;
        IFC4-PSD:propertyDef          :p84ee5080d1fc11e1800000215ad4efdf , :p80299c80d1fc11e1800000215ad4efdf , :p6ee09000d1fc11e1800000215ad4efdf , :p5b352980d1fc11e1800000215ad4efdf , :p68521880d1fc11e1800000215ad4efdf , :p60927400d1fc11e1800000215ad4efdf , :p799b2500d1fc11e1800000215ad4efdf , :p45bfff80d1fc11e1800000215ad4efdf , :p553f4880d1fc11e1800000215ad4efdf , :p73a54400d1fc11e1800000215ad4efdf .

:p68521880d1fc11e1800000215ad4efdf
        a                         IFC4-PSD:PropertyDef ;
        rdfs:comment              "The ambient temperature at which the thermal current/time-curve associated with this protection device is defined." ;
        rdfs:label                "DefinedTemperature" ;
        IFC4-PSD:definition       "The ambient temperature at which the thermal current/time-curve associated with this protection device is defined." ;
        IFC4-PSD:definitionAlias  "この保護装置が定める温度・電流/時間-カーブに関連する周囲温度。"@ja-JP , ""@en , "이 보호 장치가 정한 온도 · 전류 / 시간 - 곡선과 관련된 주위 온도."@ko-KR ;
        IFC4-PSD:ifdguid          "68521880d1fc11e1800000215ad4efdf" ;
        IFC4-PSD:name             "DefinedTemperature" ;
        IFC4-PSD:nameAlias        "Defined Temperature"@en , "설정 온도"@ko-KR , "設定温度"@ja-JP ;
        IFC4-PSD:propertyType     [ a                  IFC4-PSD:TypePropertySingleValue ;
                                    IFC4-PSD:dataType  IFC4:IfcThermodynamicTemperatureMeasure
                                  ] .

:I4     a                   rdf:Property ;
        rdfs:seeAlso        :p73a54400d1fc11e1800000215ad4efdf ;
        rdfs:subPropertyOf  IFC4-PSD:I4 .

:p84ee5080d1fc11e1800000215ad4efdf
        a                         IFC4-PSD:PropertyDef ;
        rdfs:comment              "The designation of the trippingcurve given by the manufacturer. For a MCB the designation should be in accordance with the designations given in IEC 60898." ;
        rdfs:label                "CurveDesignation" ;
        IFC4-PSD:definition       "The designation of the trippingcurve given by the manufacturer. For a MCB the designation should be in accordance with the designations given in IEC 60898." ;
        IFC4-PSD:definitionAlias  "제조 업체가 제공하는 지정된 토릿삔구 곡선. MCB 위해, 지정은 IEC 60898을 준수해야한다."@ko-KR , ""@en , "メーカーが提供する指定のトリッピングカーブ。MCBのために、指定はIEC 60898に準拠しなければならない。"@ja-JP ;
        IFC4-PSD:ifdguid          "84ee5080d1fc11e1800000215ad4efdf" ;
        IFC4-PSD:name             "CurveDesignation" ;
        IFC4-PSD:nameAlias        "곡성 지정"@ko-KR , "曲線指定"@ja-JP , "Curve Designation"@en ;
        IFC4-PSD:propertyType     [ a                  IFC4-PSD:TypePropertySingleValue ;
                                    IFC4-PSD:dataType  IFC4:IfcLabel
                                  ] .

:p60927400d1fc11e1800000215ad4efdf
        a                         IFC4-PSD:PropertyDef ;
        rdfs:comment              "The (thermal) testing time in [s] associated with the testing currents I1 and I2." ;
        rdfs:label                "T2" ;
        IFC4-PSD:definition       "The (thermal) testing time in [s] associated with the testing currents I1 and I2." ;
        IFC4-PSD:definitionAlias  "熱動式の試験時間を [s] , 関連する試験電流を I1 と I2　とする。"@ja-JP , "열 동식 시험 시간 [s] 관련 시험 전류를 I1과 I2로한다."@ko-KR , ""@en ;
        IFC4-PSD:ifdguid          "60927400d1fc11e1800000215ad4efdf" ;
        IFC4-PSD:name             "T2" ;
        IFC4-PSD:nameAlias        "T2"@ko-KR , "T2"@en , "T2"@ja-JP ;
        IFC4-PSD:propertyType     [ a                  IFC4-PSD:TypePropertySingleValue ;
                                    IFC4-PSD:dataType  IFC4:IfcTimeMeasure
                                  ] .

:p80299c80d1fc11e1800000215ad4efdf
        a                         IFC4-PSD:PropertyDef ;
        rdfs:comment              "The electromagnetic testing time in [s] associated with the testing currents I4 and I5, i.e. electromagnetic tripping time" ;
        rdfs:label                "T5" ;
        IFC4-PSD:definition       "The electromagnetic testing time in [s] associated with the testing currents I4 and I5, i.e. electromagnetic tripping time" ;
        IFC4-PSD:definitionAlias  ""@en , "전자 시험 시간 [s] 관련 시험 전류를 I4하면 I5한다."@ko-KR , "電磁の試験時間を [s] , 関連する試験電流を I4 と I5　とする。"@ja-JP ;
        IFC4-PSD:ifdguid          "80299c80d1fc11e1800000215ad4efdf" ;
        IFC4-PSD:name             "T5" ;
        IFC4-PSD:nameAlias        "T5"@en , "T5"@ja-JP , "T5"@ko-KR ;
        IFC4-PSD:propertyType     [ a                  IFC4-PSD:TypePropertySingleValue ;
                                    IFC4-PSD:dataType  IFC4:IfcTimeMeasure
                                  ] .

:TemperatureFactor  a       rdf:Property ;
        rdfs:seeAlso        :p6ee09000d1fc11e1800000215ad4efdf ;
        rdfs:subPropertyOf  IFC4-PSD:TemperatureFactor .

:p45bfff80d1fc11e1800000215ad4efdf
        a                         IFC4-PSD:PropertyDef ;
        rdfs:comment              "A list of the available types of electric magnetic tripping unit  from which that required may be selected. These cover overload, none special, short circuit, motor protection and bi-metal tripping." ;
        rdfs:label                "ElectroMagneticTrippingUnitType" ;
        IFC4-PSD:definition       "A list of the available types of electric magnetic tripping unit  from which that required may be selected. These cover overload, none special, short circuit, motor protection and bi-metal tripping." ;
        IFC4-PSD:definitionAlias  "전자 트립 장치 유형을 선택합니다. (과전류 · 배선 모터 바이메탈 기타)"@ko-KR , ""@en , "電磁トリップ装置タイプを選択する。（過電流・配線用・モーター・バイメタル・その他）"@ja-JP ;
        IFC4-PSD:ifdguid          "45bfff80d1fc11e1800000215ad4efdf" ;
        IFC4-PSD:name             "ElectroMagneticTrippingUnitType" ;
        IFC4-PSD:nameAlias        "電磁トリップ装置タイプ"@ja-JP , "전자 트립장치 유형"@ko-KR , "Electro Magnetic Tripping Unit Type"@en ;
        IFC4-PSD:propertyType     [ a                  IFC4-PSD:TypePropertyEnumeratedValue ;
                                    IFC4-PSD:enumItem  "OL" , "TMP_STD" , "TMP_SC" , "TMP_MP" , "TMP_BM" , "OTHER" , "NOTKNOWN" , "UNSET"
                                  ] .

:T2     a                   rdf:Property ;
        rdfs:seeAlso        :p60927400d1fc11e1800000215ad4efdf ;
        rdfs:subPropertyOf  IFC4-PSD:T2 .

:I2     a                   rdf:Property ;
        rdfs:seeAlso        :p5b352980d1fc11e1800000215ad4efdf ;
        rdfs:subPropertyOf  IFC4-PSD:I2 .

:ElectroMagneticTrippingUnitType
        a                   rdf:Property ;
        rdfs:seeAlso        :p45bfff80d1fc11e1800000215ad4efdf ;
        rdfs:subPropertyOf  IFC4-PSD:ElectroMagneticTrippingUnitType .

:p553f4880d1fc11e1800000215ad4efdf
        a                         IFC4-PSD:PropertyDef ;
        rdfs:comment              "The (thermal) lower testing current limit in [x In], indicating that for currents lower than I1, the tripping time shall be longer than the associated tripping time, T2." ;
        rdfs:label                "I1" ;
        IFC4-PSD:definition       "The (thermal) lower testing current limit in [x In], indicating that for currents lower than I1, the tripping time shall be longer than the associated tripping time, T2." ;
        IFC4-PSD:definitionAlias  "熱動式の低試験電流限界値を [x In]、電流は I1　よりも低い値を示す。トリップ時間は関連する T2 の時間よりも長い。"@ja-JP , "열 동식 낮은 시험 전류 한계를 [x In] 전류는 I1보다 낮은 값을 나타낸다. 트립 시간은 관련 T2 시간보다 길다."@ko-KR , ""@en ;
        IFC4-PSD:ifdguid          "553f4880d1fc11e1800000215ad4efdf" ;
        IFC4-PSD:name             "I1" ;
        IFC4-PSD:nameAlias        "I1"@ja-JP , "I1"@ko-KR , "I1"@en ;
        IFC4-PSD:propertyType     [ a                  IFC4-PSD:TypePropertySingleValue ;
                                    IFC4-PSD:dataType  IFC4:IfcReal
                                  ] .

:CurveDesignation  a        rdf:Property ;
        rdfs:seeAlso        :p84ee5080d1fc11e1800000215ad4efdf ;
        rdfs:subPropertyOf  IFC4-PSD:CurveDesignation .

<https://www.linkedbuildingdata.net/IFC4-PSD/Pset_ProtectiveDeviceTrippingUnitTypeElectroMagnetic>
        a                owl:Ontology ;
        owl:imports      <http://lbd.arch.rwth-aachen.de/ifcOWL/IFC4-PSD> ;
        owl:versionInfo  "Created with BIM-Bots PSD Repository" .

:I1     a                   rdf:Property ;
        rdfs:seeAlso        :p553f4880d1fc11e1800000215ad4efdf ;
        rdfs:subPropertyOf  IFC4-PSD:I1 .

:p5b352980d1fc11e1800000215ad4efdf
        a                         IFC4-PSD:PropertyDef ;
        rdfs:comment              "The (thermal) upper testing current limit in [x In], indicating that for currents larger than I2, the tripping time shall be shorter than the associated tripping time, T2." ;
        rdfs:label                "I2" ;
        IFC4-PSD:definition       "The (thermal) upper testing current limit in [x In], indicating that for currents larger than I2, the tripping time shall be shorter than the associated tripping time, T2." ;
        IFC4-PSD:definitionAlias  ""@en , "열 동식 높은 시험 전류 한계를 [x In], 전류 I2보다 높은 값을 나타낸다. 트립 시간은 관련 T2 시간보다 짧다."@ko-KR , "熱動式の高試験電流限界値を [x In], 電流は I2 よりも高い値を示す。トリップ時間は関連する T2 の時間よりも短い。"@ja-JP ;
        IFC4-PSD:ifdguid          "5b352980d1fc11e1800000215ad4efdf" ;
        IFC4-PSD:name             "I2" ;
        IFC4-PSD:nameAlias        "I2"@en , "I2"@ja-JP , "I2"@ko-KR ;
        IFC4-PSD:propertyType     [ a                  IFC4-PSD:TypePropertySingleValue ;
                                    IFC4-PSD:dataType  IFC4:IfcReal
                                  ] .

:p6ee09000d1fc11e1800000215ad4efdf
        a                         IFC4-PSD:PropertyDef ;
        rdfs:comment              "The correction factor (typically measured as %/deg K) for adjusting the thermal current/time to an ambient temperature different from the value given by the defined temperature." ;
        rdfs:label                "TemperatureFactor" ;
        IFC4-PSD:definition       "The correction factor (typically measured as %/deg K) for adjusting the thermal current/time to an ambient temperature different from the value given by the defined temperature." ;
        IFC4-PSD:definitionAlias  "熱の電流/時間を、定義済みの温度によって与えられる値と異なる場合に周囲温度に合わせるための補正係数（%/deg K で計測する）。"@ja-JP , ""@en , "열 전류 / 시간 미리 정의된 온도에 의해 주어진 값과 다른 경우 주위 온도에 맞추기위한 보정 계수 (% / deg K로 측정한다)."@ko-KR ;
        IFC4-PSD:ifdguid          "6ee09000d1fc11e1800000215ad4efdf" ;
        IFC4-PSD:name             "TemperatureFactor" ;
        IFC4-PSD:nameAlias        "温度係数"@ja-JP , "온도 계수"@ko-KR , "Temperature Factor"@en ;
        IFC4-PSD:propertyType     [ a                  IFC4-PSD:TypePropertySingleValue ;
                                    IFC4-PSD:dataType  IFC4:IfcRatioMeasure
                                  ] .

:T5     a                   rdf:Property ;
        rdfs:seeAlso        :p80299c80d1fc11e1800000215ad4efdf ;
        rdfs:subPropertyOf  IFC4-PSD:T5 .

:p73a54400d1fc11e1800000215ad4efdf
        a                         IFC4-PSD:PropertyDef ;
        rdfs:comment              "The lower electromagnetic testing current limit in [x In], indicating that for currents lower than I4, the tripping time shall be longer than the associated tripping time, T5, i.e. the device shall not trip instantaneous." ;
        rdfs:label                "I4" ;
        IFC4-PSD:definition       "The lower electromagnetic testing current limit in [x In], indicating that for currents lower than I4, the tripping time shall be longer than the associated tripping time, T5, i.e. the device shall not trip instantaneous." ;
        IFC4-PSD:definitionAlias  "電磁の低試験電流限界値を [x In], 電流は I4 よりも低い値を示す。トリップ時間は関連する T5 と瞬時に遮断する定格使用電流の時間よりも長い。"@ja-JP , "전자 낮은 시험 전류 한계를 [x In] 전류는 I4보다 낮은 값을 나타낸다. 트립 시간은 관련 T5 즉석에서 차단하는 정격 사용 전류의 시간보다 길다."@ko-KR , ""@en ;
        IFC4-PSD:ifdguid          "73a54400d1fc11e1800000215ad4efdf" ;
        IFC4-PSD:name             "I4" ;
        IFC4-PSD:nameAlias        "I4"@en , "I4"@ja-JP , "I4"@ko-KR ;
        IFC4-PSD:propertyType     [ a                  IFC4-PSD:TypePropertySingleValue ;
                                    IFC4-PSD:dataType  IFC4:IfcReal
                                  ] .

:DefinedTemperature  a      rdf:Property ;
        rdfs:seeAlso        :p68521880d1fc11e1800000215ad4efdf ;
        rdfs:subPropertyOf  IFC4-PSD:DefinedTemperature .

:I5     a                   rdf:Property ;
        rdfs:seeAlso        :p799b2500d1fc11e1800000215ad4efdf ;
        rdfs:subPropertyOf  IFC4-PSD:I5 .
