@prefix :      <https://www.linkedbuildingdata.net/IFC4-PSD/Pset_SlabCommon#> .
@prefix IFC4-PSD: <https://www.linkedbuildingdata.net/IFC4-PSD#> .
@prefix owl:   <http://www.w3.org/2002/07/owl#> .
@prefix rdf:   <http://www.w3.org/1999/02/22-rdf-syntax-ns#> .
@prefix rdfs:  <http://www.w3.org/2000/01/rdf-schema#> .
@prefix IFC4:  <http://lbd.arch.rwth-aachen.de/ifcOWL/IFC4#> .

:p1a431200d20811e1800000215ad4efdf
        a                         IFC4-PSD:PropertyDef ;
        rdfs:comment              "Indication whether the object is made from combustible material (TRUE) or not (FALSE)." ;
        rdfs:label                "Combustible" ;
        IFC4-PSD:definition       "Indication whether the object is made from combustible material (TRUE) or not (FALSE)." ;
        IFC4-PSD:definitionAlias  "Angabe ob das Bauteil brennbares Material enthält (WAHR) oder nicht (FALSCH)."@de-DE , "Indique si l'objet est fait de matière combustible (VRAI) ou non (FAUX)."@fr-FR , "この部材が可燃性物質で作られているかどうかを示すブーリアン値。"@ja-JP , ""@en , "表示该构件是否由可燃材料制成。"@zh-CN ;
        IFC4-PSD:ifdguid          "1a431200d20811e1800000215ad4efdf" ;
        IFC4-PSD:name             "Combustible" ;
        IFC4-PSD:nameAlias        "是否可燃"@zh-CN , "Brennbares Material"@de-DE , "可燃性区分"@ja-JP , "Combustible"@en , "Combustible"@fr-FR ;
        IFC4-PSD:propertyType     [ a                  IFC4-PSD:TypePropertySingleValue ;
                                    IFC4-PSD:dataType  IFC4:IfcBoolean
                                  ] .

:Compartmentation  a        rdf:Property ;
        rdfs:seeAlso        :p4199df00d20811e1800000215ad4efdf ;
        rdfs:subPropertyOf  IFC4-PSD:Compartmentation .

:p49598380d20811e1800000215ad4efdf
        a                         IFC4-PSD:PropertyDef ;
        rdfs:comment              "Angle of the slab to the horizontal when used as a component for the roof (specified as 0 degrees or not asserted for cases where the slab is not used as a roof component).      \n\nThe shape information is provided in addition to the shape representation and the geometric parameters used within. In cases of inconsistency between the geometric parameters and the shape properties, provided in the attached property, the geometric parameters take precedence.  For geometry editing applications, like CAD: this value should be write-only." ;
        rdfs:label                "PitchAngle" ;
        IFC4-PSD:definition       "Angle of the slab to the horizontal when used as a component for the roof (specified as 0 degrees or not asserted for cases where the slab is not used as a roof component).      \n\nThe shape information is provided in addition to the shape representation and the geometric parameters used within. In cases of inconsistency between the geometric parameters and the shape properties, provided in the attached property, the geometric parameters take precedence.  For geometry editing applications, like CAD: this value should be write-only." ;
        IFC4-PSD:definitionAlias  "Angle de la dalle avec l'horizontale quand elle est utilisée comme un élément de la couverture (valeur 0 ou non définie lorsque la dalle ne participe pas à la couverture). Cette propriété  est donnée en complément de la représentation de la forme et des paramètres géométriques qui la déterminent. En cas d'incohérence entre ces paramètres géométriques et cette propriété, ce sont les paramètres géométriques qui priment. Les applications qui déterminent la géométrie comme les logiciels de CAO ne doivent pas autoriser la modification de cette propriété."@fr-FR , ""@en , "コンポーネントが屋根として使用される場合の、水平に対するスラブの角度（スラブが屋根として使用されない場合は、0度と指定されるか、定義されない）。\n\n形状情報は形状の表現として追加され、幾何学的なパラメータが使用される。幾何学的なパラメータと追加された形状プロパティが矛盾する場合、幾何学的なパラメータが優先される。CADのような、幾何学操作アプリケーションにとって、この値は、書き込み専用であるべきだ。"@ja-JP , "Neigungswinkel der Decke gegenüber der Horizontalen wenn es sich um eine Dachfläche handelt. Angabe 0 Grad definiert eine horizontale Fläche.\n\nDieser Parameter wird zusätzlich zur geometrischen Repräsentation bereitgestellt. Im Fall der Inkonsistenz zwischen dem Parameter und der Geometrie hat die geometrische Repräsention Priorität. Dieser Parameter ist für CAD Software write-only."@de-DE ;
        IFC4-PSD:ifdguid          "49598380d20811e1800000215ad4efdf" ;
        IFC4-PSD:name             "PitchAngle" ;
        IFC4-PSD:nameAlias        "Dachflächenneigung"@de-DE , "Pitch Angle"@en , "AngleInclinaison"@fr-FR , "勾配角度"@ja-JP ;
        IFC4-PSD:propertyType     [ a                  IFC4-PSD:TypePropertySingleValue ;
                                    IFC4-PSD:dataType  IFC4:IfcPlaneAngleMeasure
                                  ] .

:Reference  a               rdf:Property ;
        rdfs:seeAlso        :pfaabe980d20711e1800000215ad4efdf ;
        rdfs:subPropertyOf  IFC4-PSD:Reference .

:LoadBearing  a             rdf:Property ;
        rdfs:seeAlso        :p3b0b6780d20811e1800000215ad4efdf ;
        rdfs:subPropertyOf  IFC4-PSD:LoadBearing .

:p3b0b6780d20811e1800000215ad4efdf
        a                         IFC4-PSD:PropertyDef ;
        rdfs:comment              "Indicates whether the object is intended to carry loads (TRUE) or not (FALSE)." ;
        rdfs:label                "LoadBearing" ;
        IFC4-PSD:definition       "Indicates whether the object is intended to carry loads (TRUE) or not (FALSE)." ;
        IFC4-PSD:definitionAlias  "荷重に関係している部材かどうかを示すブーリアン値。"@ja-JP , "表示该对象是否需要承重。"@zh-CN , "Indique si l'objet est censé porter des charges (VRAI) ou non (FAUX)."@fr-FR , "Angabe, ob dieses Bauteil tragend ist (JA) oder nichttragend (NEIN)"@de-DE , ""@en ;
        IFC4-PSD:ifdguid          "3b0b6780d20811e1800000215ad4efdf" ;
        IFC4-PSD:name             "LoadBearing" ;
        IFC4-PSD:nameAlias        "耐力部材"@ja-JP , "Porteur"@fr-FR , "Tragendes Bauteil"@de-DE , "Load Bearing"@en , "是否承重"@zh-CN ;
        IFC4-PSD:propertyType     [ a                  IFC4-PSD:TypePropertySingleValue ;
                                    IFC4-PSD:dataType  IFC4:IfcBoolean
                                  ] .

:p2e870f00d20811e1800000215ad4efdf
        a                         IFC4-PSD:PropertyDef ;
        rdfs:comment              "Thermal transmittance coefficient (U-Value) of a material. Here the total thermal transmittance coefficient through the slab (including all materials)." ;
        rdfs:label                "ThermalTransmittance" ;
        IFC4-PSD:definition       "Thermal transmittance coefficient (U-Value) of a material. Here the total thermal transmittance coefficient through the slab (including all materials)." ;
        IFC4-PSD:definitionAlias  ""@en , "材料的导热系数（U值）。\n表示穿过该板的整体导热系数（包括所有材料）。"@zh-CN , "熱貫流率U値。ここではスラブを通した熱移動の方向における全体の熱還流率を示す。"@ja-JP , "Coefficient de transmission thermique surfacique (U). C'est le coefficient global de transmission thermique à travers la dalle (tous matériaux inclus)."@fr-FR , "Wärmedurchgangskoeffizient (U-Wert) der Materialschichten.\nHier der Gesamtwärmedurchgangskoeffizient der Decke (für alle Schichten)."@de-DE ;
        IFC4-PSD:ifdguid          "2e870f00d20811e1800000215ad4efdf" ;
        IFC4-PSD:name             "ThermalTransmittance" ;
        IFC4-PSD:nameAlias        "TransmissionThermique"@fr-FR , "熱貫流率"@ja-JP , "Thermal Transmittance"@en , "U-Wert"@de-DE , "导热系数"@zh-CN ;
        IFC4-PSD:propertyType     [ a                  IFC4-PSD:TypePropertySingleValue ;
                                    IFC4-PSD:dataType  IFC4:IfcThermalTransmittanceMeasure
                                  ] .

:p00093400d20811e1800000215ad4efdf
        a                         IFC4-PSD:PropertyDef ;
        rdfs:comment              "Status of the element, predominately used in renovation or retrofitting projects. The status can be assigned to as \"New\" - element designed as new addition, \"Existing\" - element exists and remains, \"Demolish\" - element existed but is to be demolished,  \"Temporary\" - element will exists only temporary (like a temporary support structure)." ;
        rdfs:label                "Status" ;
        IFC4-PSD:definition       "Status of the element, predominately used in renovation or retrofitting projects. The status can be assigned to as \"New\" - element designed as new addition, \"Existing\" - element exists and remains, \"Demolish\" - element existed but is to be demolished,  \"Temporary\" - element will exists only temporary (like a temporary support structure)." ;
        IFC4-PSD:definitionAlias  "要素（主にリノベーションまたは改修プロジェクトにおいて）の状態。 状態は、「新規(New)」－新しく追加される要素。「既存」－要素は存在し、かつ残りもの。「破壊」－要素は存在したが、廃棄されるもの。「一時的」－一時的に存在する要素（一時的にサポートしている構造のようなもの）。"@ja-JP , "Statut de l'élément, principalement utilisé dans les projets de rénovation et de réhabilitation. Le statut a pour valeur NOUVEAU pour un nouvel élément, EXISTANT pour un élément existant qui est conservé, DEMOLI pour un élément existant à démolir et TEMPORAIRE pour un élément temporaire (comme une structure support provisoire)."@fr-FR , "Status bzw. Phase des Bauteils insbesondere beim Bauen im Bestand. \"Neu\" (new) neues Bauteil als Ergänzung, \"Bestand\" (existing) bestehendes Bauteil, dass erhalten bleibt, \"Abbruch\" (demolish) Bauteil, das abgebrochen wird, \"Temporär\" (temporary) Bauteil und andere Bauelemente, die vorübergehend eingebaut werden (wie Abstützungen, etc.)"@de-DE , ""@en ;
        IFC4-PSD:ifdguid          "00093400d20811e1800000215ad4efdf" ;
        IFC4-PSD:name             "Status" ;
        IFC4-PSD:nameAlias        "Status"@en , "Status"@de-DE , "Statut"@fr-FR , "状態"@ja-JP ;
        IFC4-PSD:propertyType     [ a                  IFC4-PSD:TypePropertyEnumeratedValue ;
                                    IFC4-PSD:enumItem  "NEW" , "EXISTING" , "DEMOLISH" , "TEMPORARY" , "OTHER" , "NOTKNOWN" , "UNSET"
                                  ] .

:IsExternal  a              rdf:Property ;
        rdfs:seeAlso        :p347cf000d20811e1800000215ad4efdf ;
        rdfs:subPropertyOf  IFC4-PSD:IsExternal .

:FireRating  a              rdf:Property ;
        rdfs:seeAlso        :p13b49a80d20811e1800000215ad4efdf ;
        rdfs:subPropertyOf  IFC4-PSD:FireRating .

:p13b49a80d20811e1800000215ad4efdf
        a                         IFC4-PSD:PropertyDef ;
        rdfs:comment              "Fire rating for this object. It is given according to the national fire safety classification." ;
        rdfs:label                "FireRating" ;
        IFC4-PSD:definition       "Fire rating for this object. It is given according to the national fire safety classification." ;
        IFC4-PSD:definitionAlias  "该构件的防火等级。\n该属性的依据为国家防火安全分级。"@zh-CN , "Classement au feu de l'élément donné selon la classification nationale de sécurité incendie."@fr-FR , "Feuerwiderstandasklasse gemäß der nationalen oder regionalen Brandschutzverordnung."@de-DE , ""@en , "主要な耐火等級。関連する建築基準法、消防法などの国家基準を参照。"@ja-JP ;
        IFC4-PSD:ifdguid          "13b49a80d20811e1800000215ad4efdf" ;
        IFC4-PSD:name             "FireRating" ;
        IFC4-PSD:nameAlias        "ResistanceAuFeu"@fr-FR , "耐火等級"@ja-JP , "Fire Rating"@en , "Feuerwiderstandsklasse"@de-DE , "防火等级"@zh-CN ;
        IFC4-PSD:propertyType     [ a                  IFC4-PSD:TypePropertySingleValue ;
                                    IFC4-PSD:dataType  IFC4:IfcLabel
                                  ] .

:p4199df00d20811e1800000215ad4efdf
        a                         IFC4-PSD:PropertyDef ;
        rdfs:comment              "Indication whether the object is designed to serve as a fire compartmentation (TRUE) or not (FALSE)." ;
        rdfs:label                "Compartmentation" ;
        IFC4-PSD:definition       "Indication whether the object is designed to serve as a fire compartmentation (TRUE) or not (FALSE)." ;
        IFC4-PSD:definitionAlias  "部材が防火区画として用いられるかどうかを示すブーリアン値（TRUE or False)。"@ja-JP , "Angabe, ob dieses Bauteil einen Brandabschnitt begrenzt (WAHR), oder nicht (FALSCH)."@de-DE , ""@en , "Indique si l'objet est conçu  pour assurer un compartimentage contre l'incendie (VRAI) ou non (FAUX)."@fr-FR ;
        IFC4-PSD:ifdguid          "4199df00d20811e1800000215ad4efdf" ;
        IFC4-PSD:name             "Compartmentation" ;
        IFC4-PSD:nameAlias        "防火区画"@ja-JP , "Compartimentage"@fr-FR , "Compartmentation"@en , "Brandabschnittsdefinierendes Bauteil"@de-DE ;
        IFC4-PSD:propertyType     [ a                  IFC4-PSD:TypePropertySingleValue ;
                                    IFC4-PSD:dataType  IFC4:IfcBoolean
                                  ] .

:p0d262300d20811e1800000215ad4efdf
        a                         IFC4-PSD:PropertyDef ;
        rdfs:comment              "Acoustic rating for this object.\nIt is provided according to the national building code. It indicates the sound transmission resistance of this object by an index ratio (instead of providing full sound absorbtion values)." ;
        rdfs:label                "AcousticRating" ;
        IFC4-PSD:definition       "Acoustic rating for this object.\nIt is provided according to the national building code. It indicates the sound transmission resistance of this object by an index ratio (instead of providing full sound absorbtion values)." ;
        IFC4-PSD:definitionAlias  "Schallschutzklasse gemäß der nationalen oder regionalen Schallschutzverordnung."@de-DE , ""@en , "该构件的隔音等级。\n该属性的依据为国家建筑规范。为表示该构件隔音效果的比率（而不是完全吸收声音的值）。"@zh-CN , "遮音等級情報。関連する建築基準法を参照。"@ja-JP , "Classement acoustique de cet objet. Donné selon le Code National du Bâtiment. Il indique la résistance à la transmission du son de cet objet par une valeur de référence (au lieu de fournir les valeurs totales d'absorption du son)."@fr-FR ;
        IFC4-PSD:ifdguid          "0d262300d20811e1800000215ad4efdf" ;
        IFC4-PSD:name             "AcousticRating" ;
        IFC4-PSD:nameAlias        "隔音等级"@zh-CN , "遮音等級"@ja-JP , "Acoustic Rating"@en , "IsolationAcoustique"@fr-FR , "Schallschutzklasse"@de-DE ;
        IFC4-PSD:propertyType     [ a                  IFC4-PSD:TypePropertySingleValue ;
                                    IFC4-PSD:dataType  IFC4:IfcLabel
                                  ] .

:pfaabe980d20711e1800000215ad4efdf
        a                         IFC4-PSD:PropertyDef ;
        rdfs:comment              "Reference ID for this specified type in this project (e.g. type 'A-1'), Also referred to as \"construction type\". It should be provided as an alternative to the name of the \"object type\", if the software does not support object types." ;
        rdfs:label                "Reference" ;
        IFC4-PSD:definition       "Reference ID for this specified type in this project (e.g. type 'A-1'), Also referred to as \"construction type\". It should be provided as an alternative to the name of the \"object type\", if the software does not support object types." ;
        IFC4-PSD:definitionAlias  "若未采用已知的分类系统，则该属性为该项目中该类型构件的参考编号（例如，类型A-1）。"@zh-CN , "Bezeichnung zur Zusammenfassung gleichartiger Bauteile zu einem Bauteiltyp (auch Konstruktionstyp genannt). Alternativ zum Namen des \"Typobjekts\", insbesondere wenn die Software keine Typen unterstützt."@de-DE , ""@en , "このプロジェクトにおける参照記号(例：A-1)。分類コードではなく内部で使用されるプロジェクトタイプとして使用されるもの。"@ja-JP , "Référence à l'identifiant d'un type spécifié dans le contexte du projet (exemple : \"type A1\") pour désigner un \"type de construction\". Une alternative au nom d'un objet type lorsque les objets types ne sont pas gérés par le logiciel."@fr-FR ;
        IFC4-PSD:ifdguid          "faabe980d20711e1800000215ad4efdf" ;
        IFC4-PSD:name             "Reference" ;
        IFC4-PSD:nameAlias        "参照記号"@ja-JP , "参考号"@zh-CN , "Reference"@en , "Reference"@fr-FR , "Bauteiltyp"@de-DE ;
        IFC4-PSD:propertyType     [ a                  IFC4-PSD:TypePropertySingleValue ;
                                    IFC4-PSD:dataType  IFC4:IfcIdentifier
                                  ] .

:PitchAngle  a              rdf:Property ;
        rdfs:seeAlso        :p49598380d20811e1800000215ad4efdf ;
        rdfs:subPropertyOf  IFC4-PSD:PitchAngle .

:Combustible  a             rdf:Property ;
        rdfs:seeAlso        :p1a431200d20811e1800000215ad4efdf ;
        rdfs:subPropertyOf  IFC4-PSD:Combustible .

:SurfaceSpreadOfFlame
        a                   rdf:Property ;
        rdfs:seeAlso        :p2038f300d20811e1800000215ad4efdf ;
        rdfs:subPropertyOf  IFC4-PSD:SurfaceSpreadOfFlame .

:ThermalTransmittance
        a                   rdf:Property ;
        rdfs:seeAlso        :p2e870f00d20811e1800000215ad4efdf ;
        rdfs:subPropertyOf  IFC4-PSD:ThermalTransmittance .

:AcousticRating  a          rdf:Property ;
        rdfs:seeAlso        :p0d262300d20811e1800000215ad4efdf ;
        rdfs:subPropertyOf  IFC4-PSD:AcousticRating .

<https://www.linkedbuildingdata.net/IFC4-PSD/Pset_SlabCommon>
        a                owl:Ontology ;
        owl:imports      <http://lbd.arch.rwth-aachen.de/ifcOWL/IFC4-PSD> ;
        owl:versionInfo  "Created with BIM-Bots PSD Repository" .

:Pset_SlabCommon  a                   IFC4-PSD:PropertySetDef ;
        rdfs:comment                  "Properties common to the definition of all occurrences of IfcSlab. Note: Properties for PitchAngle added in IFC 2x3" ;
        rdfs:label                    "Pset_SlabCommon" ;
        IFC4-PSD:applicableClass      IFC4:IfcSlab ;
        IFC4-PSD:applicableTypeValue  "IfcSlab" ;
        IFC4-PSD:definition           "Properties common to the definition of all occurrences of IfcSlab. Note: Properties for PitchAngle added in IFC 2x3" ;
        IFC4-PSD:definitionAlias      "IfcSlab(スラブ)オブジェクトに関する共通プロパティセット定義。"@ja-JP , "Définition de l'IAI : propriétés communes à la définition de toutes les instances de la classe IfcSlab. Nota : la propriété AngleInclinaison a été introduite depuis la version 2x3."@fr-FR , ""@en , "所有IfcSlab实例的定义中通用的属性。\n注：PitchAngle属性为IFC 2x3 新添。"@zh-CN ;
        IFC4-PSD:ifcVersion           [ a                 IFC4-PSD:IfcVersion ;
                                        IFC4-PSD:version  "IFC4"
                                      ] ;
        IFC4-PSD:name                 "Pset_SlabCommon" ;
        IFC4-PSD:propertyDef          :p3b0b6780d20811e1800000215ad4efdf , :p13b49a80d20811e1800000215ad4efdf , :p347cf000d20811e1800000215ad4efdf , :p1a431200d20811e1800000215ad4efdf , :pfaabe980d20711e1800000215ad4efdf , :p4199df00d20811e1800000215ad4efdf , :p2e870f00d20811e1800000215ad4efdf , :p0d262300d20811e1800000215ad4efdf , :p49598380d20811e1800000215ad4efdf , :p00093400d20811e1800000215ad4efdf , :p2038f300d20811e1800000215ad4efdf .

:p2038f300d20811e1800000215ad4efdf
        a                         IFC4-PSD:PropertyDef ;
        rdfs:comment              "Indication on how the flames spread around the surface, It is given according to the national building code that governs the fire behaviour for materials." ;
        rdfs:label                "SurfaceSpreadOfFlame" ;
        IFC4-PSD:definition       "Indication on how the flames spread around the surface, It is given according to the national building code that governs the fire behaviour for materials." ;
        IFC4-PSD:definitionAlias  ""@en , "Indique comment les flammes se propagent sur une surface. Indication donnée selon le Code National du Bâtiment régissant le comportement au feu des matériaux."@fr-FR , "Beschreibung des Brandverhaltens des Bauteils gemäß der nationalen oder regionalen  Brandschutzverordnung."@de-DE , "炎がどのように材料の表面を広がるかという指標。材料の炎に対する振る舞いについての国家建築規則に従って提供される。"@ja-JP ;
        IFC4-PSD:ifdguid          "2038f300d20811e1800000215ad4efdf" ;
        IFC4-PSD:name             "SurfaceSpreadOfFlame" ;
        IFC4-PSD:nameAlias        "Brandverhalten"@de-DE , "火炎伝播性"@ja-JP , "SurfacePropagationFlamme"@fr-FR , "Surface Spread Of Flame"@en ;
        IFC4-PSD:propertyType     [ a                  IFC4-PSD:TypePropertySingleValue ;
                                    IFC4-PSD:dataType  IFC4:IfcLabel
                                  ] .

:p347cf000d20811e1800000215ad4efdf
        a                         IFC4-PSD:PropertyDef ;
        rdfs:comment              "Indication whether the element is designed for use in the exterior (TRUE) or not (FALSE). If (TRUE) it is an external element and faces the outside of the building." ;
        rdfs:label                "IsExternal" ;
        IFC4-PSD:definition       "Indication whether the element is designed for use in the exterior (TRUE) or not (FALSE). If (TRUE) it is an external element and faces the outside of the building." ;
        IFC4-PSD:definitionAlias  "Angabe, ob dieses Bauteil ein Aussenbauteil ist (JA) oder ein Innenbauteil (NEIN). Als Aussenbauteil grenzt es an den Aussenraum (oder Erdreich, oder Wasser)."@de-DE , "Indique si l'élément est conçu pour être utilisé à l'extérieur (VRAI) ou non (FAUX). Si VRAI, c'est un élément extérieur qui donne sur l'extérieur du bâtiment."@fr-FR , ""@en , "外部の部材かどうかを示すブーリアン値。もしTRUEの場合、外部の部材で建物の外側に面している。"@ja-JP , "表示该构件是否设计为外部构件。若是，则该构件为外部构件，朝向建筑物的外侧。"@zh-CN ;
        IFC4-PSD:ifdguid          "347cf000d20811e1800000215ad4efdf" ;
        IFC4-PSD:name             "IsExternal" ;
        IFC4-PSD:nameAlias        "是否外部构件"@zh-CN , "Is External"@en , "外部区分"@ja-JP , "EstExterieur"@fr-FR , "Außenbauteil"@de-DE ;
        IFC4-PSD:propertyType     [ a                  IFC4-PSD:TypePropertySingleValue ;
                                    IFC4-PSD:dataType  IFC4:IfcBoolean
                                  ] .

:Status  a                  rdf:Property ;
        rdfs:seeAlso        :p00093400d20811e1800000215ad4efdf ;
        rdfs:subPropertyOf  IFC4-PSD:Status .
