@prefix :      <https://www.linkedbuildingdata.net/IFC4-PSD/Pset_ProtectiveDeviceTrippingFunctionLCurve#> .
@prefix IFC4-PSD: <https://www.linkedbuildingdata.net/IFC4-PSD#> .
@prefix rdf:   <http://www.w3.org/1999/02/22-rdf-syntax-ns#> .
@prefix owl:   <http://www.w3.org/2002/07/owl#> .
@prefix rdfs:  <http://www.w3.org/2000/01/rdf-schema#> .
@prefix IFC4:  <http://lbd.arch.rwth-aachen.de/ifcOWL/IFC4#> .

:LowerTime2  a              rdf:Property ;
        rdfs:seeAlso        :p39877280d1fb11e1800000215ad4efdf ;
        rdfs:subPropertyOf  IFC4-PSD:LowerTime2 .

:LowerTime1  a              rdf:Property ;
        rdfs:seeAlso        :p34c2be80d1fb11e1800000215ad4efdf ;
        rdfs:subPropertyOf  IFC4-PSD:LowerTime1 .

:p16f55980d1fb11e1800000215ad4efdf
        a                         IFC4-PSD:PropertyDef ;
        rdfs:comment              "The current in [x In], indicating the upper current limit of the upper time/current curve of the I2t part of the L-function." ;
        rdfs:label                "UpperCurrent2" ;
        IFC4-PSD:definition       "The current in [x In], indicating the upper current limit of the upper time/current curve of the I2t part of the L-function." ;
        IFC4-PSD:definitionAlias  ""@en , "[x In]の電流,電流をトリップするL関数のI2t部分は、上限時間/特性曲線よりも大きい電流を示す。"@ja-JP , "[x In] 전류 전류를 여행하는 L 함수 I2t 부분은 제한 시간 / 특성 곡선보다 큰 전류를 보여준다."@ko-KR ;
        IFC4-PSD:ifdguid          "16f55980d1fb11e1800000215ad4efdf" ;
        IFC4-PSD:name             "UpperCurrent2" ;
        IFC4-PSD:nameAlias        "上電流2"@ja-JP , "Upper Current2"@en , "상전류2"@ko-KR ;
        IFC4-PSD:propertyType     [ a                  IFC4-PSD:TypePropertySingleValue ;
                                    IFC4-PSD:dataType  IFC4:IfcElectricCurrentMeasure
                                  ] .

:UpperTime2  a              rdf:Property ;
        rdfs:seeAlso        :p21afee80d1fb11e1800000215ad4efdf ;
        rdfs:subPropertyOf  IFC4-PSD:UpperTime2 .

:p34c2be80d1fb11e1800000215ad4efdf
        a                         IFC4-PSD:PropertyDef ;
        rdfs:comment              "The time in [s], indicating that tripping times of the lower time/current curve lower than LowerTime1 is determined by the I2t part of the L-function." ;
        rdfs:label                "LowerTime1" ;
        IFC4-PSD:definition       "The time in [s], indicating that tripping times of the lower time/current curve lower than LowerTime1 is determined by the I2t part of the L-function." ;
        IFC4-PSD:definitionAlias  "[s] 시간 아래 시간보다 낮은 특성 곡선의 트립 시간은 L-함수의 I2t 부분에 의해 결정된다."@ko-KR , "[s]の時間,下時間より低い特性曲線のトリップ時間は、L-関数ののI2t部分によって決定される。"@ja-JP , ""@en ;
        IFC4-PSD:ifdguid          "34c2be80d1fb11e1800000215ad4efdf" ;
        IFC4-PSD:name             "LowerTime1" ;
        IFC4-PSD:nameAlias        "Lower Time1"@en , "하 시간 1"@ko-KR , "下時間1"@ja-JP ;
        IFC4-PSD:propertyType     [ a                  IFC4-PSD:TypePropertySingleValue ;
                                    IFC4-PSD:dataType  IFC4:IfcTimeMeasure
                                  ] .

:UpperTime1  a              rdf:Property ;
        rdfs:seeAlso        :p1c52a400d1fb11e1800000215ad4efdf ;
        rdfs:subPropertyOf  IFC4-PSD:UpperTime1 .

:p11980f00d1fb11e1800000215ad4efdf
        a                         IFC4-PSD:PropertyDef ;
        rdfs:comment              "The current in [x In], indicating that for currents larger than UpperCurrent1 the I2t part of the L-function will trip the current." ;
        rdfs:label                "UpperCurrent1" ;
        IFC4-PSD:definition       "The current in [x In], indicating that for currents larger than UpperCurrent1 the I2t part of the L-function will trip the current." ;
        IFC4-PSD:definitionAlias  ""@en , "x In] 전류 전류를 여행하는 L 함수 I2t 부분은 최대 전류 1보다 큰 전류를 보여준다."@ko-KR , "[x In]の電流,電流をトリップするL関数のI2t部分は、上限電流1よりも大きい電流を示す。"@ja-JP ;
        IFC4-PSD:ifdguid          "11980f00d1fb11e1800000215ad4efdf" ;
        IFC4-PSD:name             "UpperCurrent1" ;
        IFC4-PSD:nameAlias        "上電流1"@ja-JP , "Upper Current1"@en , "상전류1"@ko-KR ;
        IFC4-PSD:propertyType     [ a                  IFC4-PSD:TypePropertySingleValue ;
                                    IFC4-PSD:dataType  IFC4:IfcElectricCurrentMeasure
                                  ] .

:p2eccdd80d1fb11e1800000215ad4efdf
        a                         IFC4-PSD:PropertyDef ;
        rdfs:comment              "The current in [x In], indicating the upper current limit of the lower time/current curve of the I2t part of the L-function." ;
        rdfs:label                "LowerCurrent2" ;
        IFC4-PSD:definition       "The current in [x In], indicating the upper current limit of the lower time/current curve of the I2t part of the L-function." ;
        IFC4-PSD:definitionAlias  "[x In]の電流,電流をトリップするL関数のI2t部分は、特性曲線よりも小さい電流を示す。"@ja-JP , ""@en , "x In] 전류 전류를 여행하는 L 함수 I2t 부분은 곡선보다 작은 전류를 보여준다."@ko-KR ;
        IFC4-PSD:ifdguid          "2eccdd80d1fb11e1800000215ad4efdf" ;
        IFC4-PSD:name             "LowerCurrent2" ;
        IFC4-PSD:nameAlias        "下電流2"@ja-JP , "하전류 2"@ko-KR , "Lower Current2"@en ;
        IFC4-PSD:propertyType     [ a                  IFC4-PSD:TypePropertySingleValue ;
                                    IFC4-PSD:dataType  IFC4:IfcElectricCurrentMeasure
                                  ] .

:IsSelectable  a            rdf:Property ;
        rdfs:seeAlso        :p0a710100d1fb11e1800000215ad4efdf ;
        rdfs:subPropertyOf  IFC4-PSD:IsSelectable .

:UpperCurrent2  a           rdf:Property ;
        rdfs:seeAlso        :p16f55980d1fb11e1800000215ad4efdf ;
        rdfs:subPropertyOf  IFC4-PSD:UpperCurrent2 .

:p0a710100d1fb11e1800000215ad4efdf
        a                         IFC4-PSD:PropertyDef ;
        rdfs:comment              "Indication whether the L-function can be switched off or not." ;
        rdfs:label                "IsSelectable" ;
        IFC4-PSD:definition       "Indication whether the L-function can be switched off or not." ;
        IFC4-PSD:definitionAlias  "장치의 \"ON-OFF\"상태를 전기적으로 표시가 교체 가능합니까?"@ko-KR , "装置の “ON-OFF”状態を電気的表示が切り替え可能かどうか。"@ja-JP , ""@en ;
        IFC4-PSD:ifdguid          "0a710100d1fb11e1800000215ad4efdf" ;
        IFC4-PSD:name             "IsSelectable" ;
        IFC4-PSD:nameAlias        "Is Selectable"@en , "切り替え"@ja-JP , "전환"@ko-KR ;
        IFC4-PSD:propertyType     [ a                  IFC4-PSD:TypePropertySingleValue ;
                                    IFC4-PSD:dataType  IFC4:IfcBoolean
                                  ] .

:Pset_ProtectiveDeviceTrippingFunctionLCurve
        a                             IFC4-PSD:PropertySetDef ;
        rdfs:comment                  "Tripping functions are applied to electronic tripping units (i.e. tripping units having type property sets for electronic tripping defined). They are not applied to thermal, thermal magnetic or RCD tripping units.\nThis property set represent the long time protection (L-curve) of an electronic protection device" ;
        rdfs:label                    "Pset_ProtectiveDeviceTrippingFunctionLCurve" ;
        IFC4-PSD:applicableClass      IFC4:IfcProtectiveDeviceTrippingUnit ;
        IFC4-PSD:applicableTypeValue  "IfcProtectiveDeviceTrippingUnit" ;
        IFC4-PSD:definition           "Tripping functions are applied to electronic tripping units (i.e. tripping units having type property sets for electronic tripping defined). They are not applied to thermal, thermal magnetic or RCD tripping units.\nThis property set represent the long time protection (L-curve) of an electronic protection device" ;
        IFC4-PSD:definitionAlias      "トリッピング関数は、電子トリッピング装置に適用される。\n（例えば、トリッピング装置は、電子トリッピング定義されたプロパティセットタイプを持っている）\nこれらは、熱,熱電磁,RCDトリッピング装置に適用されない。\nこのプロパティセットは、電子保護装置の遅延短絡保護(L-curve)を表す。"@ja-JP , ""@en ;
        IFC4-PSD:ifcVersion           [ a                 IFC4-PSD:IfcVersion ;
                                        IFC4-PSD:version  "IFC4"
                                      ] ;
        IFC4-PSD:name                 "Pset_ProtectiveDeviceTrippingFunctionLCurve" ;
        IFC4-PSD:propertyDef          :p34c2be80d1fb11e1800000215ad4efdf , :p2eccdd80d1fb11e1800000215ad4efdf , :p0a710100d1fb11e1800000215ad4efdf , :p27a5cf80d1fb11e1800000215ad4efdf , :p39877280d1fb11e1800000215ad4efdf , :p11980f00d1fb11e1800000215ad4efdf , :p1c52a400d1fb11e1800000215ad4efdf , :p16f55980d1fb11e1800000215ad4efdf , :p21afee80d1fb11e1800000215ad4efdf .

:LowerCurrent2  a           rdf:Property ;
        rdfs:seeAlso        :p2eccdd80d1fb11e1800000215ad4efdf ;
        rdfs:subPropertyOf  IFC4-PSD:LowerCurrent2 .

:UpperCurrent1  a           rdf:Property ;
        rdfs:seeAlso        :p11980f00d1fb11e1800000215ad4efdf ;
        rdfs:subPropertyOf  IFC4-PSD:UpperCurrent1 .

:p39877280d1fb11e1800000215ad4efdf
        a                         IFC4-PSD:PropertyDef ;
        rdfs:comment              "The time in [s], indicating the tripping times of the upper time/current curve at the LowerCurrent2." ;
        rdfs:label                "LowerTime2" ;
        IFC4-PSD:definition       "The time in [s], indicating the tripping times of the upper time/current curve at the LowerCurrent2." ;
        IFC4-PSD:definitionAlias  "[s] 시간, 아래 전류 2보다 하부의 특성 곡선의 트립 시간을 보여준다."@ko-KR , "[s]の時間,下電流2より下部の特性曲線のトリップ時間を示す。"@ja-JP , ""@en ;
        IFC4-PSD:ifdguid          "39877280d1fb11e1800000215ad4efdf" ;
        IFC4-PSD:name             "LowerTime2" ;
        IFC4-PSD:nameAlias        "하 시간 2"@ko-KR , "Lower Time2"@en , "下時間2"@ja-JP ;
        IFC4-PSD:propertyType     [ a                  IFC4-PSD:TypePropertySingleValue ;
                                    IFC4-PSD:dataType  IFC4:IfcTimeMeasure
                                  ] .

:p21afee80d1fb11e1800000215ad4efdf
        a                         IFC4-PSD:PropertyDef ;
        rdfs:comment              "The time in [s], indicating the tripping times of the upper time/current curve at the UpperCurrent2." ;
        rdfs:label                "UpperTime2" ;
        IFC4-PSD:definition       "The time in [s], indicating the tripping times of the upper time/current curve at the UpperCurrent2." ;
        IFC4-PSD:definitionAlias  "[s]の時間,上電流2より上部の特性曲線のトリップ時間を示す"@ja-JP , "[s]의 시간에 전류 2보다 상단의 특성 곡선의 트립 시간을 나타냄"@ko-KR , ""@en ;
        IFC4-PSD:ifdguid          "21afee80d1fb11e1800000215ad4efdf" ;
        IFC4-PSD:name             "UpperTime2" ;
        IFC4-PSD:nameAlias        "상시간2"@ko-KR , "上時間2"@ja-JP , "Upper Time2"@en ;
        IFC4-PSD:propertyType     [ a                  IFC4-PSD:TypePropertySingleValue ;
                                    IFC4-PSD:dataType  IFC4:IfcTimeMeasure
                                  ] .

:LowerCurrent1  a           rdf:Property ;
        rdfs:seeAlso        :p27a5cf80d1fb11e1800000215ad4efdf ;
        rdfs:subPropertyOf  IFC4-PSD:LowerCurrent1 .

:p1c52a400d1fb11e1800000215ad4efdf
        a                         IFC4-PSD:PropertyDef ;
        rdfs:comment              "The time in [s], indicating that tripping times of the upper time/current curve lower than UpperTime1 is determined by the I2t part of the L-function." ;
        rdfs:label                "UpperTime1" ;
        IFC4-PSD:definition       "The time in [s], indicating that tripping times of the upper time/current curve lower than UpperTime1 is determined by the I2t part of the L-function." ;
        IFC4-PSD:definitionAlias  "[s]의 시간에 시간 더 낮은 위 시간 / 특성 곡선의 트립 시간은 L-함수의 I2t 부분에 의해 결정된다"@ko-KR , "[s]の時間,上時間より低い上部の時間/特性曲線のトリップ時間は、L-関数ののI2t部分によって決定される。"@ja-JP , ""@en ;
        IFC4-PSD:ifdguid          "1c52a400d1fb11e1800000215ad4efdf" ;
        IFC4-PSD:name             "UpperTime1" ;
        IFC4-PSD:nameAlias        "Upper Time1"@en , "上時間1"@ja-JP , "상시간1"@ko-KR ;
        IFC4-PSD:propertyType     [ a                  IFC4-PSD:TypePropertySingleValue ;
                                    IFC4-PSD:dataType  IFC4:IfcTimeMeasure
                                  ] .

:p27a5cf80d1fb11e1800000215ad4efdf
        a                         IFC4-PSD:PropertyDef ;
        rdfs:comment              "The current in [x In], indicating that for currents smaller than LowerCurrent1 the I2t part of the L-function will not trip the current," ;
        rdfs:label                "LowerCurrent1" ;
        IFC4-PSD:definition       "The current in [x In], indicating that for currents smaller than LowerCurrent1 the I2t part of the L-function will not trip the current," ;
        IFC4-PSD:definitionAlias  ""@en , "[x In] 전류 전류를 여행하는 L 함수 I2t 부분은 아래 전류 1보다 작은 전류를 보여준다."@ko-KR , "[x In]の電流,電流をトリップするL関数のI2t部分は、下電流1よりも小さい電流を示す。"@ja-JP ;
        IFC4-PSD:ifdguid          "27a5cf80d1fb11e1800000215ad4efdf" ;
        IFC4-PSD:name             "LowerCurrent1" ;
        IFC4-PSD:nameAlias        "하전류 1"@ko-KR , "Lower Current1"@en , "下電流1"@ja-JP ;
        IFC4-PSD:propertyType     [ a                  IFC4-PSD:TypePropertySingleValue ;
                                    IFC4-PSD:dataType  IFC4:IfcElectricCurrentMeasure
                                  ] .

<https://www.linkedbuildingdata.net/IFC4-PSD/Pset_ProtectiveDeviceTrippingFunctionLCurve>
        a                owl:Ontology ;
        owl:imports      <http://lbd.arch.rwth-aachen.de/ifcOWL/IFC4-PSD> ;
        owl:versionInfo  "Created with BIM-Bots PSD Repository" .
