@prefix :      <https://www.linkedbuildingdata.net/IFC4-PSD/Pset_ProtectiveDeviceTrippingFunctionGCurve#> .
@prefix IFC4-PSD: <https://www.linkedbuildingdata.net/IFC4-PSD#> .
@prefix rdf:   <http://www.w3.org/1999/02/22-rdf-syntax-ns#> .
@prefix owl:   <http://www.w3.org/2002/07/owl#> .
@prefix rdfs:  <http://www.w3.org/2000/01/rdf-schema#> .
@prefix IFC4:  <http://lbd.arch.rwth-aachen.de/ifcOWL/IFC4#> .

:Pset_ProtectiveDeviceTrippingFunctionGCurve
        a                             IFC4-PSD:PropertySetDef ;
        rdfs:comment                  "Tripping functions are applied to electronic tripping units (i.e. tripping units having type property sets for electronic tripping defined). They are not applied to thermal, thermal magnetic or RCD tripping units.\nThis property set represent the ground fault protection (G-curve) of an electronic protection device" ;
        rdfs:label                    "Pset_ProtectiveDeviceTrippingFunctionGCurve" ;
        IFC4-PSD:applicableClass      IFC4:IfcProtectiveDeviceTrippingUnit ;
        IFC4-PSD:applicableTypeValue  "IfcProtectiveDeviceTrippingUnit" ;
        IFC4-PSD:definition           "Tripping functions are applied to electronic tripping units (i.e. tripping units having type property sets for electronic tripping defined). They are not applied to thermal, thermal magnetic or RCD tripping units.\nThis property set represent the ground fault protection (G-curve) of an electronic protection device" ;
        IFC4-PSD:definitionAlias      "トリッピング関数は、電子トリッピング装置に適用される。\n（例えば、トリッピング装置は、電子トリッピング定義されたプロパティセットタイプを持っている）\nこれらは、熱,熱電磁,RCDトリッピング装置に適用されない。\nこのプロパティセットは、電子保護装置(G-curve)の地絡保護を表す。"@ja-JP , ""@en ;
        IFC4-PSD:ifcVersion           [ a                 IFC4-PSD:IfcVersion ;
                                        IFC4-PSD:version  "IFC4"
                                      ] ;
        IFC4-PSD:name                 "Pset_ProtectiveDeviceTrippingFunctionGCurve" ;
        IFC4-PSD:propertyDef          :p51122b80d1fa11e1800000215ad4efdf , :p96cef400d1fa11e1800000215ad4efdf , :p6d15cd00d1fa11e1800000215ad4efdf , :p8ae33200d1fa11e1800000215ad4efdf , :p84ed5100d1fa11e1800000215ad4efdf , :p5bccc080d1fa11e1800000215ad4efdf , :p9171a980d1fa11e1800000215ad4efdf , :p671fec00d1fa11e1800000215ad4efdf , :p57080c80d1fa11e1800000215ad4efdf , :p73a44480d1fa11e1800000215ad4efdf , :pa2221f80d1fa11e1800000215ad4efdf , :p7a32bc00d1fa11e1800000215ad4efdf , :p9c2c3e80d1fa11e1800000215ad4efdf , :p61c2a180d1fa11e1800000215ad4efdf , :p4a83b400d1fa11e1800000215ad4efdf , :p80289d00d1fa11e1800000215ad4efdf , :p42c40f80d1fa11e1800000215ad4efdf .

:p80289d00d1fa11e1800000215ad4efdf
        a                         IFC4-PSD:PropertyDef ;
        rdfs:comment              "The current limit in [x In] limiting the application of TimeTolerance1, if any. If the value is set to 0, the value of the TimeTolerance1 is valid for the whole time/current-curve." ;
        rdfs:label                "TimeToleranceLimit1" ;
        IFC4-PSD:definition       "The current limit in [x In] limiting the application of TimeTolerance1, if any. If the value is set to 0, the value of the TimeTolerance1 is valid for the whole time/current-curve." ;
        IFC4-PSD:definitionAlias  "허용 시간 1를 제한하는 전류 제한. 값이 0이면 제한이 없다"@ko-KR , ""@en , "許容時間1を制限する電流制限値。\n値が0の場合は、制限はない。"@ja-JP ;
        IFC4-PSD:ifdguid          "80289d00d1fa11e1800000215ad4efdf" ;
        IFC4-PSD:name             "TimeToleranceLimit1" ;
        IFC4-PSD:nameAlias        "Time Tolerance Limit1"@en , "許容限界時間1"@ja-JP , "허용 한계시간1"@ko-KR ;
        IFC4-PSD:propertyType     [ a                  IFC4-PSD:TypePropertySingleValue ;
                                    IFC4-PSD:dataType  IFC4:IfcElectricCurrentMeasure
                                  ] .

:CurrentTolerance1  a       rdf:Property ;
        rdfs:seeAlso        :p61c2a180d1fa11e1800000215ad4efdf ;
        rdfs:subPropertyOf  IFC4-PSD:CurrentTolerance1 .

:p51122b80d1fa11e1800000215ad4efdf
        a                         IFC4-PSD:PropertyDef ;
        rdfs:comment              "An indication if the ground fault protection may be adjusted according to an external current coil or not." ;
        rdfs:label                "ExternalAdjusted" ;
        IFC4-PSD:definition       "An indication if the ground fault protection may be adjusted according to an external current coil or not." ;
        IFC4-PSD:definitionAlias  "外部調整が可能かどうか。"@ja-JP , ""@en , "외부 조정이 가능합니까?"@ko-KR ;
        IFC4-PSD:ifdguid          "51122b80d1fa11e1800000215ad4efdf" ;
        IFC4-PSD:name             "ExternalAdjusted" ;
        IFC4-PSD:nameAlias        "External Adjusted"@en , "외부조정"@ko-KR , "外部調整"@ja-JP ;
        IFC4-PSD:propertyType     [ a                  IFC4-PSD:TypePropertySingleValue ;
                                    IFC4-PSD:dataType  IFC4:IfcBoolean
                                  ] .

:p5bccc080d1fa11e1800000215ad4efdf
        a                         IFC4-PSD:PropertyDef ;
        rdfs:comment              "The release time in [s] for the initial tripping of the relevant part. This time indicates that for current lower than the indicated release current, the tripping time will be longer than the indicated release time. The value is given as a mean value." ;
        rdfs:label                "ReleaseTime" ;
        IFC4-PSD:definition       "The release time in [s] for the initial tripping of the relevant part. This time indicates that for current lower than the indicated release current, the tripping time will be longer than the indicated release time. The value is given as a mean value." ;
        IFC4-PSD:definitionAlias  ""@en , "関連する部分の初期トリップのための[s]が放出時間。\n このトリップ時間は、リリースの電流よりも低い電流の場合、指定された動作時間よりも長くなります。\n 値が平均値として与えられる。"@ja-JP , "관련 부분의 초기 여행을위한 [s]가 방출 시간.  이 트립 시간은 릴리스 전류보다 낮은 전류의 경우 지정된 동작 시간보다 길어집니다.  값을 평균으로 주어진다."@ko-KR ;
        IFC4-PSD:ifdguid          "5bccc080d1fa11e1800000215ad4efdf" ;
        IFC4-PSD:name             "ReleaseTime" ;
        IFC4-PSD:nameAlias        "放出時間"@ja-JP , "방출 시간"@ko-KR , "Release Time"@en ;
        IFC4-PSD:propertyType     [ a                  IFC4-PSD:TypePropertySingleValue ;
                                    IFC4-PSD:dataType  IFC4:IfcTimeMeasure
                                  ] .

:p61c2a180d1fa11e1800000215ad4efdf
        a                         IFC4-PSD:PropertyDef ;
        rdfs:comment              "The tolerance for the current of time/current-curve in [%]." ;
        rdfs:label                "CurrentTolerance1" ;
        IFC4-PSD:definition       "The tolerance for the current of time/current-curve in [%]." ;
        IFC4-PSD:definitionAlias  "時間/特性曲線の許容範囲を[％]で指定。"@ja-JP , ""@en , "시간 / 특성 곡선의 허용 범위를 [%]로 지정합니다."@ko-KR ;
        IFC4-PSD:ifdguid          "61c2a180d1fa11e1800000215ad4efdf" ;
        IFC4-PSD:name             "CurrentTolerance1" ;
        IFC4-PSD:nameAlias        "許容電流1"@ja-JP , "허용 전류1"@ko-KR , "Current Tolerance1"@en ;
        IFC4-PSD:propertyType     [ a                  IFC4-PSD:TypePropertySingleValue ;
                                    IFC4-PSD:dataType  IFC4:IfcPositiveRatioMeasure
                                  ] .

:ReleaseCurrentI2tEnd
        a                   rdf:Property ;
        rdfs:seeAlso        :p9c2c3e80d1fa11e1800000215ad4efdf ;
        rdfs:subPropertyOf  IFC4-PSD:ReleaseCurrentI2tEnd .

:ReleaseTimeI2tEnd  a       rdf:Property ;
        rdfs:seeAlso        :pa2221f80d1fa11e1800000215ad4efdf ;
        rdfs:subPropertyOf  IFC4-PSD:ReleaseTimeI2tEnd .

:p7a32bc00d1fa11e1800000215ad4efdf
        a                         IFC4-PSD:PropertyDef ;
        rdfs:comment              "The tolerance for the time of time/current-curve in [%]." ;
        rdfs:label                "TimeTolerance1" ;
        IFC4-PSD:definition       "The tolerance for the time of time/current-curve in [%]." ;
        IFC4-PSD:definitionAlias  ""@en , "[％]で時間/特性曲線の許容時間を設定"@ja-JP , "[%] 시간 / 특성 곡선의 허용 시간을 설정"@ko-KR ;
        IFC4-PSD:ifdguid          "7a32bc00d1fa11e1800000215ad4efdf" ;
        IFC4-PSD:name             "TimeTolerance1" ;
        IFC4-PSD:nameAlias        "허용 시간1"@ko-KR , "許容時間1"@ja-JP , "Time Tolerance1"@en ;
        IFC4-PSD:propertyType     [ a                  IFC4-PSD:TypePropertySingleValue ;
                                    IFC4-PSD:dataType  IFC4:IfcPositiveRatioMeasure
                                  ] .

:IsSelectable  a            rdf:Property ;
        rdfs:seeAlso        :p42c40f80d1fa11e1800000215ad4efdf ;
        rdfs:subPropertyOf  IFC4-PSD:IsSelectable .

:CurrentToleranceLimit1
        a                   rdf:Property ;
        rdfs:seeAlso        :p671fec00d1fa11e1800000215ad4efdf ;
        rdfs:subPropertyOf  IFC4-PSD:CurrentToleranceLimit1 .

:IsTimeTolerancePositiveOnly
        a                   rdf:Property ;
        rdfs:seeAlso        :p8ae33200d1fa11e1800000215ad4efdf ;
        rdfs:subPropertyOf  IFC4-PSD:IsTimeTolerancePositiveOnly .

:TimeToleranceLimit1  a     rdf:Property ;
        rdfs:seeAlso        :p80289d00d1fa11e1800000215ad4efdf ;
        rdfs:subPropertyOf  IFC4-PSD:TimeToleranceLimit1 .

:pa2221f80d1fa11e1800000215ad4efdf
        a                         IFC4-PSD:PropertyDef ;
        rdfs:comment              "The release time in [s] for the end point of the I2 tripping curve of the G-function, if any. The value of ReleaseTimeI2tEnd shall be lower than ReleaseTimeI2tStart." ;
        rdfs:label                "ReleaseTimeI2tEnd" ;
        IFC4-PSD:definition       "The release time in [s] for the end point of the I2 tripping curve of the G-function, if any. The value of ReleaseTimeI2tEnd shall be lower than ReleaseTimeI2tStart." ;
        IFC4-PSD:definitionAlias  ""@en , "G 함수 I2의 특성 곡선의 끝점에서 s를 방류 시간.  I2t 종료 방류 전류 시간이 I2t 시작 방류 시간보다 낮게해야한다"@ko-KR , "G関数のI2の特性曲線のエンドポイントの[s]を放流時間。 \n I2tの終了放流電流時間がI2tの開始放流時間よりも低くしなければならない。"@ja-JP ;
        IFC4-PSD:ifdguid          "a2221f80d1fa11e1800000215ad4efdf" ;
        IFC4-PSD:name             "ReleaseTimeI2tEnd" ;
        IFC4-PSD:nameAlias        "Release Time I2t End"@en , "I2t 종료 방류 시간"@ko-KR , "I2tの終了放流時間"@ja-JP ;
        IFC4-PSD:propertyType     [ a                  IFC4-PSD:TypePropertySingleValue ;
                                    IFC4-PSD:dataType  IFC4:IfcTimeMeasure
                                  ] .

:ReleaseTime  a             rdf:Property ;
        rdfs:seeAlso        :p5bccc080d1fa11e1800000215ad4efdf ;
        rdfs:subPropertyOf  IFC4-PSD:ReleaseTime .

:TimeTolerance2  a          rdf:Property ;
        rdfs:seeAlso        :p84ed5100d1fa11e1800000215ad4efdf ;
        rdfs:subPropertyOf  IFC4-PSD:TimeTolerance2 .

:p671fec00d1fa11e1800000215ad4efdf
        a                         IFC4-PSD:PropertyDef ;
        rdfs:comment              "The time limit in [s] limiting the application of CurrentTolerance1, if any. If the value is set to 0, the value of the CurrentTolerance1 is valid for the whole time/current-curve." ;
        rdfs:label                "CurrentToleranceLimit1" ;
        IFC4-PSD:definition       "The time limit in [s] limiting the application of CurrentTolerance1, if any. If the value is set to 0, the value of the CurrentTolerance1 is valid for the whole time/current-curve." ;
        IFC4-PSD:definitionAlias  ""@en , "許容電流1を制限する時間制限。\n値が0の場合は、制限はない。"@ja-JP , "허용 전류 1 제한 시간 제한. 값이 0이면 제한이 없다."@ko-KR ;
        IFC4-PSD:ifdguid          "671fec00d1fa11e1800000215ad4efdf" ;
        IFC4-PSD:name             "CurrentToleranceLimit1" ;
        IFC4-PSD:nameAlias        "허용전류한계1"@ko-KR , "許容電流限界1"@ja-JP , "Current Tolerance Limit1"@en ;
        IFC4-PSD:propertyType     [ a                  IFC4-PSD:TypePropertySingleValue ;
                                    IFC4-PSD:dataType  IFC4:IfcTimeMeasure
                                  ] .

:p73a44480d1fa11e1800000215ad4efdf
        a                         IFC4-PSD:PropertyDef ;
        rdfs:comment              "Indication whether the value of  CurrentTolerance1 is provided as a positive tolereance only  or not. If not, the value is proved as a pluss/minus tolerance." ;
        rdfs:label                "IsCurrentTolerancePositiveOnly" ;
        IFC4-PSD:definition       "Indication whether the value of  CurrentTolerance1 is provided as a positive tolereance only  or not. If not, the value is proved as a pluss/minus tolerance." ;
        IFC4-PSD:definitionAlias  ""@en , "허용 전류 한계 값 1 만 여부  위의 경우, 전류 허용 값은 플러스 / 마이너스 값."@ko-KR , "許容電流限界1の値のみかどうか\n 上記でない場合、電流許容値はプラス/マイナスした値。"@ja-JP ;
        IFC4-PSD:ifdguid          "73a44480d1fa11e1800000215ad4efdf" ;
        IFC4-PSD:name             "IsCurrentTolerancePositiveOnly" ;
        IFC4-PSD:nameAlias        "電流許容値"@ja-JP , "Is Current Tolerance Positive Only"@en , "전류 허용 값"@ko-KR ;
        IFC4-PSD:propertyType     [ a                  IFC4-PSD:TypePropertySingleValue ;
                                    IFC4-PSD:dataType  IFC4:IfcBoolean
                                  ] .

:NominalCurrentAdjusted
        a                   rdf:Property ;
        rdfs:seeAlso        :p4a83b400d1fa11e1800000215ad4efdf ;
        rdfs:subPropertyOf  IFC4-PSD:NominalCurrentAdjusted .

:ReleaseCurrentI2tStart
        a                   rdf:Property ;
        rdfs:seeAlso        :p9171a980d1fa11e1800000215ad4efdf ;
        rdfs:subPropertyOf  IFC4-PSD:ReleaseCurrentI2tStart .

:p9171a980d1fa11e1800000215ad4efdf
        a                         IFC4-PSD:PropertyDef ;
        rdfs:comment              "The release current in [x In] for the start point of the I2t tripping curve of the G-function, if any." ;
        rdfs:label                "ReleaseCurrentI2tStart" ;
        IFC4-PSD:definition       "The release current in [x In] for the start point of the I2t tripping curve of the G-function, if any." ;
        IFC4-PSD:definitionAlias  ""@en , "G関数の特性曲線I2tの始点[x In]が開始放流電流。"@ja-JP , "G 함수 특성 곡선 I2t의 시작점 [x In]가 시작 방류 전류."@ko-KR ;
        IFC4-PSD:ifdguid          "9171a980d1fa11e1800000215ad4efdf" ;
        IFC4-PSD:name             "ReleaseCurrentI2tStart" ;
        IFC4-PSD:nameAlias        "I2t 시작 방류 전류"@ko-KR , "Release Current I2t Start"@en , "I2tの開始放流電流"@ja-JP ;
        IFC4-PSD:propertyType     [ a                  IFC4-PSD:TypePropertySingleValue ;
                                    IFC4-PSD:dataType  IFC4:IfcElectricCurrentMeasure
                                  ] .

:ReleaseTimeI2tStart  a     rdf:Property ;
        rdfs:seeAlso        :p96cef400d1fa11e1800000215ad4efdf ;
        rdfs:subPropertyOf  IFC4-PSD:ReleaseTimeI2tStart .

:ExternalAdjusted  a        rdf:Property ;
        rdfs:seeAlso        :p51122b80d1fa11e1800000215ad4efdf ;
        rdfs:subPropertyOf  IFC4-PSD:ExternalAdjusted .

<https://www.linkedbuildingdata.net/IFC4-PSD/Pset_ProtectiveDeviceTrippingFunctionGCurve>
        a                owl:Ontology ;
        owl:imports      <http://lbd.arch.rwth-aachen.de/ifcOWL/IFC4-PSD> ;
        owl:versionInfo  "Created with BIM-Bots PSD Repository" .

:p6d15cd00d1fa11e1800000215ad4efdf
        a                         IFC4-PSD:PropertyDef ;
        rdfs:comment              "The tolerance for the current of time/current-curve in [%] valid for times above CurrentTolereanceLimit1." ;
        rdfs:label                "CurrentTolerance2" ;
        IFC4-PSD:definition       "The tolerance for the current of time/current-curve in [%] valid for times above CurrentTolereanceLimit1." ;
        IFC4-PSD:definitionAlias  ""@en , "[%]로 지정된 시간 / 특성 곡선의 허용 범위는 상기의 허용 전류 한계 1 시간에 유효합니다."@ko-KR , "[％]で指定された時間/特性曲線の許容範囲は、上記の許容電流限界1の時間で有効です。"@ja-JP ;
        IFC4-PSD:ifdguid          "6d15cd00d1fa11e1800000215ad4efdf" ;
        IFC4-PSD:name             "CurrentTolerance2" ;
        IFC4-PSD:nameAlias        "허용전류 2"@ko-KR , "許容電流2"@ja-JP , "Current Tolerance2"@en ;
        IFC4-PSD:propertyType     [ a                  IFC4-PSD:TypePropertySingleValue ;
                                    IFC4-PSD:dataType  IFC4:IfcPositiveRatioMeasure
                                  ] .

:p57080c80d1fa11e1800000215ad4efdf
        a                         IFC4-PSD:PropertyDef ;
        rdfs:comment              "The release current in [x In] for the initial tripping of the S-function." ;
        rdfs:label                "ReleaseCurrent" ;
        IFC4-PSD:definition       "The release current in [x In] for the initial tripping of the S-function." ;
        IFC4-PSD:definitionAlias  "방출 전류는 S-function의 초기 특성."@ko-KR , "放出する電流は、S-functionの初期特性。"@ja-JP , ""@en ;
        IFC4-PSD:ifdguid          "57080c80d1fa11e1800000215ad4efdf" ;
        IFC4-PSD:name             "ReleaseCurrent" ;
        IFC4-PSD:nameAlias        "방출전류"@ko-KR , "放出電流"@ja-JP , "Release Current"@en ;
        IFC4-PSD:propertyType     [ a                  IFC4-PSD:TypePropertySingleValue ;
                                    IFC4-PSD:dataType  IFC4:IfcElectricCurrentMeasure
                                  ] .

:TimeTolerance1  a          rdf:Property ;
        rdfs:seeAlso        :p7a32bc00d1fa11e1800000215ad4efdf ;
        rdfs:subPropertyOf  IFC4-PSD:TimeTolerance1 .

:IsCurrentTolerancePositiveOnly
        a                   rdf:Property ;
        rdfs:seeAlso        :p73a44480d1fa11e1800000215ad4efdf ;
        rdfs:subPropertyOf  IFC4-PSD:IsCurrentTolerancePositiveOnly .

:ReleaseCurrent  a          rdf:Property ;
        rdfs:seeAlso        :p57080c80d1fa11e1800000215ad4efdf ;
        rdfs:subPropertyOf  IFC4-PSD:ReleaseCurrent .

:p96cef400d1fa11e1800000215ad4efdf
        a                         IFC4-PSD:PropertyDef ;
        rdfs:comment              "The release time in [s] for the start point of the I2t tripping curve of the G-function, if any." ;
        rdfs:label                "ReleaseTimeI2tStart" ;
        IFC4-PSD:definition       "The release time in [s] for the start point of the I2t tripping curve of the G-function, if any." ;
        IFC4-PSD:definitionAlias  ""@en , "G関数の特性曲線I2tの始点[s]が開始放流時間。"@ja-JP , "G 함수 특성 곡선 I2t의 시작점 [s]가 시작 방류 시간."@ko-KR ;
        IFC4-PSD:ifdguid          "96cef400d1fa11e1800000215ad4efdf" ;
        IFC4-PSD:name             "ReleaseTimeI2tStart" ;
        IFC4-PSD:nameAlias        "I2t 시작 방류 시간"@ko-KR , "I2tの開始放流時間"@ja-JP , "Release Time I2t Start"@en ;
        IFC4-PSD:propertyType     [ a                  IFC4-PSD:TypePropertySingleValue ;
                                    IFC4-PSD:dataType  IFC4:IfcTimeMeasure
                                  ] .

:p4a83b400d1fa11e1800000215ad4efdf
        a                         IFC4-PSD:PropertyDef ;
        rdfs:comment              "An indication if the tripping currents of the short time protection is related to the nominal current multiplied with the actual setting of the current adjustment, if any, of the long time protection part of the protective device, or not." ;
        rdfs:label                "NominalCurrentAdjusted" ;
        IFC4-PSD:definition       "An indication if the tripping currents of the short time protection is related to the nominal current multiplied with the actual setting of the current adjustment, if any, of the long time protection part of the protective device, or not." ;
        IFC4-PSD:definitionAlias  ""@en , "전류 작동 시간의 여부"@ko-KR , "電流によって、動作時間が短かかったり長かったりするかどうか。"@ja-JP ;
        IFC4-PSD:ifdguid          "4a83b400d1fa11e1800000215ad4efdf" ;
        IFC4-PSD:name             "NominalCurrentAdjusted" ;
        IFC4-PSD:nameAlias        "Nominal Current Adjusted"@en , "정격전류조정"@ko-KR , "定格調整電流"@ja-JP ;
        IFC4-PSD:propertyType     [ a                  IFC4-PSD:TypePropertySingleValue ;
                                    IFC4-PSD:dataType  IFC4:IfcBoolean
                                  ] .

:p84ed5100d1fa11e1800000215ad4efdf
        a                         IFC4-PSD:PropertyDef ;
        rdfs:comment              "The tolerance for the time of the time/current-curve in [%] valid for currents above TimeToleranceLimit1." ;
        rdfs:label                "TimeTolerance2" ;
        IFC4-PSD:definition       "The tolerance for the time of the time/current-curve in [%] valid for currents above TimeToleranceLimit1." ;
        IFC4-PSD:definitionAlias  "[％]で指定された時間/特性曲線の許容範囲は、上記の許容電流限界1の電流で有効です。"@ja-JP , ""@en , "[%]로 지정된 시간 / 특성 곡선의 허용 범위는 상기의 허용 전류 한계 1의 전류로 사용할 수 있습니다."@ko-KR ;
        IFC4-PSD:ifdguid          "84ed5100d1fa11e1800000215ad4efdf" ;
        IFC4-PSD:name             "TimeTolerance2" ;
        IFC4-PSD:nameAlias        "許容時間2"@ja-JP , "Time Tolerance2"@en , "허용시간 2"@ko-KR ;
        IFC4-PSD:propertyType     [ a                  IFC4-PSD:TypePropertySingleValue ;
                                    IFC4-PSD:dataType  IFC4:IfcPositiveRatioMeasure
                                  ] .

:p42c40f80d1fa11e1800000215ad4efdf
        a                         IFC4-PSD:PropertyDef ;
        rdfs:comment              "Indication whether the S-function can be switched off or not." ;
        rdfs:label                "IsSelectable" ;
        IFC4-PSD:definition       "Indication whether the S-function can be switched off or not." ;
        IFC4-PSD:definitionAlias  "装置の “ON-OFF”状態を電気的表示が切り替え可能かどうか。"@ja-JP , ""@en , "장치\"ON-OFF \"상태를 전기적으로 표시가 교체 가능합니까?"@ko-KR ;
        IFC4-PSD:ifdguid          "42c40f80d1fa11e1800000215ad4efdf" ;
        IFC4-PSD:name             "IsSelectable" ;
        IFC4-PSD:nameAlias        "切り替え"@ja-JP , "Is Selectable"@en , "전환"@ko-KR ;
        IFC4-PSD:propertyType     [ a                  IFC4-PSD:TypePropertySingleValue ;
                                    IFC4-PSD:dataType  IFC4:IfcBoolean
                                  ] .

:CurrentTolerance2  a       rdf:Property ;
        rdfs:seeAlso        :p6d15cd00d1fa11e1800000215ad4efdf ;
        rdfs:subPropertyOf  IFC4-PSD:CurrentTolerance2 .

:p9c2c3e80d1fa11e1800000215ad4efdf
        a                         IFC4-PSD:PropertyDef ;
        rdfs:comment              "The release current in [x In] for the end point of the I2t tripping curve of the G-function, if any. The value of ReleaseCurrentI2tEnd shall be larger than ReleaseCurrentI2tStart." ;
        rdfs:label                "ReleaseCurrentI2tEnd" ;
        IFC4-PSD:definition       "The release current in [x In] for the end point of the I2t tripping curve of the G-function, if any. The value of ReleaseCurrentI2tEnd shall be larger than ReleaseCurrentI2tStart." ;
        IFC4-PSD:definitionAlias  ""@en , "G関数のI2の特性曲線のエンドポイントの[s]を放流電流。 \n  I2tの終了放流電流がI2tの開始放流電流よりも低くしなければならない。"@ja-JP , "G 함수 I2의 특성 곡선의 끝점에서 s를 방류 전류.   I2t 종료 방류 전류가 I2t 시작 방류 전류보다 낮게해야한다. \""@ko-KR ;
        IFC4-PSD:ifdguid          "9c2c3e80d1fa11e1800000215ad4efdf" ;
        IFC4-PSD:name             "ReleaseCurrentI2tEnd" ;
        IFC4-PSD:nameAlias        "I2tの終了放流電流"@ja-JP , "I2t 종료 방류 전류"@ko-KR , "Release Current I2t End"@en ;
        IFC4-PSD:propertyType     [ a                  IFC4-PSD:TypePropertySingleValue ;
                                    IFC4-PSD:dataType  IFC4:IfcElectricCurrentMeasure
                                  ] .

:p8ae33200d1fa11e1800000215ad4efdf
        a                         IFC4-PSD:PropertyDef ;
        rdfs:comment              "Indication whether the value of  TimeTolerance1 is provided as a positive tolereance only  or not. If not, the value is proved as a pluss/minus tolerance." ;
        rdfs:label                "IsTimeTolerancePositiveOnly" ;
        IFC4-PSD:definition       "Indication whether the value of  TimeTolerance1 is provided as a positive tolereance only  or not. If not, the value is proved as a pluss/minus tolerance." ;
        IFC4-PSD:definitionAlias  ""@en , "許容時間1の値のみかどうか\n 上記でない場合、時間許容値は、プラス/マイナスした値。"@ja-JP , "허용 시간 1 값만 여부  위의 경우 시간 허용치는 플러스 / 마이너스 값."@ko-KR ;
        IFC4-PSD:ifdguid          "8ae33200d1fa11e1800000215ad4efdf" ;
        IFC4-PSD:name             "IsTimeTolerancePositiveOnly" ;
        IFC4-PSD:nameAlias        "Is Time Tolerance Positive Only"@en , "時間許容値"@ja-JP , "시간 허용치"@ko-KR ;
        IFC4-PSD:propertyType     [ a                  IFC4-PSD:TypePropertySingleValue ;
                                    IFC4-PSD:dataType  IFC4:IfcBoolean
                                  ] .
