@prefix :      <https://www.linkedbuildingdata.net/IFC4-PSD/Pset_ProtectiveDeviceBreakerUnitI2TFuseCurve#> .
@prefix IFC4-PSD: <https://www.linkedbuildingdata.net/IFC4-PSD#> .
@prefix rdf:   <http://www.w3.org/1999/02/22-rdf-syntax-ns#> .
@prefix owl:   <http://www.w3.org/2002/07/owl#> .
@prefix rdfs:  <http://www.w3.org/2000/01/rdf-schema#> .
@prefix IFC4:  <http://lbd.arch.rwth-aachen.de/ifcOWL/IFC4#> .

<https://www.linkedbuildingdata.net/IFC4-PSD/Pset_ProtectiveDeviceBreakerUnitI2TFuseCurve>
        a                owl:Ontology ;
        owl:imports      <http://lbd.arch.rwth-aachen.de/ifcOWL/IFC4-PSD> ;
        owl:versionInfo  "Created with BIM-Bots PSD Repository" .

:BreakerUnitFuseBreakingingCurve
        a                   rdf:Property ;
        rdfs:seeAlso        :p2673a300d1f911e1800000215ad4efdf ;
        rdfs:subPropertyOf  IFC4-PSD:BreakerUnitFuseBreakingingCurve .

:p2673a300d1f911e1800000215ad4efdf
        a                         IFC4-PSD:PropertyDef ;
        rdfs:comment              "A curve that establishes the let through breaking energy of a breaker unit when a particular prospective breaking current is applied.  Note that the breaker unit fuse breaking curve is defined within a Cartesian coordinate system and this fact must be:\n\n(1) Defining value: ProspectiveCurrentBreaking: A list of minimum 2 and maximum 8 numbers providing the currents in [A] for points in the\ncurrent/breaking energy log/log coordinate space. The curve is drawn as a straight line between two consecutive points.\n(2) Defined value: LetThroughBreakingEnergy: A list of minimum 2 and maximum 8 numbers providing the breaking energy whereby the fuse has provided a break, I2t, in [A2s] for points in the current/breakting_energy log/log coordinate space. The curve is drawn as a straight line between two consecutive." ;
        rdfs:label                "BreakerUnitFuseBreakingingCurve" ;
        IFC4-PSD:definition       "A curve that establishes the let through breaking energy of a breaker unit when a particular prospective breaking current is applied.  Note that the breaker unit fuse breaking curve is defined within a Cartesian coordinate system and this fact must be:\n\n(1) Defining value: ProspectiveCurrentBreaking: A list of minimum 2 and maximum 8 numbers providing the currents in [A] for points in the\ncurrent/breaking energy log/log coordinate space. The curve is drawn as a straight line between two consecutive points.\n(2) Defined value: LetThroughBreakingEnergy: A list of minimum 2 and maximum 8 numbers providing the breaking energy whereby the fuse has provided a break, I2t, in [A2s] for points in the current/breakting_energy log/log coordinate space. The curve is drawn as a straight line between two consecutive." ;
        IFC4-PSD:definitionAlias  "예상치 못한 전류가 흐를 때 차단기의 퓨즈를 녹이는 데 필요한 에너지를 나타내는 곡선.   예상외의 전류가 흘렀을 때에 차단기의 퓨즈를 녹이는 데 필요한 에너지를 나타내는 곡선.   (1) 정의 값 : 융해 전류 : 전류 / 융해 에너지에 표시된 최소 2에서 최대 8 개의 목록에서 전류 [A]를 정의합니다.    커브가 연속되는 두 개의 점을 연결하는 직선으로 그려져 있습니다.   (2) 정의 값 : 융해 에너지 :/ 전류 / 융해 에너지의 위치 [A2s에서 나타나는 2 ~ 16 예상되는 퓨즈가 용해 시작 전류 [A2s을 정의합니다. 커브가 연속되는 두 개의 점을 연결하는 직선으로 그려져 있습니다."@ko-KR , ""@en , "想定外の電流が流れた時に遮断機のフューズを溶かすために必要なエネルギーを表す曲線。\n  想定外の電流が流れた時に遮断機のフューズを溶かすために必要なエネルギーを表す曲線。\n\n  （1）定義値：融解電流：電流/ 融解エネルギーで示される最小2から最大8のリストで電流[A]を定義します。\n   カーブが連続する2つの点を結ぶ直線として描かれています。\n  （2）定義値：融解エネルギー：/電流/融解エネルギーの位置[A2s]で示される2～16の想定されるフューズが溶解始める電流[A2s]を定義します。カーブが連続する2つの点を結ぶ直線として描かれています。"@ja-JP ;
        IFC4-PSD:ifdguid          "2673a300d1f911e1800000215ad4efdf" ;
        IFC4-PSD:name             "BreakerUnitFuseBreakingingCurve" ;
        IFC4-PSD:nameAlias        "Breaker Unit Fuse Breakinging Curve"@en , "퓨즈 차단기 융해 곡선"@ko-KR , "フューズ遮断機融解曲線"@ja-JP ;
        IFC4-PSD:propertyType     [ a                       IFC4-PSD:TypePropertyTableValue ;
                                    IFC4-PSD:definedValue   IFC4:IfcReal ;
                                    IFC4-PSD:definingValue  IFC4:IfcElectricCurrentMeasure
                                  ] .

:Pset_ProtectiveDeviceBreakerUnitI2TFuseCurve
        a                             IFC4-PSD:PropertySetDef ;
        rdfs:comment                  "A coherent set of attributes representing curves for melting- and breaking-energy of a fuse. Note - A fuse may be associated with different instances of this property set providing information related to different  basic characteristics." ;
        rdfs:label                    "Pset_ProtectiveDeviceBreakerUnitI2TFuseCurve" ;
        IFC4-PSD:applicableClass      IFC4:IfcProtectiveDevice ;
        IFC4-PSD:applicableTypeValue  "IfcProtectiveDevice" ;
        IFC4-PSD:definition           "A coherent set of attributes representing curves for melting- and breaking-energy of a fuse. Note - A fuse may be associated with different instances of this property set providing information related to different  basic characteristics." ;
        IFC4-PSD:definitionAlias      "フューズの融解-遮断エネルギー曲線を表す一連のプロパティセット。\n注記-フューズは、根本的な特性に関連付けられた提供されたプロパティの情報は、　異なる実態に関連しているかもしれません。　　　　　　　　　　　　　　　　　"@ja-JP , ""@en ;
        IFC4-PSD:ifcVersion           [ a                 IFC4-PSD:IfcVersion ;
                                        IFC4-PSD:version  "IFC4"
                                      ] ;
        IFC4-PSD:name                 "Pset_ProtectiveDeviceBreakerUnitI2TFuseCurve" ;
        IFC4-PSD:propertyDef          :pf75d3180d1f811e1800000215ad4efdf , :p152a9680d1f911e1800000215ad4efdf , :p2673a300d1f911e1800000215ad4efdf .

:pf75d3180d1f811e1800000215ad4efdf
        a                         IFC4-PSD:PropertyDef ;
        rdfs:comment              "The voltage levels of the fuse for which the data of the instance is valid. More than one value may be selected in the enumeration." ;
        rdfs:label                "VoltageLevel" ;
        IFC4-PSD:definition       "The voltage levels of the fuse for which the data of the instance is valid. More than one value may be selected in the enumeration." ;
        IFC4-PSD:definitionAlias  ""@en , "전압 레벨을 선택합니다."@ko-KR , "電圧レベルを選択。"@ja-JP ;
        IFC4-PSD:ifdguid          "f75d3180d1f811e1800000215ad4efdf" ;
        IFC4-PSD:name             "VoltageLevel" ;
        IFC4-PSD:nameAlias        "Voltage Level"@en , "전압레벨"@ko-KR , "電圧レベル"@ja-JP ;
        IFC4-PSD:propertyType     [ a                  IFC4-PSD:TypePropertyEnumeratedValue ;
                                    IFC4-PSD:enumItem  "U230" , "OTHER" , "U400" , "NOTKNOWN" , "U1000" , "UNSET" , "U690" , "U525" , "U440"
                                  ] .

:p152a9680d1f911e1800000215ad4efdf
        a                         IFC4-PSD:PropertyDef ;
        rdfs:comment              "A curve that establishes the energy required to melt the fuse of a breaker unit when a particular prospective melting current is applied.  Note that the breaker unit fuse melting curve is defined within a Cartesian coordinate system and this fact must be:\n\n(1) Defining value: ProspectiveCurrentMelting :A list of minimum 2 and maximum 8 numbers providing the currents in [A] for points in the\ncurrent/melting_energy log/log coordinate space. The curve is drawn as a straight line between two consecutive points.\n(2) Defined value: MeltingEnergy: A list of minimum 2 and maximum 8 numbers providing the energy whereby the fuse is starting to melt, I2t, in [A2s] for points in the current/melting_energy log/log coordinate space. The curve is drawn as a straight line between two consecutive points." ;
        rdfs:label                "BreakerUnitFuseMeltingCurve" ;
        IFC4-PSD:definition       "A curve that establishes the energy required to melt the fuse of a breaker unit when a particular prospective melting current is applied.  Note that the breaker unit fuse melting curve is defined within a Cartesian coordinate system and this fact must be:\n\n(1) Defining value: ProspectiveCurrentMelting :A list of minimum 2 and maximum 8 numbers providing the currents in [A] for points in the\ncurrent/melting_energy log/log coordinate space. The curve is drawn as a straight line between two consecutive points.\n(2) Defined value: MeltingEnergy: A list of minimum 2 and maximum 8 numbers providing the energy whereby the fuse is starting to melt, I2t, in [A2s] for points in the current/melting_energy log/log coordinate space. The curve is drawn as a straight line between two consecutive points." ;
        IFC4-PSD:definitionAlias  "想定外の電流が流れた時に遮断機のフューズを溶かすために必要なエネルギーを表す曲線。\n  想定外の電流が流れた時に遮断機のフューズを溶かすために必要なエネルギーを表す曲線。\n\n  （1）定義値：融解電流：電流/ 融解エネルギーで示される最小2から最大8のリストで電流[A]を定義します。\n   カーブが連続する2つの点を結ぶ直線として描かれています。\n  （2）定義値：融解エネルギー：/電流/融解エネルギーの位置[A2s]で示される2～16の想定されるフューズが溶解始める電流[A2s]を定義します。カーブが連続する2つの点を結ぶ直線として描かれています。"@ja-JP , "예상치 못한 전류가 흐를 때 차단기의 퓨즈를 녹이는 데 필요한 에너지를 나타내는 곡선.   예상외의 전류가 흘렀을 때에 차단기의 퓨즈를 녹이는 데 필요한 에너지를 나타내는 곡선.   (1) 정의 값 : 융해 전류 : 전류 / 융해 에너지에 표시된 최소 2에서 최대 8 개의 목록에서 전류 [A]를 정의합니다.    커브가 연속되는 두 개의 점을 연결하는 직선으로 그려져 있습니다.   (2) 정의 값 : 융해 에너지 :/ 전류 / 융해 에너지의 위치 [A2s에서 나타나는 2 ~ 16 예상되는 퓨즈가 용해 시작 전류 [A2s을 정의합니다. 커브가 연속되는 두 개의 점을 연결하는 직선으로 그려져 있습니다."@ko-KR , ""@en ;
        IFC4-PSD:ifdguid          "152a9680d1f911e1800000215ad4efdf" ;
        IFC4-PSD:name             "BreakerUnitFuseMeltingCurve" ;
        IFC4-PSD:nameAlias        "フューズ遮断機融解曲線"@ja-JP , "Breaker Unit Fuse Melting Curve"@en , "퓨즈 차단기 융해 곡선"@ko-KR ;
        IFC4-PSD:propertyType     [ a                       IFC4-PSD:TypePropertyTableValue ;
                                    IFC4-PSD:definedValue   IFC4:IfcReal ;
                                    IFC4-PSD:definingValue  IFC4:IfcElectricCurrentMeasure
                                  ] .

:BreakerUnitFuseMeltingCurve
        a                   rdf:Property ;
        rdfs:seeAlso        :p152a9680d1f911e1800000215ad4efdf ;
        rdfs:subPropertyOf  IFC4-PSD:BreakerUnitFuseMeltingCurve .

:VoltageLevel  a            rdf:Property ;
        rdfs:seeAlso        :pf75d3180d1f811e1800000215ad4efdf ;
        rdfs:subPropertyOf  IFC4-PSD:VoltageLevel .
