@prefix :      <https://www.linkedbuildingdata.net/IFC4-PSD/Pset_TransportElementElevator#> .
@prefix IFC4-PSD: <https://www.linkedbuildingdata.net/IFC4-PSD#> .
@prefix owl:   <http://www.w3.org/2002/07/owl#> .
@prefix rdf:   <http://www.w3.org/1999/02/22-rdf-syntax-ns#> .
@prefix rdfs:  <http://www.w3.org/2000/01/rdf-schema#> .
@prefix IFC4:  <http://lbd.arch.rwth-aachen.de/ifcOWL/IFC4#> .

:p29c75880d21211e1800000215ad4efdf
        a                         IFC4-PSD:PropertyDef ;
        rdfs:comment              "Clear depth of the object (elevator). It indicates the distance from the inner surface of the elevator door to the opposite surface of the elevator car. \nThe shape information is provided in addition to the shape representation and the geometric parameters used within. In cases of inconsistency between the geometric parameters and the shape properties, provided in the attached property, the geometric parameters take precedence." ;
        rdfs:label                "ClearDepth" ;
        IFC4-PSD:definition       "Clear depth of the object (elevator). It indicates the distance from the inner surface of the elevator door to the opposite surface of the elevator car. \nThe shape information is provided in addition to the shape representation and the geometric parameters used within. In cases of inconsistency between the geometric parameters and the shape properties, provided in the attached property, the geometric parameters take precedence." ;
        IFC4-PSD:definitionAlias  "Profondeur de l'ascenseur. Elle indique la distance entre la face intérieure de la porte et la face opposée de la cabine de l'ascenseur. Cette propriété est donnée en complément de la représentation de la forme de l'élément et des paramètres géométriques qui la déterminent. En cas d'incohérence entre ces paramètres géométriques et cette propriété, ce sont les paramètres géométriques qui priment."@fr-FR , "オブジェクト（エレベータ）の奥行き。エレベータドアの内部表面から、反対側の表面までの距離を示す。\n形状表現は、Shape representation（IFCの幾何形状表現）およびそこで設定されている幾何形状パラメータにより与えられる。もし、幾何形状パラメータと形状プロパティ情報が一致しない場合は、形状パラメータの値を優先する。"@ja-JP , ""@en ;
        IFC4-PSD:ifdguid          "29c75880d21211e1800000215ad4efdf" ;
        IFC4-PSD:name             "ClearDepth" ;
        IFC4-PSD:nameAlias        "Profondeur de passage"@fr-FR , "奥行き"@ja-JP , "Clear Depth"@en ;
        IFC4-PSD:propertyType     [ a                  IFC4-PSD:TypePropertySingleValue ;
                                    IFC4-PSD:dataType  IFC4:IfcPositiveLengthMeasure
                                  ] .

:ClearHeight  a             rdf:Property ;
        rdfs:seeAlso        :p321f9380d21211e1800000215ad4efdf ;
        rdfs:subPropertyOf  IFC4-PSD:ClearHeight .

:ClearWidth  a              rdf:Property ;
        rdfs:seeAlso        :p20d68700d21211e1800000215ad4efdf ;
        rdfs:subPropertyOf  IFC4-PSD:ClearWidth .

:Pset_TransportElementElevator
        a                             IFC4-PSD:PropertySetDef ;
        rdfs:comment                  "Properties common to the definition of all occurrences of IfcTransportElement with the predefined type =\"ELEVATOR\"" ;
        rdfs:label                    "Pset_TransportElementElevator" ;
        IFC4-PSD:applicableClass      <http://lbd.arch.rwth-aachen.de/ifcOWL/IFC4#IfcTransportElement/ELEVATOR> ;
        IFC4-PSD:applicableTypeValue  "IfcTransportElement/ELEVATOR" ;
        IFC4-PSD:definition           "Properties common to the definition of all occurrences of IfcTransportElement with the predefined type =\"ELEVATOR\"" ;
        IFC4-PSD:definitionAlias      ""@en , "タイプが既定義の\"ELEVATOR\"であるIfcTransportElementすべてに共通な属性の定義。"@ja-JP , "Property Set Definition in German"@de-DE , "Définition de l'IAI : propriétés communes à la définition de toutes les instances de la classe IfcTransportElement de type ELEVATOR."@fr-FR ;
        IFC4-PSD:ifcVersion           [ a                 IFC4-PSD:IfcVersion ;
                                        IFC4-PSD:version  "IFC4"
                                      ] ;
        IFC4-PSD:name                 "Pset_TransportElementElevator" ;
        IFC4-PSD:propertyDef          :p1a480f80d21211e1800000215ad4efdf , :p321f9380d21211e1800000215ad4efdf , :p20d68700d21211e1800000215ad4efdf , :p29c75880d21211e1800000215ad4efdf .

:p321f9380d21211e1800000215ad4efdf
        a                         IFC4-PSD:PropertyDef ;
        rdfs:comment              "Clear height of the object (elevator).  \nThe shape information is provided in addition to the shape representation and the geometric parameters used within. In cases of inconsistency between the geometric parameters and the shape properties, provided in the attached property, the geometric parameters take precedence." ;
        rdfs:label                "ClearHeight" ;
        IFC4-PSD:definition       "Clear height of the object (elevator).  \nThe shape information is provided in addition to the shape representation and the geometric parameters used within. In cases of inconsistency between the geometric parameters and the shape properties, provided in the attached property, the geometric parameters take precedence." ;
        IFC4-PSD:definitionAlias  "Hauteur du passage de l'ascenseur. Cette propriété est donnée en complément de la représentation de la forme de l'élément et des paramètres géométriques qui la déterminent. En cas d'incohérence entre ces paramètres géométriques et cette propriété, ce sont les paramètres géométriques qui priment."@fr-FR , "オブジェクト（エレベータ）の高さ。エレベータドアの内部の床面から天井までの距離を示す。\n形状表現は、Shape representation（IFCの幾何形状表現）およびそこで設定されている幾何形状パラメータにより与えられる。もし、幾何形状パラメータと形状プロパティ情報が一致しない場合は、形状パラメータの値を優先する。"@ja-JP , ""@en ;
        IFC4-PSD:ifdguid          "321f9380d21211e1800000215ad4efdf" ;
        IFC4-PSD:name             "ClearHeight" ;
        IFC4-PSD:nameAlias        "Clear Height"@en , "高さ"@ja-JP , "Hauteur de passage"@fr-FR ;
        IFC4-PSD:propertyType     [ a                  IFC4-PSD:TypePropertySingleValue ;
                                    IFC4-PSD:dataType  IFC4:IfcPositiveLengthMeasure
                                  ] .

<https://www.linkedbuildingdata.net/IFC4-PSD/Pset_TransportElementElevator>
        a                owl:Ontology ;
        owl:imports      <http://lbd.arch.rwth-aachen.de/ifcOWL/IFC4-PSD> ;
        owl:versionInfo  "Created with BIM-Bots PSD Repository" .

:p20d68700d21211e1800000215ad4efdf
        a                         IFC4-PSD:PropertyDef ;
        rdfs:comment              "Clear width of the object (elevator). It indicates the distance from the inner surfaces of the elevator car left and right from the elevator door. \nThe shape information is provided in addition to the shape representation and the geometric parameters used within. In cases of inconsistency between the geometric parameters and the shape properties, provided in the attached property, the geometric parameters take precedence." ;
        rdfs:label                "ClearWidth" ;
        IFC4-PSD:definition       "Clear width of the object (elevator). It indicates the distance from the inner surfaces of the elevator car left and right from the elevator door. \nThe shape information is provided in addition to the shape representation and the geometric parameters used within. In cases of inconsistency between the geometric parameters and the shape properties, provided in the attached property, the geometric parameters take precedence." ;
        IFC4-PSD:definitionAlias  "Largeur du passage de l'ascenseur. Elle indique la distance entre les surfaces intérieures gauche et droite de la cabine depuis la porte de l'ascenseur. Cette propriété est donnée en complément de la représentation de la forme de l'élément et des paramètres géométriques qui la déterminent. En cas d'incohérence entre ces paramètres géométriques et cette propriété, ce sont les paramètres géométriques qui priment."@fr-FR , "オブジェクト（エレベータ）の幅。エレベータ昇降機内部表面の左から右の距離を示す。\n形状表現は、Shape representation（IFCの幾何形状表現）およびそこで設定されている幾何形状パラメータにより与えられる。もし、幾何形状パラメータと形状プロパティ情報が一致しない場合は、形状パラメータの値を優先する。"@ja-JP , ""@en ;
        IFC4-PSD:ifdguid          "20d68700d21211e1800000215ad4efdf" ;
        IFC4-PSD:name             "ClearWidth" ;
        IFC4-PSD:nameAlias        "Largeur du passage"@fr-FR , "Clear Width"@en , "幅員"@ja-JP ;
        IFC4-PSD:propertyType     [ a                  IFC4-PSD:TypePropertySingleValue ;
                                    IFC4-PSD:dataType  IFC4:IfcPositiveLengthMeasure
                                  ] .

:ClearDepth  a              rdf:Property ;
        rdfs:seeAlso        :p29c75880d21211e1800000215ad4efdf ;
        rdfs:subPropertyOf  IFC4-PSD:ClearDepth .

:p1a480f80d21211e1800000215ad4efdf
        a                         IFC4-PSD:PropertyDef ;
        rdfs:comment              "Indication whether the elevator is designed to serve as a fire fighting lift the case of fire (TRUE) or not (FALSE). A fire fighting lift is used by fire fighters to access the location of fire and to evacuate people." ;
        rdfs:label                "FireFightingLift" ;
        IFC4-PSD:definition       "Indication whether the elevator is designed to serve as a fire fighting lift the case of fire (TRUE) or not (FALSE). A fire fighting lift is used by fire fighters to access the location of fire and to evacuate people." ;
        IFC4-PSD:definitionAlias  ""@en , "火災時に消防エレベーターとしての利用を想定して設計されているかどうかを示す。消防エレベーターは火災現場へ消防士を運んだり人を避難させるために使われる。"@ja-JP , "Indique si l'ascenseur est conçu pour servir d'ascenseur pompier (VRAI) ou non (FAUX). Un ascenseur pompier est utilisé par les pompiers pour accéder à l'endroit du feu et évacuer les personnes."@fr-FR , "Angabe, ob der Aufzug als ein Feuerwerksaufzug vorgesehen ist (WAHR) oder nicht (FALSCH). Ein Feuerwehraufzug ist ein besonders abgesicherter Aufzug der der Feuerwehr im Branfall ein Erreichen der Branetage ermöglicht."@de-DE ;
        IFC4-PSD:ifdguid          "1a480f80d21211e1800000215ad4efdf" ;
        IFC4-PSD:name             "FireFightingLift" ;
        IFC4-PSD:nameAlias        "Fire Fighting Lift"@en , "LargeurPassage"@fr-FR , "消防エレベーター"@ja-JP , "Feuerwehraufzug"@de-DE ;
        IFC4-PSD:propertyType     [ a                  IFC4-PSD:TypePropertySingleValue ;
                                    IFC4-PSD:dataType  IFC4:IfcBoolean
                                  ] .

:FireFightingLift  a        rdf:Property ;
        rdfs:seeAlso        :p1a480f80d21211e1800000215ad4efdf ;
        rdfs:subPropertyOf  IFC4-PSD:FireFightingLift .
