@prefix :      <https://www.linkedbuildingdata.net/IFC4-PSD/Pset_ProtectiveDeviceTrippingUnitCurrentAdjustment#> .
@prefix IFC4-PSD: <https://www.linkedbuildingdata.net/IFC4-PSD#> .
@prefix rdf:   <http://www.w3.org/1999/02/22-rdf-syntax-ns#> .
@prefix owl:   <http://www.w3.org/2002/07/owl#> .
@prefix rdfs:  <http://www.w3.org/2000/01/rdf-schema#> .
@prefix IFC4:  <http://lbd.arch.rwth-aachen.de/ifcOWL/IFC4#> .

:pb87cab00d1fb11e1800000215ad4efdf
        a                         IFC4-PSD:PropertyDef ;
        rdfs:comment              "Step value of current adjustment for an AdjustmentValueType = RANGE. Note that this property should not have a value for an  AdjustmentValueType = LIST." ;
        rdfs:label                "AdjustmentRangeStepValue" ;
        IFC4-PSD:definition       "Step value of current adjustment for an AdjustmentValueType = RANGE. Note that this property should not have a value for an  AdjustmentValueType = LIST." ;
        IFC4-PSD:definitionAlias  ""@en , "時間調整の範囲をステップ値を設定。一覧表ではもっていない事を注意。"@ja-JP , "시간 조정 범위를 단계 값을 설정합니다. 목록은 갖고 있지 않은 것을주의."@ko-KR ;
        IFC4-PSD:ifdguid          "b87cab00d1fb11e1800000215ad4efdf" ;
        IFC4-PSD:name             "AdjustmentRangeStepValue" ;
        IFC4-PSD:nameAlias        "조정범위 단계값"@ko-KR , "調整範囲のステップ値"@ja-JP , "Adjustment Range Step Value"@en ;
        IFC4-PSD:propertyType     [ a                  IFC4-PSD:TypePropertySingleValue ;
                                    IFC4-PSD:dataType  IFC4:IfcElectricCurrentMeasure
                                  ] .

:AdjustmentDesignation
        a                   rdf:Property ;
        rdfs:seeAlso        :pc4686d00d1fb11e1800000215ad4efdf ;
        rdfs:subPropertyOf  IFC4-PSD:AdjustmentDesignation .

:Pset_ProtectiveDeviceTrippingUnitCurrentAdjustment
        a                             IFC4-PSD:PropertySetDef ;
        rdfs:comment                  "A set of current adjustment values that may be applied to an electronic or thermal tripping unit type." ;
        rdfs:label                    "Pset_ProtectiveDeviceTrippingUnitCurrentAdjustment" ;
        IFC4-PSD:applicableClass      IFC4:IfcProtectiveDeviceTrippingUnit ;
        IFC4-PSD:applicableTypeValue  "IfcProtectiveDeviceTrippingUnit" ;
        IFC4-PSD:definition           "A set of current adjustment values that may be applied to an electronic or thermal tripping unit type." ;
        IFC4-PSD:definitionAlias      "電磁式または熱動式のトリップ装置の電流調整値。"@ja-JP , ""@en ;
        IFC4-PSD:ifcVersion           [ a                 IFC4-PSD:IfcVersion ;
                                        IFC4-PSD:version  "IFC4"
                                      ] ;
        IFC4-PSD:name                 "Pset_ProtectiveDeviceTrippingUnitCurrentAdjustment" ;
        IFC4-PSD:propertyDef          :pbe728c00d1fb11e1800000215ad4efdf , :pa864cb80d1fb11e1800000215ad4efdf , :pb0bd0680d1fb11e1800000215ad4efdf , :pc4686d00d1fb11e1800000215ad4efdf , :pb87cab00d1fb11e1800000215ad4efdf .

:pbe728c00d1fb11e1800000215ad4efdf
        a                         IFC4-PSD:PropertyDef ;
        rdfs:comment              "A list of current adjustment values that may be applied to a tripping unit for an AdjustmentValueType = LIST. A minimum of 1 and a maximum of 16 adjustment values may be specified. Note that this property should not have a value for an  AdjustmentValueType = RANGE." ;
        rdfs:label                "AdjustmentValues" ;
        IFC4-PSD:definition       "A list of current adjustment values that may be applied to a tripping unit for an AdjustmentValueType = LIST. A minimum of 1 and a maximum of 16 adjustment values may be specified. Note that this property should not have a value for an  AdjustmentValueType = RANGE." ;
        IFC4-PSD:definitionAlias  "時間調整値を１から16で設定。範囲では、ない事を注意。"@ja-JP , ""@en , "시간 조정 값을 1에서 16로 설정. 범위는없는 것을주의."@ko-KR ;
        IFC4-PSD:ifdguid          "be728c00d1fb11e1800000215ad4efdf" ;
        IFC4-PSD:name             "AdjustmentValues" ;
        IFC4-PSD:nameAlias        "조정 값"@ko-KR , "調整値"@ja-JP , "Adjustment Values"@en ;
        IFC4-PSD:propertyType     [ a                  IFC4-PSD:TypePropertyListValue ;
                                    IFC4-PSD:dataType  IFC4:IfcElectricCurrentMeasure
                                  ] .

:AdjustmentValueType  a     rdf:Property ;
        rdfs:seeAlso        :pa864cb80d1fb11e1800000215ad4efdf ;
        rdfs:subPropertyOf  IFC4-PSD:AdjustmentValueType .

:AdjustmentRange  a         rdf:Property ;
        rdfs:seeAlso        :pb0bd0680d1fb11e1800000215ad4efdf ;
        rdfs:subPropertyOf  IFC4-PSD:AdjustmentRange .

:pa864cb80d1fb11e1800000215ad4efdf
        a                         IFC4-PSD:PropertyDef ;
        rdfs:comment              "The type of adjustment value that is applied through the property set. This determines the properties that should be asserted (see below)." ;
        rdfs:label                "AdjustmentValueType" ;
        IFC4-PSD:definition       "The type of adjustment value that is applied through the property set. This determines the properties that should be asserted (see below)." ;
        IFC4-PSD:definitionAlias  "조정 값 유형을 설정합니다."@ko-KR , "調整値のタイプを設定。"@ja-JP , ""@en ;
        IFC4-PSD:ifdguid          "a864cb80d1fb11e1800000215ad4efdf" ;
        IFC4-PSD:name             "AdjustmentValueType" ;
        IFC4-PSD:nameAlias        "調整値の型"@ja-JP , "Adjustment Value Type"@en , "조정 형식"@ko-KR ;
        IFC4-PSD:propertyType     [ a                  IFC4-PSD:TypePropertyEnumeratedValue ;
                                    IFC4-PSD:enumItem  "RANGE" , "LIST"
                                  ] .

<https://www.linkedbuildingdata.net/IFC4-PSD/Pset_ProtectiveDeviceTrippingUnitCurrentAdjustment>
        a                owl:Ontology ;
        owl:imports      <http://lbd.arch.rwth-aachen.de/ifcOWL/IFC4-PSD> ;
        owl:versionInfo  "Created with BIM-Bots PSD Repository" .

:pc4686d00d1fb11e1800000215ad4efdf
        a                         IFC4-PSD:PropertyDef ;
        rdfs:comment              "The desgnation on the device for the adjustment." ;
        rdfs:label                "AdjustmentDesignation" ;
        IFC4-PSD:definition       "The desgnation on the device for the adjustment." ;
        IFC4-PSD:definitionAlias  ""@en , "조정하는 장치를 지정합니다."@ko-KR , "調整する装置の指定。"@ja-JP ;
        IFC4-PSD:ifdguid          "c4686d00d1fb11e1800000215ad4efdf" ;
        IFC4-PSD:name             "AdjustmentDesignation" ;
        IFC4-PSD:nameAlias        "調整の指定"@ja-JP , "Adjustment Designation"@en , "조정지정"@ko-KR ;
        IFC4-PSD:propertyType     [ a                  IFC4-PSD:TypePropertySingleValue ;
                                    IFC4-PSD:dataType  IFC4:IfcLabel
                                  ] .

:pb0bd0680d1fb11e1800000215ad4efdf
        a                         IFC4-PSD:PropertyDef ;
        rdfs:comment              "Upper and lower current adjustment limits for an AdjustmentValueType = RANGE. Note that this property should not have a value for an  AdjustmentValueType = LIST." ;
        rdfs:label                "AdjustmentRange" ;
        IFC4-PSD:definition       "Upper and lower current adjustment limits for an AdjustmentValueType = RANGE. Note that this property should not have a value for an  AdjustmentValueType = LIST." ;
        IFC4-PSD:definitionAlias  "시간 조정 범위의 상한 치와 하한 치를 설정합니다. 목록은 갖고 있지 않은 것을주의."@ko-KR , "時間調整の範囲の上限値と下限値を設定。一覧表ではもっていない事を注意。"@ja-JP , ""@en ;
        IFC4-PSD:ifdguid          "b0bd0680d1fb11e1800000215ad4efdf" ;
        IFC4-PSD:name             "AdjustmentRange" ;
        IFC4-PSD:nameAlias        "조정 범위"@ko-KR , "Adjustment Range"@en , "調整範囲"@ja-JP ;
        IFC4-PSD:propertyType     [ a                  IFC4-PSD:TypePropertyBoundedValue ;
                                    IFC4-PSD:dataType  IFC4:IfcElectricCurrentMeasure
                                  ] .

:AdjustmentValues  a        rdf:Property ;
        rdfs:seeAlso        :pbe728c00d1fb11e1800000215ad4efdf ;
        rdfs:subPropertyOf  IFC4-PSD:AdjustmentValues .

:AdjustmentRangeStepValue
        a                   rdf:Property ;
        rdfs:seeAlso        :pb87cab00d1fb11e1800000215ad4efdf ;
        rdfs:subPropertyOf  IFC4-PSD:AdjustmentRangeStepValue .
