@prefix :      <https://www.linkedbuildingdata.net/IFC4-PSD/Pset_MaterialWoodBasedPanel#> .
@prefix IFC4-PSD: <https://www.linkedbuildingdata.net/IFC4-PSD#> .
@prefix rdf:   <http://www.w3.org/1999/02/22-rdf-syntax-ns#> .
@prefix owl:   <http://www.w3.org/2002/07/owl#> .
@prefix rdfs:  <http://www.w3.org/2000/01/rdf-schema#> .
@prefix IFC4:  <http://lbd.arch.rwth-aachen.de/ifcOWL/IFC4#> .

<https://www.linkedbuildingdata.net/IFC4-PSD/Pset_MaterialWoodBasedPanel>
        a                owl:Ontology ;
        owl:imports      <http://lbd.arch.rwth-aachen.de/ifcOWL/IFC4-PSD> ;
        owl:versionInfo  "Created with BIM-Bots PSD Repository" .

:InPlane  a                 rdf:Property ;
        rdfs:seeAlso        :p7b122080d1ef11e1800000215ad4efdf ;
        rdfs:subPropertyOf  IFC4-PSD:InPlane .

:p7b122080d1ef11e1800000215ad4efdf
        a                         IFC4-PSD:PropertyDef ;
        rdfs:comment              "Mechanical properties with respect to in-plane load, i.e. for function as a membrane." ;
        rdfs:label                "InPlane" ;
        IFC4-PSD:definition       "Mechanical properties with respect to in-plane load, i.e. for function as a membrane." ;
        IFC4-PSD:definitionAlias  ""@en ;
        IFC4-PSD:ifdguid          "7b122080d1ef11e1800000215ad4efdf" ;
        IFC4-PSD:name             "InPlane" ;
        IFC4-PSD:nameAlias        "In Plane"@en ;
        IFC4-PSD:propertyType     [ a  IFC4-PSD:TypeComplexProperty ] .

:pe52ac580d1ef11e1800000215ad4efdf
        a                         IFC4-PSD:PropertyDef ;
        rdfs:comment              "Mechanical properties with respect to out-of-plane load, i.e. for function as a plate; tension zone of unbalanced layups is stressed in tension." ;
        rdfs:label                "OutOfPlane" ;
        IFC4-PSD:definition       "Mechanical properties with respect to out-of-plane load, i.e. for function as a plate; tension zone of unbalanced layups is stressed in tension." ;
        IFC4-PSD:definitionAlias  ""@en ;
        IFC4-PSD:ifdguid          "e52ac580d1ef11e1800000215ad4efdf" ;
        IFC4-PSD:name             "OutOfPlane" ;
        IFC4-PSD:nameAlias        "Out Of Plane"@en ;
        IFC4-PSD:propertyType     [ a  IFC4-PSD:TypeComplexProperty ] .

:p75b4d600d1ef11e1800000215ad4efdf
        a                         IFC4-PSD:PropertyDef ;
        rdfs:comment              "Determines whether mechanical material properties are applicable to 'ASD' = allowable stress design (working stress design), 'LSD' = limit state design, or 'LRFD' = load and resistance factor design." ;
        rdfs:label                "ApplicableStructuralDesignMethod" ;
        IFC4-PSD:definition       "Determines whether mechanical material properties are applicable to 'ASD' = allowable stress design (working stress design), 'LSD' = limit state design, or 'LRFD' = load and resistance factor design." ;
        IFC4-PSD:definitionAlias  ""@en ;
        IFC4-PSD:ifdguid          "75b4d600d1ef11e1800000215ad4efdf" ;
        IFC4-PSD:name             "ApplicableStructuralDesignMethod" ;
        IFC4-PSD:nameAlias        "Applicable Structural Design Method"@en ;
        IFC4-PSD:propertyType     [ a                  IFC4-PSD:TypePropertySingleValue ;
                                    IFC4-PSD:dataType  IFC4:IfcLabel
                                  ] .

:OutOfPlaneNegative  a      rdf:Property ;
        rdfs:seeAlso        :p510d2e00d1f011e1800000215ad4efdf ;
        rdfs:subPropertyOf  IFC4-PSD:OutOfPlaneNegative .

:p510d2e00d1f011e1800000215ad4efdf
        a                         IFC4-PSD:PropertyDef ;
        rdfs:comment              "Mechanical properties with respect to out-of-plane load i.e. for function as a plate; compression zone of unbalanced layups is stressed in tension." ;
        rdfs:label                "OutOfPlaneNegative" ;
        IFC4-PSD:definition       "Mechanical properties with respect to out-of-plane load i.e. for function as a plate; compression zone of unbalanced layups is stressed in tension." ;
        IFC4-PSD:definitionAlias  ""@en ;
        IFC4-PSD:ifdguid          "510d2e00d1f011e1800000215ad4efdf" ;
        IFC4-PSD:name             "OutOfPlaneNegative" ;
        IFC4-PSD:nameAlias        "Out Of Plane Negative"@en ;
        IFC4-PSD:propertyType     [ a  IFC4-PSD:TypeComplexProperty ] .

:Pset_MaterialWoodBasedPanel
        a                             IFC4-PSD:PropertySetDef ;
        rdfs:comment                  "This is a collection of mechanical properties related to wood-based materials for panel-like products like plywood or OSB. The propositions given above for wood-based beam materials with respect to anisotropy, strength graduation according to element sizes (especially panel thickness) apply accordingly." ;
        rdfs:label                    "Pset_MaterialWoodBasedPanel" ;
        IFC4-PSD:applicableClass      <http://lbd.arch.rwth-aachen.de/ifcOWL/IFC4#IfcMaterial/Wood> ;
        IFC4-PSD:applicableTypeValue  "IfcMaterial/Wood" ;
        IFC4-PSD:definition           "This is a collection of mechanical properties related to wood-based materials for panel-like products like plywood or OSB. The propositions given above for wood-based beam materials with respect to anisotropy, strength graduation according to element sizes (especially panel thickness) apply accordingly." ;
        IFC4-PSD:definitionAlias      ""@en ;
        IFC4-PSD:ifcVersion           [ a                 IFC4-PSD:IfcVersion ;
                                        IFC4-PSD:version  "IFC4"
                                      ] ;
        IFC4-PSD:name                 "Pset_MaterialWoodBasedPanel" ;
        IFC4-PSD:propertyDef          :p75b4d600d1ef11e1800000215ad4efdf , :p510d2e00d1f011e1800000215ad4efdf , :p7b122080d1ef11e1800000215ad4efdf , :pe52ac580d1ef11e1800000215ad4efdf .

:ApplicableStructuralDesignMethod
        a                   rdf:Property ;
        rdfs:seeAlso        :p75b4d600d1ef11e1800000215ad4efdf ;
        rdfs:subPropertyOf  IFC4-PSD:ApplicableStructuralDesignMethod .

:OutOfPlane  a              rdf:Property ;
        rdfs:seeAlso        :pe52ac580d1ef11e1800000215ad4efdf ;
        rdfs:subPropertyOf  IFC4-PSD:OutOfPlane .
