@prefix :      <https://www.linkedbuildingdata.net/IFC4-PSD/Pset_DoorCommon#> .
@prefix IFC4-PSD: <https://www.linkedbuildingdata.net/IFC4-PSD#> .
@prefix owl:   <http://www.w3.org/2002/07/owl#> .
@prefix rdf:   <http://www.w3.org/1999/02/22-rdf-syntax-ns#> .
@prefix rdfs:  <http://www.w3.org/2000/01/rdf-schema#> .
@prefix IFC4:  <http://lbd.arch.rwth-aachen.de/ifcOWL/IFC4#> .

:p8f98ed80d1dc11e1800000215ad4efdf
        a                         IFC4-PSD:PropertyDef ;
        rdfs:comment              "Indication whether this object is designed to serve as an exit in the case of fire (TRUE) or not (FALSE).\nHere it defines an exit door in accordance to the national building code." ;
        rdfs:label                "FireExit" ;
        IFC4-PSD:definition       "Indication whether this object is designed to serve as an exit in the case of fire (TRUE) or not (FALSE).\nHere it defines an exit door in accordance to the national building code." ;
        IFC4-PSD:definitionAlias  "このオブジェクトが火災時の非常口として設計されているかどうかを示すブーリアン値。ここでは関連する建築基準法における出口ドアとして定義している。"@ja-JP , "Angabe, ob die Tür ein Notausgang gemäß der nationalen oder regionalen Brandschutzverordnung ist (JA), oder nicht (NEIN).."@de-DE , "Indique si cet objet est conçu pour servir de sortie en cas d'incendie (VRAI) ou non (FAUX). Définition de la sortie de secours selon le Code National."@fr-FR , ""@en , "表示该构件是否设计为火灾时的紧急出口。\n该属性的依据为国家建筑规范。"@zh-CN ;
        IFC4-PSD:ifdguid          "8f98ed80d1dc11e1800000215ad4efdf" ;
        IFC4-PSD:name             "FireExit" ;
        IFC4-PSD:nameAlias        "Fire Exit"@en , "Notausgang"@de-DE , "非常口区分"@ja-JP , "是否为紧急出口"@zh-CN , "Sortie Secours"@fr-FR ;
        IFC4-PSD:propertyType     [ a                  IFC4-PSD:TypePropertySingleValue ;
                                    IFC4-PSD:dataType  IFC4:IfcBoolean
                                  ] .

:Infiltration  a            rdf:Property ;
        rdfs:seeAlso        :p23b68500d1dc11e1800000215ad4efdf ;
        rdfs:subPropertyOf  IFC4-PSD:Infiltration .

:WaterTightnessRating
        a                   rdf:Property ;
        rdfs:seeAlso        :p5030f04224d94c74aba753294170b227 ;
        rdfs:subPropertyOf  IFC4-PSD:WaterTightnessRating .

:p2795d780d1db11e1800000215ad4efdf
        a                         IFC4-PSD:PropertyDef ;
        rdfs:comment              "Reference ID for this specified type in this project (e.g. type 'A-1'), Also referred to as \"construction type\". It should be provided as an alternative to the name of the \"object type\", if the software does not support object types." ;
        rdfs:label                "Reference" ;
        IFC4-PSD:definition       "Reference ID for this specified type in this project (e.g. type 'A-1'), Also referred to as \"construction type\". It should be provided as an alternative to the name of the \"object type\", if the software does not support object types." ;
        IFC4-PSD:definitionAlias  "このプロジェクトにおける参照記号(例：A-1)。分類コードではなく内部で使用されるプロジェクトタイプとして使用されるもの。"@ja-JP , "若未采用已知的分类系统，则该属性为该项目中该类型构件的参考编号（例如，类型A-1）。"@zh-CN , ""@en , "Référence à l'identifiant d'un type spécifié dans le contexte du projet (exemple : \"type A1\") pour désigner un \"type de construction\". Une alternative au nom d'un objet type lorsque les objets types ne sont pas gérés par le logiciel."@fr-FR , "Bezeichnung zur Zusammenfassung gleichartiger Bauteile zu einem Bauteiltyp (auch Konstruktionstyp genannt). Alternativ zum Namen des \"Typobjekts\", insbesondere wenn die Software keine Typen unterstützt."@de-DE ;
        IFC4-PSD:ifdguid          "2795d780d1db11e1800000215ad4efdf" ;
        IFC4-PSD:name             "Reference" ;
        IFC4-PSD:nameAlias        "参照記号"@ja-JP , "Bauteiltyp"@de-DE , "参考号"@zh-CN , "Reference"@en , "Reference"@fr-FR ;
        IFC4-PSD:propertyType     [ a                  IFC4-PSD:TypePropertySingleValue ;
                                    IFC4-PSD:dataType  IFC4:IfcIdentifier
                                  ] .

:pda9b78dfa88b4538887d4c597a1059dd
        a                      IFC4-PSD:PropertyDef ;
        rdfs:comment           "Mechanical load rating for this object.\nIt is provided according to the national building code." ;
        rdfs:label             "MechanicalLoadRating" ;
        IFC4-PSD:definition    "Mechanical load rating for this object.\nIt is provided according to the national building code." ;
        IFC4-PSD:ifdguid       "da9b78dfa88b4538887d4c597a1059dd" ;
        IFC4-PSD:name          "MechanicalLoadRating" ;
        IFC4-PSD:propertyType  [ a                  IFC4-PSD:TypePropertySingleValue ;
                                 IFC4-PSD:dataType  IFC4:IfcLabel
                               ] .

:SmokeStop  a               rdf:Property ;
        rdfs:seeAlso        :pcec73e80d1dc11e1800000215ad4efdf ;
        rdfs:subPropertyOf  IFC4-PSD:SmokeStop .

:p5030f04224d94c74aba753294170b227
        a                      IFC4-PSD:PropertyDef ;
        rdfs:comment           "Water tightness rating for this object.\nIt is provided according to the national building code." ;
        rdfs:label             "WaterTightnessRating" ;
        IFC4-PSD:definition    "Water tightness rating for this object.\nIt is provided according to the national building code." ;
        IFC4-PSD:ifdguid       "5030f04224d94c74aba753294170b227" ;
        IFC4-PSD:name          "WaterTightnessRating" ;
        IFC4-PSD:propertyType  [ a                  IFC4-PSD:TypePropertySingleValue ;
                                 IFC4-PSD:dataType  IFC4:IfcLabel
                               ] .

:DurabilityRating  a        rdf:Property ;
        rdfs:seeAlso        :pcde1dd00d1db11e1800000215ad4efdf ;
        rdfs:subPropertyOf  IFC4-PSD:DurabilityRating .

:pcde1dd00d1db11e1800000215ad4efdf
        a                         IFC4-PSD:PropertyDef ;
        rdfs:comment              "Durability against mechanical stress. It is given according to the national code or regulation." ;
        rdfs:label                "DurabilityRating" ;
        IFC4-PSD:definition       "Durability against mechanical stress. It is given according to the national code or regulation." ;
        IFC4-PSD:definitionAlias  ""@en , "Mechanische Widerstandsfähigkeit gegen immer wiederkehrende Bewegungen und Einflüsse gemäß der nationalen oder regionalen Richtlinie."@de-DE , "Durabilité au stress mécanique, selon une classification ou règlementation nationale."@fr-FR ;
        IFC4-PSD:ifdguid          "cde1dd00d1db11e1800000215ad4efdf" ;
        IFC4-PSD:name             "DurabilityRating" ;
        IFC4-PSD:nameAlias        "Beanspruchungsklasse"@de-DE , "Durabilité"@fr-FR , "Durability Rating"@en ;
        IFC4-PSD:propertyType     [ a                  IFC4-PSD:TypePropertySingleValue ;
                                    IFC4-PSD:dataType  IFC4:IfcLabel
                                  ] .

:pbeaf5f00d1dc11e1800000215ad4efdf
        a                         IFC4-PSD:PropertyDef ;
        rdfs:comment              "Indication whether this object is designed to close automatically after use (TRUE) or not (FALSE)." ;
        rdfs:label                "SelfClosing" ;
        IFC4-PSD:definition       "Indication whether this object is designed to close automatically after use (TRUE) or not (FALSE)." ;
        IFC4-PSD:definitionAlias  "Indique si cet objet est conçu pour une fermeture automatique après usage (VRAI) ou non (FAUX)"@fr-FR , "Angabe, ob die Tür sicher und selbständig nach der Benutzung durch einen Türschließer schließt (Ja) oder nicht (NEIN)."@de-DE , "表示该构件是否设计为自动关闭。"@zh-CN , "このドアが自動的に閉まる機能を有するかどうかのブーリアン値。"@ja-JP , ""@en ;
        IFC4-PSD:ifdguid          "beaf5f00d1dc11e1800000215ad4efdf" ;
        IFC4-PSD:name             "SelfClosing" ;
        IFC4-PSD:nameAlias        "Selbstschliessend"@de-DE , "Self Closing"@en , "是否自动关闭"@zh-CN , "自動ドア閉機能区分"@ja-JP , "FermetureAutomatique"@fr-FR ;
        IFC4-PSD:propertyType     [ a                  IFC4-PSD:TypePropertySingleValue ;
                                    IFC4-PSD:dataType  IFC4:IfcBoolean
                                  ] .

:p42b51700d1dc11e1800000215ad4efdf
        a                         IFC4-PSD:PropertyDef ;
        rdfs:comment              "Thermal transmittance coefficient (U-Value) of a material.\nIt applies to the total door construction." ;
        rdfs:label                "ThermalTransmittance" ;
        IFC4-PSD:definition       "Thermal transmittance coefficient (U-Value) of a material.\nIt applies to the total door construction." ;
        IFC4-PSD:definitionAlias  "Coefficient de transmission thermique (U) d'un matériau. Il s'applique à l'ensemble de la porte."@fr-FR , ""@en , "材料的导热系数（U值）。\n适用于门的整体结构。"@zh-CN , "Wärmedurchgangskoeffizient (U-Wert) der Materialschichten.\nHier der Gesamtwärmedurchgangskoeffizient der Tür."@de-DE , "熱貫流率U値。"@ja-JP ;
        IFC4-PSD:ifdguid          "42b51700d1dc11e1800000215ad4efdf" ;
        IFC4-PSD:name             "ThermalTransmittance" ;
        IFC4-PSD:nameAlias        "熱貫流率"@ja-JP , "U-Wert"@de-DE , "TransmissionThermique"@fr-FR , "导热系数"@zh-CN , "Thermal Transmittance"@en ;
        IFC4-PSD:propertyType     [ a                  IFC4-PSD:TypePropertySingleValue ;
                                    IFC4-PSD:dataType  IFC4:IfcThermalTransmittanceMeasure
                                  ] .

:AcousticRating  a          rdf:Property ;
        rdfs:seeAlso        :p95420380d1db11e1800000215ad4efdf ;
        rdfs:subPropertyOf  IFC4-PSD:AcousticRating .

:FireExit  a                rdf:Property ;
        rdfs:seeAlso        :p8f98ed80d1dc11e1800000215ad4efdf ;
        rdfs:subPropertyOf  IFC4-PSD:FireExit .

:MechanicalLoadRating
        a                   rdf:Property ;
        rdfs:seeAlso        :pda9b78dfa88b4538887d4c597a1059dd ;
        rdfs:subPropertyOf  IFC4-PSD:MechanicalLoadRating .

:ThermalTransmittance
        a                   rdf:Property ;
        rdfs:seeAlso        :p42b51700d1dc11e1800000215ad4efdf ;
        rdfs:subPropertyOf  IFC4-PSD:ThermalTransmittance .

:p23b68500d1dc11e1800000215ad4efdf
        a                         IFC4-PSD:PropertyDef ;
        rdfs:comment              "Infiltration flowrate of outside air for the filler object based on the area of the filler object at a pressure level of 50 Pascals. It shall be used, if the length of all joints is unknown." ;
        rdfs:label                "Infiltration" ;
        IFC4-PSD:definition       "Infiltration flowrate of outside air for the filler object based on the area of the filler object at a pressure level of 50 Pascals. It shall be used, if the length of all joints is unknown." ;
        IFC4-PSD:definitionAlias  "Taux d'infiltration de l'air extérieur lorsqu'on soumet la porte à une pression de 50 pascals. Cette valeur sera utilisée si la longueur des joints n'est pas connue."@fr-FR , ""@en , "Luftaustausch über die Fugen der geschlossenen Tür  (Q-Wert). Gibt die Luftdurchlässigkeit der gesamten Tür bei einem Luftdruckniveau von 50 Pascal an."@de-DE ;
        IFC4-PSD:ifdguid          "23b68500d1dc11e1800000215ad4efdf" ;
        IFC4-PSD:name             "Infiltration" ;
        IFC4-PSD:nameAlias        "TauxInfiltration"@fr-FR , "Luftdurchlässigkeit"@de-DE , "Infiltration"@en ;
        IFC4-PSD:propertyType     [ a                  IFC4-PSD:TypePropertySingleValue ;
                                    IFC4-PSD:dataType  IFC4:IfcVolumetricFlowRateMeasure
                                  ] .

:p32e90300d1db11e1800000215ad4efdf
        a                         IFC4-PSD:PropertyDef ;
        rdfs:comment              "Status of the element, predominately used in renovation or retrofitting projects. The status can be assigned to as \"New\" - element designed as new addition, \"Existing\" - element exists and remains, \"Demolish\" - element existed but is to be demolished,  \"Temporary\" - element will exists only temporary (like a temporary support structure)." ;
        rdfs:label                "Status" ;
        IFC4-PSD:definition       "Status of the element, predominately used in renovation or retrofitting projects. The status can be assigned to as \"New\" - element designed as new addition, \"Existing\" - element exists and remains, \"Demolish\" - element existed but is to be demolished,  \"Temporary\" - element will exists only temporary (like a temporary support structure)." ;
        IFC4-PSD:definitionAlias  ""@en , "要素（主にリノベーションまたは改修プロジェクトにおいて）の状態。 状態は、「新規(New)」－新しく追加される要素。「既存」－要素は存在し、かつ残りもの。「破壊」－要素は存在したが、廃棄されるもの。「一時的」－一時的に存在する要素（一時的にサポートしている構造のようなもの）。"@ja-JP , "Statut de l'élément, principalement utilisé dans les projets de rénovation et de réhabilitation. Le statut a pour valeur NOUVEAU pour un nouvel élément, EXISTANT pour un élément existant qui est conservé, DEMOLI pour un élément existant à démolir et TEMPORAIRE pour un élément temporaire (comme une structure support provisoire)."@fr-FR , "Status bzw. Phase des Bauteils insbesondere beim Bauen im Bestand. \"Neu\" (new) neues Bauteil als Ergänzung, \"Bestand\" (existing) bestehendes Bauteil, dass erhalten bleibt, \"Abbruch\" (demolish) Bauteil, das abgebrochen wird, \"Temporär\" (temporary) Bauteil und andere Bauelemente, die vorübergehend eingebaut werden (wie Abstützungen, etc.)"@de-DE ;
        IFC4-PSD:ifdguid          "32e90300d1db11e1800000215ad4efdf" ;
        IFC4-PSD:name             "Status" ;
        IFC4-PSD:nameAlias        "Statut"@fr-FR , "Status"@en , "Status"@de-DE , "状態"@ja-JP ;
        IFC4-PSD:propertyType     [ a                  IFC4-PSD:TypePropertyEnumeratedValue ;
                                    IFC4-PSD:enumItem  "NEW" , "EXISTING" , "DEMOLISH" , "TEMPORARY" , "OTHER" , "NOTKNOWN" , "UNSET"
                                  ] .

:p9be0892ff9324135bdafcd98782a64ff
        a                      IFC4-PSD:PropertyDef ;
        rdfs:comment           "Wind load resistance rating for this object.\nIt is provided according to the national building code." ;
        rdfs:label             "WindLoadRating" ;
        IFC4-PSD:definition    "Wind load resistance rating for this object.\nIt is provided according to the national building code." ;
        IFC4-PSD:ifdguid       "9be0892ff9324135bdafcd98782a64ff" ;
        IFC4-PSD:name          "WindLoadRating" ;
        IFC4-PSD:propertyType  [ a                  IFC4-PSD:TypePropertySingleValue ;
                                 IFC4-PSD:dataType  IFC4:IfcLabel
                               ] .

:HandicapAccessible  a      rdf:Property ;
        rdfs:seeAlso        :p76903c80d1dc11e1800000215ad4efdf ;
        rdfs:subPropertyOf  IFC4-PSD:HandicapAccessible .

:p5d878b80d1dc11e1800000215ad4efdf
        a                         IFC4-PSD:PropertyDef ;
        rdfs:comment              "Fraction of the glazing area relative to the total area of the filling element. \nIt shall be used, if the glazing area is not given separately for all panels within the filling element." ;
        rdfs:label                "GlazingAreaFraction" ;
        IFC4-PSD:definition       "Fraction of the glazing area relative to the total area of the filling element. \nIt shall be used, if the glazing area is not given separately for all panels within the filling element." ;
        IFC4-PSD:definitionAlias  ""@en , "Part de surface de vitrage par rapport à la surface totale de l'élément de remplissage. Doit être utilisée si la surface de vitrage n'est pas donnée séparément pour tous les panneaux occupant l'ouverture."@fr-FR , "Anteil der verglasten Fläche an der Gesamtfläche der Tür."@de-DE ;
        IFC4-PSD:ifdguid          "5d878b80d1dc11e1800000215ad4efdf" ;
        IFC4-PSD:name             "GlazingAreaFraction" ;
        IFC4-PSD:nameAlias        "Glasflächenanteil"@de-DE , "FractionSurfaceVitree"@fr-FR , "Glazing Area Fraction"@en ;
        IFC4-PSD:propertyType     [ a                  IFC4-PSD:TypePropertySingleValue ;
                                    IFC4-PSD:dataType  IFC4:IfcPositiveRatioMeasure
                                  ] .

:Pset_DoorCommon  a                   IFC4-PSD:PropertySetDef ;
        rdfs:comment                  "Properties common to the definition of all occurrences of IfcDoor." ;
        rdfs:label                    "Pset_DoorCommon" ;
        IFC4-PSD:applicableClass      IFC4:IfcDoor ;
        IFC4-PSD:applicableTypeValue  "IfcDoor" ;
        IFC4-PSD:definition           "Properties common to the definition of all occurrences of IfcDoor." ;
        IFC4-PSD:definitionAlias      "所有IfcDoor实例的定义中通用的属性。"@zh-CN , ""@en , "Définition de l'IAI : propriétés communes à la définition de toutes les instances de la classe IfcDoor"@fr-FR , "IfcDoor(ドア)オブジェクトに関する共通プロパティセット定義。"@ja-JP ;
        IFC4-PSD:ifcVersion           [ a                 IFC4-PSD:IfcVersion ;
                                        IFC4-PSD:version  "IFC4"
                                      ] ;
        IFC4-PSD:name                 "Pset_DoorCommon" ;
        IFC4-PSD:propertyDef          :p42b51700d1dc11e1800000215ad4efdf , :p9be0892ff9324135bdafcd98782a64ff , :p2795d780d1db11e1800000215ad4efdf , :p7ba0bc00d1db11e1800000215ad4efdf , :p23b68500d1dc11e1800000215ad4efdf , :p76903c80d1dc11e1800000215ad4efdf , :p5030f04224d94c74aba753294170b227 , :pbeaf5f00d1dc11e1800000215ad4efdf , :p32e90300d1db11e1800000215ad4efdf , :p95420380d1db11e1800000215ad4efdf , :p5d878b80d1dc11e1800000215ad4efdf , :pcde1dd00d1db11e1800000215ad4efdf , :p0aadd400d1dc11e1800000215ad4efdf , :pcec73e80d1dc11e1800000215ad4efdf , :paa6b6200d1dc11e1800000215ad4efdf , :pda9b78dfa88b4538887d4c597a1059dd , :pec47d880d1db11e1800000215ad4efdf , :pb4409580d1db11e1800000215ad4efdf , :p8f98ed80d1dc11e1800000215ad4efdf .

:WindLoadRating  a          rdf:Property ;
        rdfs:seeAlso        :p9be0892ff9324135bdafcd98782a64ff ;
        rdfs:subPropertyOf  IFC4-PSD:WindLoadRating .

:paa6b6200d1dc11e1800000215ad4efdf
        a                         IFC4-PSD:PropertyDef ;
        rdfs:comment              "Indication whether this object has an automatic drive to operate it (TRUE) or no drive (FALSE)" ;
        rdfs:label                "HasDrive" ;
        IFC4-PSD:definition       "Indication whether this object has an automatic drive to operate it (TRUE) or no drive (FALSE)" ;
        IFC4-PSD:definitionAlias  ""@en , "Angabe, ob dieses Bauteil einen automatischen Antrieb zum Öffnen und Schließen besitzt (JA) oder nicht (NEIN)."@de-DE ;
        IFC4-PSD:ifdguid          "aa6b6200d1dc11e1800000215ad4efdf" ;
        IFC4-PSD:name             "HasDrive" ;
        IFC4-PSD:nameAlias        "Has Drive"@en , "Antrieb"@de-DE ;
        IFC4-PSD:propertyType     [ a                  IFC4-PSD:TypePropertySingleValue ;
                                    IFC4-PSD:dataType  IFC4:IfcBoolean
                                  ] .

:p95420380d1db11e1800000215ad4efdf
        a                         IFC4-PSD:PropertyDef ;
        rdfs:comment              "Acoustic rating for this object.\nIt is provided according to the national building code. It indicates the sound transmission resistance of this object by an index ratio (instead of providing full sound absorbtion values)." ;
        rdfs:label                "AcousticRating" ;
        IFC4-PSD:definition       "Acoustic rating for this object.\nIt is provided according to the national building code. It indicates the sound transmission resistance of this object by an index ratio (instead of providing full sound absorbtion values)." ;
        IFC4-PSD:definitionAlias  "遮音等級情報。関連する建築基準法を参照。"@ja-JP , ""@en , "该构件的隔音等级。\n该属性的依据为国家建筑规范。为表示该构件隔音效果的比率（而不是完全吸收声音的值）。"@zh-CN , "Schallschutzklasse gemäß der nationalen oder regionalen Richtlinie die als Mindestanforderung für die Schalldämmung der Tür gewährleistet sein muss."@de-DE , "Classement acoustique de cet objet. Donné selon le Code National du Bâtiment. Il indique la résistance à la transmission du son de cet objet par une valeur de référence (au lieu de fournir les valeurs totales d'absorption du son)."@fr-FR ;
        IFC4-PSD:ifdguid          "95420380d1db11e1800000215ad4efdf" ;
        IFC4-PSD:name             "AcousticRating" ;
        IFC4-PSD:nameAlias        "遮音等級"@ja-JP , "IsolationAcoustique"@fr-FR , "Acoustic Rating"@en , "隔音等级"@zh-CN , "Schallschutzklasse"@de-DE ;
        IFC4-PSD:propertyType     [ a                  IFC4-PSD:TypePropertySingleValue ;
                                    IFC4-PSD:dataType  IFC4:IfcLabel
                                  ] .

:Status  a                  rdf:Property ;
        rdfs:seeAlso        :p32e90300d1db11e1800000215ad4efdf ;
        rdfs:subPropertyOf  IFC4-PSD:Status .

:p0aadd400d1dc11e1800000215ad4efdf
        a                         IFC4-PSD:PropertyDef ;
        rdfs:comment              "Indication whether the element is designed for use in the exterior (TRUE) or not (FALSE). If (TRUE) it is an external element and faces the outside of the building." ;
        rdfs:label                "IsExternal" ;
        IFC4-PSD:definition       "Indication whether the element is designed for use in the exterior (TRUE) or not (FALSE). If (TRUE) it is an external element and faces the outside of the building." ;
        IFC4-PSD:definitionAlias  "Angabe, ob dieses Bauteil ein Aussenbauteil ist (JA) oder ein Innenbauteil (NEIN). Als Aussenbauteil grenzt es an den Aussenraum (oder Erdreich, oder Wasser)."@de-DE , "外部の部材かどうかを示すブーリアン値。もしTRUEの場合、外部の部材で建物の外側に面している。"@ja-JP , "表示该图元是否设计为外部构件。若是，则该图元为外部图元，朝向建筑物的外部。"@zh-CN , ""@en , "Indique si l'élément est conçu pour être utilisé à l'extérieur (VRAI) ou non (FAUX). Si VRAI, c'est un élément extérieur qui donne sur l'extérieur du bâtiment."@fr-FR ;
        IFC4-PSD:ifdguid          "0aadd400d1dc11e1800000215ad4efdf" ;
        IFC4-PSD:name             "IsExternal" ;
        IFC4-PSD:nameAlias        "Is External"@en , "EstExterieur"@fr-FR , "外部区分"@ja-JP , "Außenbauteil"@de-DE , "是否外部构件"@zh-CN ;
        IFC4-PSD:propertyType     [ a                  IFC4-PSD:TypePropertySingleValue ;
                                    IFC4-PSD:dataType  IFC4:IfcBoolean
                                  ] .

:pb4409580d1db11e1800000215ad4efdf
        a                         IFC4-PSD:PropertyDef ;
        rdfs:comment              "Index based rating system indicating security level.\nIt is giving according to the national building code." ;
        rdfs:label                "SecurityRating" ;
        IFC4-PSD:definition       "Index based rating system indicating security level.\nIt is giving according to the national building code." ;
        IFC4-PSD:definitionAlias  "Système de classification par indices, indiquant le niveau de sécurité."@fr-FR , ""@en , "表示安全程度的参考性等级。\n该属性的依据为国家建筑规范。"@zh-CN , "防犯等級情報。関連する基準を参照。"@ja-JP , "Widerstandsklasse für den Einbruchschutz gemäß der nationalen oder regionalen Richtlinie die als Mindestanforderung für die Einbruchhemmung der Tür gewährleistet sein muss."@de-DE ;
        IFC4-PSD:ifdguid          "b4409580d1db11e1800000215ad4efdf" ;
        IFC4-PSD:name             "SecurityRating" ;
        IFC4-PSD:nameAlias        "Security Rating"@en , "防犯等級"@ja-JP , "Widerstandsklasse"@de-DE , "安全等级"@zh-CN , "NiveauSecurite"@fr-FR ;
        IFC4-PSD:propertyType     [ a                  IFC4-PSD:TypePropertySingleValue ;
                                    IFC4-PSD:dataType  IFC4:IfcLabel
                                  ] .

:IsExternal  a              rdf:Property ;
        rdfs:seeAlso        :p0aadd400d1dc11e1800000215ad4efdf ;
        rdfs:subPropertyOf  IFC4-PSD:IsExternal .

:pcec73e80d1dc11e1800000215ad4efdf
        a                         IFC4-PSD:PropertyDef ;
        rdfs:comment              "Indication whether the object is designed to provide a smoke stop (TRUE) or not (FALSE)." ;
        rdfs:label                "SmokeStop" ;
        IFC4-PSD:definition       "Indication whether the object is designed to provide a smoke stop (TRUE) or not (FALSE)." ;
        IFC4-PSD:definitionAlias  "このドアが煙を止める機能を有するかどうかのブーリアン値。"@ja-JP , "Angabe, ob die Tür einen Rauchschutz gemäß der nationalen oder regionalen Brandschutzverordnung gewährleistet (JA) oder nicht (NEIN). Rauchschutztüren müssen selbstschließend sein."@de-DE , "表示该构件是否设计为防烟。"@zh-CN , ""@en , "Indique si la porte est conçue pour une fonction coupe-fumée (VRAI) ou non (FAUX)"@fr-FR ;
        IFC4-PSD:ifdguid          "cec73e80d1dc11e1800000215ad4efdf" ;
        IFC4-PSD:name             "SmokeStop" ;
        IFC4-PSD:nameAlias        "Rauchschutz"@de-DE , "煙止め機能区分"@ja-JP , "CoupeFumee"@fr-FR , "Smoke Stop"@en , "是否防烟"@zh-CN ;
        IFC4-PSD:propertyType     [ a                  IFC4-PSD:TypePropertySingleValue ;
                                    IFC4-PSD:dataType  IFC4:IfcBoolean
                                  ] .

:FireRating  a              rdf:Property ;
        rdfs:seeAlso        :p7ba0bc00d1db11e1800000215ad4efdf ;
        rdfs:subPropertyOf  IFC4-PSD:FireRating .

:SecurityRating  a          rdf:Property ;
        rdfs:seeAlso        :pb4409580d1db11e1800000215ad4efdf ;
        rdfs:subPropertyOf  IFC4-PSD:SecurityRating .

<https://www.linkedbuildingdata.net/IFC4-PSD/Pset_DoorCommon>
        a                owl:Ontology ;
        owl:imports      <http://lbd.arch.rwth-aachen.de/ifcOWL/IFC4-PSD> ;
        owl:versionInfo  "Created with BIM-Bots PSD Repository" .

:p76903c80d1dc11e1800000215ad4efdf
        a                         IFC4-PSD:PropertyDef ;
        rdfs:comment              "Indication that this object is designed to be accessible by the handicapped. \nIt is giving according to the requirements of the national building code." ;
        rdfs:label                "HandicapAccessible" ;
        IFC4-PSD:definition       "Indication that this object is designed to be accessible by the handicapped. \nIt is giving according to the requirements of the national building code." ;
        IFC4-PSD:definitionAlias  "Angabe, ob die Tür behindertengerecht gemäß der nationalen oder regionalen Verordnung ist (JA), oder nicht (NEIN)."@de-DE , ""@en , "Indique que cet objet est conçu pour être accessible aux handicapés. Indication donnée selon le Code National."@fr-FR ;
        IFC4-PSD:ifdguid          "76903c80d1dc11e1800000215ad4efdf" ;
        IFC4-PSD:name             "HandicapAccessible" ;
        IFC4-PSD:nameAlias        "Handicap Accessible"@en , "AccessibleHandicapes"@fr-FR , "Behindertengerecht"@de-DE ;
        IFC4-PSD:propertyType     [ a                  IFC4-PSD:TypePropertySingleValue ;
                                    IFC4-PSD:dataType  IFC4:IfcBoolean
                                  ] .

:p7ba0bc00d1db11e1800000215ad4efdf
        a                         IFC4-PSD:PropertyDef ;
        rdfs:comment              "Fire rating for this object. It is given according to the national fire safety code or regulation." ;
        rdfs:label                "FireRating" ;
        IFC4-PSD:definition       "Fire rating for this object. It is given according to the national fire safety code or regulation." ;
        IFC4-PSD:definitionAlias  "Classement au feu de l'élément donné selon la classification nationale de sécurité incendie."@fr-FR , "主要な耐火等級。関連する建築基準法、消防法などの国家基準を参照。"@ja-JP , "Feuerwiderstandsklasse für den Brandschutz gemäß der nationalen oder regionalen Richtlinie die für den Brandschutz der Brandschutztür gewährleistet werden muss."@de-DE , ""@en , "该构件的防火等级。\n该属性的依据为国家防火安全分级。"@zh-CN ;
        IFC4-PSD:ifdguid          "7ba0bc00d1db11e1800000215ad4efdf" ;
        IFC4-PSD:name             "FireRating" ;
        IFC4-PSD:nameAlias        "防火等级"@zh-CN , "Fire Rating"@en , "耐火等級"@ja-JP , "Feuerwiderstandsklasse"@de-DE , "ResistanceAuFeu"@fr-FR ;
        IFC4-PSD:propertyType     [ a                  IFC4-PSD:TypePropertySingleValue ;
                                    IFC4-PSD:dataType  IFC4:IfcLabel
                                  ] .

:GlazingAreaFraction  a     rdf:Property ;
        rdfs:seeAlso        :p5d878b80d1dc11e1800000215ad4efdf ;
        rdfs:subPropertyOf  IFC4-PSD:GlazingAreaFraction .

:Reference  a               rdf:Property ;
        rdfs:seeAlso        :p2795d780d1db11e1800000215ad4efdf ;
        rdfs:subPropertyOf  IFC4-PSD:Reference .

:HasDrive  a                rdf:Property ;
        rdfs:seeAlso        :paa6b6200d1dc11e1800000215ad4efdf ;
        rdfs:subPropertyOf  IFC4-PSD:HasDrive .

:HygrothermalRating  a      rdf:Property ;
        rdfs:seeAlso        :pec47d880d1db11e1800000215ad4efdf ;
        rdfs:subPropertyOf  IFC4-PSD:HygrothermalRating .

:SelfClosing  a             rdf:Property ;
        rdfs:seeAlso        :pbeaf5f00d1dc11e1800000215ad4efdf ;
        rdfs:subPropertyOf  IFC4-PSD:SelfClosing .

:pec47d880d1db11e1800000215ad4efdf
        a                         IFC4-PSD:PropertyDef ;
        rdfs:comment              "Resistence against hygrothermal impact from different temperatures and humidities inside and outside. It is given according to the national code or regulation." ;
        rdfs:label                "HygrothermalRating" ;
        IFC4-PSD:definition       "Resistence against hygrothermal impact from different temperatures and humidities inside and outside. It is given according to the national code or regulation." ;
        IFC4-PSD:definitionAlias  ""@en , "Hygrothermische Widerstandsfähigkeit gegen Temperatur- und Feuchteunterschiede gemäß der nationalen oder regionalen Richtlinie als Mindestanforderung gegen die Verformung der Tür."@de-DE , "Résistance à l'impact hygrothermique des différences de température et d'humidité entre l'intérieur et l'extérieur, selon une classification ou règlementation nationale."@fr-FR ;
        IFC4-PSD:ifdguid          "ec47d880d1db11e1800000215ad4efdf" ;
        IFC4-PSD:name             "HygrothermalRating" ;
        IFC4-PSD:nameAlias        "Résistance hygrothermique"@fr-FR , "Hygrothermal Rating"@en , "Klimaklasse"@de-DE ;
        IFC4-PSD:propertyType     [ a                  IFC4-PSD:TypePropertySingleValue ;
                                    IFC4-PSD:dataType  IFC4:IfcLabel
                                  ] .
