@prefix :      <https://www.linkedbuildingdata.net/IFC4-PSD/Pset_ControllerTypeMultiPosition#> .
@prefix IFC4-PSD: <https://www.linkedbuildingdata.net/IFC4-PSD#> .
@prefix rdf:   <http://www.w3.org/1999/02/22-rdf-syntax-ns#> .
@prefix owl:   <http://www.w3.org/2002/07/owl#> .
@prefix rdfs:  <http://www.w3.org/2000/01/rdf-schema#> .
@prefix IFC4:  <http://lbd.arch.rwth-aachen.de/ifcOWL/IFC4#> .

:Labels  a                  rdf:Property ;
        rdfs:seeAlso        :p89e7db80d1cd11e1800000215ad4efdf ;
        rdfs:subPropertyOf  IFC4-PSD:Labels .

:Value  a                   rdf:Property ;
        rdfs:seeAlso        :p95d39d80d1cd11e1800000215ad4efdf ;
        rdfs:subPropertyOf  IFC4-PSD:Value .

:Range  a                   rdf:Property ;
        rdfs:seeAlso        :p910ee980d1cd11e1800000215ad4efdf ;
        rdfs:subPropertyOf  IFC4-PSD:Range .

:Pset_ControllerTypeMultiPosition
        a                             IFC4-PSD:PropertySetDef ;
        rdfs:comment                  "Properties for discrete inputs, outputs, and values within a programmable logic controller. HISTORY: New in IFC4, replaces Pset_MultiStateInput and Pset_MultiStateOutput." ;
        rdfs:label                    "Pset_ControllerTypeMultiPosition" ;
        IFC4-PSD:applicableClass      <http://lbd.arch.rwth-aachen.de/ifcOWL/IFC4#IfcController/MULTIPOSITION> ;
        IFC4-PSD:applicableTypeValue  "IfcController/MULTIPOSITION" ;
        IFC4-PSD:definition           "Properties for discrete inputs, outputs, and values within a programmable logic controller. HISTORY: New in IFC4, replaces Pset_MultiStateInput and Pset_MultiStateOutput." ;
        IFC4-PSD:definitionAlias      ""@en ;
        IFC4-PSD:ifcVersion           [ a                 IFC4-PSD:IfcVersion ;
                                        IFC4-PSD:version  "IFC4"
                                      ] ;
        IFC4-PSD:name                 "Pset_ControllerTypeMultiPosition" ;
        IFC4-PSD:propertyDef          :p89e7db80d1cd11e1800000215ad4efdf , :p7e94b000d1cd11e1800000215ad4efdf , :p910ee980d1cd11e1800000215ad4efdf , :p95d39d80d1cd11e1800000215ad4efdf .

:p910ee980d1cd11e1800000215ad4efdf
        a                         IFC4-PSD:PropertyDef ;
        rdfs:comment              "The physical range of values supported by the device." ;
        rdfs:label                "Range" ;
        IFC4-PSD:definition       "The physical range of values supported by the device." ;
        IFC4-PSD:definitionAlias  ""@en ;
        IFC4-PSD:ifdguid          "910ee980d1cd11e1800000215ad4efdf" ;
        IFC4-PSD:name             "Range" ;
        IFC4-PSD:nameAlias        "Range"@en ;
        IFC4-PSD:propertyType     [ a                  IFC4-PSD:TypePropertyBoundedValue ;
                                    IFC4-PSD:dataType  IFC4:IfcInteger
                                  ] .

<https://www.linkedbuildingdata.net/IFC4-PSD/Pset_ControllerTypeMultiPosition>
        a                owl:Ontology ;
        owl:imports      <http://lbd.arch.rwth-aachen.de/ifcOWL/IFC4-PSD> ;
        owl:versionInfo  "Created with BIM-Bots PSD Repository" .

:p7e94b000d1cd11e1800000215ad4efdf
        a                         IFC4-PSD:PropertyDef ;
        rdfs:comment              "The type of signal modification effected and applicable ports:\n\nINPUT: Controller element is a dedicated input.\nOUTPUT: Controller element is a dedicated output.\nVARIABLE: Controller element is an in-memory variable." ;
        rdfs:label                "ControlType" ;
        IFC4-PSD:definition       "The type of signal modification effected and applicable ports:\n\nINPUT: Controller element is a dedicated input.\nOUTPUT: Controller element is a dedicated output.\nVARIABLE: Controller element is an in-memory variable." ;
        IFC4-PSD:definitionAlias  ""@en ;
        IFC4-PSD:ifdguid          "7e94b000d1cd11e1800000215ad4efdf" ;
        IFC4-PSD:name             "ControlType" ;
        IFC4-PSD:nameAlias        "Control Type"@en ;
        IFC4-PSD:propertyType     [ a                  IFC4-PSD:TypePropertyEnumeratedValue ;
                                    IFC4-PSD:enumItem  "INPUT" , "OUTPUT" , "VARIABLE" , "OTHER" , "NOTKNOWN" , "UNSET"
                                  ] .

:ControlType  a             rdf:Property ;
        rdfs:seeAlso        :p7e94b000d1cd11e1800000215ad4efdf ;
        rdfs:subPropertyOf  IFC4-PSD:ControlType .

:p89e7db80d1cd11e1800000215ad4efdf
        a                         IFC4-PSD:PropertyDef ;
        rdfs:comment              "Table mapping values to labels, where each entry corresponds to an integer within the ValueRange." ;
        rdfs:label                "Labels" ;
        IFC4-PSD:definition       "Table mapping values to labels, where each entry corresponds to an integer within the ValueRange." ;
        IFC4-PSD:definitionAlias  ""@en ;
        IFC4-PSD:ifdguid          "89e7db80d1cd11e1800000215ad4efdf" ;
        IFC4-PSD:name             "Labels" ;
        IFC4-PSD:nameAlias        "Labels"@en ;
        IFC4-PSD:propertyType     [ a                       IFC4-PSD:TypePropertyTableValue ;
                                    IFC4-PSD:definedValue   IFC4:IfcLabel ;
                                    IFC4-PSD:definingValue  IFC4:IfcInteger
                                  ] .

:p95d39d80d1cd11e1800000215ad4efdf
        a                         IFC4-PSD:PropertyDef ;
        rdfs:comment              "The expected range and default value.  The LowerLimitValue and UpperLimitValue must fall within the physical Range." ;
        rdfs:label                "Value" ;
        IFC4-PSD:definition       "The expected range and default value.  The LowerLimitValue and UpperLimitValue must fall within the physical Range." ;
        IFC4-PSD:definitionAlias  ""@en ;
        IFC4-PSD:ifdguid          "95d39d80d1cd11e1800000215ad4efdf" ;
        IFC4-PSD:name             "Value" ;
        IFC4-PSD:nameAlias        "Value"@en ;
        IFC4-PSD:propertyType     [ a                  IFC4-PSD:TypePropertyBoundedValue ;
                                    IFC4-PSD:dataType  IFC4:IfcInteger
                                  ] .
