@prefix :      <https://www.linkedbuildingdata.net/IFC4-PSD/Pset_CoveringCommon#> .
@prefix IFC4-PSD: <https://www.linkedbuildingdata.net/IFC4-PSD#> .
@prefix owl:   <http://www.w3.org/2002/07/owl#> .
@prefix rdf:   <http://www.w3.org/1999/02/22-rdf-syntax-ns#> .
@prefix rdfs:  <http://www.w3.org/2000/01/rdf-schema#> .
@prefix IFC4:  <http://lbd.arch.rwth-aachen.de/ifcOWL/IFC4#> .

:Finish  a                  rdf:Property ;
        rdfs:seeAlso        :p565a8080d1d011e1800000215ad4efdf ;
        rdfs:subPropertyOf  IFC4-PSD:Finish .

:p565a8080d1d011e1800000215ad4efdf
        a                         IFC4-PSD:PropertyDef ;
        rdfs:comment              "Finish selection for this object.\nHere specification of the surface finish for informational purposes." ;
        rdfs:label                "Finish" ;
        IFC4-PSD:definition       "Finish selection for this object.\nHere specification of the surface finish for informational purposes." ;
        IFC4-PSD:definitionAlias  "仕上げ選択に関する情報。表面仕上げに関する仕様。"@ja-JP , ""@en , "Finition de cet objet. Spécification de la finition donnée à titre informatif."@fr-FR , "Oberflächenbehandlung oder Oberflächengüte, wie \"poliert\", \"schalungsrau\", imprägniert."@de-DE , "该构件的表面处理方式。仅供参考。"@zh-CN ;
        IFC4-PSD:ifdguid          "565a8080d1d011e1800000215ad4efdf" ;
        IFC4-PSD:name             "Finish" ;
        IFC4-PSD:nameAlias        "Oberflächengüte"@de-DE , "Finition"@fr-FR , "仕上げ"@ja-JP , "Finish"@en , "表面处理"@zh-CN ;
        IFC4-PSD:propertyType     [ a                  IFC4-PSD:TypePropertySingleValue ;
                                    IFC4-PSD:dataType  IFC4:IfcText
                                  ] .

:AcousticRating  a          rdf:Property ;
        rdfs:seeAlso        :p2e6b1d00d1d011e1800000215ad4efdf ;
        rdfs:subPropertyOf  IFC4-PSD:AcousticRating .

:p50fd3600d1d011e1800000215ad4efdf
        a                         IFC4-PSD:PropertyDef ;
        rdfs:comment              "Thermal transmittance coefficient (U-Value) of an element. \nHere the total thermal transmittance coefficient through the covering (including all materials)." ;
        rdfs:label                "ThermalTransmittance" ;
        IFC4-PSD:definition       "Thermal transmittance coefficient (U-Value) of an element. \nHere the total thermal transmittance coefficient through the covering (including all materials)." ;
        IFC4-PSD:definitionAlias  ""@en , "材料的导热系数（U值）。\n表示穿过该覆盖层的整体导热系数（包括所有材料）。"@zh-CN , "Coefficient de transmission thermique surfacique (U). C'est le coefficient global de transmission thermique à travers le revêtement dans la direction du flux thermique (tous matériaux inclus). Nouvelle propriété de la version 2x4."@fr-FR , "熱貫流率U値。ここではカバリングを通した熱移動の方向における全体の熱還流率を示す。"@ja-JP , "Wärmedurchgangskoeffizient (U-Wert) der Materialschichten.\nHier der Gesamtwärmedurchgangskoeffizient der Bekleidung (für alle Schichten)."@de-DE ;
        IFC4-PSD:ifdguid          "50fd3600d1d011e1800000215ad4efdf" ;
        IFC4-PSD:name             "ThermalTransmittance" ;
        IFC4-PSD:nameAlias        "导热系数"@zh-CN , "Transmission thermique surfacique"@fr-FR , "U-Wert"@de-DE , "熱貫流率"@ja-JP , "Thermal Transmittance"@en ;
        IFC4-PSD:propertyType     [ a                  IFC4-PSD:TypePropertySingleValue ;
                                    IFC4-PSD:dataType  IFC4:IfcThermalTransmittanceMeasure
                                  ] .

:Pset_CoveringCommon  a               IFC4-PSD:PropertySetDef ;
        rdfs:comment                  "Properties common to the definition of all occurrence and type objects of covering" ;
        rdfs:label                    "Pset_CoveringCommon" ;
        IFC4-PSD:applicableClass      IFC4:IfcCovering ;
        IFC4-PSD:applicableTypeValue  "IfcCovering" ;
        IFC4-PSD:definition           "Properties common to the definition of all occurrence and type objects of covering" ;
        IFC4-PSD:definitionAlias      "IfcCoveringオブジェクトに関する共通プロパティセット定義。"@ja-JP , ""@en , "所有IfcCovering实例的定义中通用的属性。"@zh-CN ;
        IFC4-PSD:ifcVersion           [ a                 IFC4-PSD:IfcVersion ;
                                        IFC4-PSD:version  "IFC4"
                                      ] ;
        IFC4-PSD:name                 "Pset_CoveringCommon" ;
        IFC4-PSD:propertyDef          :p14c9d580d1d011e1800000215ad4efdf , :p3460fe00d1d011e1800000215ad4efdf , :p4b9feb80d1d011e1800000215ad4efdf , :p28753c00d1d011e1800000215ad4efdf , :p2e6b1d00d1d011e1800000215ad4efdf , :p39be4880d1d011e1800000215ad4efdf , :p45aa0a80d1d011e1800000215ad4efdf , :p1a272000d1d011e1800000215ad4efdf , :p565a8080d1d011e1800000215ad4efdf , :p50fd3600d1d011e1800000215ad4efdf , :p3f1b9300d1d011e1800000215ad4efdf .

:IsExternal  a              rdf:Property ;
        rdfs:seeAlso        :p4b9feb80d1d011e1800000215ad4efdf ;
        rdfs:subPropertyOf  IFC4-PSD:IsExternal .

:p3460fe00d1d011e1800000215ad4efdf
        a                         IFC4-PSD:PropertyDef ;
        rdfs:comment              "Flammability Rating for this object.\nIt is given according to the national building code that governs the rating of flammability for materials." ;
        rdfs:label                "FlammabilityRating" ;
        IFC4-PSD:definition       "Flammability Rating for this object.\nIt is given according to the national building code that governs the rating of flammability for materials." ;
        IFC4-PSD:definitionAlias  "Angabe zur Entflammbarkeit des Materials gemäß der nationalen oder regionalen Normen."@de-DE , "Classement de l'inflammabilité de l'élément selon la classification nationale de sécurité incendie."@fr-FR , "可燃性等級。当該国の建築法規による。"@ja-JP , ""@en ;
        IFC4-PSD:ifdguid          "3460fe00d1d011e1800000215ad4efdf" ;
        IFC4-PSD:name             "FlammabilityRating" ;
        IFC4-PSD:nameAlias        "Entflammbarkeitsklasse"@de-DE , "可燃性等級"@ja-JP , "Inflammabilité"@fr-FR , "Flammability Rating"@en ;
        IFC4-PSD:propertyType     [ a                  IFC4-PSD:TypePropertySingleValue ;
                                    IFC4-PSD:dataType  IFC4:IfcLabel
                                  ] .

:p14c9d580d1d011e1800000215ad4efdf
        a                         IFC4-PSD:PropertyDef ;
        rdfs:comment              "Reference ID for this specified type in this project (e.g. type 'A-1'), Also referred to as \"construction type\". It should be provided as an alternative to the name of the \"object type\", if the software does not support object types." ;
        rdfs:label                "Reference" ;
        IFC4-PSD:definition       "Reference ID for this specified type in this project (e.g. type 'A-1'), Also referred to as \"construction type\". It should be provided as an alternative to the name of the \"object type\", if the software does not support object types." ;
        IFC4-PSD:definitionAlias  "该项目中该类型构件的参考编号（例如，类型A-1）。"@zh-CN , "Référence à l'identifiant d'un type spécifié dans le contexte du projet (exemple : \"type A1\") pour désigner un \"type de construction\". Une alternative au nom d'un objet type lorsque les objets types ne sont pas gérés par le logiciel."@fr-FR , "このプロジェクトにおける参照記号(例：A-1)"@ja-JP , ""@en , "Bezeichnung zur Zusammenfassung gleichartiger Bauteile zu einem Bauteiltyp (auch Konstruktionstyp genannt). Alternativ zum Namen des \"Typobjekts\", insbesondere wenn die Software keine Typen unterstützt."@de-DE ;
        IFC4-PSD:ifdguid          "14c9d580d1d011e1800000215ad4efdf" ;
        IFC4-PSD:name             "Reference" ;
        IFC4-PSD:nameAlias        "参考号"@zh-CN , "参照記号"@ja-JP , "Bauteiltyp"@de-DE , "Reference"@en , "Référence"@fr-FR ;
        IFC4-PSD:propertyType     [ a                  IFC4-PSD:TypePropertySingleValue ;
                                    IFC4-PSD:dataType  IFC4:IfcIdentifier
                                  ] .

:p39be4880d1d011e1800000215ad4efdf
        a                         IFC4-PSD:PropertyDef ;
        rdfs:comment              "Indication on the fragility of the covering (e.g., under fire conditions).  It is given according to the national building code that might provide a classification for fragility." ;
        rdfs:label                "FragilityRating" ;
        IFC4-PSD:definition       "Indication on the fragility of the covering (e.g., under fire conditions).  It is given according to the national building code that might provide a classification for fragility." ;
        IFC4-PSD:definitionAlias  "脆弱性等級。当該国の建築法規による。"@ja-JP , ""@en , "Indication de la fragilité du revêtement selon une classification nationale."@fr-FR , "Angabe zur Zerbrechlichkeit des Materials (zum Beispiel unter Brandlast oder Erschütterung) gemäß der nationalen oder regionalen Normen."@de-DE ;
        IFC4-PSD:ifdguid          "39be4880d1d011e1800000215ad4efdf" ;
        IFC4-PSD:name             "FragilityRating" ;
        IFC4-PSD:nameAlias        "脆弱性等級"@ja-JP , "Fragilitätsklasse"@de-DE , "Fragilité"@fr-FR , "Fragility Rating"@en ;
        IFC4-PSD:propertyType     [ a                  IFC4-PSD:TypePropertySingleValue ;
                                    IFC4-PSD:dataType  IFC4:IfcLabel
                                  ] .

:SurfaceSpreadOfFlame
        a                   rdf:Property ;
        rdfs:seeAlso        :p3f1b9300d1d011e1800000215ad4efdf ;
        rdfs:subPropertyOf  IFC4-PSD:SurfaceSpreadOfFlame .

:ThermalTransmittance
        a                   rdf:Property ;
        rdfs:seeAlso        :p50fd3600d1d011e1800000215ad4efdf ;
        rdfs:subPropertyOf  IFC4-PSD:ThermalTransmittance .

:p3f1b9300d1d011e1800000215ad4efdf
        a                         IFC4-PSD:PropertyDef ;
        rdfs:comment              "Indication on how the flames spread around the surface,\nIt is given according to the national building code that governs the fire behaviour for materials." ;
        rdfs:label                "SurfaceSpreadOfFlame" ;
        IFC4-PSD:definition       "Indication on how the flames spread around the surface,\nIt is given according to the national building code that governs the fire behaviour for materials." ;
        IFC4-PSD:definitionAlias  "Beschreibung des Brandverhaltens des Bauteils gemäß der nationalen oder regionalen  Brandschutzverordnung."@de-DE , "Indique comment les flammes se propagent sur une surface. Indication donnée selon le Code National du Bâtiment régissant le comportement au feu des matériaux."@fr-FR , ""@en , "火炎表面伝播性。当該国の建築法規による。"@ja-JP ;
        IFC4-PSD:ifdguid          "3f1b9300d1d011e1800000215ad4efdf" ;
        IFC4-PSD:name             "SurfaceSpreadOfFlame" ;
        IFC4-PSD:nameAlias        "Surface Spread Of Flame"@en , "Propagation des flammes en surface"@fr-FR , "Brandverhalten"@de-DE , "火炎表面伝播性"@ja-JP ;
        IFC4-PSD:propertyType     [ a                  IFC4-PSD:TypePropertySingleValue ;
                                    IFC4-PSD:dataType  IFC4:IfcLabel
                                  ] .

:p28753c00d1d011e1800000215ad4efdf
        a                         IFC4-PSD:PropertyDef ;
        rdfs:comment              "Fire rating for this object.\nIt is given according to the national fire safety classification." ;
        rdfs:label                "FireRating" ;
        IFC4-PSD:definition       "Fire rating for this object.\nIt is given according to the national fire safety classification." ;
        IFC4-PSD:definitionAlias  ""@en , "耐火等級。当該国の建築法規による。"@ja-JP , "该构件的防火等级。\n该属性的依据为国家防火安全分级。"@zh-CN , "Feuerwiderstandsklasse gemäß der nationalen oder regionalen Brandschutzverordnung."@de-DE , "Classement au feu de l'élément donné selon la classification nationale de sécurité incendie."@fr-FR ;
        IFC4-PSD:ifdguid          "28753c00d1d011e1800000215ad4efdf" ;
        IFC4-PSD:name             "FireRating" ;
        IFC4-PSD:nameAlias        "防火等级"@zh-CN , "Fire Rating"@en , "Feuerwiderstandsklasse"@de-DE , "耐火等級"@ja-JP , "Résistance au feu"@fr-FR ;
        IFC4-PSD:propertyType     [ a                  IFC4-PSD:TypePropertySingleValue ;
                                    IFC4-PSD:dataType  IFC4:IfcLabel
                                  ] .

:FireRating  a              rdf:Property ;
        rdfs:seeAlso        :p28753c00d1d011e1800000215ad4efdf ;
        rdfs:subPropertyOf  IFC4-PSD:FireRating .

:p45aa0a80d1d011e1800000215ad4efdf
        a                         IFC4-PSD:PropertyDef ;
        rdfs:comment              "Indication whether the object is made from combustible material (TRUE) or not (FALSE)." ;
        rdfs:label                "Combustible" ;
        IFC4-PSD:definition       "Indication whether the object is made from combustible material (TRUE) or not (FALSE)." ;
        IFC4-PSD:definitionAlias  "Angabe ob das Bauteil brennbares Material enthält (WAHR) oder nicht (FALSCH)."@de-DE , "Indique si l'objet est réalisé à partir de matériau combustible (VRAI) ou non (FAUX)."@fr-FR , "表示该构件是否由可燃材料制成。"@zh-CN , ""@en , "この部材が可燃性物質で作られているかどうかを示すブーリアン値。"@ja-JP ;
        IFC4-PSD:ifdguid          "45aa0a80d1d011e1800000215ad4efdf" ;
        IFC4-PSD:name             "Combustible" ;
        IFC4-PSD:nameAlias        "可燃性区分"@ja-JP , "是否可燃"@zh-CN , "Combustible"@fr-FR , "Combustible"@en , "Brennbares Material"@de-DE ;
        IFC4-PSD:propertyType     [ a                  IFC4-PSD:TypePropertySingleValue ;
                                    IFC4-PSD:dataType  IFC4:IfcBoolean
                                  ] .

:FragilityRating  a         rdf:Property ;
        rdfs:seeAlso        :p39be4880d1d011e1800000215ad4efdf ;
        rdfs:subPropertyOf  IFC4-PSD:FragilityRating .

:Reference  a               rdf:Property ;
        rdfs:seeAlso        :p14c9d580d1d011e1800000215ad4efdf ;
        rdfs:subPropertyOf  IFC4-PSD:Reference .

:Status  a                  rdf:Property ;
        rdfs:seeAlso        :p1a272000d1d011e1800000215ad4efdf ;
        rdfs:subPropertyOf  IFC4-PSD:Status .

:p1a272000d1d011e1800000215ad4efdf
        a                         IFC4-PSD:PropertyDef ;
        rdfs:comment              "Status of the element, predominately used in renovation or retrofitting projects. The status can be assigned to as \"New\" - element designed as new addition, \"Existing\" - element exists and remains, \"Demolish\" - element existed but is to be demolished,  \"Temporary\" - element will exists only temporary (like a temporary support structure)." ;
        rdfs:label                "Status" ;
        IFC4-PSD:definition       "Status of the element, predominately used in renovation or retrofitting projects. The status can be assigned to as \"New\" - element designed as new addition, \"Existing\" - element exists and remains, \"Demolish\" - element existed but is to be demolished,  \"Temporary\" - element will exists only temporary (like a temporary support structure)." ;
        IFC4-PSD:definitionAlias  ""@en , "Statut de l'élément, principalement utilisé dans les projets de rénovation et de réhabilitation. Le statut a pour valeur NOUVEAU pour un nouvel élément, EXISTANT pour un élément existant qui est conservé, DEMOLI pour un élément existant à démolir et TEMPORAIRE pour un élément temporaire (comme une structure support provisoire)."@fr-FR , "Status bzw. Phase des Bauteils insbesondere beim Bauen im Bestand. \"Neu\" (new) neues Bauteil als Ergänzung, \"Bestand\" (existing) bestehendes Bauteil, dass erhalten bleibt, \"Abbruch\" (demolish) Bauteil, das abgebrochen wird, \"Temporär\" (temporary) Bauteil und andere Bauelemente, die vorübergehend eingebaut werden (wie Abstützungen, etc.)"@de-DE , "要素（主にリノベーションまたは改修プロジェクトにおいて）の状態。 状態は、「新規(New)」－新しく追加される要素。「既存」－要素は存在し、かつ残りもの。「破壊」－要素は存在したが、廃棄されるもの。「一時的」－一時的に存在する要素（一時的にサポートしている構造のようなもの）。"@ja-JP ;
        IFC4-PSD:ifdguid          "1a272000d1d011e1800000215ad4efdf" ;
        IFC4-PSD:name             "Status" ;
        IFC4-PSD:nameAlias        "Status"@en , "Status"@de-DE , "状態"@ja-JP , "Statut"@fr-FR ;
        IFC4-PSD:propertyType     [ a                  IFC4-PSD:TypePropertyEnumeratedValue ;
                                    IFC4-PSD:enumItem  "NEW" , "EXISTING" , "DEMOLISH" , "TEMPORARY" , "OTHER" , "NOTKNOWN" , "UNSET"
                                  ] .

<https://www.linkedbuildingdata.net/IFC4-PSD/Pset_CoveringCommon>
        a                owl:Ontology ;
        owl:imports      <http://lbd.arch.rwth-aachen.de/ifcOWL/IFC4-PSD> ;
        owl:versionInfo  "Created with BIM-Bots PSD Repository" .

:p2e6b1d00d1d011e1800000215ad4efdf
        a                         IFC4-PSD:PropertyDef ;
        rdfs:comment              "Acoustic rating for this object.\nIt is giving according to the national building code. It indicates the sound transmission resistance of this object by an index ration (instead of providing full sound absorbtion values)." ;
        rdfs:label                "AcousticRating" ;
        IFC4-PSD:definition       "Acoustic rating for this object.\nIt is giving according to the national building code. It indicates the sound transmission resistance of this object by an index ration (instead of providing full sound absorbtion values)." ;
        IFC4-PSD:definitionAlias  ""@en , "Classement acoustique de cet objet. Donné selon le Code National du Bâtiment. Il indique la résistance à la transmission du son de cet objet par une valeur de référence (au lieu de fournir les valeurs totales d'absorption du son)."@fr-FR , "遮音等級。当該国の建築法規による。\nこのオブジェクトの音の透過損失を等級値で示す。"@ja-JP , "Schallschutzklasse gemäß der nationalen oder regionalen Schallschutzverordnung."@de-DE , "该构件的隔音等级。\n该属性的依据为国家建筑规范。为表示该构件隔音效果的比率（而不是完全吸收声音的值）。"@zh-CN ;
        IFC4-PSD:ifdguid          "2e6b1d00d1d011e1800000215ad4efdf" ;
        IFC4-PSD:name             "AcousticRating" ;
        IFC4-PSD:nameAlias        "Acoustic Rating"@en , "遮音等級"@ja-JP , "Schallschutzklasse"@de-DE , "Isolation acoustique"@fr-FR , "隔音等级"@zh-CN ;
        IFC4-PSD:propertyType     [ a                  IFC4-PSD:TypePropertySingleValue ;
                                    IFC4-PSD:dataType  IFC4:IfcLabel
                                  ] .

:Combustible  a             rdf:Property ;
        rdfs:seeAlso        :p45aa0a80d1d011e1800000215ad4efdf ;
        rdfs:subPropertyOf  IFC4-PSD:Combustible .

:p4b9feb80d1d011e1800000215ad4efdf
        a                         IFC4-PSD:PropertyDef ;
        rdfs:comment              "Indication whether the element is designed for use in the exterior (TRUE) or not (FALSE). If (TRUE) it is an external element and faces the outside of the building." ;
        rdfs:label                "IsExternal" ;
        IFC4-PSD:definition       "Indication whether the element is designed for use in the exterior (TRUE) or not (FALSE). If (TRUE) it is an external element and faces the outside of the building." ;
        IFC4-PSD:definitionAlias  "Indique si l'élément est conçu pour être utilisé à l'extérieur (VRAI) ou non (FAUX). Si VRAI, c'est un élément extérieur qui donne sur l'extérieur du bâtiment."@fr-FR , "表示该构件是否设计为外部构件。若是，则该构件为外部构件，朝向建筑物的外侧。"@zh-CN , "Angabe, ob dieser Bekleidung eine Außenbekleidung ist (JA) oder ein Innenbekleidung (NEIN)."@de-DE , "外部の部材かどうかを示すブーリアン値。もしTRUEの場合、外部の部材で建物の外側に面している。"@ja-JP , ""@en ;
        IFC4-PSD:ifdguid          "4b9feb80d1d011e1800000215ad4efdf" ;
        IFC4-PSD:name             "IsExternal" ;
        IFC4-PSD:nameAlias        "外部区分"@ja-JP , "Est extérieur"@fr-FR , "Is External"@en , "是否外部构件"@zh-CN , "Außenbauteil"@de-DE ;
        IFC4-PSD:propertyType     [ a                  IFC4-PSD:TypePropertySingleValue ;
                                    IFC4-PSD:dataType  IFC4:IfcBoolean
                                  ] .

:FlammabilityRating  a      rdf:Property ;
        rdfs:seeAlso        :p3460fe00d1d011e1800000215ad4efdf ;
        rdfs:subPropertyOf  IFC4-PSD:FlammabilityRating .
