# baseURI: http://www.buildingsmart-tech.org/ifcOWL/IFC4-PSD
# imports: http://www.buildingsmart-tech.org/ifcOWL/IFC4
# prefix: PSD 

@base          <http://www.buildingsmart-tech.org/ifcOWL/IFC4-PSD> .
@prefix :      <http://www.buildingsmart-tech.org/ifcOWL/IFC4-PSD#> .
@prefix PSD:   <http://www.buildingsmart-tech.org/ifcOWL/IFC4-PSD#> .
@prefix owl:   <http://www.w3.org/2002/07/owl#> .
@prefix rdf:   <http://www.w3.org/1999/02/22-rdf-syntax-ns#> .
@prefix xsd:   <http://www.w3.org/2001/XMLSchema#> .
@prefix rdfs:  <http://www.w3.org/2000/01/rdf-schema#> .
@prefix IFC4:  <http://www.buildingsmart-tech.org/ifcOWL/IFC4#> .

PSD:InternalRefrigerantVolume
        a             rdf:Property ;
        rdfs:comment  "Internal volume of condenser (refrigerant side)."@en ;
        rdfs:label    "Internal refrigerant volume"@en .

PSD:FrictionLoss  a   rdf:Property ;
        rdfs:comment  "The pressure loss due to friction per unit length. (Data type = PressureMeasure/LengthMeasure)"@en ;
        rdfs:label    "FrictionLoss"@en .

PSD:TreadLengthAtOffset
        a           rdf:Property ;
        rdfs:label  "Tread length at offset"@en .

PSD:VentilationAirFlowrate
        a             rdf:Property ;
        rdfs:comment  "Ventilation outside air requirement for the space."@en ;
        rdfs:label    "VentilationAirFlowrate"@en .

PSD:IntegratedLightingType
        a             rdf:Property ;
        rdfs:comment  "Integrated lighting in cooled beam."@en ;
        rdfs:label    "IntegratedLightingType"@en .

PSD:RequiredSlope  a  rdf:Property ;
        rdfs:comment  "Required sloping angle of the object  - relative to horizontal (0.0 degrees).\\nRequired maximum slope for the passageway according to the applicable building code or additional requirements."@en ;
        rdfs:label    "Required slope"@en .

PSD:NosingLength  a  rdf:Property ;
        rdfs:label  "Nosing length"@en .

PSD:YearOfLastRefurbishment
        a           rdf:Property ;
        rdfs:label  "Year of last refurbishment"@en .

PSD:Twisting  a     rdf:Property ;
        rdfs:label  "Twisting"@en .

PSD:AccuracyOfFireSensor
        a             rdf:Property ;
        rdfs:comment  "The accuracy of the sensor."@en ;
        rdfs:label    "AccuracyOfFireSensor"@en .

PSD:ConstructionToleranceClass
        a           rdf:Property ;
        rdfs:label  "Construction tolerance class"@en .

PSD:Headroom  a       rdf:Property ;
        rdfs:comment  "Actual headroom clearance for the passageway according to the current design. \\nThe shape information is provided in addition to the shape representation and the geometric parameters used within. In cases of inconsistency between the geometric parameters and the shape properties, provided in the attached property, the geometric parameters take precedence."@en ;
        rdfs:label    "Headroom"@en .

PSD:Options  a        rdf:Property ;
        rdfs:comment  "A statement of the options available in the agreement."@en ;
        rdfs:label    "Options"@en .

PSD:UpstreamPressure  a  rdf:Property ;
        rdfs:comment  "The operating pressure of the fluid upstream of the pressure reducing valve."@en ;
        rdfs:label    "UpstreamPressure"@en .

PSD:SetPointTemperature
        a             rdf:Property ;
        rdfs:comment  "The temperature value to be sensed. Use IfcPropertyBoundedValue.SetPointValue to set the set point value."@en ;
        rdfs:label    "SetPointTemperature"@en .

PSD:NumberOfCircuits  a  rdf:Property ;
        rdfs:comment  "Number of parallel fluid tube circuits."@en ;
        rdfs:label    "NumberOfCircuits"@en .

PSD:Position  a       rdf:Property ;
        rdfs:comment  "Indicates position of the actuator over time where 0.0 is fully closed and 1.0 is fully open."@en ;
        rdfs:label    "Position"@en .

PSD:ConcreteCover  a  rdf:Property ;
        rdfs:label  "Concrete cover"@en .

PSD:IsHighPressure  a  rdf:Property ;
        rdfs:comment  "Indication of whether the flushing valve is suitable for use on a high pressure water main (set TRUE) or not (set FALSE)."@en ;
        rdfs:label    "IsHighPressure"@en .

PSD:MechanicalEfficiency
        a             rdf:Property ;
        rdfs:comment  "Ratio of the work (as measured) delivered to the gas to the work input to the compressor shaft."@en , "The pumps operational mechanical efficiency."@en ;
        rdfs:label    "MechanicalEfficiency"@en .

PSD:CoreSetHorizontal
        a             rdf:Property ;
        rdfs:comment  "Degree of horizontal (in the X-axis of the LocalPlacement) blade set from the centerline."@en ;
        rdfs:label    "Core set horizontal"@en .

PSD:FlowCondition  a  rdf:Property ;
        rdfs:comment  "Defines the flow condition as a percentage of the cross-sectional area."@en ;
        rdfs:label    "FlowCondition"@en .

PSD:Azimuth  a        rdf:Property ;
        rdfs:comment  "The azimuth of the outward normal for the outward or upward facing surface."@en ;
        rdfs:label    "Azimuth"@en .

PSD:DynamicViscosity  a  rdf:Property ;
        rdfs:comment  "A measure of the viscous resistance of the material."@en ;
        rdfs:label    "DynamicViscosity"@en .

PSD:HoseNozzleType  a  rdf:Property ;
        rdfs:comment  "Identifies the predefined types of nozzle (in terms of spray pattern) fitted to the end of the hose from which the type required may be set."@en ;
        rdfs:label    "HoseNozzleType"@en .

PSD:ModelReference  a  rdf:Property ;
        rdfs:comment  "The model number or designator of the product model (or product line) as assigned by the manufacturer of the manufactured item."@en ;
        rdfs:label    "ModelReference"@en .

PSD:MarketSubCategory
        a             rdf:Property ;
        rdfs:comment  "ubset of category of use e.g. multi-family, 2 bedroom, low rise."@en , "Subset of category of use e.g. multi-family, 2 bedroom, low rise."@en ;
        rdfs:label    "Market sub category"@en , "MarketSubCategory"@en .

PSD:PrevailingWindDirection
        a             rdf:Property ;
        rdfs:comment  "The prevailing wind angle direction measured from True North (0 degrees) in a clockwise direction."@en ;
        rdfs:label    "PrevailingWindDirection"@en .

PSD:Type  a           rdf:Property ;
        rdfs:comment  "Defines the allowed values for selection of the flow meter operation type."@en ;
        rdfs:label    "Type"@en .

PSD:FreezingPoint  a  rdf:Property ;
        rdfs:comment  "The freezing point of the material (fluid)."@en ;
        rdfs:label    "FreezingPoint"@en .

PSD:NetPositiveSuctionHead
        a             rdf:Property ;
        rdfs:comment  "Minimum liquid pressure at the pump inlet to prevent cavitation."@en ;
        rdfs:label    "NetPositiveSuctionHead"@en .

PSD:AssessmentCondition
        a             rdf:Property ;
        rdfs:comment  "The overall condition of a product based on an assessment of the contributions to the overall condition made by the various criteria considered. The meanings given to the values of assessed condition should be agreed and documented by local agreements. For instance, is overall condition measured on a scale of 1 - 10 or by assigning names such as Good, OK, Poor."@en ;
        rdfs:label    "Assessment condition"@en .

PSD:SpaceRelativeHumidity
        a             rdf:Property ;
        rdfs:comment  "The relative humidity of the space."@en ;
        rdfs:label    "SpaceRelativeHumidity"@en .

PSD:IsPluggableOutlet
        a             rdf:Property ;
        rdfs:comment  "Indication of whether the outlet accepts a loose plug connection (= TRUE) or whether it is directly connected (= FALSE) or whether the form of connection has not yet been determined (= UNKNOWN)."@en ;
        rdfs:label    "Is pluggable outlet"@en .

PSD:NumberOfChairs  a  rdf:Property ;
        rdfs:comment  "Maximum number of chairs that can fit with the table for normal use."@en ;
        rdfs:label    "NumberOfChairs"@en .

PSD:StandardFixingPlateDepth
        a             rdf:Property ;
        rdfs:comment  "The depth of the standard fixing plate."@en ;
        rdfs:label    "StandardFixingPlateDepth"@en .

PSD:ContributedLuminousFlux
        a             rdf:Property ;
        rdfs:comment  "Luminous flux is a photometric measure of radiant flux, i.e. the volume of light emitted from a light source. Luminous flux is measured either for the interior as a whole or for a part of the interior (partial luminous flux for a solid angle). All other photometric parameters are derivatives of luminous flux. Luminous flux is measured in lumens (lm). The luminous flux is given as a nominal value for each lamp."@en ;
        rdfs:label    "Contributed luminous flux"@en .

PSD:IsolatingPurpose  a  rdf:Property ;
        rdfs:comment  "Defines the purpose for which the isolating valve is used since the way in which the valve is identified as an isolating valve may be in the context of its use. Note that unless there is a contextual name for the isolating valve (as in the case of a Landing Valve on a rising fire main), then the value assigned shoulkd be UNSET."@en ;
        rdfs:label    "IsolatingPurpose"@en .

PSD:I2TApplicability  a  rdf:Property ;
        rdfs:comment  "The applicability of the time adjustment related to the tripping function."@en ;
        rdfs:label    "I2TApplicability"@en .

PSD:SetPointConductance
        a             rdf:Property ;
        rdfs:comment  "The fill level value to be sensed. Use IfcPropertyBoundedValue.SetPointValue to set the set point value."@en ;
        rdfs:label    "SetPointConductance"@en .

PSD:ReinforcementAreaRatio
        a           rdf:Property ;
        rdfs:label  "Reinforcement area ratio"@en .

PSD:TypePropertyEnumeratedValue
        a                 owl:Class ;
        rdfs:label        "Type property enumerated value"@en ;
        rdfs:subClassOf   PSD:PropertyType ;
        rdfs:subClassOf   [ a                owl:Restriction ;
                            owl:cardinality  "1"^^xsd:nonNegativeInteger ;
                            owl:onProperty   PSD:name
                          ] ;
        owl:disjointWith  PSD:TypePropertyTableValue , PSD:TypePropertyReferenceValue , PSD:TypePropertyBoundedValue , PSD:TypePropertyListValue , PSD:TypeComplexProperty , PSD:TypePropertySingleValue .

PSD:IfNotAccomplished
        a             rdf:Property ;
        rdfs:comment  "Comments if the job is not accomplished."@en ;
        rdfs:label    "IfNotAccomplished"@en .

PSD:ConvectorType  a  rdf:Property ;
        rdfs:comment  "Indicates the type of convector, whether forced air (mechanically driven) or natural (gravity)."@en ;
        rdfs:label    "ConvectorType"@en .

PSD:Mode  a           rdf:Property ;
        rdfs:comment  "Table mapping operation mode identifiers to descriptive labels, which may be used for interpreting Pset_UnitaryControlElementPHistory.Mode."@en , "Indicates operation mode corresponding to Pset_UnitaryControlTypeCommon.Mode.  For example, 'HEAT', 'COOL', 'AUTO'."@en ;
        rdfs:label    "Mode"@en .

PSD:Relaxations  a    rdf:Property ;
        rdfs:comment  "Measures of decrease in stress over long time intervals resulting from plastic flow. Different relaxation values for different initial stress levels for a material may be given. It describes the time dependent relative relaxation value for a given initial stress level at constant strain.\\nRelating values are the \\\"RelaxationValue\\\". Related values are the \\\"InitialStress\\\""@en ;
        rdfs:label    "Relaxations"@en .

PSD:OuterDiameter  a  rdf:Property ;
        rdfs:comment  "The actual outer diameter of the pipe."@en ;
        rdfs:label    "OuterDiameter"@en .

PSD:VisibleTransmittance
        a             rdf:Property ;
        rdfs:comment  "Transmittance at normal incidence (visible). Defines the fraction of the visible spectrum of solar radiation that passes through per unit area, perpendicular to the surface."@en ;
        rdfs:label    "VisibleTransmittance"@en .

PSD:ColumnShoeCasingHeight
        a             rdf:Property ;
        rdfs:comment  "The height of the column shoe casing."@en ;
        rdfs:label    "ColumnShoeCasingHeight"@en .

PSD:PipeConnection  a  rdf:Property ;
        rdfs:comment  "The manner in which the pipe connection is made to the cooled beam."@en ;
        rdfs:label    "PipeConnection"@en .

PSD:ParticleAbsorptionCurve
        a             rdf:Property ;
        rdfs:comment  "Ratio of particles that are removed by the filter.  Each entry describes the ratio of particles absorbed greater than equal to the specified size and less than the next specified size.  For example,  given for 3 significant particle sizes >= 0,1 micro m, >= 1 micro m, >= 5 micro m"@en ;
        rdfs:label    "ParticleAbsorptionCurve"@en .

PSD:DesignLocationNumber
        a           rdf:Property ;
        rdfs:label  "Design location number"@en .

PSD:HigherHeatingValue
        a             rdf:Property ;
        rdfs:comment  "Higher Heating Value is defined as the amount of energy released (MJ/kg) when a fuel is burned completely, and H2O is in liquid form in the combustion products."@en ;
        rdfs:label    "HigherHeatingValue"@en .

PSD:ThermalConductivity
        a             rdf:Property ;
        rdfs:comment  "The thermal conductivity of the fin."@en , "The rate at which thermal energy is transmitted through the material."@en , "The thermal conductivity of the tube."@en ;
        rdfs:label    "ThermalConductivity"@en .

PSD:z   a             rdf:Property ;
        rdfs:comment  "Measure z according to ISO 2553"@en ;
        rdfs:label    "z"@en .

PSD:ClearDepth  a     rdf:Property ;
        rdfs:comment  "Clear unobstructed depth available for cable inclusion within the junction box."@en , "The clear depth of the culvert."@en ;
        rdfs:label    "Clear depth"@en , "ClearDepth"@en .

PSD:ScrapFactor  a    rdf:Property ;
        rdfs:comment  "Sheet metal scrap factor."@en ;
        rdfs:label    "ScrapFactor"@en .

PSD:TemperatureFactor
        a             rdf:Property ;
        rdfs:comment  "The correction factor (typically measured as %/deg K) for adjusting the thermal current/time to an ambient temperature different from the value given by the defined temperature."@en ;
        rdfs:label    "TemperatureFactor"@en .

PSD:DesignName  a     rdf:Property ;
        rdfs:comment  "A name for the design values."@en ;
        rdfs:label    "DesignName"@en .

PSD:MassDensity  a  rdf:Property ;
        rdfs:label  "Mass density"@en .

PSD:AngleBetweenComponentAxes
        a           rdf:Property ;
        rdfs:label  "Angle between component axes"@en .

PSD:BathType  a       rdf:Property ;
        rdfs:comment  "The property enumeration defines the types of bath that may be specified within the property set."@en ;
        rdfs:label    "BathType"@en .

PSD:ShipMethod  a     rdf:Property ;
        rdfs:comment  "Method of shipping that will be used for goods or services."@en ;
        rdfs:label    "ShipMethod"@en .

PSD:TypePropertySingleValue
        a                 owl:Class ;
        rdfs:comment      "Type of IfcPropertySingleValue."@en ;
        rdfs:label        "Type property single value"@en ;
        rdfs:subClassOf   PSD:PropertyType ;
        rdfs:subClassOf   [ a                owl:Restriction ;
                            owl:cardinality  "1"^^xsd:nonNegativeInteger ;
                            owl:onProperty   PSD:dataType
                          ] ;
        rdfs:subClassOf   [ a                   owl:Restriction ;
                            owl:maxCardinality  "1"^^xsd:nonNegativeInteger ;
                            owl:onProperty      PSD:unitType
                          ] ;
        owl:disjointWith  PSD:TypePropertyBoundedValue , PSD:TypePropertyTableValue , PSD:TypePropertyListValue , PSD:TypeComplexProperty , PSD:TypePropertyReferenceValue , PSD:TypePropertyEnumeratedValue .

PSD:HeatingCapacity  a  rdf:Property ;
        rdfs:comment  "Heating capacity."@en ;
        rdfs:label    "HeatingCapacity"@en .

PSD:StemBaseFillet  a  rdf:Property ;
        rdfs:comment  "Stem base fillet of the profile."@en ;
        rdfs:label    "StemBaseFillet"@en .

PSD:HazardousWastePerUnit
        a           rdf:Property ;
        rdfs:label  "Hazardous waste per unit"@en .

PSD:FanPowerRate  a   rdf:Property ;
        rdfs:comment  "Fan power consumption."@en ;
        rdfs:label    "FanPowerRate"@en .

PSD:ColumnShoeCasingDepth
        a             rdf:Property ;
        rdfs:comment  "The depth of the column shoe casing."@en ;
        rdfs:label    "ColumnShoeCasingDepth"@en .

PSD:InternalWaterVolume
        a             rdf:Property ;
        rdfs:comment  "Internal volume of condenser (water side)."@en ;
        rdfs:label    "Internal water volume"@en .

PSD:BladeEdge  a      rdf:Property ;
        rdfs:comment  "Blade edge."@en ;
        rdfs:label    "BladeEdge"@en .

PSD:NumberofBlades  a  rdf:Property ;
        rdfs:comment  "Number of blades."@en ;
        rdfs:label    "NumberofBlades"@en .

PSD:ReleaseTimeI2tStart
        a             rdf:Property ;
        rdfs:comment  "The release time in [s] for the start point of the I2t tripping curve of the G-function, if any."@en , "The release time in [s] for the start point of the I2t tripping curve of the S-function, if any"@en ;
        rdfs:label    "ReleaseTimeI2tStart"@en .

PSD:TotalHeatingCapacity
        a             rdf:Property ;
        rdfs:comment  "Total heating capacity. This includes heating capacity of beam and heating capacity of supply air."@en ;
        rdfs:label    "TotalHeatingCapacity"@en .

PSD:TotalHeatGain  a  rdf:Property ;
        rdfs:comment  "The total amount of heat or energy gained by the space at the time of the space's peak cooling conditions."@en ;
        rdfs:label    "TotalHeatGain"@en .

PSD:PowerState  a     rdf:Property ;
        rdfs:comment  "Indicates the power state of the device where True is on and False is off."@en ;
        rdfs:label    "PowerState"@en .

PSD:Type2  a          rdf:Property ;
        rdfs:comment  "See Type1."@en ;
        rdfs:label    "Type2"@en .

PSD:Description  a    rdf:Property ;
        rdfs:comment  "The description of the air side system."@en , "Description of the reinforcement."@en ;
        rdfs:label    "Description"@en .

PSD:HoseReelMountingType
        a             rdf:Property ;
        rdfs:comment  "Identifies the predefined types of hose reel mounting from which the type required may be set."@en ;
        rdfs:label    "HoseReelMountingType"@en .

PSD:AgreementType  a  rdf:Property ;
        rdfs:comment  "Identifies the predefined types of property agreement from which the type required may be set."@en ;
        rdfs:label    "AgreementType"@en .

PSD:Width  a          rdf:Property ;
        rdfs:comment  "The width of the sump."@en , "The requested width (horizontal extension in elevation) of the provision for void, only provided if the Shape property is set to 'rectangle'."@en , "The width of the pit."@en , "The width of the trench."@en ;
        rdfs:label    "Width"@en .

PSD:MaximumVelocity  a  rdf:Property ;
        rdfs:comment  "The maximum design velocity of the air in the duct or fitting."@en ;
        rdfs:label    "MaximumVelocity"@en .

PSD:DesignLevel  a    rdf:Property ;
        rdfs:comment  "Adjustment of the service life resulting from the effect of design level employed."@en ;
        rdfs:label    "DesignLevel"@en .

PSD:DefinedTemperature
        a             rdf:Property ;
        rdfs:comment  "The ambient temperature at which the thermal current/time-curve associated with this protection device is defined."@en ;
        rdfs:label    "DefinedTemperature"@en .

PSD:LiftingStrength  a  rdf:Property ;
        rdfs:label  "Lifting strength"@en .

PSD:Porosity  a     rdf:Property ;
        rdfs:label  "Porosity"@en .

PSD:SecondCurvatureRadius
        a             rdf:Property ;
        rdfs:comment  "SecondCurvatureRadius should be defined as the top or right side radius of curvature value."@en ;
        rdfs:label    "SecondCurvatureRadius"@en .

PSD:HeatingDesignDay  a  rdf:Property ;
        rdfs:comment  "The month, day and time that has been selected for the heating design calculations."@en ;
        rdfs:label    "HeatingDesignDay"@en .

PSD:DistanceBetweenComponentAxes
        a           rdf:Property ;
        rdfs:label  "Distance between component axes"@en .

PSD:SeatingHeight  a  rdf:Property ;
        rdfs:comment  "The value of seating height if the chair height is not adjustable."@en ;
        rdfs:label    "SeatingHeight"@en .

PSD:ShortCircuit3PolePowerFactorMaximumState
        a             rdf:Property ;
        rdfs:comment  "Power factor of the maximum 3 pole short circuit current provided at the point of supply."@en ;
        rdfs:label    "ShortCircuit3PolePowerFactorMaximumState"@en .

PSD:SupplyAirConnectionType
        a             rdf:Property ;
        rdfs:comment  "The manner in which the pipe connection is made to the cooled beam."@en ;
        rdfs:label    "SupplyAirConnectionType"@en .

PSD:TimeConstant  a   rdf:Property ;
        rdfs:comment  "The time constant of the sensor."@en ;
        rdfs:label    "TimeConstant"@en .

PSD:FlangeChamfer  a  rdf:Property ;
        rdfs:comment  "Flange chamfer of the profile."@en ;
        rdfs:label    "FlangeChamfer"@en .

PSD:ClearHeight  a  rdf:Property ;
        rdfs:label  "Clear height"@en .

PSD:AdjustmentDesignation
        a             rdf:Property ;
        rdfs:comment  "The desgnation on the device for the adjustment."@en ;
        rdfs:label    "AdjustmentDesignation"@en .

PSD:LandID  a         rdf:Property ;
        rdfs:comment  "Identification number assigned by the statutory registration authority to a land parcel."@en ;
        rdfs:label    "LandID"@en .

PSD:CorrosionTreatment
        a             rdf:Property ;
        rdfs:comment  "Determines corrosion treatment for metal components. This property is provided if the requirement needs to be expressed (a) independently of a material specification and (b) as a mere requirements statement rather than a workshop design/ processing feature."@en ;
        rdfs:label    "Corrosion treatment"@en .

PSD:Span  a         rdf:Property ;
        rdfs:label  "Span"@en .

PSD:Style  a          rdf:Property ;
        rdfs:comment  "Description of the furniture style."@en ;
        rdfs:label    "Style"@en .

PSD:Operation  a      rdf:Property ;
        rdfs:comment  "The operational mechanism for the damper operation."@en ;
        rdfs:label    "Operation"@en .

PSD:SolarTransmittance
        a             rdf:Property ;
        rdfs:comment  "Transmittance at normal incidence (solar). Defines the fraction of solar radiation that passes through per unit area, perpendicular to the surface."@en ;
        rdfs:label    "Solar transmittance"@en , "SolarTransmittance"@en .

PSD:WashersCount  a   rdf:Property ;
        rdfs:comment  "Count of washers to be mounted on one bolt"@en ;
        rdfs:label    "WashersCount"@en .

PSD:AcidityConcentration
        a             rdf:Property ;
        rdfs:comment  "Maximum CaCO3 equivalent that would neutralize the acid."@en ;
        rdfs:label    "AcidityConcentration"@en .

PSD:HasGrabHandles  a  rdf:Property ;
        rdfs:comment  "Indicates whether the bath is fitted with handles that provide assistance to a bather in entering or leaving the bath."@en ;
        rdfs:label    "HasGrabHandles"@en .

PSD:PropertyDef  a       owl:Class ;
        rdfs:comment     "Element of property definition."@en ;
        rdfs:label       "Property definition"@en ;
        rdfs:subClassOf  owl:Thing ;
        rdfs:subClassOf  [ a                   owl:Restriction ;
                           owl:maxCardinality  "1"^^xsd:nonNegativeInteger ;
                           owl:onProperty      PSD:name
                         ] ;
        rdfs:subClassOf  [ a                   owl:Restriction ;
                           owl:maxCardinality  "1"^^xsd:nonNegativeInteger ;
                           owl:onProperty      PSD:definition
                         ] .

PSD:InternalWidth  a  rdf:Property ;
        rdfs:comment  "The internal width of the culvert."@en ;
        rdfs:label    "InternalWidth"@en .

PSD:StemBaseChamfer  a  rdf:Property ;
        rdfs:comment  "Stem base chamfer of the profile."@en ;
        rdfs:label    "StemBaseChamfer"@en .

PSD:FireSensorSetPoint
        a             rdf:Property ;
        rdfs:comment  "The temperature value to be sensed to indicate the presence of fire."@en ;
        rdfs:label    "FireSensorSetPoint"@en .

PSD:SetPointSound  a  rdf:Property ;
        rdfs:comment  "The sound pressure value to be sensed. Use IfcPropertyBoundedValue.SetPointValue to set the set point value."@en ;
        rdfs:label    "SetPointSound"@en .

PSD:Compartmentation  a  rdf:Property ;
        rdfs:label  "Compartmentation"@en .

PSD:WaterFilterType  a  rdf:Property ;
        rdfs:comment  "Further qualifies the type of water filter.  Filtration removes undissolved matter; Purification removes dissolved matter; Softening replaces dissolved matter."@en ;
        rdfs:label    "WaterFilterType"@en .

PSD:I4  a             rdf:Property ;
        rdfs:comment  "The lower electromagnetic testing current limit in [x In], indicating that for currents lower than I4, the tripping time shall be longer than the associated tripping time, T5, i.e. the device shall not trip instantaneous."@en ;
        rdfs:label    "I4"@en .

PSD:Identifier  a     rdf:Property ;
        rdfs:comment  "The identifier assigned to the agreement for the purposes of tracking."@en ;
        rdfs:label    "Identifier"@en .

PSD:BuildingID  a   rdf:Property ;
        rdfs:label  "Building ID"@en .

PSD:TotalRadiantLoad  a  rdf:Property ;
        rdfs:comment  "Total electromagnetic energy added or removed by emission or absorption.  If a value is less than zero (negative), then the thermal load is lost from the space. If a value is greater than zero (positive), then the thermal load is a gain to the space."@en ;
        rdfs:label    "TotalRadiantLoad"@en .

PSD:IfcVersion  a        owl:Class ;
        rdfs:comment     "Version information of IFC release and sub schema."@en ;
        rdfs:label       "IFC version"@en ;
        rdfs:subClassOf  owl:Thing .

PSD:NominalWaterFlowHeating
        a             rdf:Property ;
        rdfs:comment  "Nominal water flow (refers to nominal heating capacity)."@en ;
        rdfs:label    "NominalWaterFlowHeating"@en .

PSD:MaximumPlenumSensibleLoad
        a             rdf:Property ;
        rdfs:comment  "Maximum or Peak sensible thermal load contributed to return air plenum by the light fixture."@en ;
        rdfs:label    "MaximumPlenumSensibleLoad"@en .

PSD:EutrophicationPerUnit
        a           rdf:Property ;
        rdfs:label  "Eutrophication per unit"@en .

PSD:LongInsideEndTopBarPitch
        a             rdf:Property ;
        rdfs:comment  "The pitch length of the long inside end top bar."@en ;
        rdfs:label    "LongInsideEndTopBarPitch"@en .

PSD:VaristorType  a   rdf:Property ;
        rdfs:comment  "A list of the available types of varistor  from which that required may be selected."@en ;
        rdfs:label    "VaristorType"@en .

PSD:DischargeDirection
        a             rdf:Property ;
        rdfs:comment  "Discharge direction of the air terminal.\\n\\nParallel: discharges parallel to mounting surface designed so that flow attaches to the surface.\\nPerpendicular:  discharges away from mounting surface.\\nAdjustable: both parallel and perpendicular discharge."@en ;
        rdfs:label    "Discharge direction"@en .

PSD:ActuatorInputPower
        a             rdf:Property ;
        rdfs:comment  "Maximum input power requirement."@en ;
        rdfs:label    "Actuator input power"@en .

PSD:parent  a        owl:TransitiveProperty , owl:FunctionalProperty ;
        rdfs:domain  PSD:InformationDeliverySpecification ;
        rdfs:label   "Parent information delivery specification"@en ;
        rdfs:range   PSD:InformationDeliverySpecification .

PSD:FragilityRating  a  rdf:Property ;
        rdfs:label  "Fragility rating"@en .

PSD:CompressorCondenserHeatGain
        a             rdf:Property ;
        rdfs:comment  "Heat gain between condenser inlet to compressor outlet."@en ;
        rdfs:label    "CompressorCondenserHeatGain"@en .

PSD:Illuminance  a    rdf:Property ;
        rdfs:comment  "Required average illuminance value for this space."@en ;
        rdfs:label    "Illuminance"@en .

PSD:SupportDuringTransportDocReference
        a           rdf:Property ;
        rdfs:label  "Support during transport doc reference"@en .

PSD:UserCorrectionFactor
        a             rdf:Property ;
        rdfs:comment  "An arbitrary correction factor that may be applied by the user."@en ;
        rdfs:label    "UserCorrectionFactor"@en .

PSD:ConstructionMethod
        a           rdf:Property ;
        rdfs:label  "Construction method"@en .

PSD:applicableClass  a  owl:ObjectProperty ;
        rdfs:comment  "Applicable entity type, i.e., \"IfcWallStandardCase\". Multiple value is accepted, and format is: \"ENTYT_TYPE_1, ENTITY_TYPE_2, ...\"."@en ;
        rdfs:domain   PSD:PropertySetDef ;
        rdfs:label    "applicable class" ;
        rdfs:range    owl:Class .

PSD:CoolingDryBulb  a  rdf:Property ;
        rdfs:comment  "Inside dry bulb temperature for cooling design."@en , "Outside dry bulb temperature for cooling design."@en ;
        rdfs:label    "CoolingDryBulb"@en .

PSD:RegeneratedSoundCurve
        a             rdf:Property ;
        rdfs:comment  "Regenerated sound versus air flow rate."@en ;
        rdfs:label    "RegeneratedSoundCurve"@en .

PSD:StemTopFillet  a  rdf:Property ;
        rdfs:comment  "Stem top fillet of the profile."@en ;
        rdfs:label    "StemTopFillet"@en .

PSD:BoltSize  a       rdf:Property ;
        rdfs:comment  "Size of the bolts securing the flange."@en ;
        rdfs:label    "BoltSize"@en .

PSD:XDirectionLowerBarCount
        a             rdf:Property ;
        rdfs:comment  "The number of bars with X direction lower bar."@en ;
        rdfs:label    "XDirectionLowerBarCount"@en .

PSD:Manufacturer  a   rdf:Property ;
        rdfs:comment  "The organization that manufactured and/or assembled the item."@en ;
        rdfs:label    "Manufacturer"@en .

PSD:CoreBaseHeight  a  rdf:Property ;
        rdfs:comment  "Core base height of the profile."@en ;
        rdfs:label    "CoreBaseHeight"@en .

PSD:VacancyRateInCategoryFuture
        a             rdf:Property ;
        rdfs:comment  "Percentage of vacancy found in the particular category expected in the future."@en ;
        rdfs:label    "Vacancy rate in category future"@en .

PSD:DualDeck  a       rdf:Property ;
        rdfs:comment  "Does the AirHandler have a dual deck? TRUE = Yes, FALSE = No."@en ;
        rdfs:label    "DualDeck"@en .

PSD:VideoResolutionHeight
        a             rdf:Property ;
        rdfs:comment  "Indicates the number of vertical pixels, e.g. 1080."@en , "Indicates the number of vertical pixels (the largest native video resolution height)."@en ;
        rdfs:label    "VideoResolutionHeight"@en .

PSD:CenterCoreBaseWidth
        a             rdf:Property ;
        rdfs:comment  "Center core base width of the profile."@en ;
        rdfs:label    "CenterCoreBaseWidth"@en .

PSD:CoreMiddleHeight  a  rdf:Property ;
        rdfs:comment  "Core middle height of the profile."@en ;
        rdfs:label    "CoreMiddleHeight"@en .

PSD:MotorDriveType  a  rdf:Property ;
        rdfs:comment  "Motor drive type:\\nDIRECTDRIVE: Direct drive. \\nBELTDRIVE: Belt drive. \\nCOUPLING: Coupling. \\nOTHER: Other type of motor drive. \\nUNKNOWN: Unknown motor drive type."@en ;
        rdfs:label    "Motor drive type"@en .

PSD:WorkFinishTime  a  rdf:Property ;
        rdfs:comment  "The default time of day a task is scheduled to finish. For presentation purposes, if the finish time of a task matches the WorkFinishTime, then applications may choose to display the date only. Conversely when entering dates without specifying time, applications may automatically append the WorkFinishTime."@en ;
        rdfs:label    "Work finish time"@en .

PSD:NominalSupplyWaterTemperatureHeating
        a             rdf:Property ;
        rdfs:comment  "Nominal supply water temperature (refers to nominal heating capacity)."@en ;
        rdfs:label    "NominalSupplyWaterTemperatureHeating"@en .

PSD:PropertyName  a   rdf:Property ;
        rdfs:comment  "Addressing details of the property as stated within the agreement."@en ;
        rdfs:label    "PropertyName"@en .

PSD:MaximumShortCircuitTemperature
        a             rdf:Property ;
        rdfs:comment  "The maximum short circuit temperature at which a cable or bus is certified to operate."@en ;
        rdfs:label    "MaximumShortCircuitTemperature"@en .

PSD:ThermalIrEmissivityBack
        a             rdf:Property ;
        rdfs:comment  "Thermal IR emissivity: back side. Defines the fraction of thermal energy emitted per unit area to 'blackbody' at the same temperature, through the 'back' side of the material."@en ;
        rdfs:label    "ThermalIrEmissivityBack"@en .

PSD:JunctionType  a   rdf:Property ;
        rdfs:comment  "The type of junction. TEE=3 ports, CROSS = 4 ports."@en ;
        rdfs:label    "JunctionType"@en .

PSD:AcquisitionDate  a  rdf:Property ;
        rdfs:comment  "The date that the manufactured item was purchased."@en ;
        rdfs:label    "AcquisitionDate"@en .

PSD:UpperTime2  a     rdf:Property ;
        rdfs:comment  "The time in [s], indicating the tripping times of the upper time/current curve at the UpperCurrent2."@en ;
        rdfs:label    "UpperTime2"@en .

PSD:LongInsideCenterLowerBarPitch
        a             rdf:Property ;
        rdfs:comment  "The pitch length of the long inside center lower bar."@en ;
        rdfs:label    "LongInsideCenterLowerBarPitch"@en .

PSD:HoseDiameter  a   rdf:Property ;
        rdfs:comment  "Notional diameter (bore) of the hose."@en ;
        rdfs:label    "HoseDiameter"@en .

PSD:CompressorSpeed  a  rdf:Property ;
        rdfs:comment  "Compressor speed."@en ;
        rdfs:label    "CompressorSpeed"@en .

PSD:SolarReflectanceFront
        a             rdf:Property ;
        rdfs:comment  "Reflectance at normal incidence (solar): front side. Defines the fraction of the solar ray that is reflected and not transmitted when the ray passes from one medium into another, at the 'front' side of the other material, perpendicular to the surface. Dependent on material and surface characteristics."@en ;
        rdfs:label    "SolarReflectanceFront"@en .

PSD:ExternalAdjusted  a  rdf:Property ;
        rdfs:comment  "An indication if the ground fault protection may be adjusted according to an external current coil or not."@en ;
        rdfs:label    "ExternalAdjusted"@en .

PSD:SpecialConstruction
        a             rdf:Property ;
        rdfs:comment  "Special construction capabilities like self-supporting, flat devidable cable or bus flat non devidable cable or bus supporting elements inside (steal, textile, concentric conductor). Note that materials used should be agreed between exchange participants before use."@en ;
        rdfs:label    "SpecialConstruction"@en .

PSD:NominalSurroundingTemperatureCooling
        a             rdf:Property ;
        rdfs:comment  "Nominal surrounding temperature (refers to nominal cooling capacity)."@en ;
        rdfs:label    "NominalSurroundingTemperatureCooling"@en .

PSD:WireLoopLength  a  rdf:Property ;
        rdfs:comment  "The length of the fastening loop part of the wire."@en ;
        rdfs:label    "WireLoopLength"@en .

PSD:ReheatType  a     rdf:Property ;
        rdfs:comment  "Terminal box reheat type."@en ;
        rdfs:label    "Reheat type"@en .

PSD:MaximumCableLength
        a             rdf:Property ;
        rdfs:comment  "Maximum cable length based on voltagedrop. NOTE: This value may also be specified as a constraint within an IFC model if required but is included within the property set at this stage pending implementation of the required capabilities within software applications."@en ;
        rdfs:label    "MaximumCableLength"@en .

PSD:AmplifierType  a  rdf:Property ;
        rdfs:comment  "Indicates the type of amplifier."@en ;
        rdfs:label    "AmplifierType"@en .

PSD:ShortInsideEndLowerBarPitch
        a             rdf:Property ;
        rdfs:comment  "The pitch length of the short inside end lower bar."@en ;
        rdfs:label    "ShortInsideEndLowerBarPitch"@en .

PSD:CoolingDesignAirflow
        a             rdf:Property ;
        rdfs:comment  "The air flowrate required during the peak cooling conditions."@en ;
        rdfs:label    "CoolingDesignAirflow"@en .

PSD:LeakageCurve  a   rdf:Property ;
        rdfs:comment  "Leakage versus pressure drop; Leakage = f (pressure)."@en , "Leakage per unit length curve versus working pressure. If a scalar is expressed then it represents LeakageClass which is flowrate per unit area at a specified pressure rating (e.g., ASHRAE Fundamentals 2001 34.16.)."@en , "Leakage per unit length curve versus working pressure."@en ;
        rdfs:label    "LeakageCurve"@en .

PSD:ElectroMagneticTrippingUnitType
        a             rdf:Property ;
        rdfs:comment  "A list of the available types of electric magnetic tripping unit  from which that required may be selected. These cover overload, none special, short circuit, motor protection and bi-metal tripping."@en ;
        rdfs:label    "ElectroMagneticTrippingUnitType"@en .

PSD:SolarReflectanceBack
        a             rdf:Property ;
        rdfs:comment  "Reflectance at normal incidence (solar): back side. Defines the fraction of the solar ray that is reflected and not transmitted when the ray passes from one medium into another, at the 'back' side of the other material, perpendicular to the surface. Dependent on material and surface characteristics."@en ;
        rdfs:label    "SolarReflectanceBack"@en .

PSD:FlowResistanceRange
        a             rdf:Property ;
        rdfs:comment  "Allowable range of frictional resistance against which the fluid is being pumped."@en ;
        rdfs:label    "FlowResistanceRange"@en .

PSD:StandardFixingPlateThickness
        a             rdf:Property ;
        rdfs:comment  "The thickness of the standard fixing plate."@en ;
        rdfs:label    "StandardFixingPlateThickness"@en .

PSD:EnergyLoss  a     rdf:Property ;
        rdfs:comment  "The sum of energy losses for the spaces served by the system during the peak heating conditions."@en ;
        rdfs:label    "Energy loss"@en .

PSD:Temperature  a    rdf:Property ;
        rdfs:comment  "The temperature of the fuel."@en , "Temperature of the fluid. For air this value represents the dry bulb temperature."@en , "Indicates the current measured temperature."@en ;
        rdfs:label    "Temperature"@en .

PSD:AdjustmentRangeStepValue
        a             rdf:Property ;
        rdfs:comment  "Step value of current adjustment for an AdjustmentValueType = RANGE. Note that this property should not have a value for an  AdjustmentValueType = LIST."@en , "Step value of time adjustment for an AdjustmentValueType = RANGE. Note that this property should not have a value for an  AdjustmentValueType = LIST."@en ;
        rdfs:label    "AdjustmentRangeStepValue"@en .

PSD:BaseChamfer  a    rdf:Property ;
        rdfs:comment  "Base chamfer of the profile."@en ;
        rdfs:label    "BaseChamfer"@en .

PSD:SetPoint  a       rdf:Property ;
        rdfs:comment  "Indicates the switch position over time according to Pset_SwitchingDeviceTypeCommon.SetPoint."@en , "Indicates the temperature setpoint.  For thermostats with setbacks or separate high and low setpoints, then the time series may contain a pair of values at each entry where the first value is the heating setpoint (low) and the second value is the cooling setpoint (high)."@en ;
        rdfs:label    "SetPoint"@en .

PSD:RefreshRate  a    rdf:Property ;
        rdfs:comment  "Indicates the display refresh frequency."@en ;
        rdfs:label    "RefreshRate"@en .

PSD:AtmosphericPressure
        a             rdf:Property ;
        rdfs:comment  "Ambient atmospheric pressure."@en ;
        rdfs:label    "Atmospheric pressure"@en , "AtmosphericPressure"@en .

PSD:OutsideAirFlowrate
        a             rdf:Property ;
        rdfs:comment  "Flow rate of outside air entering the unit."@en ;
        rdfs:label    "OutsideAirFlowrate"@en .

PSD:Roll  a         rdf:Property ;
        rdfs:label  "Roll"@en .

PSD:GlassThickness3  a  rdf:Property ;
        rdfs:label  "Glass thickness 3"@en .

PSD:MomentaryType  a  rdf:Property ;
        rdfs:comment  "A list of the available types of momentary switch from which that required may be selected."@en ;
        rdfs:label    "MomentaryType"@en .

PSD:SprinklerProtectionAutomatic
        a           rdf:Property ;
        rdfs:label  "Sprinkler protection automatic"@en .

PSD:FullLoadRatio  a  rdf:Property ;
        rdfs:comment  "Ratio of actual power to full load power as a quadratic function of part load, at certain condensing and evaporating temperature, FracFullLoadPower = f ( PartLoadRatio)."@en ;
        rdfs:label    "FullLoadRatio"@en .

PSD:ReinforcementSpacing
        a             rdf:Property ;
        rdfs:comment  "The spacing between reinforcing elements."@en ;
        rdfs:label    "ReinforcementSpacing"@en .

PSD:HasIntegralShutOffDevice
        a             rdf:Property ;
        rdfs:comment  "Indication of whether the flushing valve has an integral shut off device fitted (set TRUE) or not (set FALSE)."@en ;
        rdfs:label    "HasIntegralShutOffDevice"@en .

PSD:ToppingType  a  rdf:Property ;
        rdfs:label  "Topping type"@en .

PSD:WaterFlowControlSystemType
        a             rdf:Property ;
        rdfs:comment  "Factory fitted waterflow control system."@en ;
        rdfs:label    "WaterFlowControlSystemType"@en .

PSD:SwitchUsage  a    rdf:Property ;
        rdfs:comment  "A list of the available usages for toggle switches from which that required may be selected."@en , "A list of the available usages for selector switches from which that required may be selected."@en ;
        rdfs:label    "SwitchUsage"@en .

PSD:HighestSeatingHeight
        a             rdf:Property ;
        rdfs:comment  "The value of seating height of high level if the chair height is adjustable."@en ;
        rdfs:label    "HighestSeatingHeight"@en .

PSD:CornerFixingPlateFlangeWidthInPlaneZ
        a             rdf:Property ;
        rdfs:comment  "The flange width of the L-shaped corner plate in plane Z."@en ;
        rdfs:label    "CornerFixingPlateFlangeWidthInPlaneZ"@en .

PSD:DownstreamPressure
        a             rdf:Property ;
        rdfs:comment  "The operating pressure of the fluid downstream of the pressure reducing valve."@en ;
        rdfs:label    "DownstreamPressure"@en .

PSD:NominalMoistureGain
        a             rdf:Property ;
        rdfs:comment  "Nominal rate of water vapor added into the airstream."@en ;
        rdfs:label    "Nominal moisture gain"@en .

PSD:ActualCost  a     rdf:Property ;
        rdfs:comment  "The actual cost on behalf of the resource allocation."@en ;
        rdfs:label    "ActualCost"@en .

PSD:upperBoundValue  a  owl:FunctionalProperty , owl:DatatypeProperty ;
        rdfs:domain  PSD:TypePropertyBoundedValue ;
        rdfs:label   "Upper bound value"@en ;
        rdfs:range   xsd:string .

PSD:Location3Local  a  rdf:Property ;
        rdfs:comment  "Local x,y coordinates of the point in which Thickness3 is given"@en ;
        rdfs:label    "Location3Local"@en .

PSD:MinimumHeight  a  rdf:Property ;
        rdfs:comment  "The minimum duct height for rectangular, oval or round duct."@en ;
        rdfs:label    "MinimumHeight"@en .

PSD:CoolingTemperatureDelta
        a             rdf:Property ;
        rdfs:comment  "Cooling temperature difference for calculating space air flow rates."@en ;
        rdfs:label    "CoolingTemperatureDelta"@en .

PSD:HasDeflector  a   rdf:Property ;
        rdfs:comment  "Indication of whether the sprinkler has a deflector (baffle) fitted to diffuse the discharge on activation (= TRUE) or not (= FALSE)."@en ;
        rdfs:label    "HasDeflector"@en .

PSD:HazardousWaste  a  rdf:Property ;
        rdfs:label  "Hazardous waste"@en .

PSD:EdgeFixingPlateLength
        a             rdf:Property ;
        rdfs:comment  "The length of the L-shaped edge plate."@en ;
        rdfs:label    "EdgeFixingPlateLength"@en .

PSD:Height  a         rdf:Property ;
        rdfs:comment  "Length of the fin as measured perpendicular to the direction of airflow."@en , "Height of the object. It is the upper hight of the railing above the floor or stair.\\nThe size information is provided in addition to the shape representation and the geometric parameters used within. In cases of inconsistency between the geometric parameters and the size properties, provided in the attached property set, the geometric parameters take precedence."@en , "The requested height (vertical extension in elevation) of the provision for void', only provided if the Shape property is set to 'rectangle'."@en ;
        rdfs:label    "Height"@en .

PSD:Thickness1  a     rdf:Property ;
        rdfs:comment  "First thickness parameter of a surface member with varying thickness"@en ;
        rdfs:label    "Thickness1"@en .

PSD:LeftFlangeWidth  a  rdf:Property ;
        rdfs:comment  "Left flange width of the profile."@en ;
        rdfs:label    "LeftFlangeWidth"@en .

PSD:LowestSeatingHeight
        a             rdf:Property ;
        rdfs:comment  "The value of seating height of low level if the chair height is adjustable."@en ;
        rdfs:label    "LowestSeatingHeight"@en .

PSD:HygrothermalRating
        a           rdf:Property ;
        rdfs:label  "Hygrothermal rating"@en .

PSD:TotalEffectivenessTable
        a             rdf:Property ;
        rdfs:comment  "Total heat transfer effectiveness curve as a function of the primary and secondary air flow rate."@en ;
        rdfs:label    "TotalEffectivenessTable"@en .

PSD:CurrentTolerance1
        a             rdf:Property ;
        rdfs:comment  "The tolerance for the current of time/current-curve in [%]."@en ;
        rdfs:label    "CurrentTolerance1"@en .

PSD:BeamHeatingCapacity
        a             rdf:Property ;
        rdfs:comment  "Heating capacity of beam. This excludes heating capacity of supply air."@en ;
        rdfs:label    "BeamHeatingCapacity"@en .

PSD:TemperatureSetPoint
        a             rdf:Property ;
        rdfs:comment  "The temperature setpoint range and default setpoint."@en ;
        rdfs:label    "TemperatureSetPoint"@en .

PSD:PressureClass  a  rdf:Property ;
        rdfs:comment  "Nominal pressure rating of the system components. (Data type = PressureMeasure)"@en , "The test or rated pressure classification of the fitting."@en , "Pressure classification as defined by the authority having jurisdiction (e.g., SMACNA, etc.)."@en ;
        rdfs:label    "PressureClass"@en , "Pressure class"@en .

PSD:SupplyAirTemperatureCooling
        a             rdf:Property ;
        rdfs:comment  "Supply air temperature in cooling mode."@en ;
        rdfs:label    "SupplyAirTemperatureCooling"@en .

PSD:Status  a         rdf:Property ;
        rdfs:comment  "Status of the element, predominately used in renovation or retrofitting projects. The status can be assigned to as 'New' - element designed as new addition, 'Existing' - element exists and remains, 'Demolish' - element existed but is to be demolished,  'Temporary' - element will exists only temporary (like a temporary support structure)."@en , "Indicates an error code or identifier, whose meaning is specific to the particular automation system.  Example values include: 'ConfigurationError', 'NotConnected', 'DeviceFailure', 'SensorFailure', 'LastKnown, 'CommunicationsFailure', 'OutOfService'."@en ;
        rdfs:label    "Status"@en .

PSD:FaceArea  a       rdf:Property ;
        rdfs:comment  "Face area open to the airstream."@en ;
        rdfs:label    "FaceArea"@en .

PSD:FlangeThickness  a  rdf:Property ;
        rdfs:comment  "Thickness of the material from which the pipe bend is constructed."@en ;
        rdfs:label    "FlangeThickness"@en .

PSD:IsSelectable  a   rdf:Property ;
        rdfs:comment  "Indication whether the L-function can be switched off or not."@en , "Indication whether the S-function can be switched off or not."@en ;
        rdfs:label    "IsSelectable"@en .

PSD:QualityOfComponents
        a             rdf:Property ;
        rdfs:comment  "Adjustment of the service life resulting from the effect of the quality of components used."@en ;
        rdfs:label    "QualityOfComponents"@en .

PSD:WaterFoulingResistance
        a             rdf:Property ;
        rdfs:comment  "Fouling resistance on water/air side."@en ;
        rdfs:label    "WaterFoulingResistance"@en .

PSD:MoistureDiffusivity
        a             rdf:Property ;
        rdfs:comment  "Moisture diffusivity is a transport property that is frequently used in the hygrothermal analysis of building envelope components."@en ;
        rdfs:label    "MoistureDiffusivity"@en .

PSD:HasExteriorInsulation
        a             rdf:Property ;
        rdfs:comment  "TRUE if the silencer has exterior insulation. FALSE if it does not."@en ;
        rdfs:label    "HasExteriorInsulation"@en .

PSD:Force  a          rdf:Property ;
        rdfs:comment  "Indicates the maximum close-off force for the actuator."@en ;
        rdfs:label    "Force"@en .

PSD:ReleaseCurrentI2tStart
        a             rdf:Property ;
        rdfs:comment  "The release current in [x In] for the start point of the I2t tripping curve of the G-function, if any."@en , "The release current in [x In] for the start point of the I2t tripping curve of the S-function, if any."@en ;
        rdfs:label    "ReleaseCurrentI2tStart"@en .

PSD:WaterImpermeability
        a           rdf:Property ;
        rdfs:label  "Water impermeability"@en .

PSD:VentilatingPipeSize
        a             rdf:Property ;
        rdfs:comment  "Size of the ventilating pipe(s)."@en ;
        rdfs:label    "VentilatingPipeSize"@en .

PSD:Activation  a     rdf:Property ;
        rdfs:comment  "Identifies the predefined methods of sprinkler activation from which that required may be set."@en ;
        rdfs:label    "Activation"@en .

PSD:BarAllocationType
        a             rdf:Property ;
        rdfs:comment  "Defines the type of the reinforcement bar allocation."@en ;
        rdfs:label    "BarAllocationType"@en .

PSD:a   a             rdf:Property ;
        rdfs:comment  "Measure a according to ISO 2553"@en ;
        rdfs:label    "a"@en .

PSD:SetPointFrost  a  rdf:Property ;
        rdfs:comment  "The detection of frost."@en ;
        rdfs:label    "SetPointFrost"@en .

PSD:DuctSizingMethod  a  rdf:Property ;
        rdfs:comment  "Enumeration that identifies the methodology to be used to size system components."@en ;
        rdfs:label    "DuctSizingMethod"@en .

PSD:SetPointLevel  a  rdf:Property ;
        rdfs:comment  "The fill level value to be sensed. Use IfcPropertyBoundedValue.SetPointValue to set the set point value."@en ;
        rdfs:label    "SetPointLevel"@en .

PSD:EarthFault1PolePowerFactorMinimumState
        a             rdf:Property ;
        rdfs:comment  "Power factor of the minimum 1 pole earth fault current provided at the point of supply i.e. the fault between 1 phase and PE/PEN."@en ;
        rdfs:label    "EarthFault1PolePowerFactorMinimumState"@en .

PSD:CurrentForTimeDelay
        a             rdf:Property ;
        rdfs:comment  "The tripping current in [x In] at which the time delay is specified. A value for this property should only be asserted for time delay of L-function, and for I2t of the S and G function."@en ;
        rdfs:label    "CurrentForTimeDelay"@en .

PSD:NominalBodyWidth  a  rdf:Property ;
        rdfs:comment  "Nominal or quoted length measured along the y-axis in the local coordinate system of the drain."@en , "Nominal or quoted length, measured along the y-axis of the local coordinate system of the object, of the body of the object."@en , "Nominal or quoted length measured along the y-axis in the local coordinate system of the waste."@en ;
        rdfs:label    "NominalBodyWidth"@en .

PSD:NominalCurrentAdjusted
        a             rdf:Property ;
        rdfs:comment  "An indication if the tripping currents of the short time protection is related to the nominal current multiplied with the actual setting of the current adjustment, if any, of the long time protection part of the protective device, or not."@en ;
        rdfs:label    "NominalCurrentAdjusted"@en .

PSD:NominalDamperDiameter
        a             rdf:Property ;
        rdfs:comment  "Nominal damper diameter."@en ;
        rdfs:label    "Nominal damper diameter"@en .

PSD:requiredPset  a  owl:ObjectProperty ;
        rdfs:domain  PSD:InformationDeliverySpecification ;
        rdfs:range   PSD:RequiredPset .

PSD:Standard  a       rdf:Property ;
        rdfs:comment  "The designation of the standard applicable for the definition of the Cable/Bus used."@en , "The designation of the standard applicable for the definition of the core used."@en ;
        rdfs:label    "Standard"@en .

PSD:IsNormallyOpen  a  rdf:Property ;
        rdfs:comment  "If TRUE, the valve is normally open. If FALSE is is normally closed."@en ;
        rdfs:label    "IsNormallyOpen"@en .

PSD:ShortCircuit1PolePowerFactorMaximumState
        a             rdf:Property ;
        rdfs:comment  "Power factor of the maximum 1 pole short circuit current provided at the point of supply i.e. the fault between 1 phase and N."@en ;
        rdfs:label    "ShortCircuit1PolePowerFactorMaximumState"@en .

PSD:CompressorTotalEfficiency
        a             rdf:Property ;
        rdfs:comment  "Ratio of the thermal cooling capacity to electrical input."@en ;
        rdfs:label    "CompressorTotalEfficiency"@en .

PSD:ThermometerType  a  rdf:Property ;
        rdfs:comment  "Identifies the means by which temperature is displayed."@en ;
        rdfs:label    "ThermometerType"@en .

PSD:ShortCircuit1PoleMaximumState
        a             rdf:Property ;
        rdfs:comment  "Maximum 1 pole short circuit current provided at the point of supply i.e. the fault between 1 phase and N."@en ;
        rdfs:label    "ShortCircuit1PoleMaximumState"@en .

PSD:NeckAirVelocity  a  rdf:Property ;
        rdfs:comment  "Air velocity at the neck."@en ;
        rdfs:label    "NeckAirVelocity"@en .

PSD:Spectrum  a       rdf:Property ;
        rdfs:comment  "The spectrum of radiation describes its composition with regard to wavelength. Light, for example, as the portion of electromagnetic radiation that is visible to the human eye, is radiation with wavelengths in the range of approx. 380 to 780 nm (1 nm = 10 m). The corresponding range of colours varies from violet to indigo, blue, green, yellow, orange, and red. These colours form a continuous spectrum, in which the various spectral sectors merge into each other."@en ;
        rdfs:label    "Spectrum"@en .

PSD:Surface2  a       rdf:Property ;
        rdfs:comment  "See Surface1."@en ;
        rdfs:label    "Surface2"@en .

PSD:BulbLiquidColor  a  rdf:Property ;
        rdfs:comment  "The color of the liquid in the bulb for a bulb activated sprinkler. Note that the liquid color varies according to the activation temperature requirement of the sprinkler head. Note also that this property does not need to be asserted for quick response activated sprinklers."@en ;
        rdfs:label    "BulbLiquidColor"@en .

PSD:IsMountedFlatCable
        a             rdf:Property ;
        rdfs:comment  "Indication of whether the cable occurrences are mounted flat (= TRUE) or in a trefoil pattern (= FALSE)."@en ;
        rdfs:label    "IsMountedFlatCable"@en .

PSD:ReasonForChange  a  rdf:Property ;
        rdfs:comment  "A description of the problem for why a change is needed."@en ;
        rdfs:label    "ReasonForChange"@en .

PSD:Diameter  a       rdf:Property ;
        rdfs:comment  "Actual diameter of a fin for circular fins only."@en , "Diameter of the object. It is the diameter of the handrail of the railing.\\nThe size information is provided in addition to the shape representation and the geometric parameters used within. In cases of inconsistency between the geometric parameters and the size properties, provided in the attached property set, the geometric parameters take precedence.\\nHere the diameter of the hand or guardrail within the railing."@en , "The requested diameter (in elevation) of the provision for void, only provided if the Shape property is set to 'round'."@en ;
        rdfs:label    "Diameter"@en .

PSD:ColorTemperature  a  rdf:Property ;
        rdfs:comment  "The color temperature of any source of radiation is defined as the temperature (in Kelvin) of a black-body or Planckian radiator whose radiation has the same chromaticity as the source of radiation. Often the values are only approximate color temperatures as the black-body radiator cannot emit radiation of every chromaticity value. The color temperatures of the commonest artificial light sources range from less than 3000K (warm white) to 4000K (intermediate) and over 5000K (daylight)."@en ;
        rdfs:label    "Color temperature"@en .

PSD:CondenserMeanVoidFraction
        a             rdf:Property ;
        rdfs:comment  "Mean void fraction in condenser."@en ;
        rdfs:label    "CondenserMeanVoidFraction"@en .

PSD:VisibleRefractionIndex
        a             rdf:Property ;
        rdfs:comment  "Index of refraction (visible) defines the \\\"bending\\\" of the sola! r ray in the visible spectrum when it passes from one medium into another."@en ;
        rdfs:label    "Visible refraction index"@en .

PSD:ImpellerDiameter  a  rdf:Property ;
        rdfs:comment  "Diameter of compressor impeller - used to scale performance of geometrically similar compressors."@en ;
        rdfs:label    "Impeller diameter"@en .

PSD:LoadBearingCapacity
        a           rdf:Property ;
        rdfs:label  "Load bearing capacity"@en .

PSD:PowerLoss  a      rdf:Property ;
        rdfs:comment  "Total loss of power across this cable."@en ;
        rdfs:label    "PowerLoss"@en .

PSD:EdgeFixingPlateFlangeWidthInPlaneZ
        a             rdf:Property ;
        rdfs:comment  "The flange width of the L-shaped edge plate in plane Z."@en ;
        rdfs:label    "EdgeFixingPlateFlangeWidthInPlaneZ"@en .

PSD:Species  a        rdf:Property ;
        rdfs:comment  "Wood species of a solid wood or laminated wood product."@en ;
        rdfs:label    "Species"@en .

PSD:CrossSectionalArea
        a             rdf:Property ;
        rdfs:comment  "Cross section area of the phase(s) lead(s)."@en ;
        rdfs:label    "CrossSectionalArea"@en .

PSD:ConditionTermination
        a             rdf:Property ;
        rdfs:comment  "Condition of property required on termination of the agreement e.g. cold shell, warm lit shell, broom clean, turn-key."@en ;
        rdfs:label    "ConditionTermination"@en .

PSD:LadderConfiguration
        a             rdf:Property ;
        rdfs:comment  "Description of the configuration of the ladder structure used."@en ;
        rdfs:label    "LadderConfiguration"@en .

PSD:RadioactiveWastePerUnit
        a           rdf:Property ;
        rdfs:label  "Radioactive waste per unit"@en .

PSD:applicability  a  owl:FunctionalProperty , owl:DatatypeProperty ;
        rdfs:comment  "Description of applicability and usecases, i.e., \"IfcDoor entity\", \"Common Pset of Ifc...\""@en ;
        rdfs:domain   PSD:PropertySetDef ;
        rdfs:label    "Applicability"@en ;
        rdfs:range    xsd:string .

PSD:HollowCorePlugging
        a           rdf:Property ;
        rdfs:label  "Hollow core plugging"@en .

PSD:Construction  a   rdf:Property ;
        rdfs:comment  "Purpose of informing on how the vonductor is constucted (interwined or solid). I.e. Solid (IEV 461-01-06), stranded (IEV 461-01-07), solid-/finestranded(IEV 461-01-11) (not flexible/flexible)."@en ;
        rdfs:label    "Construction"@en .

PSD:FireFightingLift  a  rdf:Property ;
        rdfs:label  "Fire fighting lift"@en .

PSD:SetPointMoisture  a  rdf:Property ;
        rdfs:comment  "The moisture value to be sensed. Use IfcPropertyBoundedValue.SetPointValue to set the set point value."@en ;
        rdfs:label    "SetPointMoisture"@en .

PSD:VisibleReflectanceBack
        a             rdf:Property ;
        rdfs:comment  "Reflectance at normal incidence (visible): back side. Defines the fraction of the solar ray in the visible spectrum that is reflected and not transmitted when the ray passes from one medium into another, at the 'back' side of the other material, perpendicular to the surface. Dependent on material and surface characteristics."@en ;
        rdfs:label    "VisibleReflectanceBack"@en .

PSD:MaximumFlowRate  a  rdf:Property ;
        rdfs:comment  "Maximum rate of flow which the meter is expected to pass."@en ;
        rdfs:label    "MaximumFlowRate"@en .

PSD:PercentageOpen  a  rdf:Property ;
        rdfs:comment  "The ratio between the amount that the valve is open to the full open position of the valve."@en ;
        rdfs:label    "PercentageOpen"@en .

PSD:BatterAtEnd  a  rdf:Property ;
        rdfs:label  "Batter at end"@en .

PSD:PropertySetDef  a    owl:Class ;
        rdfs:comment     "Top node element of PSD."@en ;
        rdfs:label       "Property set definition"@en ;
        rdfs:subClassOf  owl:Thing ;
        rdfs:subClassOf  [ a                   owl:Restriction ;
                           owl:maxCardinality  "1"^^xsd:nonNegativeInteger ;
                           owl:onProperty      PSD:name
                         ] ;
        rdfs:subClassOf  [ a                   owl:Restriction ;
                           owl:maxCardinality  "1"^^xsd:nonNegativeInteger ;
                           owl:onProperty      PSD:definition
                         ] ;
        rdfs:subClassOf  [ a                  owl:Restriction ;
                           owl:allValuesFrom  IFC4:IfcProduct ;
                           owl:onProperty     PSD:applicableClass
                         ] .

PSD:Workability  a  rdf:Property ;
        rdfs:label  "Workability"@en .

PSD:TreadLength  a  rdf:Property ;
        rdfs:label  "Tread length"@en .

PSD:BatchReference  a  rdf:Property ;
        rdfs:comment  "The identity of the batch reference from which an occurrence of a product is taken."@en ;
        rdfs:label    "BatchReference"@en .

PSD:NominalPartLoadRatio
        a             rdf:Property ;
        rdfs:comment  "Allowable part load ratio range."@en ;
        rdfs:label    "Nominal part load ratio"@en .

PSD:NominalStaticPressure
        a             rdf:Property ;
        rdfs:comment  "The static pressure within the air stream that the fan must overcome to insure designed circulation of air."@en ;
        rdfs:label    "Nominal static pressure"@en .

PSD:JunctionLeftRadius
        a             rdf:Property ;
        rdfs:comment  "The radius of bending for the left junction."@en ;
        rdfs:label    "JunctionLeftRadius"@en .

PSD:HasPartWinding  a  rdf:Property ;
        rdfs:comment  "Indication of whether the motor is single speed, i.e. has a single winding (= FALSE) or multi-speed i.e.has part winding (= TRUE) ."@en ;
        rdfs:label    "HasPartWinding"@en .

PSD:HeatingTemperatureDelta
        a             rdf:Property ;
        rdfs:comment  "Heating temperature difference for calculating space air flow rates."@en ;
        rdfs:label    "Heating temperature delta"@en .

PSD:NumberOfBoltholes
        a             rdf:Property ;
        rdfs:comment  "Number of boltholes in the flange."@en ;
        rdfs:label    "NumberOfBoltholes"@en .

PSD:ShortInsideCenterTopBarPitch
        a             rdf:Property ;
        rdfs:comment  "The pitch length of the short inside center top bar."@en ;
        rdfs:label    "ShortInsideCenterTopBarPitch"@en .

PSD:CompressedAirFilterType
        a             rdf:Property ;
        rdfs:comment  "ACTIVATEDCARBON: absorbs oil vapor and odor; PARTICLE_FILTER: used to absorb solid particles of medium size; COALESCENSE_FILTER: used to absorb fine solid, oil, and water particles, also called micro filter"@en ;
        rdfs:label    "CompressedAirFilterType"@en .

PSD:IsMain  a         rdf:Property ;
        rdfs:comment  "Identifies if the current instance is a main distribution point or topmost level in an electrical distribution hierarchy (= TRUE) or a sub-main distribution point (= FALSE)."@en ;
        rdfs:label    "IsMain"@en .

PSD:ThreadLength  a   rdf:Property ;
        rdfs:comment  "Nominal length of the thread"@en ;
        rdfs:label    "ThreadLength"@en .

PSD:ScheduleCost  a   rdf:Property ;
        rdfs:comment  "The budgeted cost on behalf of the resource allocation."@en ;
        rdfs:label    "ScheduleCost"@en .

PSD:PoissonRatio  a   rdf:Property ;
        rdfs:comment  "A measure of the lateral deformations in the elastic range."@en ;
        rdfs:label    "PoissonRatio"@en .

PSD:NumberOfPlates  a  rdf:Property ;
        rdfs:comment  "Number of plates used by the plate heat exchanger."@en ;
        rdfs:label    "NumberOfPlates"@en .

PSD:MaximumPressureLoss
        a             rdf:Property ;
        rdfs:comment  "Pressure loss expected across the meter under conditions of maximum flow."@en ;
        rdfs:label    "MaximumPressureLoss"@en .

PSD:TunerType  a      rdf:Property ;
        rdfs:comment  "Indicates the tuner type."@en ;
        rdfs:label    "TunerType"@en .

PSD:AudioVolume  a    rdf:Property ;
        rdfs:comment  "Indicates discrete audio volume levels and corresponding sound power offsets, if applicable.  Missing values may be interpolated."@en ;
        rdfs:label    "Audio volume"@en .

PSD:TotalWattage  a   rdf:Property ;
        rdfs:comment  "Wattage on whole lightfitting device with all sources intact."@en ;
        rdfs:label    "TotalWattage"@en .

PSD:LampBallastType  a  rdf:Property ;
        rdfs:comment  "The type of ballast used to stabilise gas discharge by limiting the current during operation and to deliver the necessary striking voltage for starting. Ballasts are needed to operate Discharge Lamps such as Fluorescent, Compact Fluorescent, High-pressure Mercury, Metal Halide and High-pressure Sodium Lamps. \\nMagnetic ballasts are chokes which limit the current passing through a lamp connected in series on the principle of self-induction. The resultant current and power are decisive for the efficient operation of the lamp. A specially designed ballast is required for every type of lamp to comply with lamp rating in terms of Luminous Flux, Color Appearance and service life. The two types of magnetic ballasts for fluorescent lamps are KVG Conventional   (EC-A series) and VVG Low-loss ballasts (EC-B series). Low-loss ballasts have a higher efficiency, which means reduced ballast losses and a lower thermal load. Electronic ballasts are used to run fluorescent lamps at high frequencies (approx. 35 - 40 kHz)."@en ;
        rdfs:label    "Lamp ballast type"@en .

PSD:LeakageClass  a   rdf:Property ;
        rdfs:comment  "Nominal leakage rating for the system components."@en ;
        rdfs:label    "LeakageClass"@en .

PSD:Process  a        rdf:Property ;
        rdfs:comment  "Reference number of the welding process according to ISO 4063, an up to three digits long code"@en ;
        rdfs:label    "Process"@en .

PSD:VideoCaptionMode  a  rdf:Property ;
        rdfs:comment  "Indicates video closed captioning modes."@en , "Indicates closed captioning modes."@en ;
        rdfs:label    "VideoCaptionMode"@en .

PSD:ExposureClass  a  rdf:Property ;
        rdfs:label  "Exposure class"@en .

PSD:AirPressureDropCurves
        a             rdf:Property ;
        rdfs:comment  "Air pressure drop as function of air flow rate."@en ;
        rdfs:label    "AirPressureDropCurves"@en .

PSD:SelfExtinguishing60332_1
        a             rdf:Property ;
        rdfs:comment  "Self Extinguishing cable/core according to IEC 60332.1."@en ;
        rdfs:label    "SelfExtinguishing60332_1"@en .

PSD:definedValue  a  owl:ObjectProperty ;
        rdfs:domain  PSD:TypePropertyTableValue ;
        rdfs:label   "Defining value"@en ;
        rdfs:range   PSD:Value .

PSD:ShearModulus  a   rdf:Property ;
        rdfs:comment  "A measure of the shear modulus of elasticity of the material."@en ;
        rdfs:label    "ShearModulus"@en .

PSD:Shortening  a   rdf:Property ;
        rdfs:label  "Shortening"@en .

PSD:LadderTrussCrossBarSpacing
        a             rdf:Property ;
        rdfs:comment  "The spacing between the straight cross-bars."@en ;
        rdfs:label    "LadderTrussCrossBarSpacing"@en .

PSD:StirrupBarPitch  a  rdf:Property ;
        rdfs:comment  "The pitch length of the stirrup bar."@en ;
        rdfs:label    "StirrupBarPitch"@en .

PSD:BoilingPoint  a   rdf:Property ;
        rdfs:comment  "The boiling point of the material (fluid)."@en ;
        rdfs:label    "BoilingPoint"@en .

PSD:LongInsideEndLowerBarPitch
        a             rdf:Property ;
        rdfs:comment  "The pitch length of the long inside end lower bar."@en ;
        rdfs:label    "LongInsideEndLowerBarPitch"@en .

PSD:MaximumCurrent  a  rdf:Property ;
        rdfs:comment  "The maximum allowed current that a device is certified to handle."@en ;
        rdfs:label    "MaximumCurrent"@en .

PSD:PressureGaugeType
        a             rdf:Property ;
        rdfs:comment  "Identifies the means by which pressure is displayed."@en ;
        rdfs:label    "PressureGaugeType"@en .

PSD:ExhaustAirFlowrate
        a             rdf:Property ;
        rdfs:comment  "Design exhaust air flow rate for the space."@en ;
        rdfs:label    "ExhaustAirFlowrate"@en .

PSD:AreaPerOccupant  a  rdf:Property ;
        rdfs:comment  "Design occupancy loading for this type of usage assigned to this space."@en ;
        rdfs:label    "AreaPerOccupant"@en .

PSD:ThermalIrEmissivityFront
        a             rdf:Property ;
        rdfs:comment  "Thermal IR emissivity: front side. Defines the fraction of thermal energy emitted per unit area to 'blackbody' at the same temperature, through the 'front' side of the material."@en ;
        rdfs:label    "ThermalIrEmissivityFront"@en .

PSD:PlayerMediaEject  a  rdf:Property ;
        rdfs:comment  "Indicates whether the media can be ejected from the player (if physical media)."@en ;
        rdfs:label    "PlayerMediaEject"@en .

PSD:ResidualFlowingPressure
        a             rdf:Property ;
        rdfs:comment  "The residual flowing pressure in the pipeline at which the discharge flow rate is determined."@en ;
        rdfs:label    "ResidualFlowingPressure"@en .

PSD:HasReturnAir  a   rdf:Property ;
        rdfs:comment  "Terminal box has return air mixed with supply air from duct work."@en ;
        rdfs:label    "Has return air"@en .

PSD:LockedRotorCurrent
        a             rdf:Property ;
        rdfs:comment  "Input current when a motor armature is energized but not rotating."@en ;
        rdfs:label    "LockedRotorCurrent"@en .

PSD:ManualOverride  a  rdf:Property ;
        rdfs:comment  "Identifies whether hand-operated operation is provided as an override (= TRUE) or not (= FALSE). Note that this value should be set to FALSE by default in the case of a Hand Operated Actuator."@en ;
        rdfs:label    "Manual override"@en .

PSD:valueItem  a    owl:DatatypeProperty ;
        rdfs:label  "Value item"@en ;
        rdfs:range  xsd:string .

PSD:Finishing  a      rdf:Property ;
        rdfs:comment  "The finishing applied to system furniture elements of this type e.g. walnut, fabric."@en ;
        rdfs:label    "Finishing"@en .

PSD:FinishType  a     rdf:Property ;
        rdfs:comment  "The type of finish for the air terminal."@en ;
        rdfs:label    "Finish type"@en .

PSD:Category  a       rdf:Property ;
        rdfs:comment  "Designation of the category into which the actors in the population belong."@en ;
        rdfs:label    "Category"@en .

PSD:UACurve  a        rdf:Property ;
        rdfs:comment  "UA value as a  function of fan speed at certain water flow rate, UA = f ( fan speed)."@en , "UA curve as function of ambient temperature and surface temperature; UA = f (Tambient, Tsurface)"@en ;
        rdfs:label    "UACurve"@en .

PSD:OperationTemperatureRange
        a             rdf:Property ;
        rdfs:comment  "Allowable operation ambient air temperature range."@en ;
        rdfs:label    "Operation temperature range"@en .

PSD:CommencementDate  a  rdf:Property ;
        rdfs:comment  "Date on which the agreement commences."@en ;
        rdfs:label    "CommencementDate"@en .

PSD:InductionRatio  a  rdf:Property ;
        rdfs:comment  "Induction ratio versus distance from the diffuser and its discharge direction; induction ratio (or entrainment ratio) is the ratio of the volumetric flow rate in the jet to the volumetric flow rate at the air terminal."@en ;
        rdfs:label    "InductionRatio"@en .

PSD:IsTimeTolerancePositiveOnly
        a             rdf:Property ;
        rdfs:comment  "Indication whether the value of  TimeTolerance1 is provided as a positive tolereance only  or not. If not, the value is proved as a pluss/minus tolerance."@en ;
        rdfs:label    "IsTimeTolerancePositiveOnly"@en .

PSD:ElectricMotorEfficiency
        a             rdf:Property ;
        rdfs:comment  "The ratio of output capacity to intake capacity."@en ;
        rdfs:label    "ElectricMotorEfficiency"@en .

PSD:AtmosphericAcidification
        a           rdf:Property ;
        rdfs:label  "Atmospheric acidification"@en .

PSD:CountedEfficiency
        a             rdf:Property ;
        rdfs:comment  "Filter efficiency based the particle counts concentration before and after filter against particles with certain size distribution."@en ;
        rdfs:label    "CountedEfficiency"@en .

PSD:IsFreeHanging  a  rdf:Property ;
        rdfs:comment  "Is it free hanging type (not mounted in a false ceiling)?"@en ;
        rdfs:label    "IsFreeHanging"@en .

PSD:RemainingCost  a  rdf:Property ;
        rdfs:comment  "The remaining cost on behalf of the resource allocation."@en ;
        rdfs:label    "RemainingCost"@en .

PSD:ShortCircuit3PoleMaximumState
        a             rdf:Property ;
        rdfs:comment  "Maximum 3 pole short circuit current provided at the point of supply."@en ;
        rdfs:label    "ShortCircuit3PoleMaximumState"@en .

PSD:SelectorType  a   rdf:Property ;
        rdfs:comment  "A list of the available types of selector switch from which that required may be selected."@en ;
        rdfs:label    "SelectorType"@en .

PSD:OverallDepth  a   rdf:Property ;
        rdfs:comment  "Overall depth of the profile."@en ;
        rdfs:label    "OverallDepth"@en .

PSD:InertWastePerUnit
        a           rdf:Property ;
        rdfs:label  "Inert waste per unit"@en .

PSD:PlanningControlStatus
        a             rdf:Property ;
        rdfs:comment  "Label of zoning category or class, or planning control category for the site or facility."@en ;
        rdfs:label    "Planning control status"@en , "PlanningControlStatus"@en .

PSD:Version  a        rdf:Property ;
        rdfs:comment  "The version number of the agreement that is identified."@en ;
        rdfs:label    "Version"@en .

PSD:RelativeHumidity  a  rdf:Property ;
        rdfs:comment  "Loads from the relative humidity."@en ;
        rdfs:label    "RelativeHumidity"@en .

PSD:ParkingUnits  a   rdf:Property ;
        rdfs:comment  "Indicates the number of transporation units of the type specified by the property ParkingUse that may be accommodated within the space. Generally, this value should default to 1 unit. However, where the parking space is for motorcycles or bicycles, provision may be made for more than one unit in the space."@en ;
        rdfs:label    "ParkingUnits"@en .

PSD:CarrierStackNumber
        a             rdf:Property ;
        rdfs:comment  "Number of carrier segments (tray, ladder etc.) that are vertically stacked (vertical is measured as the z-axis of the local coordinate system of the carrier segment)."@en ;
        rdfs:label    "CarrierStackNumber"@en .

PSD:KeyShape  a       rdf:Property ;
        rdfs:comment  "If applicable, shape of the head's slot, e.g. 'Slot', 'Allen'"@en ;
        rdfs:label    "KeyShape"@en .

PSD:LadderTrussBaseBarDiameter
        a             rdf:Property ;
        rdfs:comment  "The nominal diameter of the base bar."@en ;
        rdfs:label    "LadderTrussBaseBarDiameter"@en .

PSD:NonHazardousWastePerUnit
        a           rdf:Property ;
        rdfs:label  "Non hazardous waste per unit"@en .

PSD:SwitchOperation  a  rdf:Property ;
        rdfs:comment  "Indicates operation of emergency stop switch."@en ;
        rdfs:label    "SwitchOperation"@en .

PSD:WindSensorType  a  rdf:Property ;
        rdfs:comment  "Enumeration that Identifies the types of wind sensors that can be specified."@en ;
        rdfs:label    "WindSensorType"@en .

PSD:CoreType  a       rdf:Property ;
        rdfs:comment  "Identifies the way the core of the AirTerminal is constructed."@en ;
        rdfs:label    "Core type"@en .

PSD:StratosphericOzoneLayerDestruction
        a           rdf:Property ;
        rdfs:label  "Stratospheric ozone layer destruction"@en .

PSD:AssetInsuranceType
        a             rdf:Property ;
        rdfs:comment  "Identifies the predefined types of insurance rating from which the type required may be set."@en ;
        rdfs:label    "Asset insurance type"@en .

PSD:Type1  a          rdf:Property ;
        rdfs:comment  "Type of weld seam according to ISO 2553.  Note, combined welds are given by two corresponding symbols in the direction of the normal axis of the coordinate system.  For example, an X weld is specified by Type1 = 'V' and Type2 = 'V'."@en ;
        rdfs:label    "Type1"@en .

PSD:TiltAngle  a      rdf:Property ;
        rdfs:comment  "The angle of tilt defined in the plane perpendicular to the extrusion axis (X-Axis of the local placement). The angle shall be measured from the orientation of the Z-Axis in the local placement."@en ;
        rdfs:label    "TiltAngle"@en .

PSD:SecurityRating  a  rdf:Property ;
        rdfs:label  "Security rating"@en .

PSD:StemTopWidth  a   rdf:Property ;
        rdfs:comment  "Stem top width of the profile."@en ;
        rdfs:label    "StemTopWidth"@en .

PSD:WaterPressureDropCurves
        a             rdf:Property ;
        rdfs:comment  "Water pressure drop as function of water flow rate."@en ;
        rdfs:label    "WaterPressureDropCurves"@en .

PSD:LossCoefficient  a  rdf:Property ;
        rdfs:comment  "Dimensionless loss coefficient used for calculating fluid resistance representing the ratio of total pressure loss to velocity pressure at a referenced cross-section."@en ;
        rdfs:label    "LossCoefficient"@en .

PSD:PhotochemicalOzoneFormationPerUnit
        a           rdf:Property ;
        rdfs:label  "Photochemical ozone formation per unit"@en .

PSD:TerminationDate  a  rdf:Property ;
        rdfs:comment  "Date on which the agreement terminates."@en ;
        rdfs:label    "TerminationDate"@en .

PSD:SprinklerProtection
        a           rdf:Property ;
        rdfs:label  "Sprinkler protection"@en .

PSD:CoilLength  a     rdf:Property ;
        rdfs:comment  "Length of coil."@en ;
        rdfs:label    "CoilLength"@en .

PSD:CoilWidth  a      rdf:Property ;
        rdfs:comment  "Width of coil."@en ;
        rdfs:label    "CoilWidth"@en .

PSD:SolarAbsorption  a  rdf:Property ;
        rdfs:label  "Solar absorption"@en .

PSD:NominalInletAirPressure
        a             rdf:Property ;
        rdfs:comment  "Nominal airflow inlet static pressure."@en ;
        rdfs:label    "Nominal inlet air pressure"@en .

PSD:HousingThickness  a  rdf:Property ;
        rdfs:comment  "Air terminal box housing material thickness."@en ;
        rdfs:label    "Housing thickness"@en .

PSD:IsAutomatic  a    rdf:Property ;
        rdfs:comment  "Indication of whether the valve is automatically operated (TRUE) or manually operated (FALSE)."@en ;
        rdfs:label    "IsAutomatic"@en .

PSD:ApplicableStructuralDesignMethod
        a             rdf:Property ;
        rdfs:comment  "Determines whether mechanical material properties are applicable to 'ASD' = allowable stress design (working stress design), 'LSD' = limit state design, or 'LRFD' = load and resistance factor design."@en ;
        rdfs:label    "ApplicableStructuralDesignMethod"@en .

PSD:ToggleSwitchType  a  rdf:Property ;
        rdfs:comment  "A list of the available types of toggle switch from which that required may be selected."@en ;
        rdfs:label    "ToggleSwitchType"@en .

PSD:ReleaseTime  a    rdf:Property ;
        rdfs:comment  "The release time in [s] for the initial tripping of the relevant part. This time indicates that for current lower than the indicated release current, the tripping time will be longer than the indicated release time. The value is given as a mean value."@en ;
        rdfs:label    "ReleaseTime"@en .

PSD:MeasuredPressureDrop
        a             rdf:Property ;
        rdfs:comment  "The actual pressure drop in the fluid measured across the valve."@en ;
        rdfs:label    "MeasuredPressureDrop"@en .

PSD:WarrantyContent  a  rdf:Property ;
        rdfs:comment  "The content of the warranty."@en ;
        rdfs:label    "WarrantyContent"@en .

PSD:SaturationEfficiency
        a             rdf:Property ;
        rdfs:comment  "Saturation efficiency: Ratio of leaving air absolute humidity to the maximum absolute humidity."@en ;
        rdfs:label    "SaturationEfficiency"@en .

PSD:TotalAirflow  a   rdf:Property ;
        rdfs:comment  "The total design supply air flowrate required for the system for either heating or cooling conditions, whichever is greater."@en ;
        rdfs:label    "Total airflow"@en .

PSD:BeamCoolingCapacity
        a             rdf:Property ;
        rdfs:comment  "Cooling capacity of beam. This excludes cooling capacity of supply air."@en ;
        rdfs:label    "BeamCoolingCapacity"@en .

PSD:Infiltration  a  rdf:Property ;
        rdfs:label  "Infiltration"@en .

PSD:MaximumPartLoadRatio
        a             rdf:Property ;
        rdfs:comment  "Maximum part load ratio as a fraction of nominal capacity."@en ;
        rdfs:label    "Maximum part load ratio"@en .

PSD:AirHandlerFanCoilArrangement
        a             rdf:Property ;
        rdfs:comment  "Enumeration defining the arrangement of the supply air fan and the cooling coil."@en ;
        rdfs:label    "AirHandlerFanCoilArrangement"@en .

PSD:LadderTrussHeight
        a             rdf:Property ;
        rdfs:comment  "The overall height of the truss connector."@en ;
        rdfs:label    "LadderTrussHeight"@en .

PSD:BladePositionAngle
        a             rdf:Property ;
        rdfs:comment  "Blade position angle; angle between the blade and flow direction ( 0 - 90)."@en ;
        rdfs:label    "BladePositionAngle"@en .

PSD:ActualWork  a     rdf:Property ;
        rdfs:comment  "The actual work on behalf of the resource allocation."@en ;
        rdfs:label    "ActualWork"@en .

PSD:SelfTestFunction  a  rdf:Property ;
        rdfs:comment  "The type of self test function."@en ;
        rdfs:label    "SelfTestFunction"@en .

PSD:ColorCode  a      rdf:Property ;
        rdfs:comment  "Name of a color for identifying the connector, if applicable."@en ;
        rdfs:label    "ColorCode"@en .

PSD:YoungModulus  a   rdf:Property ;
        rdfs:comment  "A measure of the Young's modulus of elasticity of the material."@en ;
        rdfs:label    "YoungModulus"@en .

PSD:ShortCircuit2PolePowerFactorMinimumState
        a             rdf:Property ;
        rdfs:comment  "Power factor of the minimum 2 pole short circuit current provided at the point of supply."@en ;
        rdfs:label    "ShortCircuit2PolePowerFactorMinimumState"@en .

PSD:StartCurrentFactor
        a             rdf:Property ;
        rdfs:comment  "IEC. Start current factor defines how large the peak starting current will become on the engine. StartCurrentFactor is multiplied to NominalCurrent and to give the start current."@en , "IEC. Start current factor defines how large the peek starting current will become on the engine. StartCurrentFactor is multiplied to NominalCurrent and we get the start current."@en ;
        rdfs:label    "StartCurrentFactor"@en .

PSD:FractionRadiantHeatTransfer
        a             rdf:Property ;
        rdfs:comment  "Fraction of the total heat transfer rate as the radiant heat transfer."@en ;
        rdfs:label    "FractionRadiantHeatTransfer"@en .

PSD:ConditionCommencement
        a             rdf:Property ;
        rdfs:comment  "Condition of property provided on commencement of the agreement e.g. cold shell, warm lit shell, broom clean, turn-key."@en ;
        rdfs:label    "ConditionCommencement"@en .

PSD:GasPressure  a    rdf:Property ;
        rdfs:comment  "Fill pressure (e.g. for between-pane gas fills): the pressure exerted by a mass of gas confined in a constant volume."@en ;
        rdfs:label    "Gas pressure"@en .

PSD:Pressure  a       rdf:Property ;
        rdfs:comment  "The pressure of the fuel."@en , "The pressure of the fluid."@en ;
        rdfs:label    "Pressure"@en .

PSD:CeilingRAPlenum  a  rdf:Property ;
        rdfs:comment  "Ceiling plenum used for return air or not. TRUE = Yes, FALSE = No."@en ;
        rdfs:label    "CeilingRAPlenum"@en .

PSD:OpenPressureDrop  a  rdf:Property ;
        rdfs:comment  "Total pressure drop across damper."@en ;
        rdfs:label    "OpenPressureDrop"@en .

PSD:DesignAmbientTemperature
        a             rdf:Property ;
        rdfs:comment  "The highest and lowest local ambient temperature likely to be encountered."@en ;
        rdfs:label    "DesignAmbientTemperature"@en .

PSD:definitionAlias  a  owl:DatatypeProperty ;
        rdfs:comment  "Definition alias in local language."@en ;
        rdfs:domain   [ a            owl:Class ;
                        owl:unionOf  ( PSD:PropertySetDef PSD:PropertyDef )
                      ] ;
        rdfs:label    "Definition alias"@en ;
        rdfs:range    xsd:string .

PSD:RefrigerantFoulingResistance
        a             rdf:Property ;
        rdfs:comment  "Fouling resistance on the refrigerant side."@en ;
        rdfs:label    "RefrigerantFoulingResistance"@en .

PSD:DuctSealant  a    rdf:Property ;
        rdfs:comment  "Type of sealant used on the duct and fittings."@en ;
        rdfs:label    "DuctSealant"@en .

PSD:ShortInsideEndTopBarPitch
        a             rdf:Property ;
        rdfs:comment  "The pitch length of the short inside end top bar."@en ;
        rdfs:label    "ShortInsideEndTopBarPitch"@en .

PSD:StandardFixingPlateWidth
        a             rdf:Property ;
        rdfs:comment  "The width of the standard fixing plate."@en ;
        rdfs:label    "StandardFixingPlateWidth"@en .

PSD:LubricantPumpHeatGain
        a             rdf:Property ;
        rdfs:comment  "Lubricant pump heat gain."@en ;
        rdfs:label    "LubricantPumpHeatGain"@en .

PSD:Torque  a         rdf:Property ;
        rdfs:comment  "Indicates the maximum close-off torque for the actuator."@en ;
        rdfs:label    "Torque"@en .

PSD:PressureRange  a  rdf:Property ;
        rdfs:comment  "Allowable maximum and minimum working pressure (relative to ambient pressure)."@en ;
        rdfs:label    "Pressure range"@en , "PressureRange"@en .

PSD:ThermalExpansionCoefficient
        a             rdf:Property ;
        rdfs:comment  "A measure of the expansion coefficient for warming up the material about one Kelvin."@en ;
        rdfs:label    "ThermalExpansionCoefficient"@en .

PSD:Effectiveness  a  rdf:Property ;
        rdfs:comment  "Ratio of the change in dry bulb temperature of the (primary) air stream to the difference between the entering dry bulb temperature of the (primary) air and the wet-bulb temperature of the (secondary) air."@en , "Ratio of the real heat transfer rate to the maximum possible heat transfer rate."@en ;
        rdfs:label    "Effectiveness"@en .

PSD:ReadOutType  a    rdf:Property ;
        rdfs:comment  "Indication of the form that readout from the meter takes. In the case of a dial read out, this may comprise multiple dials that give a cumulative reading and/or a mechanical odometer."@en ;
        rdfs:label    "Read out type"@en .

PSD:AirFlowConfiguration
        a             rdf:Property ;
        rdfs:comment  "Air flow configuration type of cooled beam."@en ;
        rdfs:label    "AirFlowConfiguration"@en .

PSD:LowerCurrent2  a  rdf:Property ;
        rdfs:comment  "The current in [x In], indicating the upper current limit of the lower time/current curve of the I2t part of the L-function."@en ;
        rdfs:label    "LowerCurrent2"@en .

PSD:MarketSubCategoriesAvailableFuture
        a             rdf:Property ;
        rdfs:comment  "A list of the sub categories of property that are expected to be available in the future expressed in terms of IfcLabel."@en ;
        rdfs:label    "Market sub categories available future"@en .

PSD:UsePurpose  a     rdf:Property ;
        rdfs:comment  "The principal purpose for which the work surface is intended to be used e.g. writing/reading, computer, meeting, printer, reference files, etc."@en ;
        rdfs:label    "UsePurpose"@en .

PSD:ApplianceDiversity
        a             rdf:Property ;
        rdfs:comment  "Diversity of appliance load."@en ;
        rdfs:label    "ApplianceDiversity"@en , "Appliance diversity"@en .

PSD:CompressionEfficiency
        a             rdf:Property ;
        rdfs:comment  "Ratio of the work required for isentropic compression of the gas to the work delivered to the gas within the compression volume (as obtained by measurement)."@en ;
        rdfs:label    "CompressionEfficiency"@en .

PSD:ShaftPower  a     rdf:Property ;
        rdfs:comment  "The actual shaft power input to the compressor."@en ;
        rdfs:label    "ShaftPower"@en .

PSD:NominalHeight  a  rdf:Property ;
        rdfs:comment  "The nominal height of the duct segment."@en , "The nominal height of the segment."@en , "The nominal height of the furniture of this type. The size information is provided in addition to the shape representation and the geometric parameters used within. In cases of inconsistency between the geometric parameters and the size properties, provided in the attached property set, the geometric parameters take precedence."@en , "The nominal height of the system furniture elements of this type. The size information is provided in addition to the shape representation and the geometric parameters used within. In cases of inconsistency between the geometric parameters and the size properties, provided in the attached property set, the geometric parameters take precedence."@en ;
        rdfs:label    "NominalHeight"@en , "Nominal height"@en .

PSD:NominalWaterFlowCooling
        a             rdf:Property ;
        rdfs:comment  "Nominal water flow (refers to nominal cooling capacity)."@en ;
        rdfs:label    "NominalWaterFlowCooling"@en .

PSD:Velocity  a       rdf:Property ;
        rdfs:comment  "The velocity of the fluid."@en ;
        rdfs:label    "Velocity"@en .

PSD:FixingSocketTypeReference
        a             rdf:Property ;
        rdfs:comment  "Type reference for the fixing socket according to local standards."@en ;
        rdfs:label    "FixingSocketTypeReference"@en .

PSD:IsOffWhenLfunctionOn
        a             rdf:Property ;
        rdfs:comment  "Indication whether the S-function is automatically switched off when the I-function is switched on."@en ;
        rdfs:label    "IsOffWhenLfunctionOn"@en .

PSD:MediaSource  a    rdf:Property ;
        rdfs:comment  "Indicates media sources and corresponding names of ports (IfcDistributionPort with FlowDirection=SINK and PredefinedType=AUDIOVISUAL) or aggregated audio/video components (IfcAudioVisualAppliance)."@en ;
        rdfs:label    "MediaSource"@en .

PSD:ImpuritiesContent
        a             rdf:Property ;
        rdfs:comment  "Fraction of impurities such as dust to the total amount of water. This is measured in weight of impurities per weight of water and is therefore unitless."@en ;
        rdfs:label    "ImpuritiesContent"@en .

PSD:Fuel  a           rdf:Property ;
        rdfs:comment  "The amount of fuel consumed during the period specified in the time series."@en ;
        rdfs:label    "Fuel"@en .

PSD:SetPointSpeed  a  rdf:Property ;
        rdfs:comment  "The wind speed value to be sensed. Use IfcPropertyBoundedValue.SetPointValue to set the set point value."@en ;
        rdfs:label    "SetPointSpeed"@en .

PSD:GrossPlannedArea  a  rdf:Property ;
        rdfs:label  "Gross planned area"@en .

PSD:DiagonalTrussLength
        a             rdf:Property ;
        rdfs:comment  "The overall length of the truss connector."@en ;
        rdfs:label    "DiagonalTrussLength"@en .

PSD:UpperTime1  a     rdf:Property ;
        rdfs:comment  "The time in [s], indicating that tripping times of the upper time/current curve lower than UpperTime1 is determined by the I2t part of the L-function."@en ;
        rdfs:label    "UpperTime1"@en .

PSD:EvaporatorMeanVoidFraction
        a             rdf:Property ;
        rdfs:comment  "Mean void fraction in evaporator."@en ;
        rdfs:label    "EvaporatorMeanVoidFraction"@en .

PSD:Plies  a          rdf:Property ;
        rdfs:comment  "Number of plies."@en ;
        rdfs:label    "Plies"@en .

PSD:Location  a       rdf:Property ;
        rdfs:comment  "Location  (a single type of diffuser can be used for multiple locations); high means close to ceiling."@en ;
        rdfs:label    "Location"@en .

PSD:ProtectedOpening  a  rdf:Property ;
        rdfs:label  "Protected opening"@en .

PSD:InitialResistance
        a             rdf:Property ;
        rdfs:comment  "Initial new filter fluid resistance (i.e., pressure drop at the maximum air flowrate across the filter when the filter is new per ASHRAE Standard 52.1)."@en ;
        rdfs:label    "Initial resistance"@en .

PSD:HasCover  a       rdf:Property ;
        rdfs:comment  "Indication of whether the cable tray has a cover (=TRUE) or not (= FALSE). By default, this value should be set to FALSE.."@en ;
        rdfs:label    "HasCover"@en .

PSD:InputPower  a     rdf:Property ;
        rdfs:comment  "Input power to the compressor motor."@en ;
        rdfs:label    "InputPower"@en .

PSD:Color  a          rdf:Property ;
        rdfs:comment  "Color selection for this object."@en ;
        rdfs:label    "Color"@en .

PSD:T2  a             rdf:Property ;
        rdfs:comment  "The (thermal) testing time in [s] associated with the testing currents I1 and I2."@en ;
        rdfs:label    "T2"@en .

PSD:DimensionalChangeCoefficient
        a             rdf:Property ;
        rdfs:comment  "Weighted dimensional change coefficient, relative to 1% change in moisture content."@en ;
        rdfs:label    "DimensionalChangeCoefficient"@en .

PSD:NominalParticleGeometricStandardDeviation
        a             rdf:Property ;
        rdfs:comment  "Particle geometric standard deviation associated with nominal efficiency."@en ;
        rdfs:label    "Nominal particle geometric standard deviation"@en .

PSD:CondenserFlowrate
        a             rdf:Property ;
        rdfs:comment  "Flow rate of fluid through the condenser."@en ;
        rdfs:label    "CondenserFlowrate"@en .

PSD:ThermalTransmittanceWinter
        a           rdf:Property ;
        rdfs:label  "Thermal transmittance winter"@en .

PSD:CapacityWeight  a  rdf:Property ;
        rdfs:label  "Capacity weight"@en .

PSD:PlasticStrain  a  rdf:Property ;
        rdfs:comment  "A measure of the permanent displacement, as in slip or twinning, which remains after the stress has been removed. Currently applied to a strain of 0.2% proportional stress of the material."@en ;
        rdfs:label    "Plastic strain"@en .

PSD:Depth  a          rdf:Property ;
        rdfs:comment  "The requested depth or thickness of the provision for void."@en , "The depth of the pit."@en , "The depth of the trench."@en ;
        rdfs:label    "Depth"@en .

PSD:OccupancyType  a  rdf:Property ;
        rdfs:comment  "Occupancy type for this object. It is defined according to the presiding national building code."@en ;
        rdfs:label    "OccupancyType"@en , "Occupancy type"@en .

PSD:NumberOfSlots  a  rdf:Property ;
        rdfs:comment  "Number of slots."@en ;
        rdfs:label    "Number of slots"@en .

PSD:NominalSupplyWaterTemperatureCooling
        a             rdf:Property ;
        rdfs:comment  "Nominal supply water temperature (refers to nominal cooling capacity)."@en ;
        rdfs:label    "NominalSupplyWaterTemperatureCooling"@en .

PSD:DishwasherType  a  rdf:Property ;
        rdfs:comment  "Type of dishwasher."@en ;
        rdfs:label    "DishwasherType"@en .

PSD:HeatingRelativeHumidity
        a             rdf:Property ;
        rdfs:comment  "Inside relative humidity for heating design."@en ;
        rdfs:label    "HeatingRelativeHumidity"@en .

PSD:InfiltrationDiversityWinter
        a             rdf:Property ;
        rdfs:comment  "Diversity factor for Winter infiltration."@en ;
        rdfs:label    "InfiltrationDiversityWinter"@en , "Infiltration diversity winter"@en .

PSD:OccupancyNumberPeak
        a             rdf:Property ;
        rdfs:comment  "Maximal number of people required for the activity assigned to this space in peak time."@en ;
        rdfs:label    "OccupancyNumberPeak"@en .

PSD:NumberOfActors  a  rdf:Property ;
        rdfs:comment  "The number of actors that are to be dealt with together in the population."@en ;
        rdfs:label    "Number of actors"@en .

PSD:DamperPosition  a  rdf:Property ;
        rdfs:comment  "Damper position (0-1); damper position ( 0=closed=90deg position angle, 1=open=0deg position angle."@en , "Control damper position, ranging from 0 to 1."@en ;
        rdfs:label    "DamperPosition"@en , "Damper position"@en .

PSD:Ventilation  a    rdf:Property ;
        rdfs:comment  "Required outside air ventilation."@en ;
        rdfs:label    "Ventilation"@en .

PSD:CurrentToleranceLimit1
        a             rdf:Property ;
        rdfs:comment  "The time limit in [s] limiting the application of CurrentTolerance1, if any. If the value is set to 0, the value of the CurrentTolerance1 is valid for the whole time/current-curve."@en ;
        rdfs:label    "CurrentToleranceLimit1"@en .

PSD:SensibleLoadToRadiant
        a             rdf:Property ;
        rdfs:comment  "Percent of sensible thermal load to radiant heat."@en ;
        rdfs:label    "SensibleLoadToRadiant"@en .

PSD:DischargeFlowRate
        a             rdf:Property ;
        rdfs:comment  "The volumetric rate of fluid discharge."@en ;
        rdfs:label    "DischargeFlowRate"@en .

PSD:LongOutsideLowerBarPitch
        a             rdf:Property ;
        rdfs:comment  "The pitch length of the long outside lower bar."@en ;
        rdfs:label    "LongOutsideLowerBarPitch"@en .

PSD:HasSillExternal  a  rdf:Property ;
        rdfs:label  "Has sill external"@en .

PSD:ReleaseTimeI2tEnd
        a             rdf:Property ;
        rdfs:comment  "The release time in [s] for the end point of the I2 tripping curve of the G-function, if any. The value of ReleaseTimeI2tEnd shall be lower than ReleaseTimeI2tStart."@en , "The release time in [s] for the end point of the I2 tripping curve of the S-function, if any. The value of ReleaseTimeI2tEnd shall be lower than ReleaseTimeI2tStart."@en ;
        rdfs:label    "ReleaseTimeI2tEnd"@en .

PSD:MolecularWeight  a  rdf:Property ;
        rdfs:label  "Molecular weight"@en .

PSD:GlassThickness2  a  rdf:Property ;
        rdfs:label  "Glass thickness 2"@en .

PSD:PowerFactor  a    rdf:Property ;
        rdfs:comment  "Power factor."@en ;
        rdfs:label    "PowerFactor"@en .

PSD:CoreSetVertical  a  rdf:Property ;
        rdfs:comment  "Degree of vertical (in the Y-axis of the LocalPlacement) blade set from the centerline."@en ;
        rdfs:label    "Core set vertical"@en .

PSD:MoistureContent  a  rdf:Property ;
        rdfs:comment  "Total weight of moisture relative to oven-dried weight of the wood."@en ;
        rdfs:label    "MoistureContent"@en .

PSD:SpeakerType  a    rdf:Property ;
        rdfs:comment  "Indicates the type of speaker."@en ;
        rdfs:label    "SpeakerType"@en .

PSD:ReceptacleLoadIntensity
        a             rdf:Property ;
        rdfs:comment  "Average power use intensity of appliances and other non-HVAC equipment in the space per unit area.(PowerMeasure/IfcAreaMeasure)."@en ;
        rdfs:label    "ReceptacleLoadIntensity"@en .

PSD:NominalDiameter  a  rdf:Property ;
        rdfs:comment  "The nominal diameter of the pipe segment."@en , "Nominal diameter or width of the tubes in the tube bundle."@en ;
        rdfs:label    "NominalDiameter"@en .

PSD:NominalPowerRate  a  rdf:Property ;
        rdfs:comment  "Nominal fan power rate."@en ;
        rdfs:label    "Nominal power rate"@en .

PSD:TemperatureRating
        a             rdf:Property ;
        rdfs:comment  "Temperature rating."@en ;
        rdfs:label    "TemperatureRating"@en .

PSD:ExtendToStructure
        a           rdf:Property ;
        rdfs:label  "Extend to structure"@en .

PSD:ProductionLotId  a  rdf:Property ;
        rdfs:comment  "The manufacturer's production lot identifier."@en ;
        rdfs:label    "ProductionLotId"@en .

PSD:e   a             rdf:Property ;
        rdfs:comment  "Measure e according to ISO 2553"@en ;
        rdfs:label    "e"@en .

PSD:MaximumPowerOutput
        a             rdf:Property ;
        rdfs:comment  "The maximum output power rating of the engine."@en ;
        rdfs:label    "MaximumPowerOutput"@en .

PSD:unitType  a     owl:DatatypeProperty ;
        rdfs:label  "Unit type"@en ;
        rdfs:range  [ a            owl:Class ;
                      owl:unionOf  ( IFC4:IfcDerivedUnit IFC4:IfcNamedUnit )
                    ] .

PSD:Leakage  a        rdf:Property ;
        rdfs:comment  "Air leakage rate."@en ;
        rdfs:label    "Leakage"@en .

PSD:ColorAppearance  a  rdf:Property ;
        rdfs:comment  "In both the DIN and CIE standards, artificial light sources are classified in terms of their color appearance. To the human eye they all appear to be white; the difference can only be detected by direct comparison. Visual performance is not directly affected by differences in color appearance."@en ;
        rdfs:label    "Color appearance"@en .

PSD:ProjectorType  a  rdf:Property ;
        rdfs:comment  "Indicates the type of projector."@en ;
        rdfs:label    "ProjectorType"@en .

PSD:Severity  a       rdf:Property ;
        rdfs:comment  "Indicates alarm severity over time, where the scale of values is determined by the control system configuration.  A zero value indicates no present alarm."@en ;
        rdfs:label    "Severity"@en .

PSD:WaterRequirement  a  rdf:Property ;
        rdfs:comment  "Make-up water requirement."@en ;
        rdfs:label    "Water requirement"@en .

PSD:IdealShaftPower  a  rdf:Property ;
        rdfs:comment  "Compressor shaft power under ideal conditions."@en ;
        rdfs:label    "Ideal shaft power"@en .

PSD:LatentCoolingCapacity
        a             rdf:Property ;
        rdfs:comment  "Latent cooling capacity."@en ;
        rdfs:label    "LatentCoolingCapacity"@en .

PSD:FoulingFactor  a  rdf:Property ;
        rdfs:comment  "Fouling factor of the tubes in the tube bundle."@en ;
        rdfs:label    "FoulingFactor"@en .

PSD:ifcVersion  a     owl:ObjectProperty , owl:FunctionalProperty ;
        rdfs:comment  "Version information of IFC release and sub schema."@en ;
        rdfs:domain   PSD:PropertySetDef ;
        rdfs:label    "IFC version"@en ;
        rdfs:range    PSD:IfcVersion .

PSD:EvaporatorCoolant
        a             rdf:Property ;
        rdfs:comment  "The fluid used for the coolant in the evaporator."@en ;
        rdfs:label    "Evaporator coolant"@en .

PSD:CrossingLowerBarPitch
        a             rdf:Property ;
        rdfs:comment  "The pitch length of the crossing lower bar."@en ;
        rdfs:label    "CrossingLowerBarPitch"@en .

PSD:TenureModesAvailableFuture
        a             rdf:Property ;
        rdfs:comment  "A list of the tenure modes that are expected to be available in the future expressed in terms of IfcLabel."@en ;
        rdfs:label    "Tenure modes available future"@en .

PSD:NumberOfRows  a   rdf:Property ;
        rdfs:comment  "Number of tube rows in the tube bundle assembly."@en ;
        rdfs:label    "NumberOfRows"@en .

PSD:N20Content  a     rdf:Property ;
        rdfs:comment  "Nitrous oxide (N2O) content of the products of combustion. This is measured in weight of N2O per unit weight and is therefore unitless."@en ;
        rdfs:label    "N20Content"@en .

PSD:DiagonalTrussSecondaryBarDiameter
        a             rdf:Property ;
        rdfs:comment  "The nominal diameter of the secondary bar."@en ;
        rdfs:label    "DiagonalTrussSecondaryBarDiameter"@en .

PSD:IsHorizontalBusbar
        a             rdf:Property ;
        rdfs:comment  "Indication of whether the busbar occurrences are routed horizontally (= TRUE) or vertically (= FALSE)."@en ;
        rdfs:label    "IsHorizontalBusbar"@en .

PSD:HasIntegralControl
        a             rdf:Property ;
        rdfs:comment  "If TRUE, a self powered temperature control is included in the AirTerminal."@en ;
        rdfs:label    "Has integral control"@en .

PSD:AssessmentDate  a  rdf:Property ;
        rdfs:comment  "Date on which the overall condition is assessed"@en ;
        rdfs:label    "Assessment date"@en .

PSD:AirHandlerConstruction
        a             rdf:Property ;
        rdfs:comment  "Enumeration defining how the air handler might be fabricated."@en ;
        rdfs:label    "AirHandlerConstruction"@en .

PSD:TeTime  a         rdf:Property ;
        rdfs:comment  "The maximum time (in s) at which the motor could run with locked rotor when the motor is used in an EX-environment. The time indicates that a protective device should trip before this time when the starting current of the motor is slowing through the device."@en ;
        rdfs:label    "TeTime"@en .

PSD:MaintenanceLevel  a  rdf:Property ;
        rdfs:comment  "Adjustment of the service life resulting from the effect of the level or degree of maintenance applied to dcomponents."@en ;
        rdfs:label    "MaintenanceLevel"@en .

PSD:VisibleLightReflectance
        a           rdf:Property ;
        rdfs:label  "Visible light reflectance"@en .

PSD:version  a        owl:FunctionalProperty , owl:DatatypeProperty ;
        rdfs:comment  "Version of IFC, i.e., \"2x3 TC1\", \"IFC4\"."@en ;
        rdfs:domain   PSD:IfcVersion ;
        rdfs:label    "Version"@en ;
        rdfs:range    xsd:string .

PSD:AirflowSensible  a  rdf:Property ;
        rdfs:comment  "The air flowrate required to satisfy the sensible peak loads."@en ;
        rdfs:label    "Airflow sensible"@en .

PSD:BreechingInletType
        a             rdf:Property ;
        rdfs:comment  "Defines the type of breeching inlet."@en ;
        rdfs:label    "BreechingInletType"@en .

PSD:NutsCount  a      rdf:Property ;
        rdfs:comment  "Count of nuts to be mounted on one bolt"@en ;
        rdfs:label    "NutsCount"@en .

PSD:SoilConductivity  a  rdf:Property ;
        rdfs:comment  "Thermal conductivity of soil. Generally, within standards such as IEC 60364-5-52, table 52A-16, the resistivity of soil is required (measured in [SI] units of degK.m /W). This is the reciprocal of the conductivity value and needs to be calculated accordingly."@en ;
        rdfs:label    "SoilConductivity"@en .

PSD:Location3Global  a  rdf:Property ;
        rdfs:comment  "Global X,Y,Z coordinates of the point in which Thickness3 is given"@en ;
        rdfs:label    "Location3Global"@en .

PSD:ReactivePower  a  rdf:Property ;
        rdfs:comment  "Reactive power."@en ;
        rdfs:label    "ReactivePower"@en .

PSD:AsBuiltLocationNumber
        a             rdf:Property ;
        rdfs:comment  "Defines a unique location within a structure, the slot into which the piece was installed. Where pieces share the same piece mark, they can be interchanged. The value is only known after erection."@en ;
        rdfs:label    "AsBuiltLocationNumber"@en .

PSD:Arrangement  a    rdf:Property ;
        rdfs:comment  "Defines the basic flow arrangements for the heat exchanger:\\n\\nCOUNTERFLOW: Counterflow heat exchanger arrangement. \\nCROSSFLOW: Crossflow heat exchanger arrangement. \\nPARALLELFLOW: Parallel flow heat exchanger arrangement. \\nMULTIPASS: Multipass flow heat exchanger arrangement. \\nOTHER: Other type of heat exchanger flow arrangement not defined above."@en ;
        rdfs:label    "Arrangement"@en .

PSD:SensibleEffectivenessTable
        a             rdf:Property ;
        rdfs:comment  "Sensible heat transfer effectiveness curve as a function of the primary and secondary air flow rate."@en ;
        rdfs:label    "SensibleEffectivenessTable"@en .

PSD:ActualProductionDate
        a             rdf:Property ;
        rdfs:comment  "Production date (stripped from form)."@en ;
        rdfs:label    "ActualProductionDate"@en .

PSD:RemainingWork  a  rdf:Property ;
        rdfs:comment  "The remaining work on behalf of the resource allocation."@en ;
        rdfs:label    "RemainingWork"@en .

PSD:EfficiencyCurve  a  rdf:Property ;
        rdfs:comment  "Fan efficiency =f (flow rate)."@en ;
        rdfs:label    "Efficiency curve"@en .

PSD:InstallationMethodFlagEnum
        a             rdf:Property ;
        rdfs:comment  "Special installation conditions relating to particular types of installation based on IEC60364-5-52:2001 reference installation methods C and D."@en ;
        rdfs:label    "InstallationMethodFlagEnum"@en .

PSD:ReleaseCurrentI2tEnd
        a             rdf:Property ;
        rdfs:comment  "The release current in [x In] for the end point of the I2t tripping curve of the G-function, if any. The value of ReleaseCurrentI2tEnd shall be larger than ReleaseCurrentI2tStart."@en , "The release current in [x In] for the end point of the I2t tripping curve of the S-function, if any. The value of ReleaseCurrentI2tEnd shall be larger than ReleaseCurrentI2tStart."@en ;
        rdfs:label    "ReleaseCurrentI2tEnd"@en .

PSD:RadioactiveWaste  a  rdf:Property ;
        rdfs:label  "Radioactive waste"@en .

PSD:DrainConnectionSize
        a             rdf:Property ;
        rdfs:comment  "Size of the drain connection inlet to the waste disposal unit."@en ;
        rdfs:label    "DrainConnectionSize"@en .

PSD:MaximumOperatingTemperature
        a             rdf:Property ;
        rdfs:comment  "The maximum temperature at which a cable or bus is certified to operate."@en ;
        rdfs:label    "MaximumOperatingTemperature"@en .

PSD:WireEmbeddingLength
        a             rdf:Property ;
        rdfs:comment  "The length of the part of wire which is embedded in the precast concrete element."@en ;
        rdfs:label    "WireEmbeddingLength"@en .

PSD:Material  a       rdf:Property ;
        rdfs:comment  "Type of material from which the conductor is constructed."@en ;
        rdfs:label    "Material"@en .

PSD:LightFixtureMountingType
        a             rdf:Property ;
        rdfs:comment  "A list of the available types of mounting for light fixtures from which that required may be selected."@en ;
        rdfs:label    "LightFixtureMountingType"@en .

PSD:LongOutsideTopBarPitch
        a             rdf:Property ;
        rdfs:comment  "The pitch length of the long outside top bar."@en ;
        rdfs:label    "LongOutsideTopBarPitch"@en .

PSD:Surface1  a       rdf:Property ;
        rdfs:comment  "Aspect of weld seam surface, i.e. 'plane', 'curved' or 'hollow'.  Combined welds are given by two corresponding symbols analogous to Type1 and Type2."@en ;
        rdfs:label    "Surface1"@en .

PSD:CurveDesignation  a  rdf:Property ;
        rdfs:comment  "The designation of the trippingcurve given by the manufacturer. For a MCB the designation should be in accordance with the designations given in IEC 60898."@en ;
        rdfs:label    "CurveDesignation"@en .

PSD:IsWired  a      rdf:Property ;
        rdfs:label  "Is wired"@en .

PSD:IsExtendedWarranty
        a             rdf:Property ;
        rdfs:comment  "Indication of whether this is an extended warranty whose duration is greater than that normally assigned to an artefact (=TRUE) or not (= FALSE)."@en ;
        rdfs:label    "IsExtendedWarranty"@en .

PSD:Volume  a         rdf:Property ;
        rdfs:comment  "Total volume of fluid in the tubes and their headers."@en ;
        rdfs:label    "Volume"@en .

PSD:HasNonSkidSurface
        a             rdf:Property ;
        rdfs:comment  "Indication whether the surface finish is designed to prevent slippery (TRUE) or not (FALSE)."@en ;
        rdfs:label    "HasNonSkidSurface"@en , "Has non skid surface"@en .

PSD:EnergyGainTotal  a  rdf:Property ;
        rdfs:comment  "The total amount of energy gains for the spaces served by the system during the peak cooling conditions, plus any system-level total energy gains."@en ;
        rdfs:label    "Energy gain total"@en .

PSD:IsHorizontalCable
        a             rdf:Property ;
        rdfs:comment  "Indication of whether the cable occurrences are mounted horizontally (= TRUE) or vertically (= FALSE)."@en ;
        rdfs:label    "IsHorizontalCable"@en .

PSD:SurfaceSpreadOfFlame
        a           rdf:Property ;
        rdfs:label  "Surface spread of flame"@en .

PSD:RentalRatesInCategoryNow
        a             rdf:Property ;
        rdfs:comment  "Range of the cost rates for property currently available in the required category."@en ;
        rdfs:label    "Rental rates in category now"@en .

PSD:JunctionRightAngle
        a             rdf:Property ;
        rdfs:comment  "The change of direction of flow for the right junction where 0 indicates straight segment."@en ;
        rdfs:label    "JunctionRightAngle"@en .

PSD:XDirectionUpperBarCount
        a             rdf:Property ;
        rdfs:comment  "The number of bars with X direction upper bar."@en ;
        rdfs:label    "XDirectionUpperBarCount"@en .

PSD:TimeToleranceLimit1
        a             rdf:Property ;
        rdfs:comment  "The current limit in [x In] limiting the application of TimeTolerance1, if any. If the value is set to 0, the value of the TimeTolerance1 is valid for the whole time/current-curve."@en ;
        rdfs:label    "TimeToleranceLimit1"@en .

PSD:SetPointConcentration
        a             rdf:Property ;
        rdfs:comment  "The ion concentration value to be sensed. Use IfcPropertyBoundedValue.SetPointValue to set the set point value."@en , "The gas concentration value to be sensed. Use IfcPropertyBoundedValue.SetPointValue to set the set point value."@en , "The carbon dioxide concentration to be sensed. Use IfcPropertyBoundedValue.SetPointValue to set the set point value."@en , "The smoke concentration value to be sensed. Use IfcPropertyBoundedValue.SetPointValue to set the set point value."@en ;
        rdfs:label    "SetPointConcentration"@en .

PSD:Quality  a        rdf:Property ;
        rdfs:comment  "Indicates the quality of measurement or failure condition, which may be further qualified by the Status.  True: measured values are considered reliable; False: measured values are considered not reliable (i.e. a fault has been detected); Unknown: reliability of values is uncertain."@en ;
        rdfs:label    "Quality"@en .

PSD:DiagonalTrussCrossBarSpacing
        a             rdf:Property ;
        rdfs:comment  "The spacing between diagonal cross-bar sections."@en ;
        rdfs:label    "DiagonalTrussCrossBarSpacing"@en .

PSD:VentilationOutdoorAir
        a             rdf:Property ;
        rdfs:comment  "Ventilation loads from outdoor air."@en ;
        rdfs:label    "VentilationOutdoorAir"@en .

PSD:StemBaseWidth  a  rdf:Property ;
        rdfs:comment  "Stem base width of the profile."@en ;
        rdfs:label    "StemBaseWidth"@en .

PSD:IsExternal  a     rdf:Property ;
        rdfs:comment  "Indication of whether the junction box type is allowed for exposure to outdoor elements (set TRUE where external exposure is allowed)."@en ;
        rdfs:label    "Is external"@en , "IsExternal"@en .

PSD:ShortCircuit1PoleMinimumState
        a             rdf:Property ;
        rdfs:comment  "Minimum 1 pole short circuit current provided at the point of supply i.e. the fault between 1 phase and N."@en ;
        rdfs:label    "ShortCircuit1PoleMinimumState"@en .

PSD:VerticalSpacing  a  rdf:Property ;
        rdfs:comment  "Vertical spacing between tubes in the tube bundle."@en ;
        rdfs:label    "VerticalSpacing"@en .

PSD:WorkWeekDuration  a  rdf:Property ;
        rdfs:comment  "The elapsed time within a worktime-based week. For presentation purposes, applications may choose to display IfcTask durations in work weeks where IfcTaskTime.DurationType=WORKTIME. This value must be less than or equal to 168 hours (an elapsed week); if omitted then 40 hours is assumed."@en ;
        rdfs:label    "Work week duration"@en .

PSD:WheelTipSpeed  a  rdf:Property ;
        rdfs:comment  "Fan blade tip speed, typically defined as the linear speed of the tip of the fan blade furthest from the shaft."@en ;
        rdfs:label    "WheelTipSpeed"@en .

PSD:NominalMediaSurfaceVelocity
        a             rdf:Property ;
        rdfs:comment  "Average fluid velocity at the media surface."@en ;
        rdfs:label    "Nominal media surface velocity"@en .

PSD:Reference  a      rdf:Property ;
        rdfs:comment  "Reference ID for this specified type in this project (e.g. type 'A-1')."@en , "Reference ID for this specific instance of a distribution system, or sub-system (e.g. 'WWS/VS1', which indicates the system to be WWS, subsystems VSI/400). The reference values depend on the local code of practice."@en , "Reference ID for this specific instance (e.g.  'WWS/VS1/400/001', which indicates the occurrence belongs to system WWS, subsystems VSI/400, and has the component number 001)."@en , "Reference ID for this specified type in this project (e.g. type 'A-1'), provided, if there is no classification reference to a recognized classification system used."@en , "A descriptive label for the general reinforcement type."@en ;
        rdfs:label    "Reference"@en .

PSD:LowerTime2  a     rdf:Property ;
        rdfs:comment  "The time in [s], indicating the tripping times of the upper time/current curve at the LowerCurrent2."@en ;
        rdfs:label    "LowerTime2"@en .

PSD:IsLandmarked  a  rdf:Property ;
        rdfs:label  "Is landmarked"@en .

PSD:FanRotationSpeed  a  rdf:Property ;
        rdfs:comment  "Fan rotation speed."@en ;
        rdfs:label    "FanRotationSpeed"@en .

PSD:DryBulbTemperature
        a             rdf:Property ;
        rdfs:comment  "Loads from the dry bulb temperature."@en ;
        rdfs:label    "DryBulbTemperature"@en .

PSD:SensibleHeatTransferRate
        a             rdf:Property ;
        rdfs:comment  "Sensible heat transfer rate."@en , "Sensible heat transfer rate to primary air flow."@en ;
        rdfs:label    "SensibleHeatTransferRate"@en .

PSD:PlacingType  a    rdf:Property ;
        rdfs:comment  "Location at which the type of junction box can be located."@en ;
        rdfs:label    "PlacingType"@en .

PSD:YDirectionLowerBarCount
        a             rdf:Property ;
        rdfs:comment  "The number of bars with Y direction lower bar."@en ;
        rdfs:label    "YDirectionLowerBarCount"@en .

PSD:NominalReturnWaterTemperatureHeating
        a             rdf:Property ;
        rdfs:comment  "Nominal return water temperature (refers to nominal heating capacity)."@en ;
        rdfs:label    "NominalReturnWaterTemperatureHeating"@en .

PSD:Shape  a          rdf:Property ;
        rdfs:comment  "Cross sectional shape. Note that this shape is uniform throughout the length of the segment. For nonuniform shapes, a transition fitting should be used instead."@en , "Indication of the shape of the conductor."@en , "Shape of the air terminal. Slot is typically a long narrow supply device with an aspect ratio generally greater than 10 to 1."@en , "The shape form of the provision for void, the minimum set of agreed values includes 'Rectangle', 'Round', and 'Undefined'."@en ;
        rdfs:label    "Shape"@en .

PSD:VolumetricFlowRate
        a             rdf:Property ;
        rdfs:comment  "The volumetric flow rate of the fluid."@en ;
        rdfs:label    "VolumetricFlowRate"@en .

PSD:Response  a       rdf:Property ;
        rdfs:comment  "Identifies the predefined methods of sprinkler response from which that required may be set."@en ;
        rdfs:label    "Response"@en .

PSD:VideoResolutionMode
        a             rdf:Property ;
        rdfs:comment  "Indicates video resolution modes."@en ;
        rdfs:label    "VideoResolutionMode"@en .

PSD:name  a         owl:DatatypeProperty ;
        rdfs:label  "Name"@en ;
        rdfs:range  xsd:string .

PSD:TypePropertyBoundedValue
        a                 owl:Class ;
        rdfs:label        "Type property bounded value"@en ;
        rdfs:subClassOf   PSD:PropertyType ;
        rdfs:subClassOf   [ a                owl:Restriction ;
                            owl:cardinality  "1"^^xsd:nonNegativeInteger ;
                            owl:onProperty   PSD:dataType
                          ] ;
        rdfs:subClassOf   [ a                   owl:Restriction ;
                            owl:maxCardinality  "1"^^xsd:nonNegativeInteger ;
                            owl:onProperty      PSD:unitType
                          ] ;
        owl:disjointWith  PSD:TypeComplexProperty , PSD:TypePropertySingleValue , PSD:TypePropertyReferenceValue , PSD:TypePropertyEnumeratedValue , PSD:TypePropertyTableValue , PSD:TypePropertyListValue .

PSD:SetPointPressure  a  rdf:Property ;
        rdfs:comment  "The pressure value to be sensed. Use IfcPropertyBoundedValue.SetPointValue to set the set point value."@en ;
        rdfs:label    "SetPointPressure"@en .

PSD:Throw  a          rdf:Property ;
        rdfs:comment  "Distance cooled beam throws the air."@en ;
        rdfs:label    "Throw"@en .

PSD:MechanicalLoadRating
        a           rdf:Property ;
        rdfs:label  "Mechanical load rating"@en .

PSD:HasHoseUnion  a   rdf:Property ;
        rdfs:comment  "Indicates whether the gas tap is fitted with a hose union connection (= TRUE) or not (= FALSE)."@en , "Indicates whether the drawoff cock is fitted with a hose union connection (= TRUE) or not (= FALSE)."@en ;
        rdfs:label    "HasHoseUnion"@en .

PSD:FractionConvectiveHeatTransfer
        a             rdf:Property ;
        rdfs:comment  "Fraction of the total heat transfer rate as the convective heat transfer."@en ;
        rdfs:label    "FractionConvectiveHeatTransfer"@en .

PSD:FanPower  a       rdf:Property ;
        rdfs:comment  "Fan motor loads contributing to the cooling load."@en ;
        rdfs:label    "Fan power"@en .

PSD:Water  a          rdf:Property ;
        rdfs:comment  "The amount of water consumed during the period specified in the time series."@en ;
        rdfs:label    "Water"@en .

PSD:ManufacturingToleranceClass
        a           rdf:Property ;
        rdfs:label  "Manufacturing tolerance class"@en .

PSD:DiagonalTrussBaseBarDiameter
        a             rdf:Property ;
        rdfs:comment  "The nominal diameter of the base bar."@en ;
        rdfs:label    "DiagonalTrussBaseBarDiameter"@en .

PSD:TendonRelaxation  a  rdf:Property ;
        rdfs:label  "Tendon relaxation"@en .

PSD:VaporPermeability
        a             rdf:Property ;
        rdfs:comment  "The rate of water vapor transmission per unit area per unit of vapor pressure differential under test conditions."@en ;
        rdfs:label    "VaporPermeability"@en .

PSD:MovementSensingType
        a             rdf:Property ;
        rdfs:comment  "Enumeration that identifies the type of movement sensing mechanism."@en ;
        rdfs:label    "MovementSensingType"@en .

PSD:Impedence  a      rdf:Property ;
        rdfs:comment  "Indicates the speaker impedence."@en ;
        rdfs:label    "Impedence"@en .

PSD:EarthFault1PoleMaximumState
        a             rdf:Property ;
        rdfs:comment  "Maximum 1 pole earth fault current provided at the point of supply i.e. the fault between 1 phase and PE/PEN."@en ;
        rdfs:label    "EarthFault1PoleMaximumState"@en .

PSD:FlushingRate  a   rdf:Property ;
        rdfs:comment  "The predetermined quantity of water to be flushed."@en ;
        rdfs:label    "FlushingRate"@en .

PSD:LongitudinalSeam  a  rdf:Property ;
        rdfs:comment  "The type of seam to be used along the longitudinal axis of the duct segment."@en ;
        rdfs:label    "LongitudinalSeam"@en .

PSD:IsRigid  a        rdf:Property ;
        rdfs:comment  "Indication of whether the conduit is rigid (= TRUE) or flexible (= FALSE)."@en ;
        rdfs:label    "IsRigid"@en .

PSD:WireLoopBasePlateLength
        a             rdf:Property ;
        rdfs:comment  "The length of the base plate."@en ;
        rdfs:label    "WireLoopBasePlateLength"@en .

PSD:PowerSource  a    rdf:Property ;
        rdfs:comment  "Type of power driving the compressor."@en ;
        rdfs:label    "Power source"@en .

PSD:SpecialInstructions
        a             rdf:Property ;
        rdfs:comment  "Special instructions that affect the move."@en ;
        rdfs:label    "SpecialInstructions"@en .

PSD:ResourceDepletionPerUnit
        a           rdf:Property ;
        rdfs:label  "Resource depletion per unit"@en .

PSD:SupplyWaterTemperatureHeating
        a             rdf:Property ;
        rdfs:comment  "Supply water temperature in heating mode."@en ;
        rdfs:label    "SupplyWaterTemperatureHeating"@en .

PSD:CloseOffRating  a  rdf:Property ;
        rdfs:comment  "Close off rating."@en ;
        rdfs:label    "CloseOffRating"@en .

PSD:BendRadius  a     rdf:Property ;
        rdfs:comment  "The radius of bending if circular arc or zero if sharp bend."@en ;
        rdfs:label    "BendRadius"@en .

PSD:ParkingUse  a     rdf:Property ;
        rdfs:comment  "Identifies the type of transporation for which the parking space is designed. Values are not predefined but might include car, compact car, motorcycle, bicycle, truck, bus etc."@en ;
        rdfs:label    "ParkingUse"@en .

PSD:WorksurfaceArea  a  rdf:Property ;
        rdfs:comment  "The value of the work surface area of the desk."@en , "The value of the work surface area of the desk.."@en ;
        rdfs:label    "WorksurfaceArea"@en .

PSD:NominalSurroundingTemperatureHeating
        a             rdf:Property ;
        rdfs:comment  "Nominal surrounding temperature (refers to nominal heating capacity)."@en ;
        rdfs:label    "NominalSurroundingTemperatureHeating"@en .

PSD:Value  a             owl:Class , rdf:Property ;
        rdfs:comment     "Indicates values over time which may be recorded continuously or only when changed beyond a particular deadband.  The range of possible values is defined by the Value property on the corresponding occurrence property set (Pset_ControllerTypeFloating, Pset_ControllerTypeProportional, Pset_ControllerTypeMultiPosition, or Pset_ControllerTypeTwoPosition)."@en , "Indicates measured values over time which may be recorded continuously or only when changed beyond a particular deadband."@en , "Indicates sensed values over time which may be recorded continuously or only when changed beyond a particular deadband.  The range of possible values is defined by the SetPoint property of the corresponding sensor type property set."@en ;
        rdfs:label       "Value"@en , "Defining value"@en ;
        rdfs:subClassOf  owl:Thing ;
        rdfs:subClassOf  [ a                   owl:Restriction ;
                           owl:maxCardinality  "1"^^xsd:nonNegativeInteger ;
                           owl:onProperty      PSD:unitType
                         ] ;
        rdfs:subClassOf  [ a                   owl:Restriction ;
                           owl:minCardinality  "0"^^xsd:nonNegativeInteger ;
                           owl:onProperty      PSD:valueItem
                         ] ;
        rdfs:subClassOf  [ a                owl:Restriction ;
                           owl:cardinality  "1"^^xsd:nonNegativeInteger ;
                           owl:onProperty   PSD:dataType
                         ] .

PSD:DisplayWidth  a   rdf:Property ;
        rdfs:comment  "Indicates the physical width of the screen (only the display surface)."@en ;
        rdfs:label    "DisplayWidth"@en .

PSD:LoadBearing  a  rdf:Property ;
        rdfs:label  "Load bearing"@en .

PSD:FirstCurvatureRadius
        a             rdf:Property ;
        rdfs:comment  "FirstCurvatureRadius should be defined as the base or left side radius of curvature value."@en ;
        rdfs:label    "FirstCurvatureRadius"@en .

PSD:MaximumSpaceSensibleLoad
        a             rdf:Property ;
        rdfs:comment  "Maximum or Peak sensible thermal load contributed to the conditioned space by the light fixture."@en ;
        rdfs:label    "MaximumSpaceSensibleLoad"@en .

PSD:MountingType  a   rdf:Property ;
        rdfs:comment  "The way the air terminal is mounted to the ceiling, wall, etc.\\n\\nSurface: mounted to the surface of something (e.g., wall, duct, etc.).\\nFlat flush: mounted flat and flush with a surface.\\nLay-in: mounted in a lay-in type ceiling (e.g., a dropped ceiling grid)."@en , "Method of mounting to be adopted for the type of junction box."@en ;
        rdfs:label    "Mounting type"@en , "MountingType"@en .

PSD:FrictionHeatGain  a  rdf:Property ;
        rdfs:comment  "Friction heat gain."@en ;
        rdfs:label    "FrictionHeatGain"@en .

PSD:RatedTemperature  a  rdf:Property ;
        rdfs:comment  "The range of allowed temerature that a device is certified to handle. The upper bound of this value is the maximum."@en ;
        rdfs:label    "RatedTemperature"@en .

PSD:YDirectionTieHoopBarPitch
        a             rdf:Property ;
        rdfs:comment  "The Y direction pitch length of the tie hoop."@en ;
        rdfs:label    "YDirectionTieHoopBarPitch"@en .

PSD:ConnectedConductorFunction
        a             rdf:Property ;
        rdfs:comment  "Function of the conductors to which the load is connected."@en ;
        rdfs:label    "ConnectedConductorFunction"@en .

PSD:YDirectionTieHoopCount
        a             rdf:Property ;
        rdfs:comment  "The number of bars with Y direction tie hoop bars."@en ;
        rdfs:label    "YDirectionTieHoopCount"@en .

PSD:InPlaneNegative  a  rdf:Property ;
        rdfs:comment  "Mechanical properties with respect to in-plane load, i.e. bending about the strong axis; compression zone of unbalanced layups is stressed in tension."@en ;
        rdfs:label    "InPlaneNegative"@en .

PSD:NonHazardousWaste
        a           rdf:Property ;
        rdfs:label  "Non hazardous waste"@en .

PSD:ControlType  a    rdf:Property ;
        rdfs:comment  "The type of control used to operate the damper (e.g., Open/Closed Indicator, Resetable Temperature Sensor, Temperature Override, etc.)."@en , "The type of control used to operate the damper (e.g., Open/Closed Indicator, Resetable Temperature Sensor, Temperature Override, etc.) ."@en ;
        rdfs:label    "ControlType"@en .

PSD:InfiltrationDiversitySummer
        a             rdf:Property ;
        rdfs:comment  "Diversity factor for Summer infiltration."@en ;
        rdfs:label    "InfiltrationDiversitySummer"@en , "Infiltration diversity summer"@en .

PSD:NominalBodyDepth  a  rdf:Property ;
        rdfs:comment  "Nominal or quoted length measured along the z-axis in the local coordinate system of the drain."@en , "Nominal or quoted =length, measured along the z-axis of the local coordinate system of the object, of the body of the object."@en , "Nominal or quoted length measured along the z-axis in the local coordinate system of the waste."@en ;
        rdfs:label    "NominalBodyDepth"@en .

PSD:OperationalCriteria
        a             rdf:Property ;
        rdfs:comment  "Time of operation at maximum operational ambient air temperature."@en ;
        rdfs:label    "Operational criteria"@en .

PSD:SetPointIdentifier
        a             rdf:Property ;
        rdfs:comment  "The detected tag value."@en ;
        rdfs:label    "SetPointIdentifier"@en .

PSD:AdjustmentValueType
        a             rdf:Property ;
        rdfs:comment  "The type of adjustment value that is applied through the property set. This determines the properties that should be asserted (see below)."@en ;
        rdfs:label    "AdjustmentValueType"@en .

PSD:SpacingBarPitch  a  rdf:Property ;
        rdfs:comment  "The pitch length of the spacing bar."@en ;
        rdfs:label    "SpacingBarPitch"@en .

PSD:SerialNumber  a   rdf:Property ;
        rdfs:comment  "The serial number assigned to an occurrence of a product."@en , "The manufacturer's serial number for the precast concrete element."@en ;
        rdfs:label    "SerialNumber"@en .

PSD:NominalFrequency  a  rdf:Property ;
        rdfs:comment  "The nominal frequency of the supply."@en ;
        rdfs:label    "NominalFrequency"@en .

PSD:AtmosphericAcidificationPerUnit
        a           rdf:Property ;
        rdfs:label  "Atmospheric acidification per unit"@en .

PSD:FrameThickness  a  rdf:Property ;
        rdfs:comment  "The thickness of the damper frame material."@en ;
        rdfs:label    "FrameThickness"@en .

PSD:InvertLevel  a    rdf:Property ;
        rdfs:comment  "The lowest point in the cross section of the sump."@en , "Level of the lowest part of the cross section as measured from ground level."@en ;
        rdfs:label    "InvertLevel"@en .

PSD:HasSillInternal  a  rdf:Property ;
        rdfs:label  "Has sill internal"@en .

PSD:applicableTypeValue
        a             owl:DatatypeProperty ;
        rdfs:comment  "The format of applicable type value is ENTITY_TYPE/PREDEFINED_TYPE. Multiple value is accepted, and format is: \"TYPE_1 | TYPE_2 ...\"."@en ;
        rdfs:domain   PSD:PropertySetDef ;
        rdfs:label    "Applicable type value"@en ;
        rdfs:range    xsd:string .

PSD:WorkStartTime  a  rdf:Property ;
        rdfs:comment  "The default time of day a task is scheduled to start. For presentation purposes, if the start time of a task matches the WorkStartTime, then applications may choose to display the date only. Conversely when entering dates without specifying time, applications may automatically append the WorkStartTime."@en ;
        rdfs:label    "Work start time"@en .

PSD:ReleaseStrength  a  rdf:Property ;
        rdfs:label  "Release strength"@en .

PSD:WaterConsumptionPerUnit
        a           rdf:Property ;
        rdfs:label  "Water consumption per unit"@en .

PSD:COContent  a      rdf:Property ;
        rdfs:comment  "Carbon monoxide (CO) content of the products of combustion. This is measured in weight of CO per unit weight and is therefore unitless."@en ;
        rdfs:label    "COContent"@en .

PSD:s   a             rdf:Property ;
        rdfs:comment  "Measure s according to ISO 2553"@en ;
        rdfs:label    "s"@en .

PSD:Lighting  a       rdf:Property ;
        rdfs:comment  "Lighting loads."@en ;
        rdfs:label    "Lighting"@en .

PSD:SetPointMovement  a  rdf:Property ;
        rdfs:comment  "The movement to be sensed."@en ;
        rdfs:label    "SetPointMovement"@en .

PSD:ActualCompletion  a  rdf:Property ;
        rdfs:comment  "The actual completion percentage of the allocation."@en ;
        rdfs:label    "ActualCompletion"@en .

PSD:ifdguid  a        owl:FunctionalProperty , owl:DatatypeProperty ;
        rdfs:comment  "GUID of IFD."@en ;
        rdfs:domain   PSD:PropertyDef ;
        rdfs:label    "IFD GUID"@en ;
        rdfs:range    xsd:string .

PSD:FlangeDepth  a    rdf:Property ;
        rdfs:comment  "Flange depth of the profile."@en ;
        rdfs:label    "FlangeDepth"@en .

PSD:ActuationType  a  rdf:Property ;
        rdfs:comment  "Enumeration that identifies the different types of dampers."@en ;
        rdfs:label    "ActuationType"@en .

PSD:IsFOB  a          rdf:Property ;
        rdfs:comment  "Indication of whether contents of the purchase order are delivered 'Free on Board' (= True) or not (= False). FOB is a shipping term which indicates that the supplier pays the shipping costs (and usually also the insurance costs) from the point of manufacture to a specified destination, at which point the buyer takes responsibility."@en ;
        rdfs:label    "IsFOB"@en .

PSD:MeasuredFlowRate  a  rdf:Property ;
        rdfs:comment  "The rate of flow of a fluid measured across the valve."@en ;
        rdfs:label    "MeasuredFlowRate"@en .

PSD:LadderTrussCrossBarDiameter
        a             rdf:Property ;
        rdfs:comment  "The nominal diameter of the straight cross-bars."@en ;
        rdfs:label    "LadderTrussCrossBarDiameter"@en .

PSD:NominalHeatTransferCoefficient
        a             rdf:Property ;
        rdfs:comment  "Nominal overall heat transfer coefficient associated with nominal heat transfer area."@en ;
        rdfs:label    "Nominal heat transfer coefficient"@en .

PSD:Steam  a          rdf:Property ;
        rdfs:comment  "The amount of steam consumed during the period specified in the time series."@en ;
        rdfs:label    "Steam"@en .

PSD:TotalLatentLoad  a  rdf:Property ;
        rdfs:comment  "Total energy added or removed from air that affects its humidity or concentration of water vapor.  If a value is less than zero (negative), then the thermal load is lost from the space. If a value is greater than zero (positive), then the thermal load is a gain to the space."@en ;
        rdfs:label    "TotalLatentLoad"@en .

PSD:definingValue  a  owl:ObjectProperty ;
        rdfs:domain  PSD:TypePropertyTableValue ;
        rdfs:label   "Defining value"@en ;
        rdfs:range   PSD:Value .

PSD:HangingHeight  a  rdf:Property ;
        rdfs:comment  "The hanging height of the worksurface."@en ;
        rdfs:label    "HangingHeight"@en .

PSD:TreadLengthAtInnerSide
        a           rdf:Property ;
        rdfs:label  "Tread length at inner side"@en .

PSD:CarbonContent  a  rdf:Property ;
        rdfs:comment  "The carbon content in the fuel. This is measured in weight of carbon per unit weight of fuel and is therefore unitless."@en ;
        rdfs:label    "CarbonContent"@en .

PSD:NominalLength  a  rdf:Property ;
        rdfs:comment  "Nominal or quoted length of the object. The size information is provided in addition to the shape representation and the geometric parameters used within. In cases of inconsistency between the geometric parameters and the size properties, provided in the attached property set, the geometric parameters take precedence."@en ;
        rdfs:label    "Nominal length"@en .

PSD:RenewableEnergyConsumptionPerUnit
        a           rdf:Property ;
        rdfs:label  "Renewable energy consumption per unit"@en .

PSD:WorkDayDuration  a  rdf:Property ;
        rdfs:comment  "The elapsed time within a worktime-based day. For presentation purposes, applications may choose to display IfcTask durations in work days where IfcTaskTime.DurationType=WORKTIME. This value must be less than or equal to 24 hours (an elapsed day); if omitted then 8 hours is assumed."@en ;
        rdfs:label    "Work day duration"@en .

PSD:FireRating  a   rdf:Property ;
        rdfs:label  "Fire rating"@en .

PSD:ShadingCoefficient
        a           rdf:Property ;
        rdfs:label  "Shading coefficient"@en .

PSD:MountingMethod  a  rdf:Property ;
        rdfs:comment  "The method of mounting cable segment occurrences on a cable carrier occurrence from which the method required can be selected. This is for the purpose of carrying out 'worst case' cable sizing calculations and may be a conceptual requirement rather than a statement of the physical occurrences of cable and carrier segments."@en ;
        rdfs:label    "MountingMethod"@en .

PSD:Flowrate  a       rdf:Property ;
        rdfs:comment  "The flowrate of the fuel."@en , "The actual operational fluid flowrate."@en ;
        rdfs:label    "Flowrate"@en .

PSD:CorrectionFactorForHeating
        a             rdf:Property ;
        rdfs:comment  "Correction factor k as a function of water flow rate (used to calculate heating capacity)."@en ;
        rdfs:label    "CorrectionFactorForHeating"@en .

PSD:AccuracyQualityObtained
        a             rdf:Property ;
        rdfs:comment  "A measure of the accuracy quality of survey points as obtained expressed in percentage terms."@en ;
        rdfs:label    "AccuracyQualityObtained"@en .

PSD:XDirectionTieHoopBarPitch
        a             rdf:Property ;
        rdfs:comment  "The X direction pitch length of the tie hoop."@en ;
        rdfs:label    "XDirectionTieHoopBarPitch"@en .

PSD:I2  a             rdf:Property ;
        rdfs:comment  "The (thermal) upper testing current limit in [x In], indicating that for currents larger than I2, the tripping time shall be shorter than the associated tripping time, T2."@en ;
        rdfs:label    "I2"@en .

PSD:ElectricActuatorType
        a             rdf:Property ;
        rdfs:comment  "Enumeration that identifies electric actuator as defined by its operational principle."@en ;
        rdfs:label    "Electric actuator type"@en .

PSD:IndoorEnvironment
        a             rdf:Property ;
        rdfs:comment  "Adjustment of the service life resulting from the effect of the indoor environment (where appropriate)."@en ;
        rdfs:label    "IndoorEnvironment"@en .

PSD:HoopBarPitch  a   rdf:Property ;
        rdfs:comment  "The pitch length of the hoop bar."@en ;
        rdfs:label    "HoopBarPitch"@en .

PSD:CouplingType  a   rdf:Property ;
        rdfs:comment  "Defines the type coupling on the inlet of the breeching inlet."@en ;
        rdfs:label    "CouplingType"@en .

PSD:AudioMode  a      rdf:Property ;
        rdfs:comment  "Indicates audio sound modes and corresponding labels, if applicable."@en ;
        rdfs:label    "AudioMode"@en .

PSD:LightFixturePlacingType
        a             rdf:Property ;
        rdfs:comment  "A list of the available types of placing specification for light fixtures from which that required may be selected."@en ;
        rdfs:label    "LightFixturePlacingType"@en .

PSD:WarrantyPeriod  a  rdf:Property ;
        rdfs:comment  "The time duration during which a manufacturer or supplier guarantees or warrants the performance of an artefact."@en ;
        rdfs:label    "WarrantyPeriod"@en .

PSD:SupplyAirTemperatureHeating
        a             rdf:Property ;
        rdfs:comment  "Supply air temperature in heating mode."@en ;
        rdfs:label    "SupplyAirTemperatureHeating"@en .

PSD:InertWaste  a   rdf:Property ;
        rdfs:label  "Inert waste"@en .

PSD:NarrativeText  a  rdf:Property ;
        rdfs:comment  "Added information relating to the adjacent building use that is not appropriate to the general descriptive text associated with an entity through the inherited IfcRoot.Description."@en ;
        rdfs:label    "Narrative text"@en , "NarrativeText"@en .

PSD:ClimateChange  a  rdf:Property ;
        rdfs:label  "Climate change"@en .

PSD:TenureModesAvailableNow
        a             rdf:Property ;
        rdfs:comment  "A list of the tenure modes that are currently available expressed in terms of IfcLabel."@en ;
        rdfs:label    "Tenure modes available now"@en .

PSD:FireExit  a     rdf:Property ;
        rdfs:label  "Fire exit"@en .

PSD:AngleToFirstAxis  a  rdf:Property ;
        rdfs:label  "Angle to first axis"@en .

PSD:ConcreteCoverAtLinks
        a           rdf:Property ;
        rdfs:label  "Concrete cover at links"@en .

PSD:TimeTolerance2  a  rdf:Property ;
        rdfs:comment  "The tolerance for the time of the time/current-curve in [%] valid for currents above TimeToleranceLimit1."@en ;
        rdfs:label    "TimeTolerance2"@en .

PSD:NominalSupplyVoltageOffset
        a             rdf:Property ;
        rdfs:comment  "The maximum and minimum allowed voltage of the supply e.g. boundaries of 380V/440V may be applied for a nominal voltage of 400V."@en ;
        rdfs:label    "NominalSupplyVoltageOffset"@en .

PSD:ApparentPower  a  rdf:Property ;
        rdfs:comment  "Apparent power."@en ;
        rdfs:label    "ApparentPower"@en .

PSD:n   a             rdf:Property ;
        rdfs:comment  "Count n according to ISO 2553"@en ;
        rdfs:label    "n"@en .

PSD:HeatTransferCoefficient
        a             rdf:Property ;
        rdfs:comment  "Heat transfer coefficient-area product."@en ;
        rdfs:label    "HeatTransferCoefficient"@en .

PSD:SensibleCoolingCapacity
        a             rdf:Property ;
        rdfs:comment  "Sensible cooling capacity."@en ;
        rdfs:label    "SensibleCoolingCapacity"@en .

PSD:ExpectedServiceLife
        a           rdf:Property ;
        rdfs:label  "Expected service life"@en .

PSD:OutOfPlaneNegative
        a             rdf:Property ;
        rdfs:comment  "Mechanical properties with respect to out-of-plane load i.e. for function as a plate; compression zone of unbalanced layups is stressed in tension."@en ;
        rdfs:label    "OutOfPlaneNegative"@en .

PSD:PressureCurve  a  rdf:Property ;
        rdfs:comment  "Pressure rise = f (flow rate)."@en ;
        rdfs:label    "Pressure curve"@en .

PSD:LowerCurrent1  a  rdf:Property ;
        rdfs:comment  "The current in [x In], indicating that for currents smaller than LowerCurrent1 the I2t part of the L-function will not trip the current,"@en ;
        rdfs:label    "LowerCurrent1"@en .

PSD:CornerChamfer  a  rdf:Property ;
        rdfs:label  "Corner chamfer"@en .

PSD:TorqueRange  a    rdf:Property ;
        rdfs:comment  "Torque range: minimum operational torque to maximum allowable torque."@en ;
        rdfs:label    "TorqueRange"@en .

PSD:expression  a     owl:FunctionalProperty , owl:DatatypeProperty ;
        rdfs:comment  "Information about the expression for the derivation of defined values from the defining values."@en ;
        rdfs:domain   PSD:TypePropertyTableValue ;
        rdfs:label    "Expression"@en ;
        rdfs:range    xsd:string .

PSD:Eutrophication  a  rdf:Property ;
        rdfs:label  "Eutrophication"@en .

PSD:NumberOfCores  a  rdf:Property ;
        rdfs:comment  "The number of cores in Cable/Bus."@en , "Number of cores."@en ;
        rdfs:label    "NumberOfCores"@en .

PSD:CenterCoreTopWidth
        a             rdf:Property ;
        rdfs:comment  "Center core top width of the profile."@en ;
        rdfs:label    "CenterCoreTopWidth"@en .

PSD:EvaporatingTemperature
        a             rdf:Property ;
        rdfs:comment  "Refrigerant evaporating temperature."@en ;
        rdfs:label    "EvaporatingTemperature"@en .

PSD:RequiredPset  a      owl:Class ;
        rdfs:label       "Required property set" ;
        rdfs:subClassOf  owl:Thing ;
        rdfs:subClassOf  [ a                owl:Restriction ;
                           owl:cardinality  "1"^^xsd:nonNegativeInteger ;
                           owl:onProperty   PSD:propertySetDef
                         ] .

PSD:CapacityControlType
        a             rdf:Property ;
        rdfs:comment  "InletVane: Control by adjusting inlet vane.\\nVariableSpeedDrive: Control by variable speed drive. \\nBladePitchAngle: Control by adjusting blade pitch angle.\\nTwoSpeed: Control by switch between high and low speed.\\nDischargeDamper: Control by modulating discharge damper."@en ;
        rdfs:label    "Capacity control type"@en .

PSD:ArticleNumber  a  rdf:Property ;
        rdfs:comment  "Article number or reference that is be applied to a configured product according to a standard scheme for article number definition as defined by the manufacturer. It is often used as the purchasing number."@en ;
        rdfs:label    "ArticleNumber"@en .

PSD:PatternType  a    rdf:Property ;
        rdfs:comment  "Defines the types of pattern (or shape of a tank that may be specified."@en ;
        rdfs:label    "PatternType"@en .

PSD:SetPointFlow  a   rdf:Property ;
        rdfs:comment  "The volumetric flow value to be sensed. Use IfcPropertyBoundedValue.SetPointValue to set the set point value."@en ;
        rdfs:label    "SetPointFlow"@en .

PSD:FlowrateLeakage  a  rdf:Property ;
        rdfs:comment  "Leakage flowrate versus pressure difference."@en ;
        rdfs:label    "FlowrateLeakage"@en .

PSD:SetPointIlluminance
        a             rdf:Property ;
        rdfs:comment  "The illuminance value to be sensed. Use IfcPropertyBoundedValue.SetPointValue to set the set point value."@en ;
        rdfs:label    "SetPointIlluminance"@en .

PSD:NominalEnergyConsumption
        a             rdf:Property ;
        rdfs:comment  "Nominal fuel consumption rate required to produce the total boiler heat output."@en ;
        rdfs:label    "Nominal energy consumption"@en .

PSD:LightingPercentLoadToReturnAir
        a             rdf:Property ;
        rdfs:comment  "Percent of lighting load to the return air plenum."@en ;
        rdfs:label    "LightingPercentLoadToReturnAir"@en .

PSD:HandicapAccessible
        a             rdf:Property ;
        rdfs:comment  "Indication that this object is designed to be accessible by the handicapped. \\nSet to (TRUE) if this ramp is rated as handicap accessible  according the local building codes, otherwise (FALSE)."@en ;
        rdfs:label    "Handicap accessible"@en .

PSD:EnergySource  a   rdf:Property ;
        rdfs:comment  "Enumeration defining the energy source or fuel cumbusted to generate heat."@en ;
        rdfs:label    "Energy source"@en .

PSD:ConduitShapeType  a  rdf:Property ;
        rdfs:comment  "The shape of the conduit segment."@en ;
        rdfs:label    "ConduitShapeType"@en .

PSD:RentalRatesInCategoryFuture
        a             rdf:Property ;
        rdfs:comment  "Range of the cost rates for property expected to be available in the future in the required category."@en ;
        rdfs:label    "Rental rates in category future"@en .

PSD:EarthFault1PolePowerFactorMaximumState
        a             rdf:Property ;
        rdfs:comment  "Power factor of the maximum 1 pole earth fault  current provided at the point of supply i.e. the fault between 1 phase and PE/PEN."@en ;
        rdfs:label    "EarthFault1PolePowerFactorMaximumState"@en .

PSD:BackflowPreventerType
        a             rdf:Property ;
        rdfs:comment  "Identifies the type of backflow preventer installed to prevent the backflow of contaminated or polluted water from an irrigation/reticulation system to a potable water supply."@en ;
        rdfs:label    "BackflowPreventerType"@en .

PSD:OutletDiameter  a  rdf:Property ;
        rdfs:comment  "The outlet diameter of the breeching inlet."@en ;
        rdfs:label    "OutletDiameter"@en .

PSD:InputPressure  a  rdf:Property ;
        rdfs:comment  "Maximum design pressure for the actuator."@en ;
        rdfs:label    "Input pressure"@en .

PSD:AirFlowRate  a    rdf:Property ;
        rdfs:comment  "Air flow rate."@en , "The actual airflow rate as designed."@en , "Volumetric flow rate."@en , "Volumetric air flow rate."@en ;
        rdfs:label    "AirFlowRate"@en .

PSD:BuildingThermalExposure
        a             rdf:Property ;
        rdfs:comment  "The thermal exposure expected by the building based on surrounding site conditions."@en ;
        rdfs:label    "BuildingThermalExposure"@en .

PSD:VentilationAirFlowRate
        a             rdf:Property ;
        rdfs:comment  "Ventilation air flow rate in the space."@en ;
        rdfs:label    "VentilationAirFlowRate"@en .

PSD:StructuralClass  a  rdf:Property ;
        rdfs:label  "Structural class"@en .

PSD:ReinforcementStrengthClass
        a           rdf:Property ;
        rdfs:label  "Reinforcement strength class"@en .

PSD:ClosureRatingEnum
        a             rdf:Property ;
        rdfs:comment  "Enumeration that identifies the closure rating for the damper."@en ;
        rdfs:label    "ClosureRatingEnum"@en .

PSD:ReceiverType  a   rdf:Property ;
        rdfs:comment  "Indicates the type of receiver."@en ;
        rdfs:label    "ReceiverType"@en .

PSD:Capacity  a       rdf:Property ;
        rdfs:comment  "Cooling tower capacity in terms of heat transfer rate of the cooling tower between air stream and water stream."@en ;
        rdfs:label    "Capacity"@en .

PSD:RequestSourceName
        a             rdf:Property ;
        rdfs:comment  "The person making the request, where known."@en ;
        rdfs:label    "Request source name"@en .

PSD:AppliancePercentLoadToRadiant
        a             rdf:Property ;
        rdfs:comment  "Percent of sensible load to radiant heat."@en ;
        rdfs:label    "AppliancePercentLoadToRadiant"@en .

PSD:WorkExecutionLevel
        a             rdf:Property ;
        rdfs:comment  "Adjustment of the service life resulting from the effect of the quality of work executed."@en ;
        rdfs:label    "WorkExecutionLevel"@en .

PSD:CounterSlope  a   rdf:Property ;
        rdfs:comment  "Sloping angle of the object, measured perpendicular to the slope  - relative to horizontal (0.0 degrees). \\nActual maximum slope for the passageway measured perpendicular to the direction of travel according to the current design. The shape information is provided in addition to the shape representation and the geometric parameters used within. In cases of inconsistency between the geometric parameters and the shape properties, provided in the attached property, the geometric parameters take precedence. \\nNote: new property in IFC4."@en ;
        rdfs:label    "Counter slope"@en .

PSD:SecurityLightingType
        a             rdf:Property ;
        rdfs:comment  "The type of security lighting."@en ;
        rdfs:label    "SecurityLightingType"@en .

PSD:CoefficientOfPerformance
        a             rdf:Property ;
        rdfs:comment  "Coefficient of performance (COP)."@en ;
        rdfs:label    "CoefficientOfPerformance"@en .

PSD:WeightedEfficiency
        a             rdf:Property ;
        rdfs:comment  "Filter efficiency based the particle weight concentration before and after filter against particles with certain size distribution."@en ;
        rdfs:label    "WeightedEfficiency"@en .

PSD:OverallDiameter  a  rdf:Property ;
        rdfs:comment  "The overall diameter of a Cable/Bus."@en , "The overall diameter of a core (maximun space used)."@en ;
        rdfs:label    "OverallDiameter"@en .

PSD:CombustionTemperature
        a             rdf:Property ;
        rdfs:comment  "Combustion temperature of the material when air is at 298 K and 100 kPa."@en ;
        rdfs:label    "CombustionTemperature"@en .

PSD:CenterCoreTopHeight
        a             rdf:Property ;
        rdfs:comment  "Center core top height of the profile."@en ;
        rdfs:label    "CenterCoreTopHeight"@en .

PSD:WindLoadRating  a  rdf:Property ;
        rdfs:label  "Wind load rating"@en .

PSD:PressureRating  a  rdf:Property ;
        rdfs:comment  "Nominal pressure rating of the boiler as rated by the agency having jurisdiction."@en ;
        rdfs:label    "Pressure rating"@en .

PSD:CapacityPeople  a  rdf:Property ;
        rdfs:label  "Capacity people"@en .

PSD:ReliefPressure  a  rdf:Property ;
        rdfs:comment  "The pressure at which the spring or weight in the valve is set to discharge fluid."@en ;
        rdfs:label    "ReliefPressure"@en .

PSD:AssetTaxType  a   rdf:Property ;
        rdfs:comment  "Identifies the predefined types of taxation group from which the type required may be set."@en ;
        rdfs:label    "Asset tax type"@en .

PSD:DisplayHeight  a  rdf:Property ;
        rdfs:comment  "Indicates the physical height of the screen (only the display surface)."@en ;
        rdfs:label    "DisplayHeight"@en .

PSD:ScreenDiameter  a  rdf:Property ;
        rdfs:comment  "The diameter of the screen around a cable or bus segment (if present)."@en , "The diameter of the screen around a core segment (if present)."@en ;
        rdfs:label    "ScreenDiameter"@en .

PSD:HeatingDryBulb  a  rdf:Property ;
        rdfs:comment  "Inside dry bulb temperature for heating design."@en , "Outside dry bulb temperature for heating design."@en ;
        rdfs:label    "HeatingDryBulb"@en .

PSD:BendAngle  a      rdf:Property ;
        rdfs:comment  "The change of direction of flow."@en ;
        rdfs:label    "BendAngle"@en .

PSD:PointOfContact  a  rdf:Property ;
        rdfs:comment  "The organization that should be contacted for action under the terms of the warranty. Note that the role of the organization (manufacturer, supplier, installer etc.) is determined by the IfcActorRole attribute of IfcOrganization."@en ;
        rdfs:label    "PointOfContact"@en .

PSD:HorizontalBarPitch
        a             rdf:Property ;
        rdfs:comment  "The pitch length of the horizontal bar."@en ;
        rdfs:label    "HorizontalBarPitch"@en .

PSD:ChargePressure  a  rdf:Property ;
        rdfs:comment  "Nominal or design operating pressure of the tank."@en ;
        rdfs:label    "ChargePressure"@en .

PSD:HasDrive  a     rdf:Property ;
        rdfs:label  "Has drive"@en .

PSD:CompressorCondenserPressureDrop
        a             rdf:Property ;
        rdfs:comment  "Pressure drop between condenser inlet and compressor outlet."@en ;
        rdfs:label    "CompressorCondenserPressureDrop"@en .

PSD:SolarHeatGainTransmittance
        a           rdf:Property ;
        rdfs:label  "Solar heat gain transmittance"@en .

PSD:Weight  a         rdf:Property ;
        rdfs:comment  "The weight of the silencer."@en , "Weight of cable kg/km."@en , "Weight of filter/humidifier."@en , "Weight of core kg/km."@en ;
        rdfs:label    "Weight"@en .

PSD:NominalHeatTransferArea
        a             rdf:Property ;
        rdfs:comment  "Nominal heat transfer surface area associated with nominal overall heat transfer coefficient."@en ;
        rdfs:label    "Nominal heat transfer area"@en .

PSD:HardeningModule  a  rdf:Property ;
        rdfs:comment  "A measure of the hardening module of the material (slope of stress versus strain curve after yield range)."@en ;
        rdfs:label    "Hardening module"@en .

PSD:IsCurrentTolerancePositiveOnly
        a             rdf:Property ;
        rdfs:comment  "Indication whether the value of  CurrentTolerance1 is provided as a positive tolereance only  or not. If not, the value is proved as a pluss/minus tolerance."@en ;
        rdfs:label    "IsCurrentTolerancePositiveOnly"@en .

PSD:WorkMonthDuration
        a             rdf:Property ;
        rdfs:comment  "The elapsed time within a worktime-based month. For presentation purposes, applications may choose to display IfcTask durations in work months where IfcTaskTime.DurationType=WORKTIME. This value must be less than or equal to 744 hours (an elapsed month of 31 days); if omitted then 160 hours is assumed."@en ;
        rdfs:label    "Work month duration"@en .

PSD:SpaceMeanRadiantTemperature
        a             rdf:Property ;
        rdfs:comment  "Mean radiant temperature in the space."@en ;
        rdfs:label    "SpaceMeanRadiantTemperature"@en .

PSD:FurniturePanelType
        a             rdf:Property ;
        rdfs:comment  "Available panel types from which that required may be selected."@en ;
        rdfs:label    "FurniturePanelType"@en .

PSD:CoolingEfficiency
        a             rdf:Property ;
        rdfs:comment  "Coefficient of Performance: Ratio of cooling energy output to energy input under full load operating conditions."@en ;
        rdfs:label    "CoolingEfficiency"@en .

PSD:ThermalIrTransmittance
        a             rdf:Property ;
        rdfs:comment  "Thermal IR transmittance at normal incidence. Defines the fraction of thermal energy that passes through per unit area, perpendicular to the surface."@en ;
        rdfs:label    "ThermalIrTransmittance"@en .

PSD:Location2Global  a  rdf:Property ;
        rdfs:comment  "Global X,Y,Z coordinates of the point in which Thickness2 is given"@en ;
        rdfs:label    "Location2Global"@en .

PSD:CoolingDesignDay  a  rdf:Property ;
        rdfs:comment  "The month, day  and time that has been selected for the cooling design calculations."@en ;
        rdfs:label    "CoolingDesignDay"@en .

PSD:ShortOutsideLowerBarPitch
        a             rdf:Property ;
        rdfs:comment  "The pitch length of the short outside lower bar."@en ;
        rdfs:label    "ShortOutsideLowerBarPitch"@en .

PSD:GlassThickness1  a  rdf:Property ;
        rdfs:label  "Glass thickness 1"@en .

PSD:SensibleEffectiveness
        a             rdf:Property ;
        rdfs:comment  "Sensible heat transfer effectiveness, where effectiveness is defined as the ratio of heat transfer to maximum possible heat transfer."@en ;
        rdfs:label    "SensibleEffectiveness"@en .

PSD:CompressorEvaporatorHeatGain
        a             rdf:Property ;
        rdfs:comment  "Heat gain between the evaporator outlet and the compressor inlet."@en ;
        rdfs:label    "CompressorEvaporatorHeatGain"@en .

PSD:TemperatureRange  a  rdf:Property ;
        rdfs:comment  "Allowable operational range of the fluid temperature."@en , "Allowable minimum and maximum temperature."@en , "Allowable maximum and minimum temperature. Temperature range within which the air terminal is designed to operate."@en , "Temperature range."@en , "Allowable maximum and minimum temperature."@en ;
        rdfs:label    "Temperature range"@en , "TemperatureRange"@en .

PSD:FanEfficiency  a  rdf:Property ;
        rdfs:comment  "Fan mechanical efficiency."@en ;
        rdfs:label    "FanEfficiency"@en .

PSD:WorkingPressureRange
        a             rdf:Property ;
        rdfs:comment  "Allowable minimum and maximum  working pressure (relative to ambient pressure)."@en ;
        rdfs:label    "WorkingPressureRange"@en .

PSD:CornerFixingPlateFlangeWidthInPlaneX
        a             rdf:Property ;
        rdfs:comment  "The flange width of the L-shaped corner plate in plane X."@en ;
        rdfs:label    "CornerFixingPlateFlangeWidthInPlaneX"@en .

PSD:PartialLoadEfficiencyCurves
        a             rdf:Property ;
        rdfs:comment  "Boiler efficiency as a function of the partial load factor; E = f (partialLaodfactor)."@en ;
        rdfs:label    "Partial load efficiency curves"@en .

PSD:NominalSupplyVoltage
        a             rdf:Property ;
        rdfs:comment  "The nominal voltage of the supply."@en ;
        rdfs:label    "NominalSupplyVoltage"@en .

PSD:ClimateChangePerUnit
        a           rdf:Property ;
        rdfs:label  "Climate change per unit"@en .

PSD:d   a             rdf:Property ;
        rdfs:comment  "Measure d according to ISO 2553"@en ;
        rdfs:label    "d"@en .

PSD:CoverLength  a    rdf:Property ;
        rdfs:comment  "The length measured along the x-axis in the local coordinate system or the radius (in the case of a circular shape in plan) of the cover of the drain."@en , "The length measured along the x-axis in the local coordinate system or the radius (in the case of a circular shape in plan) of the cover of the oil interceptor."@en , "The length measured along the x-axis in the local coordinate system or the radius (in the case of a circular shape in plan) of the cover of the waste."@en ;
        rdfs:label    "CoverLength"@en .

PSD:HeatingAirFlowRate
        a             rdf:Property ;
        rdfs:comment  "Heating air flow rate in the space."@en ;
        rdfs:label    "HeatingAirFlowRate"@en .

PSD:EdgeDraft  a      rdf:Property ;
        rdfs:comment  "Edge draft of the profile."@en ;
        rdfs:label    "EdgeDraft"@en .

PSD:ThrowLength  a    rdf:Property ;
        rdfs:comment  "The horizontal or vertical axial distance an airstream travels after leaving an AirTerminal before the maximum stream velocity is reduced to a specified terminal velocity under isothermal conditions at the upper value of the AirFlowrateRange."@en ;
        rdfs:label    "Throw length"@en .

PSD:definition  a   owl:DatatypeProperty ;
        rdfs:label  "Definition"@en ;
        rdfs:range  xsd:string .

PSD:FillGas  a      rdf:Property ;
        rdfs:label  "Fill gas"@en .

PSD:WarrantyStartDate
        a             rdf:Property ;
        rdfs:comment  "The date on which the warranty commences."@en ;
        rdfs:label    "WarrantyStartDate"@en .

PSD:MinimumHeadroom  a  rdf:Property ;
        rdfs:comment  "Headroom required for the activity assigned to this space."@en ;
        rdfs:label    "MinimumHeadroom"@en .

PSD:FloorAreaRatio  a  rdf:Property ;
        rdfs:comment  "The ratio of all floor areas to the buildable area as the maximum floor area utilization of the site as a maximum value according to local building codes."@en ;
        rdfs:label    "Floor area ratio"@en .

PSD:TypePropertyReferenceValue
        a                 owl:Class ;
        rdfs:label        "Type property reference value"@en ;
        rdfs:subClassOf   PSD:PropertyType ;
        rdfs:subClassOf   [ a                   owl:Restriction ;
                            owl:minCardinality  "0"^^xsd:nonNegativeInteger ;
                            owl:onProperty      PSD:dataType
                          ] ;
        owl:disjointWith  PSD:TypeComplexProperty , PSD:TypePropertyEnumeratedValue , PSD:TypePropertySingleValue , PSD:TypePropertyBoundedValue , PSD:TypePropertyListValue , PSD:TypePropertyTableValue .

PSD:SpeakerMounting  a  rdf:Property ;
        rdfs:comment  "Indicates how the speaker is designed to be mounted."@en ;
        rdfs:label    "SpeakerMounting"@en .

PSD:CoolingAirFlowRate
        a             rdf:Property ;
        rdfs:comment  "Cooling air flow rate in the space."@en ;
        rdfs:label    "CoolingAirFlowRate"@en .

PSD:MinimumWidth  a   rdf:Property ;
        rdfs:comment  "The minimum duct width for oval or rectangular duct."@en ;
        rdfs:label    "MinimumWidth"@en .

PSD:AboveGround  a  rdf:Property ;
        rdfs:label  "Above ground"@en .

PSD:Fan  a            rdf:Property ;
        rdfs:comment  "Indicates fan operation where True is on, False is off, and Unknown is automatic."@en ;
        rdfs:label    "Fan"@en .

PSD:IsGuarded  a      rdf:Property ;
        rdfs:comment  "Indication of whether the motor enclosure is guarded (= TRUE) or not (= FALSE)."@en ;
        rdfs:label    "IsGuarded"@en .

PSD:NominalEfficiency
        a             rdf:Property ;
        rdfs:comment  "The nominal efficiency of the boiler as defined by the manufacturer. For steam boilers, a function of inlet temperature versus steam pressure.  Note: as two variables are used, DefiningValues and DefinedValues are null, and values are stored in IfcTable in the following order: InletTemperature(IfcThermodynamicTemperatureMeasure) and OutletTemperature(IfcThermodynamicTemperatureMeasure) in DefiningValues, and NominalEfficiency(IfcNormalisedRatioMeasure) in DefinedValues. For example, DefininfValues(InletTemp, OutletTemp), DefinedValues(null, NominalEfficiency).  The IfcTable is related to IfcPropertyTableValue using IfcMetric and IfcPropertyConstraintRelationship."@en , "The nominal efficiency of the boiler as defined by the manufacturer. For water boilers, a function of inlet versus outlet temperature. Note: as two variables are used, DefiningValues and DefinedValues are null, and values are stored in IfcTable in the following order: InletTemperature(IfcThermodynamicTemperatureMeasure), OutletTemperature(IfcThermodynamicTemperatureMeasure), NominalEfficiency(IfcNormalizedRatioMeasure).  The IfcTable is related to IfcPropertyTableValue using IfcMetric and IfcPropertyConstraintRelationship."@en ;
        rdfs:label    "NominalEfficiency"@en .

PSD:NominalAirFlowRate
        a             rdf:Property ;
        rdfs:comment  "Nominal rate of air flow into which water vapor is added."@en , "Nominal air flow rate."@en ;
        rdfs:label    "Nominal air flow rate"@en , "NominalAirFlowRate"@en .

PSD:dataType  a     owl:ObjectProperty ;
        rdfs:label  "Data  type"@en .

PSD:CoreTopHeight  a  rdf:Property ;
        rdfs:comment  "Core top height of the profile."@en ;
        rdfs:label    "CoreTopHeight"@en .

PSD:PubliclyAccessible
        a           rdf:Property ;
        rdfs:label  "Publicly accessible"@en .

PSD:MaintenanceFactor
        a             rdf:Property ;
        rdfs:comment  "The arithmetical allowance made for depreciation of lamps and reflective equipment from their initial values due to dirt, fumes, or age."@en ;
        rdfs:label    "MaintenanceFactor"@en .

PSD:DrivePowerLoss  a  rdf:Property ;
        rdfs:comment  "Fan drive power losses associated with the type of connection between the motor and the fan wheel."@en ;
        rdfs:label    "DrivePowerLoss"@en .

PSD:WireLoopBasePlateWidth
        a             rdf:Property ;
        rdfs:comment  "The width of the base plate."@en ;
        rdfs:label    "WireLoopBasePlateWidth"@en .

PSD:AirflowRateRange  a  rdf:Property ;
        rdfs:comment  "Range of airflow that can be delivered."@en , "Possible range of airflow that can be delivered."@en ;
        rdfs:label    "Airflow rate range"@en , "AirflowRateRange"@en .

PSD:IsAisle  a        rdf:Property ;
        rdfs:comment  "Indicates that this parking zone is for accessing the parking units, i.e. an aisle (TRUE) and not a parking unit itself (FALSE)"@en ;
        rdfs:label    "IsAisle"@en .

PSD:RequiredHeadroom  a  rdf:Property ;
        rdfs:comment  "Required headroom clearance for the passageway according to the applicable building code or additional requirements."@en ;
        rdfs:label    "Required headroom"@en .

PSD:CoreIdentifier  a  rdf:Property ;
        rdfs:comment  "The core identification used  Identifiers may be used such as by color (Black, Brown, Grey) or by number (1, 2, 3) or by IEC phase reference (L1, L2, L3) etc."@en ;
        rdfs:label    "CoreIdentifier"@en .

PSD:ProductDescription
        a             rdf:Property ;
        rdfs:comment  "A textual description of the products that require the work."@en ;
        rdfs:label    "ProductDescription"@en .

PSD:SwitchActivation  a  rdf:Property ;
        rdfs:comment  "A list of the available activations for toggle switches from which that required may be selected."@en , "A list of the available activations for selector switches from which that required may be selected."@en ;
        rdfs:label    "SwitchActivation"@en .

PSD:SetPointHumidity  a  rdf:Property ;
        rdfs:comment  "The humidity value to be sensed. Use IfcPropertyBoundedValue.SetPointValue to set the set point value."@en ;
        rdfs:label    "SetPointHumidity"@en .

PSD:Staggered  a      rdf:Property ;
        rdfs:comment  "If intermittent weld, staggered or not"@en ;
        rdfs:label    "Staggered"@en .

PSD:HalogenProof  a   rdf:Property ;
        rdfs:comment  "Produces small amount of smoke and irritating Deaerator/Gas."@en , "Produces small amount of smoke and irritating deaerator/gas."@en ;
        rdfs:label    "HalogenProof"@en .

PSD:ReinforcementBarType
        a             rdf:Property ;
        rdfs:comment  "Defines the type of the reinforcement bar."@en ;
        rdfs:label    "ReinforcementBarType"@en .

PSD:KeypadType  a     rdf:Property ;
        rdfs:comment  "A list of the available types of keypad switch from which that required may be selected."@en ;
        rdfs:label    "KeypadType"@en .

PSD:CO2Content  a     rdf:Property ;
        rdfs:comment  "Carbon dioxide (CO2) content of the products of combustion. This is measured in weight of CO2 per unit weight and is therefore unitless."@en ;
        rdfs:label    "CO2Content"@en .

PSD:AuxiliaryEnergySourceConsumption
        a             rdf:Property ;
        rdfs:comment  "Auxiliary energy source consumption."@en ;
        rdfs:label    "AuxiliaryEnergySourceConsumption"@en .

PSD:SaturationEfficiencyCurve
        a             rdf:Property ;
        rdfs:comment  "Saturation efficiency as a function of the air flow rate."@en ;
        rdfs:label    "Saturation efficiency curve"@en .

PSD:Direction  a      rdf:Property ;
        rdfs:comment  "Indicates sensed direction for sensors capturing magnitude and direction measured from True North (0 degrees) in a clockwise direction."@en ;
        rdfs:label    "Direction"@en .

PSD:WithLock  a       rdf:Property ;
        rdfs:comment  "Indicates whether the file cabinet is lockable (= TRUE) or not (= FALSE)."@en ;
        rdfs:label    "WithLock"@en .

PSD:AlkalinityConcentration
        a             rdf:Property ;
        rdfs:comment  "Maximum alkalinity concentration (maximum sum of concentrations of each of the negative ions substances measured as CaCO3)."@en ;
        rdfs:label    "AlkalinityConcentration"@en .

PSD:FrameType  a      rdf:Property ;
        rdfs:comment  "The type of frame used by the damper (e.g., Standard, Single Flange, Single Reversed Flange, Double Flange, etc.)."@en ;
        rdfs:label    "FrameType"@en .

PSD:ThermalTransmittance
        a           rdf:Property ;
        rdfs:label  "Thermal transmittance"@en .

PSD:MaxAggregateSize  a  rdf:Property ;
        rdfs:label  "Max aggregate size"@en .

PSD:StartingTime  a   rdf:Property ;
        rdfs:comment  "The time (in s) needed for the motor to reach its rated speed with its driven equipment attached, starting from standstill and at the nominal voltage applied at its terminals."@en ;
        rdfs:label    "StartingTime"@en .

PSD:Location1Local  a  rdf:Property ;
        rdfs:comment  "Local x,y coordinates of the point in which Thickness1 is given"@en ;
        rdfs:label    "Location1Local"@en .

PSD:WaistThickness  a  rdf:Property ;
        rdfs:label  "Waist thickness"@en .

PSD:PlayerType  a     rdf:Property ;
        rdfs:comment  "Indicates the type of player."@en ;
        rdfs:label    "PlayerType"@en .

PSD:Voltage  a        rdf:Property ;
        rdfs:comment  "Log of electrical voltage."@en ;
        rdfs:label    "Voltage"@en .

PSD:EntranceLevel  a  rdf:Property ;
        rdfs:label  "Entrance level"@en .

PSD:Restrictions  a   rdf:Property ;
        rdfs:comment  "Restrictions that may be placed by a  competent authority."@en ;
        rdfs:label    "Restrictions"@en .

PSD:ModelLabel  a     rdf:Property ;
        rdfs:comment  "The descriptive model name of the product model (or product line) as assigned by the manufacturer of the manufactured item."@en ;
        rdfs:label    "ModelLabel"@en .

PSD:ColumnShoeBasePlateDepth
        a             rdf:Property ;
        rdfs:comment  "The depth of the column shoe base plate."@en ;
        rdfs:label    "ColumnShoeBasePlateDepth"@en .

PSD:WaterStorageCapacity
        a             rdf:Property ;
        rdfs:comment  "Water storage capacity."@en ;
        rdfs:label    "Water storage capacity"@en .

PSD:PropertyType  a      owl:Class ;
        rdfs:label       "Property type"@en ;
        rdfs:subClassOf  owl:Thing .

PSD:AirflowCurve  a   rdf:Property ;
        rdfs:comment  "Air flowrate versus damper position relationship;airflow = f ( valve position)."@en ;
        rdfs:label    "Airflow curve"@en .

PSD:StrengthGrade  a  rdf:Property ;
        rdfs:comment  "Grade with respect to mechanical strength and stiffness."@en ;
        rdfs:label    "StrengthGrade"@en .

PSD:TotalHeatTransferRate
        a             rdf:Property ;
        rdfs:comment  "Total heat transfer rate."@en , "Total heat transfer rate to primary air flow."@en ;
        rdfs:label    "TotalHeatTransferRate"@en .

PSD:InletDiameter  a  rdf:Property ;
        rdfs:comment  "The inlet diameter of the breeching inlet."@en ;
        rdfs:label    "InletDiameter"@en .

PSD:reftype  a        owl:ObjectProperty , owl:FunctionalProperty ;
        rdfs:comment  "Reference type based on SELECT Type IfcObjectReferenceSelect." ;
        rdfs:domain   PSD:TypePropertyReferenceValue ;
        rdfs:range    IFC4:IfcObjectReferenceSelect .

PSD:AirExchangeRate  a  rdf:Property ;
        rdfs:comment  "Loads from the air exchange rate."@en ;
        rdfs:label    "AirExchangeRate"@en .

PSD:FireProtectionClass
        a           rdf:Property ;
        rdfs:label  "Fire protection class"@en .

PSD:InformationDeliverySpecification
        a                owl:Class ;
        rdfs:label       "Information delivery specification"@en ;
        rdfs:subClassOf  owl:Thing ;
        rdfs:subClassOf  [ a                   owl:Restriction ;
                           owl:maxCardinality  "1"^^xsd:nonNegativeInteger ;
                           owl:onProperty      PSD:name
                         ] .

PSD:ProportionalStress
        a             rdf:Property ;
        rdfs:comment  "A measure of the proportional stress of the material. It describes the stress before the first plastic deformation occurs and is commonly measured at a deformation of 0.01%."@en ;
        rdfs:label    "Proportional stress"@en .

PSD:EdgeFixingPlateFlangeWidthInPlaneX
        a             rdf:Property ;
        rdfs:comment  "The flange width of the L-shaped edge plate in plane X."@en ;
        rdfs:label    "EdgeFixingPlateFlangeWidthInPlaneX"@en .

PSD:AirFlowrateRange  a  rdf:Property ;
        rdfs:comment  "Possible range of airflow that can be delivered."@en , "Air flowrate range within which the air terminal is designed to operate."@en ;
        rdfs:label    "AirFlowrateRange"@en , "Air flowrate range"@en .

PSD:PressureRise  a   rdf:Property ;
        rdfs:comment  "The developed pressure."@en ;
        rdfs:label    "PressureRise"@en .

PSD:UpperCurrent2  a  rdf:Property ;
        rdfs:comment  "The current in [x In], indicating the upper current limit of the upper time/current curve of the I2t part of the L-function."@en ;
        rdfs:label    "UpperCurrent2"@en .

PSD:YieldStress  a    rdf:Property ;
        rdfs:comment  "A measure of the yield stress (or characteristic 0.2 percent proof stress) of the material."@en ;
        rdfs:label    "Yield stress"@en .

PSD:CompressorEvaporatorPressureDrop
        a             rdf:Property ;
        rdfs:comment  "Pressure drop between the evaporator outlet and the compressor inlet."@en ;
        rdfs:label    "CompressorEvaporatorPressureDrop"@en .

PSD:Spacing  a        rdf:Property ;
        rdfs:comment  "Distance between fins on a tube in the tube bundle."@en ;
        rdfs:label    "Spacing"@en .

PSD:SoundCurve  a     rdf:Property ;
        rdfs:comment  "Table of sound frequencies and sound power measured in decibels at a reference power of 1 picowatt(10^(-12) watt) for the referenced octave band frequency."@en , "Regenerated sound versus air-flow rate."@en ;
        rdfs:label    "SoundCurve"@en .

PSD:BudgetSource  a   rdf:Property ;
        rdfs:comment  "The budget source requested."@en ;
        rdfs:label    "BudgetSource"@en .

PSD:LampMaintenanceFactor
        a             rdf:Property ;
        rdfs:comment  "Non recoverable losses of luminous flux of a lamp due to lamp depreciation; i.e. the decreasing of light output of a luminaire due to aging and dirt."@en ;
        rdfs:label    "Lamp maintenance factor"@en .

PSD:NumberOfSources  a  rdf:Property ;
        rdfs:comment  "Number of sources ."@en ;
        rdfs:label    "NumberOfSources"@en .

PSD:AirFlowLeakage  a  rdf:Property ;
        rdfs:comment  "Volumetric leakage flow rate."@en ;
        rdfs:label    "AirFlowLeakage"@en .

PSD:IsLaminated  a  rdf:Property ;
        rdfs:label  "Is laminated"@en .

PSD:LowerTime1  a     rdf:Property ;
        rdfs:comment  "The time in [s], indicating that tripping times of the lower time/current curve lower than LowerTime1 is determined by the I2t part of the L-function."@en ;
        rdfs:label    "LowerTime1"@en .

PSD:ThermalTrippingUnitType
        a             rdf:Property ;
        rdfs:comment  "A list of the available types of thermal tripping unit  from which that required may be selected."@en ;
        rdfs:label    "ThermalTrippingUnitType"@en .

PSD:HasSoundAttenuator
        a             rdf:Property ;
        rdfs:comment  "If TRUE, the air terminal has sound attenuation."@en ;
        rdfs:label    "Has sound attenuator"@en .

PSD:ViscosityTemperatureDerivative
        a             rdf:Property ;
        rdfs:comment  "Viscosity temperature derivative."@en ;
        rdfs:label    "Viscosity temperature derivative"@en .

PSD:Orientation  a    rdf:Property ;
        rdfs:comment  "The intended orientation for the damper as specified by the manufacturer."@en ;
        rdfs:label    "Orientation"@en .

PSD:AirPressureDropCurve
        a             rdf:Property ;
        rdfs:comment  "Air pressure drop versus air-flow rate."@en , "Air pressure drop curve, pressure drop  flow rate curve, AirPressureDrop = f (AirflowRate)."@en , "Air pressure drop as a function of air flow rate."@en ;
        rdfs:label    "Air pressure drop curve"@en , "AirPressureDropCurve"@en .

PSD:AcquisitionMethod
        a             rdf:Property ;
        rdfs:comment  "The means by which survey data was acquired."@en ;
        rdfs:label    "AcquisitionMethod"@en .

PSD:NominalWidth  a   rdf:Property ;
        rdfs:comment  "The nominal width of the segment."@en , "Nominal or quoted width of the object."@en , "The nominal width of the system furniture elements of this type. The size information is provided in addition to the shape representation and the geometric parameters used within. In cases of inconsistency between the geometric parameters and the size properties, provided in the attached property set, the geometric parameters take precedence."@en ;
        rdfs:label    "NominalWidth"@en , "Nominal width"@en .

PSD:DraftBaseOffset  a  rdf:Property ;
        rdfs:comment  "Draft base offset of the profile."@en ;
        rdfs:label    "DraftBaseOffset"@en .

PSD:FrequencyResponse
        a             rdf:Property ;
        rdfs:comment  "Indicates the output over a specified range of frequencies."@en ;
        rdfs:label    "FrequencyResponse"@en .

PSD:ShapeType  a      rdf:Property ;
        rdfs:comment  "Shape of the junction box."@en ;
        rdfs:label    "ShapeType"@en .

PSD:DischargeVelocity
        a             rdf:Property ;
        rdfs:comment  "The speed at which air discharges from the fan through the fan housing discharge opening."@en ;
        rdfs:label    "DischargeVelocity"@en .

PSD:IP_Code  a        rdf:Property ;
        rdfs:comment  "IEC 60529 (1989) Classification of degrees of protection provided by enclosures (IP Code)."@en ;
        rdfs:label    "IP_Code"@en .

PSD:TunerFrequency  a  rdf:Property ;
        rdfs:comment  "Indicates the tuner frequencies, if applicable."@en ;
        rdfs:label    "TunerFrequency"@en .

PSD:SubstanceDetected
        a             rdf:Property ;
        rdfs:comment  "Identification of the substance that is being detected according to chemical formula.  For example, calcium carbonate is 'CaCO3'"@en ;
        rdfs:label    "SubstanceDetected"@en .

PSD:WaterConsumption  a  rdf:Property ;
        rdfs:label  "Water consumption"@en .

PSD:ColorRenderingIndex
        a             rdf:Property ;
        rdfs:comment  "The CRI indicates how well a light source renders eight standard colors compared to perfect reference lamp with the same color temperature. The CRI scale ranges from 1 to 100, with 100 representing perfect rendering properties."@en ;
        rdfs:label    "Color rendering index"@en .

PSD:NutShape  a       rdf:Property ;
        rdfs:comment  "Shape of the nut, e.g. 'Hexagon', 'Cap', 'Castle', 'Wing'"@en ;
        rdfs:label    "NutShape"@en .

PSD:TypeComplexProperty
        a                 owl:Class ;
        rdfs:label        "Type property complex property"@en ;
        rdfs:subClassOf   PSD:PropertyType ;
        rdfs:subClassOf   [ a                owl:Restriction ;
                            owl:cardinality  "1"^^xsd:nonNegativeInteger ;
                            owl:onProperty   PSD:name
                          ] ;
        owl:disjointWith  PSD:TypePropertyListValue , PSD:TypePropertySingleValue , PSD:TypePropertyReferenceValue , PSD:TypePropertyEnumeratedValue , PSD:TypePropertyBoundedValue , PSD:TypePropertyTableValue .

PSD:HeatingDesignAirflow
        a             rdf:Property ;
        rdfs:comment  "The air flowrate required during the peak heating conditions, but could also be determined by minimum ventilation requirement or minimum air change requirements."@en ;
        rdfs:label    "HeatingDesignAirflow"@en .

PSD:Current  a        rdf:Property ;
        rdfs:comment  "Log of electrical current."@en ;
        rdfs:label    "Current"@en .

PSD:CondenserEnteringTemperature
        a             rdf:Property ;
        rdfs:comment  "Temperature of fluid entering condenser."@en ;
        rdfs:label    "CondenserEnteringTemperature"@en .

PSD:SpecificHeatCapacity
        a             rdf:Property ;
        rdfs:comment  "Defines the specific heat of the material: heat energy absorbed per temperature unit."@en , "Specific heat of the products of combustion: heat energy absorbed per temperature unit."@en ;
        rdfs:label    "SpecificHeatCapacity"@en .

PSD:NominalReturnWaterTemperatureCooling
        a             rdf:Property ;
        rdfs:comment  "Nominal return water temperature (refers to nominal cooling capacity)."@en ;
        rdfs:label    "NominalReturnWaterTemperatureCooling"@en .

PSD:enumItem  a       owl:DatatypeProperty ;
        rdfs:comment  "Enumeration item in uppercase."@en ;
        rdfs:domain   PSD:TypePropertyEnumeratedValue ;
        rdfs:label    "Enumeration item"@en ;
        rdfs:range    xsd:string .

PSD:IsTempered  a   rdf:Property ;
        rdfs:label  "Is tempered"@en .

PSD:DimensionalAccuracyClass
        a           rdf:Property ;
        rdfs:label  "Dimensional accuracy class"@en .

PSD:DimmerType  a     rdf:Property ;
        rdfs:comment  "A list of the available types of dimmer switch from which that required may be selected."@en ;
        rdfs:label    "DimmerType"@en .

PSD:JunctionLeftAngle
        a             rdf:Property ;
        rdfs:comment  "The change of direction of flow for the left junction."@en ;
        rdfs:label    "JunctionLeftAngle"@en .

PSD:NominalFlowrate  a  rdf:Property ;
        rdfs:comment  "Nominal fluid flow rate through the filter."@en ;
        rdfs:label    "Nominal flowrate"@en .

PSD:ExternalSurfaceArea
        a             rdf:Property ;
        rdfs:comment  "External surface area (both primary and secondary area)."@en ;
        rdfs:label    "External surface area"@en .

PSD:PitchAngle  a   rdf:Property ;
        rdfs:label  "Pitch angle"@en .

PSD:Finish  a       rdf:Property ;
        rdfs:label  "Finish"@en .

PSD:Location2Local  a  rdf:Property ;
        rdfs:comment  "Local x,y coordinates of the point in which Thickness2 is given"@en ;
        rdfs:label    "Location2Local"@en .

PSD:EarthFault1PoleMinimumState
        a             rdf:Property ;
        rdfs:comment  "Minimum 1 pole earth fault current provided at the point of supply i.e. the fault between 1 phase and PE/PEN."@en ;
        rdfs:label    "EarthFault1PoleMinimumState"@en .

PSD:DraftSideOffset  a  rdf:Property ;
        rdfs:comment  "Draft side offset of the profile."@en ;
        rdfs:label    "DraftSideOffset"@en .

PSD:SupportType  a    rdf:Property ;
        rdfs:comment  "Available support types from which that required may be selected."@en ;
        rdfs:label    "SupportType"@en .

PSD:Acknowledge  a    rdf:Property ;
        rdfs:comment  "Indicates acknowledgement status where False indicates acknowlegement is required and outstanding, True indicates condition has been acknowedged, and Unknown indicates no acknowledgement is required.  Upon resetting the condition, then acknowledgement reverts to Unknown."@en ;
        rdfs:label    "Acknowledge"@en .

PSD:Hardness  a       rdf:Property ;
        rdfs:comment  "Water hardness as positive, multivalent ion concentration in the water (usually concentrations of calcium and magnesium ions in terms of calcium carbonate)."@en ;
        rdfs:label    "Hardness"@en .

PSD:EndShapeType  a   rdf:Property ;
        rdfs:comment  "Defines the types of end shapes that can be used for preformed tanks. The convention for reading these enumerated values is that for a vertical cylinder, the first value is the base and the second is the top; for a horizontal cylinder, the order of reading should be left to right. For a speherical tank, the value UNSET should be used."@en ;
        rdfs:label    "EndShapeType"@en .

PSD:SlotWidth  a      rdf:Property ;
        rdfs:comment  "Slot width."@en ;
        rdfs:label    "Slot width"@en .

PSD:VideoScaleMode  a  rdf:Property ;
        rdfs:comment  "Indicates video scaling modes."@en ;
        rdfs:label    "VideoScaleMode"@en .

PSD:SetPointPH  a     rdf:Property ;
        rdfs:comment  "The fill level value to be sensed. Use IfcPropertyBoundedValue.SetPointValue to set the set point value."@en ;
        rdfs:label    "SetPointPH"@en .

PSD:RotationSpeed  a  rdf:Property ;
        rdfs:comment  "Pump rotational speed."@en ;
        rdfs:label    "RotationSpeed"@en .

PSD:Slope  a          rdf:Property ;
        rdfs:comment  "Angle of the gutter to allow for drainage."@en , "Sloping angle of the object  - relative to horizontal (0.0 degrees). \\nActual maximum slope for the passageway according to the current design.\\nThe shape information is provided in addition to the shape representation and the geometric parameters used within. In cases of inconsistency between the geometric parameters and the shape properties, provided in the attached property, the geometric parameters take precedence."@en ;
        rdfs:label    "Slope"@en .

PSD:FinishColor  a    rdf:Property ;
        rdfs:comment  "Finish color for cooled beam."@en , "The finish color for the air terminal."@en ;
        rdfs:label    "FinishColor"@en , "Finish color"@en .

PSD:DischargePressureLoss
        a             rdf:Property ;
        rdfs:comment  "Fan discharge pressure loss associated with the discharge arrangement."@en ;
        rdfs:label    "DischargePressureLoss"@en .

PSD:WeatherDataDate  a  rdf:Property ;
        rdfs:comment  "The date for which the weather data was gathered."@en ;
        rdfs:label    "WeatherDataDate"@en .

PSD:ShortOutsideTopBarPitch
        a             rdf:Property ;
        rdfs:comment  "The pitch length of the short outside top bar."@en ;
        rdfs:label    "ShortOutsideTopBarPitch"@en .

PSD:TotalEffectiveness
        a             rdf:Property ;
        rdfs:comment  "Total heat transfer effectiveness: The ratio of heat transfer to the maximum possible heat transfer."@en ;
        rdfs:label    "TotalEffectiveness"@en .

PSD:NominalThickness  a  rdf:Property ;
        rdfs:comment  "The nominal thickness of the panel."@en , "The nominal thickness of the work surface."@en ;
        rdfs:label    "NominalThickness"@en , "Nominal thickness"@en .

PSD:DeliveryType  a   rdf:Property ;
        rdfs:comment  "Determines how the accessory will be delivered to the site."@en ;
        rdfs:label    "Delivery type"@en .

PSD:ControlDamperOperation
        a             rdf:Property ;
        rdfs:comment  "The inherent characteristic of the control damper operation."@en ;
        rdfs:label    "ControlDamperOperation"@en .

PSD:SupplyWaterTemperatureCooling
        a             rdf:Property ;
        rdfs:comment  "Supply water temperature in cooling mode."@en ;
        rdfs:label    "SupplyWaterTemperatureCooling"@en .

PSD:Layup  a          rdf:Property ;
        rdfs:comment  "Configuration of the lamination."@en ;
        rdfs:label    "Layup"@en .

PSD:AdmixturesDescription
        a           rdf:Property ;
        rdfs:label  "Admixtures description"@en .

PSD:ArtificialLighting
        a             rdf:Property ;
        rdfs:comment  "Indication whether this space  requires artificial lighting (as natural lighting would be not sufficient). (TRUE) indicates yes (FALSE) otherwise."@en ;
        rdfs:label    "ArtificialLighting"@en .

PSD:FormStrippingStrength
        a           rdf:Property ;
        rdfs:label  "Form stripping strength"@en .

PSD:OutputCapacityCurve
        a             rdf:Property ;
        rdfs:comment  "Partial output capacity curve (as a function of water temperature); Q = f (Twater)."@en ;
        rdfs:label    "OutputCapacityCurve"@en .

PSD:PieceMark  a      rdf:Property ;
        rdfs:comment  "Defines a unique piece for production purposes. All pieces with the same piece mark value are identical and interchangeable. The piece mark may be composed of sub-parts that have specific locally defined meaning (e.g. B-1A may denote a beam, of generic type 1 and specific shape A)."@en ;
        rdfs:label    "Piece mark"@en , "PieceMark"@en .

PSD:ReturnAirFractionRange
        a             rdf:Property ;
        rdfs:comment  "Allowable return air fraction range as a fraction of discharge airflow."@en ;
        rdfs:label    "Return air fraction range"@en .

PSD:InstallationMethod
        a             rdf:Property ;
        rdfs:comment  "Method of installation of cable/conductor. Installation methods are typically defined by reference in standards such as IEC 60364-5-52, table 52A-1 or BS7671 Appendix 4 Table 4A1 etc. Selection of the value to be used should be determined from such a standard according to local usage."@en ;
        rdfs:label    "InstallationMethod"@en .

PSD:StemTopChamfer  a  rdf:Property ;
        rdfs:comment  "Stem top chamfer of the profile."@en ;
        rdfs:label    "StemTopChamfer"@en .

PSD:FunctionalUnitReference
        a           rdf:Property ;
        rdfs:label  "Functional unit reference"@en .

PSD:NeckArea  a       rdf:Property ;
        rdfs:comment  "Neck area of the air terminal."@en ;
        rdfs:label    "Neck area"@en .

PSD:GroupCode  a      rdf:Property ;
        rdfs:comment  "e.g. panels, worksurfaces, storage, etc."@en ;
        rdfs:label    "GroupCode"@en .

PSD:NominalHeatingCapacity
        a             rdf:Property ;
        rdfs:comment  "Nominal heating capacity."@en ;
        rdfs:label    "NominalHeatingCapacity"@en .

PSD:SolarRefractionIndex
        a             rdf:Property ;
        rdfs:comment  "Index of refraction (solar) defines the \\\"bending\\\" of the solar ray when it passes from one medium into another."@en ;
        rdfs:label    "Solar refraction index"@en .

PSD:CrossingUpperBarPitch
        a             rdf:Property ;
        rdfs:comment  "The pitch length of the crossing upper bar."@en ;
        rdfs:label    "CrossingUpperBarPitch"@en .

PSD:PrevailingWindVelocity
        a             rdf:Property ;
        rdfs:comment  "The design wind velocity coming from the direction specified by the PrevailingWindDirection attribute."@en ;
        rdfs:label    "PrevailingWindVelocity"@en .

PSD:DiagonalTrussCrossBarDiameter
        a             rdf:Property ;
        rdfs:comment  "The nominal diameter of the diagonal cross-bars."@en ;
        rdfs:label    "DiagonalTrussCrossBarDiameter"@en .

PSD:EffectiveArea  a  rdf:Property ;
        rdfs:comment  "Effective discharge area of the air terminal."@en ;
        rdfs:label    "Effective area"@en .

PSD:AutomaticCondensateDischarge
        a             rdf:Property ;
        rdfs:comment  "Whether or not the condensing water or oil is discharged automatically from the filter."@en ;
        rdfs:label    "AutomaticCondensateDischarge"@en .

PSD:AssessmentDescription
        a             rdf:Property ;
        rdfs:comment  "Qualitative description of the condition."@en ;
        rdfs:label    "Assessment description"@en .

PSD:Function  a       rdf:Property ;
        rdfs:comment  "Type of function for which the conductor is intended."@en ;
        rdfs:label    "Function"@en .

PSD:YearOfConstruction
        a           rdf:Property ;
        rdfs:label  "Year of construction"@en .

PSD:TotalArea  a      rdf:Property ;
        rdfs:comment  "Total planned area for the site. Used for programming the site space."@en ;
        rdfs:label    "Total area"@en .

PSD:VacancyRateInCategoryNow
        a             rdf:Property ;
        rdfs:comment  "Percentage of vacancy found in the particular category currently."@en ;
        rdfs:label    "Vacancy rate in category now"@en .

PSD:HasHotGasBypass  a  rdf:Property ;
        rdfs:comment  "Whether or not hot gas bypass is provided for the compressor. TRUE = Yes, FALSE = No."@en ;
        rdfs:label    "Has hot gas bypass"@en .

PSD:Unit  a         rdf:Property ;
        rdfs:label  "Unit"@en .

PSD:PlayerMediaFormat
        a             rdf:Property ;
        rdfs:comment  "Indicates supported media formats."@en ;
        rdfs:label    "PlayerMediaFormat"@en .

PSD:HasCoating  a     rdf:Property ;
        rdfs:comment  "TRUE if the fin has a coating, FALSE if it does not."@en ;
        rdfs:label    "HasCoating"@en .

PSD:NominalCapacity  a  rdf:Property ;
        rdfs:comment  "Compressor nameplate capacity."@en ;
        rdfs:label    "Nominal capacity"@en .

PSD:BuildableArea  a  rdf:Property ;
        rdfs:comment  "The ratio of the utilization,  TotalArea / BuildableArea, expressed as a maximum value. The ratio value may be used to derive BuildableArea."@en ;
        rdfs:label    "Buildable area"@en .

PSD:WarrantyEndDate  a  rdf:Property ;
        rdfs:comment  "The date on which the warranty expires."@en ;
        rdfs:label    "WarrantyEndDate"@en .

PSD:IsCoated  a     rdf:Property ;
        rdfs:label  "Is coated"@en .

PSD:LandTitleID  a    rdf:Property ;
        rdfs:comment  "Identification number assigned by the statutory registration authority to the title to a land parcel."@en ;
        rdfs:label    "LandTitleID"@en .

PSD:FittingLossFactor
        a             rdf:Property ;
        rdfs:comment  "A factor that determines the pressure loss due to friction through the fitting."@en ;
        rdfs:label    "Fitting loss factor"@en .

PSD:ExteriorHeatTransferCoefficient
        a             rdf:Property ;
        rdfs:comment  "Exterior heat transfer coefficient associated with exterior surface area."@en ;
        rdfs:label    "ExteriorHeatTransferCoefficient"@en .

PSD:IsSwitch  a       rdf:Property ;
        rdfs:comment  "Identifies if the sensor also functions as a switch at the set point (=TRUE) or not (= FALSE)."@en ;
        rdfs:label    "IsSwitch"@en .

PSD:propertyDef  a   owl:ObjectProperty ;
        rdfs:domain  [ a            owl:Class ;
                       owl:unionOf  ( PSD:PropertySetDef PSD:TypeComplexProperty )
                     ] ;
        rdfs:label   "Property definition"@en ;
        rdfs:range   PSD:PropertyDef .

PSD:MaximumAirFlowRate
        a             rdf:Property ;
        rdfs:comment  "Maximum allowable air flow rate."@en ;
        rdfs:label    "MaximumAirFlowRate"@en .

PSD:PhotochemicalOzoneFormation
        a           rdf:Property ;
        rdfs:label  "Photochemical ozone formation"@en .

PSD:SprinklerType  a  rdf:Property ;
        rdfs:comment  "Identifies the predefined types of sprinkler  from which the type required may be set."@en ;
        rdfs:label    "SprinklerType"@en .

PSD:GasDetected  a    rdf:Property ;
        rdfs:comment  "Identification of the gas that is being detected, according to chemical formula.  For example, carbon monoxide is 'CO', carbon dioxide is 'CO2', oxygen is 'O2'."@en ;
        rdfs:label    "GasDetected"@en .

PSD:NominalRotationSpeed
        a             rdf:Property ;
        rdfs:comment  "Pump rotational speed under nominal conditions."@en , "Nominal fan wheel speed."@en ;
        rdfs:label    "NominalRotationSpeed"@en , "Nominal rotation speed"@en .

PSD:LightEmitterNominalPower
        a             rdf:Property ;
        rdfs:comment  "Light emitter nominal power."@en ;
        rdfs:label    "Light emitter nominal power"@en .

PSD:TrippingUnitReleaseCurrent
        a             rdf:Property ;
        rdfs:comment  "The value of tripping or residual current for which the device has the possibility to be equipped. The values are given in mA."@en ;
        rdfs:label    "TrippingUnitReleaseCurrent"@en .

PSD:WireLoopBasePlateThickness
        a             rdf:Property ;
        rdfs:comment  "The thickness of the base plate."@en ;
        rdfs:label    "WireLoopBasePlateThickness"@en .

PSD:DiagonalTrussHeight
        a             rdf:Property ;
        rdfs:comment  "The overall height of the truss connector."@en ;
        rdfs:label    "DiagonalTrussHeight"@en .

PSD:HeatTransferSurfaceArea
        a             rdf:Property ;
        rdfs:comment  "Total heat transfer area of the vessel."@en ;
        rdfs:label    "Heat transfer surface area"@en .

PSD:ClassOfService  a  rdf:Property ;
        rdfs:comment  "A classification of usage of the hose reel that may be applied."@en ;
        rdfs:label    "ClassOfService"@en .

PSD:I1  a             rdf:Property ;
        rdfs:comment  "The (thermal) lower testing current limit in [x In], indicating that for currents lower than I1, the tripping time shall be longer than the associated tripping time, T2."@en ;
        rdfs:label    "I1"@en .

PSD:HasFan  a         rdf:Property ;
        rdfs:comment  "Terminal box has a fan inside (fan powered box)."@en ;
        rdfs:label    "Has fan"@en .

PSD:CoreBaseWidth  a  rdf:Property ;
        rdfs:comment  "Core base width of the profile."@en ;
        rdfs:label    "CoreBaseWidth"@en .

PSD:RemoteReading  a  rdf:Property ;
        rdfs:comment  "Indicates whether the meter has a connection for remote reading through connection of a communication device (set TRUE) or not (set FALSE)."@en ;
        rdfs:label    "Remote reading"@en .

PSD:DischargeCoefficient
        a             rdf:Property ;
        rdfs:comment  "The coefficient of flow at the sprinkler."@en ;
        rdfs:label    "DischargeCoefficient"@en .

PSD:LowerHeatingValue
        a             rdf:Property ;
        rdfs:comment  "Lower Heating Value is defined as the amount of energy released (MJ/kg) when a fuel is burned completely, and H2O is in vapor form in the combustion products."@en ;
        rdfs:label    "LowerHeatingValue"@en .

PSD:OverallEfficiency
        a             rdf:Property ;
        rdfs:comment  "Total efficiency of motor and fan."@en , "The pump and motor overall operational efficiency."@en ;
        rdfs:label    "OverallEfficiency"@en .

PSD:Electricity  a    rdf:Property ;
        rdfs:comment  "The amount of electricity consumed during the period specified in the time series."@en ;
        rdfs:label    "Electricity"@en .

PSD:ThicknessSwelling
        a             rdf:Property ;
        rdfs:comment  "Swelling ratio relative to board depth."@en ;
        rdfs:label    "ThicknessSwelling"@en .

PSD:TimeTolerance1  a  rdf:Property ;
        rdfs:comment  "The tolerance for the time of time/current-curve in [%]."@en ;
        rdfs:label    "TimeTolerance1"@en .

PSD:T5  a             rdf:Property ;
        rdfs:comment  "The electromagnetic testing time in [s] associated with the testing currents I4 and I5, i.e. electromagnetic tripping time"@en ;
        rdfs:label    "T5"@en .

PSD:OutsideDiameter  a  rdf:Property ;
        rdfs:comment  "Actual outside diameter of the tube in the tube bundle."@en ;
        rdfs:label    "OutsideDiameter"@en .

PSD:propertySetDef  a  owl:ObjectProperty ;
        rdfs:domain  PSD:RequiredPset ;
        rdfs:range   PSD:PropertySetDef .

PSD:FlowControlType  a  rdf:Property ;
        rdfs:comment  "Type of flow control element that may be included as a part of the construction of the air terminal."@en ;
        rdfs:label    "Flow control type"@en .

PSD:BackupSupplySystem
        a             rdf:Property ;
        rdfs:comment  "The type of backup supply system."@en ;
        rdfs:label    "BackupSupplySystem"@en .

PSD:SpecificHeatTemperatureDerivative
        a             rdf:Property ;
        rdfs:comment  "Specific heat temperature derivative."@en ;
        rdfs:label    "Specific heat temperature derivative"@en .

PSD:Stroke  a         rdf:Property ;
        rdfs:comment  "Indicates the maximum distance the actuator must traverse."@en ;
        rdfs:label    "Stroke"@en .

PSD:FaceVelocity  a   rdf:Property ;
        rdfs:comment  "Air velocity through the coil."@en ;
        rdfs:label    "FaceVelocity"@en .

PSD:StaggeredRowSpacing
        a             rdf:Property ;
        rdfs:comment  "Staggered tube row spacing."@en ;
        rdfs:label    "StaggeredRowSpacing"@en .

PSD:FixtureHeight  a  rdf:Property ;
        rdfs:comment  "The height of the fixture, such as the text height of an exit sign."@en ;
        rdfs:label    "FixtureHeight"@en .

PSD:CoolingRelativeHumidity
        a             rdf:Property ;
        rdfs:comment  "Inside relative humidity for cooling design."@en ;
        rdfs:label    "CoolingRelativeHumidity"@en .

PSD:InputFlowrate  a  rdf:Property ;
        rdfs:comment  "Maximum hydraulic flowrate requirement."@en ;
        rdfs:label    "Input flowrate"@en .

PSD:CorrectionFactorForCooling
        a             rdf:Property ;
        rdfs:comment  "Correction factor k as a function of water flow rate (used to calculate cooling capacity)."@en ;
        rdfs:label    "CorrectionFactorForCooling"@en .

PSD:NumberOfTreads  a  rdf:Property ;
        rdfs:label  "Number of treads"@en .

PSD:OccupancyDiversity
        a             rdf:Property ;
        rdfs:comment  "Diversity factor that may be applied to the number of people in the space."@en ;
        rdfs:label    "OccupancyDiversity"@en .

PSD:Brightness  a     rdf:Property ;
        rdfs:comment  "Indicates the display brightness."@en ;
        rdfs:label    "Brightness"@en .

PSD:UltimateStrain  a  rdf:Property ;
        rdfs:comment  "A measure of the (engineering) strain at the state of ultimate stress of the material."@en ;
        rdfs:label    "Ultimate strain"@en .

PSD:SumpHeaterPower  a  rdf:Property ;
        rdfs:comment  "Electrical heat power of sump heater."@en ;
        rdfs:label    "SumpHeaterPower"@en .

PSD:SpaceTemperature  a  rdf:Property ;
        rdfs:comment  "Temperature of the space."@en ;
        rdfs:label    "SpaceTemperature"@en .

PSD:Location1Global  a  rdf:Property ;
        rdfs:comment  "Global X,Y,Z coordinates of the point in which Thickness1 is given"@en ;
        rdfs:label    "Location1Global"@en .

PSD:ProductionYear  a  rdf:Property ;
        rdfs:comment  "The year of production of the manufactured item."@en ;
        rdfs:label    "ProductionYear"@en .

PSD:DisplayType  a    rdf:Property ;
        rdfs:comment  "Indicates the type of display."@en ;
        rdfs:label    "DisplayType"@en .

PSD:KeyHeight  a      rdf:Property ;
        rdfs:comment  "Key height of the profile."@en ;
        rdfs:label    "KeyHeight"@en .

PSD:YDirectionUpperBarCount
        a             rdf:Property ;
        rdfs:comment  "The number of bars with Y direction upper bar."@en ;
        rdfs:label    "YDirectionUpperBarCount"@en .

PSD:KeyDepth  a       rdf:Property ;
        rdfs:comment  "Key depth of the profile."@en ;
        rdfs:label    "KeyDepth"@en .

PSD:SkillLevel  a     rdf:Property ;
        rdfs:comment  "Skill level exhibited by the actor and which indicates an extent of their capability to perform actions on the artefacts upon which they can act."@en ;
        rdfs:label    "Skill level"@en .

PSD:Exclusions  a     rdf:Property ;
        rdfs:comment  "Items, conditions or actions that may be excluded from the warranty or that may cause the warranty to become void."@en ;
        rdfs:label    "Exclusions"@en .

PSD:IsothermalMoistureCapacity
        a             rdf:Property ;
        rdfs:comment  "Based on water vapor density."@en ;
        rdfs:label    "IsothermalMoistureCapacity"@en .

PSD:FireResistanceRating
        a             rdf:Property ;
        rdfs:comment  "Measure of the fire resistance rating in hours (e.g., 1.5 hours, 2 hours, etc.)."@en ;
        rdfs:label    "FireResistanceRating"@en .

PSD:CoreTopWidth  a   rdf:Property ;
        rdfs:comment  "Core top width of the profile."@en ;
        rdfs:label    "CoreTopWidth"@en .

PSD:BoreSize  a       rdf:Property ;
        rdfs:comment  "The nominal bore of the pipe flange."@en ;
        rdfs:label    "BoreSize"@en .

PSD:IsUsed  a         rdf:Property ;
        rdfs:comment  "Indicates whether the element is being used in a workstation (= TRUE) or not.(= FALSE)."@en ;
        rdfs:label    "IsUsed"@en .

PSD:InteriorHeatTransferCoefficient
        a             rdf:Property ;
        rdfs:comment  "Interior heat transfer coefficient associated with interior surface area."@en ;
        rdfs:label    "InteriorHeatTransferCoefficient"@en .

PSD:Performance  a    rdf:Property ;
        rdfs:comment  "Water temperature change as a function of wet-bulb temperature, water entering temperature, water flow rate, air flow rate, Tdiff = f ( Twet-bulb, Twater,in, mwater, mair)."@en ;
        rdfs:label    "Performance"@en .

PSD:TotalCoolingCapacity
        a             rdf:Property ;
        rdfs:comment  "Total cooling capacity. This includes cooling capacity of beam and cooling capacity of supply air."@en ;
        rdfs:label    "TotalCoolingCapacity"@en .

PSD:AdjustmentRange  a  rdf:Property ;
        rdfs:comment  "Upper and lower current adjustment limits for an AdjustmentValueType = RANGE. Note that this property should not have a value for an  AdjustmentValueType = LIST."@en , "Upper and lower time adjustment limits for an AdjustmentValueType = RANGE. Note that this property should not have a value for an  AdjustmentValueType = LIST."@en ;
        rdfs:label    "AdjustmentRange"@en .

PSD:System  a         rdf:Property ;
        rdfs:comment  "he building service system that requires the provision for voids, e.g. 'Air Conditioning', 'Plumbing', 'Electro', etc."@en ;
        rdfs:label    "System"@en .

PSD:RateOfTemperatureRise
        a             rdf:Property ;
        rdfs:comment  "The rate of temperature rise that is to be sensed as being hazardous."@en ;
        rdfs:label    "RateOfTemperatureRise"@en .

PSD:UAcurves  a       rdf:Property ;
        rdfs:comment  "UV = f (VExterior, VInterior), UV as a function of interior and exterior fluid flow velocity at the entrance."@en ;
        rdfs:label    "UAcurves"@en .

PSD:UpperVaporResistanceFactor
        a             rdf:Property ;
        rdfs:comment  "The vapor permeability relationship of air/material (typically value > 1), measured in high relative humidity (typically in 95/50 % RH)."@en ;
        rdfs:label    "UpperVaporResistanceFactor"@en .

PSD:SpeakerDriverSize
        a             rdf:Property ;
        rdfs:comment  "Indicates the number of drivers and their sizes."@en ;
        rdfs:label    "SpeakerDriverSize"@en .

PSD:AirSideSystemType
        a             rdf:Property ;
        rdfs:comment  "This enumeration specifies the basic types of possible air side systems (e.g., Constant Volume, Variable Volume, etc.)."@en ;
        rdfs:label    "Air side system type"@en .

PSD:InternalControl  a  rdf:Property ;
        rdfs:comment  "Internal modulation control."@en ;
        rdfs:label    "Internal control"@en .

PSD:TemperatureSensorType
        a             rdf:Property ;
        rdfs:comment  "Enumeration that Identifies the types of temperature sensor that can be specified."@en ;
        rdfs:label    "TemperatureSensorType"@en .

PSD:DurabilityRating  a  rdf:Property ;
        rdfs:label  "Durability rating"@en .

PSD:AudioAmplification
        a             rdf:Property ;
        rdfs:comment  "Indicates audio amplification frequency ranges."@en ;
        rdfs:label    "AudioAmplification"@en .

PSD:WarrantyIdentifier
        a             rdf:Property ;
        rdfs:comment  "The identifier assigned to a warranty."@en ;
        rdfs:label    "WarrantyIdentifier"@en .

PSD:SupportDuringTransportDescription
        a           rdf:Property ;
        rdfs:label  "Support during transport description"@en .

PSD:TypePropertyListValue
        a                 owl:Class ;
        rdfs:label        "Type property list value"@en ;
        rdfs:subClassOf   PSD:PropertyType ;
        rdfs:subClassOf   [ a                   owl:Restriction ;
                            owl:minCardinality  "0"^^xsd:nonNegativeInteger ;
                            owl:onProperty      PSD:valueItem
                          ] ;
        rdfs:subClassOf   [ a                   owl:Restriction ;
                            owl:maxCardinality  "1"^^xsd:nonNegativeInteger ;
                            owl:onProperty      PSD:unitType
                          ] ;
        rdfs:subClassOf   [ a                owl:Restriction ;
                            owl:cardinality  "1"^^xsd:nonNegativeInteger ;
                            owl:onProperty   PSD:dataType
                          ] ;
        owl:disjointWith  PSD:TypeComplexProperty , PSD:TypePropertyTableValue , PSD:TypePropertySingleValue , PSD:TypePropertyEnumeratedValue , PSD:TypePropertyBoundedValue , PSD:TypePropertyReferenceValue .

PSD:TransportationStrength
        a           rdf:Property ;
        rdfs:label  "Transportation strength"@en .

PSD:ConnectionSize  a  rdf:Property ;
        rdfs:comment  "The connection size of the to and from the pump."@en , "Duct connection diameter."@en , "Size of the inlet connection to the sprinkler."@en , "Defines the size of inlet and outlet pipe connections to the meter."@en ;
        rdfs:label    "ConnectionSize"@en .

<>      a                owl:Ontology ;
        owl:imports      <IFC4> ;
        owl:versionInfo  "Created with TopBraid Composer" .

PSD:TouchScreen  a    rdf:Property ;
        rdfs:comment  "Indicates touchscreen support."@en ;
        rdfs:label    "TouchScreen"@en .

PSD:RatedVoltage  a   rdf:Property ;
        rdfs:comment  "The range of allowed voltage that a device is certified to handle. The upper bound of this value is the maximum."@en ;
        rdfs:label    "RatedVoltage"@en .

PSD:FlangeStandard  a  rdf:Property ;
        rdfs:comment  "Designation of the standard describing the flange table."@en ;
        rdfs:label    "FlangeStandard"@en .

PSD:StratosphericOzoneLayerDestructionPerUnit
        a           rdf:Property ;
        rdfs:label  "Stratospheric ozone layer destruction per unit"@en .

PSD:GasType  a        rdf:Property ;
        rdfs:comment  "Defines the types of gas that may be specified."@en ;
        rdfs:label    "GasType"@en .

PSD:InLineRowSpacing  a  rdf:Property ;
        rdfs:comment  "In-line tube row spacing."@en ;
        rdfs:label    "InLineRowSpacing"@en .

PSD:InletConnectionSize
        a             rdf:Property ;
        rdfs:comment  "Size of the inlet connection."@en , "Size of the inlet connection to the hose reel."@en ;
        rdfs:label    "InletConnectionSize"@en .

PSD:Thickness3  a     rdf:Property ;
        rdfs:comment  "Third thickness parameter of a surface member with varying thickness"@en ;
        rdfs:label    "Thickness3"@en .

PSD:NominalSurroundingHumidityCooling
        a             rdf:Property ;
        rdfs:comment  "Nominal surrounding humidity (refers to nominal cooling capacity)."@en ;
        rdfs:label    "NominalSurroundingHumidityCooling"@en .

PSD:IsBuiltIn  a      rdf:Property ;
        rdfs:comment  "Indicates whether the furniture type is intended to be 'built in' i.e. physically attached to a building or facility (= TRUE) or not i.e. Loose and movable (= FALSE)."@en ;
        rdfs:label    "Is built in"@en .

PSD:FlangeBaseFillet  a  rdf:Property ;
        rdfs:comment  "Flange base fillet of the profile."@en ;
        rdfs:label    "FlangeBaseFillet"@en .

PSD:MinimumPartLoadRatio
        a             rdf:Property ;
        rdfs:comment  "Minimum part load ratio as a fraction of nominal capacity."@en ;
        rdfs:label    "Minimum part load ratio"@en .

PSD:ReturnWaterTemperatureHeating
        a             rdf:Property ;
        rdfs:comment  "Return water temperature in heating mode."@en ;
        rdfs:label    "ReturnWaterTemperatureHeating"@en .

PSD:AdjustmentValues  a  rdf:Property ;
        rdfs:comment  "A list of current adjustment values that may be applied to a tripping unit for an AdjustmentValueType = LIST. A minimum of 1 and a maximum of 16 adjustment values may be specified. Note that this property should not have a value for an  AdjustmentValueType = RANGE."@en , "A list of time adjustment values that may be applied to a tripping unit for an AdjustmentValueType = LIST. A minimum of 1 and a maximum of 16 adjustment values may be specified. Note that this property should not have a value for an  AdjustmentValueType = RANGE."@en ;
        rdfs:label    "AdjustmentValues"@en .

PSD:SmokeStop  a    rdf:Property ;
        rdfs:label  "Smoke stop"@en .

PSD:People  a         rdf:Property ;
        rdfs:comment  "Heat gains and losses from people."@en ;
        rdfs:label    "People"@en .

PSD:SetPointRadioactivity
        a             rdf:Property ;
        rdfs:comment  "The radioactivity value to be sensed. Use IfcPropertyBoundedValue.SetPointValue to set the set point value."@en ;
        rdfs:label    "SetPointRadioactivity"@en .

PSD:DissolvedSolidsContent
        a             rdf:Property ;
        rdfs:comment  "Fraction of the dissolved solids to the total amount of water. This is measured in weight of dissolved solids per weight of water and is therefore unitless."@en ;
        rdfs:label    "DissolvedSolidsContent"@en .

PSD:FlangeDiameter  a  rdf:Property ;
        rdfs:comment  "Overall diameter of the flange."@en ;
        rdfs:label    "FlangeDiameter"@en .

PSD:LifeCyclePhase  a  rdf:Property ;
        rdfs:label  "Life cycle phase"@en .

PSD:ClearWidth  a     rdf:Property ;
        rdfs:comment  "Actual clear width measured as the clear space for accessibility and egress; it is a measured distance betwen the two handrails or the wall and a handrail on a ramp.\\nThe shape information is provided in addition to the shape representation and the geometric parameters used within. In cases of inconsistency between the geometric parameters and the shape properties, provided in the attached property, the geometric parameters take precedence."@en ;
        rdfs:label    "Clear width"@en .

PSD:ContrastRatio  a  rdf:Property ;
        rdfs:comment  "Indicates the display contrast ratio."@en ;
        rdfs:label    "ContrastRatio"@en .

PSD:ExhaustAir  a     rdf:Property ;
        rdfs:comment  "Loads from exhaust air."@en ;
        rdfs:label    "ExhaustAir"@en .

PSD:NominalParticleGeometricMeanDiameter
        a             rdf:Property ;
        rdfs:comment  "Particle geometric mean diameter associated with nominal efficiency."@en ;
        rdfs:label    "Nominal particle geometric mean diameter"@en .

PSD:LightingLoadIntensity
        a             rdf:Property ;
        rdfs:comment  "Average lighting load intensity in the space per unit area (PowerMeasure/IfcAreaMeasure)."@en ;
        rdfs:label    "LightingLoadIntensity"@en .

PSD:PressureDrop  a   rdf:Property ;
        rdfs:comment  "Pressure drop."@en , "Drop in total pressure between inlet and outlet at nominal air-flow rate."@en ;
        rdfs:label    "PressureDrop"@en .

PSD:OperatingMode  a  rdf:Property ;
        rdfs:comment  "Identifies the operating mode of the boiler."@en ;
        rdfs:label    "Operating mode"@en .

PSD:Layers  a         rdf:Property ;
        rdfs:comment  "Number of layers."@en ;
        rdfs:label    "Layers"@en .

PSD:c   a             rdf:Property ;
        rdfs:comment  "Measure c according to ISO 2553"@en ;
        rdfs:label    "c"@en .

PSD:ExhaustAirFlowRate
        a             rdf:Property ;
        rdfs:comment  "Exhaust air flow rate in the space."@en ;
        rdfs:label    "ExhaustAirFlowRate"@en .

PSD:PortNumber  a     rdf:Property ;
        rdfs:comment  "The port index for logically ordering the port within the containing element or element type."@en ;
        rdfs:label    "PortNumber"@en .

PSD:Application  a    rdf:Property ;
        rdfs:comment  "Indicates application of actuator or humidifier application.\\n\\nFixed: Humidifier installed in a ducted flow distribution system.\\nPortable: Humidifier is not installed in a ducted flow distribution system."@en , "The application of the unitary control element."@en ;
        rdfs:label    "Application"@en .

PSD:MaximumWorkingPressure
        a             rdf:Property ;
        rdfs:comment  "Maximum working pressure."@en , "Maximum pressure that the object is manufactured to withstand."@en ;
        rdfs:label    "MaximumWorkingPressure"@en .

PSD:FrameDepth  a     rdf:Property ;
        rdfs:comment  "The length (or depth) of the damper frame."@en ;
        rdfs:label    "FrameDepth"@en .

PSD:RecirculatedAir  a  rdf:Property ;
        rdfs:comment  "Loads from recirculated air."@en ;
        rdfs:label    "RecirculatedAir"@en .

PSD:MaximumOutletPressure
        a             rdf:Property ;
        rdfs:comment  "Maximum steam outlet pressure."@en ;
        rdfs:label    "MaximumOutletPressure"@en .

PSD:ColumnShoeCasingWidth
        a             rdf:Property ;
        rdfs:comment  "The width of the column shoe casing."@en ;
        rdfs:label    "ColumnShoeCasingWidth"@en .

PSD:CoverWidth  a     rdf:Property ;
        rdfs:comment  "The length measured along the y-axis in the local coordinate system of the cover of the  drain."@en , "The length measured along the x-axis in the local coordinate system of the cover of the oil interceptor."@en , "The length measured along the y-axis in the local coordinate system of the cover of the  waste."@en ;
        rdfs:label    "CoverWidth"@en .

PSD:HeatingWetBulb  a  rdf:Property ;
        rdfs:comment  "Outside wet bulb temperature for heating design."@en ;
        rdfs:label    "HeatingWetBulb"@en .

PSD:Duration  a       rdf:Property ;
        rdfs:comment  "The period of time for the lease."@en ;
        rdfs:label    "Duration"@en .

PSD:VentilationIndoorAir
        a             rdf:Property ;
        rdfs:comment  "Ventilation loads from indoor air."@en ;
        rdfs:label    "VentilationIndoorAir"@en .

PSD:WaterContent  a   rdf:Property ;
        rdfs:comment  "Weight of water content within the heater."@en ;
        rdfs:label    "WaterContent"@en .

PSD:Intermittent  a   rdf:Property ;
        rdfs:comment  "If fillet weld, intermittent or not"@en ;
        rdfs:label    "Intermittent"@en .

PSD:EquipmentSensible
        a             rdf:Property ;
        rdfs:comment  "Heat gains and losses from equipment."@en ;
        rdfs:label    "EquipmentSensible"@en .

PSD:SolarReflectance  a  rdf:Property ;
        rdfs:label  "Solar reflectance"@en .

PSD:SetPointRadiation
        a             rdf:Property ;
        rdfs:comment  "The radiation power value to be sensed. Use IfcPropertyBoundedValue.SetPointValue to set the set point value."@en ;
        rdfs:label    "SetPointRadiation"@en .

PSD:Length  a         rdf:Property ;
        rdfs:comment  "Length of the fin as measured parallel to the direction of airflow."@en , "The finished length of the silencer."@en , "The length of the sump."@en , "The length of the pit."@en , "Length of the tubes in the tube bundle."@en ;
        rdfs:label    "Length"@en .

PSD:RequestComments  a  rdf:Property ;
        rdfs:comment  "Comments that may be made on the request."@en ;
        rdfs:label    "Request comments"@en .

PSD:HasProtectiveEarth
        a             rdf:Property ;
        rdfs:comment  "One core has protective earth marked insulation, Yellow/Green."@en ;
        rdfs:label    "HasProtectiveEarth"@en .

PSD:TypePropertyTableValue
        a                 owl:Class ;
        rdfs:label        "Type property table value"@en ;
        rdfs:subClassOf   PSD:PropertyType ;
        rdfs:subClassOf   [ a                owl:Restriction ;
                            owl:cardinality  "1"^^xsd:nonNegativeInteger ;
                            owl:onProperty   PSD:definingValue
                          ] ;
        rdfs:subClassOf   [ a                owl:Restriction ;
                            owl:cardinality  "1"^^xsd:nonNegativeInteger ;
                            owl:onProperty   PSD:definedValue
                          ] ;
        owl:disjointWith  PSD:TypePropertySingleValue , PSD:TypePropertyListValue , PSD:TypeComplexProperty , PSD:TypePropertyBoundedValue , PSD:TypePropertyReferenceValue , PSD:TypePropertyEnumeratedValue .

PSD:ShortInsideCenterLowerBarPitch
        a             rdf:Property ;
        rdfs:comment  "The pitch length of the short inside center lower bar."@en ;
        rdfs:label    "ShortInsideCenterLowerBarPitch"@en .

PSD:FlowRating  a     rdf:Property ;
        rdfs:comment  "Actual flow capacity for the gutter. Value of 0.00 means this value has not been set."@en ;
        rdfs:label    "FlowRating"@en .

PSD:HorizontalSpacing
        a             rdf:Property ;
        rdfs:comment  "Horizontal spacing between tubes in the tube bundle."@en ;
        rdfs:label    "HorizontalSpacing"@en .

PSD:lowerBoundValue  a  owl:FunctionalProperty , owl:DatatypeProperty ;
        rdfs:domain  PSD:TypePropertyBoundedValue ;
        rdfs:label   "Lower bound value"@en ;
        rdfs:range   xsd:string .

PSD:BoltholePitch  a  rdf:Property ;
        rdfs:comment  "Diameter of the circle along which the boltholes are placed."@en ;
        rdfs:label    "BoltholePitch"@en .

PSD:ClassificationAuthority
        a             rdf:Property ;
        rdfs:comment  "The name of the authority that applies the classification of service to the hose reel (e.g. NFPA/FEMA)."@en ;
        rdfs:label    "ClassificationAuthority"@en .

PSD:AssetAccountingType
        a             rdf:Property ;
        rdfs:comment  "Identifies the predefined types of risk from which the type required may be set."@en ;
        rdfs:label    "Asset accounting type"@en .

PSD:FluidFlowLeakage  a  rdf:Property ;
        rdfs:comment  "Volumetric leakage flow rate."@en ;
        rdfs:label    "FluidFlowLeakage"@en .

PSD:FusibleLinkTemperature
        a             rdf:Property ;
        rdfs:comment  "The temperature that the fusible link melts."@en ;
        rdfs:label    "FusibleLinkTemperature"@en .

PSD:NominalFilterFaceVelocity
        a             rdf:Property ;
        rdfs:comment  "Filter face velocity."@en ;
        rdfs:label    "Nominal filter face velocity"@en .

PSD:CondensingTemperature
        a             rdf:Property ;
        rdfs:comment  "Refrigerant condensing temperature."@en ;
        rdfs:label    "CondensingTemperature"@en .

PSD:NominalCoolingCapacity
        a             rdf:Property ;
        rdfs:comment  "Nominal cooling capacity."@en ;
        rdfs:label    "NominalCoolingCapacity"@en .

PSD:NonRenewableEnergyConsumption
        a           rdf:Property ;
        rdfs:label  "Non renewable energy consumption"@en .

PSD:OutdoorEnvironment
        a             rdf:Property ;
        rdfs:comment  "Adjustment of the service life resulting from the effect of the outdoor environment (where appropriate)"@en ;
        rdfs:label    "OutdoorEnvironment"@en .

PSD:TunerMode  a      rdf:Property ;
        rdfs:comment  "Indicates the tuner modes (or bands).  For example, 'AnalogCable', 'DigitalAir', 'AM', 'FM'."@en ;
        rdfs:label    "TunerMode"@en .

PSD:SiteCoverageRatio
        a             rdf:Property ;
        rdfs:comment  "The ratio of the utilization,  TotalArea / BuildableArea, expressed as a maximum value. The ratio value may be used to derive BuildableArea."@en ;
        rdfs:label    "SiteCoverageRatio"@en .

PSD:EnergyGainSensible
        a             rdf:Property ;
        rdfs:comment  "The sum of total energy gains for the spaces served by the system during the peak cooling conditions, plus any system-level sensible energy gains."@en ;
        rdfs:label    "Energy gain sensible"@en .

PSD:NominalDiameterOrWidth
        a             rdf:Property ;
        rdfs:comment  "The nominal diameter or width of the duct segment."@en ;
        rdfs:label    "NominalDiameterOrWidth"@en .

PSD:AirflowType  a    rdf:Property ;
        rdfs:comment  "Enumeration defining the functional type of air flow through the terminal."@en ;
        rdfs:label    "AirflowType"@en .

PSD:LoadSafetyFactor  a  rdf:Property ;
        rdfs:comment  "Load safety factor."@en ;
        rdfs:label    "LoadSafetyFactor"@en , "Load safety factor"@en .

PSD:HasOpening  a     rdf:Property ;
        rdfs:comment  "indicates whether the panel has an opening (= TRUE) or not (= FALSE)."@en ;
        rdfs:label    "HasOpening"@en .

PSD:FrameSize  a      rdf:Property ;
        rdfs:comment  "Designation of the frame size according to the named range of frame sizes designated at the place of use or according to a given standard."@en ;
        rdfs:label    "FrameSize"@en .

PSD:HumidityEffectiveness
        a             rdf:Property ;
        rdfs:comment  "Humidity heat transfer effectiveness: The ratio of primary airflow absolute humidity changes to maximum possible absolute humidity changes."@en ;
        rdfs:label    "HumidityEffectiveness"@en .

PSD:CompressorCapacity
        a             rdf:Property ;
        rdfs:comment  "The product of the  ideal capacity and the overall volumetric efficiency of the compressor."@en ;
        rdfs:label    "CompressorCapacity"@en .

PSD:Addressablility  a  rdf:Property ;
        rdfs:comment  "The type of addressability."@en ;
        rdfs:label    "Addressablility"@en .

PSD:GlassColor  a   rdf:Property ;
        rdfs:label  "Glass color"@en .

PSD:schema  a         owl:FunctionalProperty , owl:DatatypeProperty ;
        rdfs:comment  "Sub schema name, i.e., \"IfcSharedBldgElements\"."@en ;
        rdfs:domain   PSD:IfcVersion ;
        rdfs:label    "Schema"@en ;
        rdfs:range    xsd:string .

PSD:GlazingAreaFraction
        a           rdf:Property ;
        rdfs:label  "Glazing area fraction"@en .

PSD:AppearanceGrade  a  rdf:Property ;
        rdfs:comment  "Grade with respect to visual quality."@en ;
        rdfs:label    "AppearanceGrade"@en .

PSD:PictogramEscapeDirection
        a             rdf:Property ;
        rdfs:comment  "The direction of escape pictogram."@en ;
        rdfs:label    "PictogramEscapeDirection"@en .

PSD:ShapeDescription  a  rdf:Property ;
        rdfs:comment  "A description of the shape of the work surface e.g. corner square, rectangle, etc."@en ;
        rdfs:label    "ShapeDescription"@en .

PSD:NumberOfParallelCircuits
        a             rdf:Property ;
        rdfs:comment  "Number of parallel circuits."@en ;
        rdfs:label    "NumberOfParallelCircuits"@en .

PSD:ReleaseCurrent  a  rdf:Property ;
        rdfs:comment  "The release current in [x In] for the initial tripping of the S-function."@en ;
        rdfs:label    "ReleaseCurrent"@en .

PSD:EvaporatorMediumType
        a             rdf:Property ;
        rdfs:comment  "ColdLiquid: Evaporator is using liquid type of fluid to exchange heat with refrigerant.\\nColdAir: Evaporator is using air to exchange heat with refrigerant."@en ;
        rdfs:label    "Evaporator medium type"@en .

PSD:CoverageArea  a   rdf:Property ;
        rdfs:comment  "The floor area that is covered by the sensor (typically measured as a circle whose center is at the location of the sensor)."@en , "The area that the sprinkler is designed to protect."@en , "The area that is covered by the sensor (typically measured as a circle whose center is at the location of the sensor)."@en ;
        rdfs:label    "CoverageArea"@en .

PSD:SetPointContact  a  rdf:Property ;
        rdfs:comment  "The contact value to be sensed. Use IfcPropertyBoundedValue.SetPointValue to set the set point value."@en ;
        rdfs:label    "SetPointContact"@en .

PSD:Enabled  a        rdf:Property ;
        rdfs:comment  "Indicates whether alarm is enabled or disabled over time."@en ;
        rdfs:label    "Enabled"@en .

PSD:HasTurbulator  a  rdf:Property ;
        rdfs:comment  "TRUE if the tube has a turbulator, FALSE if it does not."@en ;
        rdfs:label    "HasTurbulator"@en .

PSD:PressureRegulatorSetting
        a             rdf:Property ;
        rdfs:comment  "Pressure that is automatically maintained in the tank."@en ;
        rdfs:label    "PressureRegulatorSetting"@en .

PSD:AcousticRating  a  rdf:Property ;
        rdfs:label  "Acoustic rating"@en .

PSD:CurrentCarryingCapasity
        a             rdf:Property ;
        rdfs:comment  "Maximum value of electric current which can be carried continuously by a conductor, a device or an apparatus, under specified conditions without its steady-state temperature exceeding a  specified value. Based on IEC60826-11-13. NOTE: The temperature specified value is maximum Design Ambient Temperature."@en ;
        rdfs:label    "CurrentCarryingCapasity"@en .

PSD:InfiltrationSensible
        a             rdf:Property ;
        rdfs:comment  "Heat gains and losses from infiltration."@en ;
        rdfs:label    "InfiltrationSensible"@en .

PSD:MinimumAllowableSupportLength
        a           rdf:Property ;
        rdfs:label  "Minimum allowable support length"@en .

PSD:BladeThickness  a  rdf:Property ;
        rdfs:comment  "The thickness of the damper blade."@en ;
        rdfs:label    "BladeThickness"@en .

PSD:ArrangementType  a  rdf:Property ;
        rdfs:comment  "Terminal box arrangement.\\nSingleDuct: Terminal box receives warm or cold air from a single air supply duct.\\nDualDuct: Terminal box receives warm and cold air from separate air supply ducts."@en ;
        rdfs:label    "Arrangement type"@en .

PSD:UpperCurrent1  a  rdf:Property ;
        rdfs:comment  "The current in [x In], indicating that for currents larger than UpperCurrent1 the I2t part of the L-function will trip the current."@en ;
        rdfs:label    "UpperCurrent1"@en .

PSD:CornerFixingPlateThickness
        a             rdf:Property ;
        rdfs:comment  "The thickness of the L-shaped corner plate."@en ;
        rdfs:label    "CornerFixingPlateThickness"@en .

PSD:OutletTemperatureRange
        a             rdf:Property ;
        rdfs:comment  "Allowable outlet temperature of either the water or the steam."@en ;
        rdfs:label    "Outlet temperature range"@en .

PSD:FixingSocketThreadLength
        a             rdf:Property ;
        rdfs:comment  "The length of the threaded part of the fixing socket."@en ;
        rdfs:label    "FixingSocketThreadLength"@en .

PSD:SelfExtinguishing60332_3
        a             rdf:Property ;
        rdfs:comment  "Self Extinguishing cable/core according to IEC 60332.3."@en ;
        rdfs:label    "SelfExtinguishing60332_3"@en .

PSD:VideoResolutionWidth
        a             rdf:Property ;
        rdfs:comment  "Indicates the number of horizontal pixels, e.g. 1920."@en , "Indicates the number of horizontal pixels (the largest native video resolution width)."@en ;
        rdfs:label    "VideoResolutionWidth"@en .

PSD:ElectricCookerType
        a             rdf:Property ;
        rdfs:comment  "Type of electric cooker."@en ;
        rdfs:label    "ElectricCookerType"@en .

PSD:LadderTrussSecondaryBarDiameter
        a             rdf:Property ;
        rdfs:comment  "The nominal diameter of the secondary bar."@en ;
        rdfs:label    "LadderTrussSecondaryBarDiameter"@en .

PSD:AirFlowrateVersusFlowControlElement
        a             rdf:Property ;
        rdfs:comment  "Air flowrate versus flow control element position at nominal pressure drop."@en ;
        rdfs:label    "Air flowrate versus flow control element"@en .

PSD:FinalResistance  a  rdf:Property ;
        rdfs:comment  "Filter fluid resistance when replacement is required (i.e., Pressure drop at the maximum air flowrate across the filter when the filter needs replacement per ASHRAE Standard 52.1)."@en ;
        rdfs:label    "Final resistance"@en .

PSD:BuildingHeightLimit
        a             rdf:Property ;
        rdfs:comment  "Allowed maximum height of buildings on this site - according to local building codes."@en ;
        rdfs:label    "Building height limit"@en .

PSD:CenterCoreSpacing
        a             rdf:Property ;
        rdfs:comment  "Center core spacing of the profile."@en ;
        rdfs:label    "CenterCoreSpacing"@en .

PSD:NumberOfDrafts  a  rdf:Property ;
        rdfs:label  "Number of drafts"@en .

PSD:CoolingWaterFlowRate
        a             rdf:Property ;
        rdfs:comment  "Water flow rate for cooling."@en ;
        rdfs:label    "CoolingWaterFlowRate"@en .

PSD:FixingSocketThreadDiameter
        a             rdf:Property ;
        rdfs:comment  "The nominal diameter of the thread."@en ;
        rdfs:label    "FixingSocketThreadDiameter"@en .

PSD:InternalSurfaceArea
        a             rdf:Property ;
        rdfs:comment  "Internal surface area."@en ;
        rdfs:label    "Internal surface area"@en .

PSD:CloggingIndicator
        a             rdf:Property ;
        rdfs:comment  "Whether the filter has an indicator to display the degree of clogging of the filter."@en ;
        rdfs:label    "CloggingIndicator"@en .

PSD:RiserHeight  a  rdf:Property ;
        rdfs:label  "Riser height"@en .

PSD:ContractualType  a  rdf:Property ;
        rdfs:comment  "The contractual type of the work."@en ;
        rdfs:label    "ContractualType"@en .

PSD:CenterCoreMiddleHeight
        a             rdf:Property ;
        rdfs:comment  "Center core middle height of the profile."@en ;
        rdfs:label    "CenterCoreMiddleHeight"@en .

PSD:WaterPressureRange
        a             rdf:Property ;
        rdfs:comment  "Allowable water circuit working pressure range."@en ;
        rdfs:label    "WaterPressureRange"@en .

PSD:propertyType  a  owl:ObjectProperty , owl:FunctionalProperty ;
        rdfs:domain  PSD:PropertyDef ;
        rdfs:label   "Property type"@en ;
        rdfs:range   PSD:PropertyType .

PSD:ElectricGeneratorEfficiency
        a             rdf:Property ;
        rdfs:comment  "The ratio of output capacity to intake capacity."@en ;
        rdfs:label    "ElectricGeneratorEfficiency"@en .

PSD:WorkTypeRequested
        a             rdf:Property ;
        rdfs:comment  "Work type requested in circumstances where there are categorizations of types of work task. It could be used to identify a remedial task, minor work task, electrical task etc."@en ;
        rdfs:label    "WorkTypeRequested"@en .

PSD:InPlane  a        rdf:Property ;
        rdfs:comment  "Mechanical properties with respect to in-plane load, i.e. for function as a membrane."@en , "Mechanical properties with respect to in-plane load, i.e. bending about the strong axis; tension zone of unbalanced layups is stressed in tension."@en ;
        rdfs:label    "InPlane"@en .

PSD:NominalToppingThickness
        a           rdf:Property ;
        rdfs:label  "Nominal topping thickness"@en .

PSD:HydraulicDiameter
        a             rdf:Property ;
        rdfs:comment  "Hydraulic diameter."@en ;
        rdfs:label    "HydraulicDiameter"@en .

PSD:AirDiffusionPerformanceIndex
        a             rdf:Property ;
        rdfs:comment  "The Air Diffusion Performance Index (ADPI) is used for cooling mode conditions. If several measurements of air velocity and air temperature are made throughout the occupied zone of a space, the ADPI is the percentage of locations where measurements were taken that meet the specifications for effective draft temperature and air velocity."@en ;
        rdfs:label    "Air diffusion performance index"@en .

PSD:WeatherDataStation
        a             rdf:Property ;
        rdfs:comment  "The site weather data station description or reference to the data source from which weather data was obtained for use in calculations."@en ;
        rdfs:label    "WeatherDataStation"@en .

PSD:OutletConnectionSize
        a             rdf:Property ;
        rdfs:comment  "The size of the pipework connection from the mixing valve."@en , "Size of the outlet connection."@en , "Size of the outlet connection from the object."@en , "Size of the outlet connection from the waste disposal unit."@en ;
        rdfs:label    "OutletConnectionSize"@en .

PSD:ReinforcementVolumeRatio
        a           rdf:Property ;
        rdfs:label  "Reinforcement volume ratio"@en .

PSD:IsOutlookDesirable
        a             rdf:Property ;
        rdfs:comment  "An indication of whether the outlook is desirable (set TRUE) or not (set FALSE)"@en ;
        rdfs:label    "IsOutlookDesirable"@en .

PSD:ShortCircuit1PolePowerFactorMinimumState
        a             rdf:Property ;
        rdfs:comment  "Power factor of the minimum 1 pole short circuit current provided at the point of supply i.e. the fault between 1 phase and N."@en ;
        rdfs:label    "ShortCircuit1PolePowerFactorMinimumState"@en .

PSD:Purpose  a        rdf:Property ;
        rdfs:comment  "Enumeration defining the purpose of the flow meter occurrence."@en ;
        rdfs:label    "Purpose"@en .

PSD:Power  a          rdf:Property ;
        rdfs:comment  "The actual power consumption of the pump."@en ;
        rdfs:label    "Power"@en .

PSD:LightingDiversity
        a             rdf:Property ;
        rdfs:comment  "Lighting diversity."@en ;
        rdfs:label    "LightingDiversity"@en , "Lighting diversity"@en .

PSD:ConcreteCoverAtMainBars
        a           rdf:Property ;
        rdfs:label  "Concrete cover at main bars"@en .

PSD:VisibleLightTransmittance
        a           rdf:Property ;
        rdfs:label  "Visible light transmittance"@en .

PSD:LongInsideCenterTopBarPitch
        a             rdf:Property ;
        rdfs:comment  "The pitch length of the long inside center top bar."@en ;
        rdfs:label    "LongInsideCenterTopBarPitch"@en .

PSD:IdealCapacity  a  rdf:Property ;
        rdfs:comment  "Compressor capacity under ideal conditions."@en ;
        rdfs:label    "Ideal capacity"@en .

PSD:ThreadDiameter  a  rdf:Property ;
        rdfs:comment  "Nominal diameter of the thread, if different from the bolt's overall nominal diameter"@en ;
        rdfs:label    "ThreadDiameter"@en .

PSD:FixingSocketHeight
        a             rdf:Property ;
        rdfs:comment  "The overall height of the fixing socket."@en ;
        rdfs:label    "FixingSocketHeight"@en .

PSD:FunctionReliable  a  rdf:Property ;
        rdfs:comment  "Cable/bus maintain given properties/functions over a given (tested) time and conditions. According to IEC standard."@en , "Core maintain given properties/functions over a given (tested) time and conditions. According to (IEC) standard."@en ;
        rdfs:label    "FunctionReliable"@en .

PSD:InUseConditions  a  rdf:Property ;
        rdfs:comment  "Adjustment of the service life resulting from the effect of the conditions in which components are operating."@en ;
        rdfs:label    "InUseConditions"@en .

PSD:NetPlannedArea  a  rdf:Property ;
        rdfs:label  "Net planned area"@en .

PSD:PressureLossCoefficient
        a             rdf:Property ;
        rdfs:comment  "Pressure loss coefficient."@en ;
        rdfs:label    "PressureLossCoefficient"@en .

PSD:OutOfPlane  a     rdf:Property ;
        rdfs:comment  "Mechanical properties with respect to out-of-plane load, i.e. for function as a plate; tension zone of unbalanced layups is stressed in tension."@en , "Mechanical properties with respect to out-of-plane load, i.e. bending about the weak axis."@en ;
        rdfs:label    "OutOfPlane"@en .

PSD:EnergyEfficiencyRatio
        a             rdf:Property ;
        rdfs:comment  "Energy efficiency ratio (EER)."@en ;
        rdfs:label    "EnergyEfficiencyRatio"@en .

PSD:ColumnShoeBasePlateThickness
        a             rdf:Property ;
        rdfs:comment  "The thickness of the column shoe base plate."@en ;
        rdfs:label    "ColumnShoeBasePlateThickness"@en .

PSD:HeatOutput  a     rdf:Property ;
        rdfs:comment  "Total nominal heat output as listed by the Boiler manufacturer. For steam boilers, it is a function of inlet temperature versus steam pressure.  Note: as two variables are used, DefiningValues and DefinedValues are null, and values are stored in IfcTable in the following order: InletTemperature(IfcThermodynamicTemperatureMeasure) and OutletTemperature(IfcThermodynamicTemperatureMeasure) in DefiningValues, and HeatOutput(IfcEnergyMeasure) in DefinedValues. For example, DefiningValues(InletTemp, OutletTemp), DefinedValues(null, HeatOutput). The IfcTable is related to IfcPropertyTableValue using IfcMetric and IfcPropertyConstraintRelationship."@en , "Total nominal heat output as listed by the Boiler manufacturer. For water boilers, it is a function of inlet versus outlet temperature. For steam boilers, it is a function of inlet temperature versus steam pressure.  Note: as two variables are used, DefiningValues and DefinedValues are null, and values are stored in IfcTable in the following order: InletTemperature(IfcThermodynamicTemperatureMeasure), OutletTemperature(IfcThermodynamicTemperatureMeasure), HeatOutput(IfcEnergyMeasure).  The IfcTable is related to IfcPropertyTableValue using IfcMetric and IfcPropertyConstraintRelationship."@en ;
        rdfs:label    "HeatOutput"@en .

PSD:BatterAtStart  a  rdf:Property ;
        rdfs:label  "Batter at start"@en .

PSD:HeatingEfficiency
        a             rdf:Property ;
        rdfs:comment  "Heating efficiency under full load heating conditions."@en ;
        rdfs:label    "HeatingEfficiency"@en .

PSD:HoseReelType  a   rdf:Property ;
        rdfs:comment  "Identifies the predefined types of hose arrangement from which the type required may be set."@en ;
        rdfs:label    "HoseReelType"@en .

PSD:RefrigerantClass  a  rdf:Property ;
        rdfs:comment  "Refrigerant class used by the compressor/condenser.\\n\\nCFC: Chlorofluorocarbons.\\nHCFC: Hydrochlorofluorocarbons.\\nHFC: Hydrofluorocarbons."@en ;
        rdfs:label    "Refrigerant class"@en .

PSD:HasSoundAttenuation
        a             rdf:Property ;
        rdfs:comment  "TRUE if the coil has sound attenuation, FALSE if it does not."@en ;
        rdfs:label    "HasSoundAttenuation"@en .

PSD:EdgeFixingPlateThickness
        a             rdf:Property ;
        rdfs:comment  "The thickness of the L-shaped edge plate."@en ;
        rdfs:label    "EdgeFixingPlateThickness"@en .

PSD:AccuracyQualityExpected
        a             rdf:Property ;
        rdfs:comment  "A measure of the accuracy quality of survey points as expected expressed in percentage terms."@en ;
        rdfs:label    "AccuracyQualityExpected"@en .

PSD:I5  a             rdf:Property ;
        rdfs:comment  "The upper electromagnetic testing current limit in [x In], indicating that for currents larger than I5, the tripping time shall be shorter than or equal to the associated tripping time, T5, i.e. the device shall trip instantaneous."@en ;
        rdfs:label    "I5"@en .

PSD:WireDiameter  a   rdf:Property ;
        rdfs:comment  "The nominal diameter of the wire."@en ;
        rdfs:label    "WireDiameter"@en .

PSD:CornerFixingPlateLength
        a             rdf:Property ;
        rdfs:comment  "The length of the L-shaped corner plate."@en ;
        rdfs:label    "CornerFixingPlateLength"@en .

PSD:AssemblyPlace  a  rdf:Property ;
        rdfs:comment  "Enumeration defining where the assembly is intended to take place, either in a factory or on the building site."@en , "Enumeration defining where the assembly is intended to take place, either in a factory, other offsite location or on the building site."@en ;
        rdfs:label    "AssemblyPlace"@en .

PSD:RightFlangeWidth  a  rdf:Property ;
        rdfs:comment  "Right flange width of the profile."@en ;
        rdfs:label    "RightFlangeWidth"@en .

PSD:MotorEnclosureType
        a             rdf:Property ;
        rdfs:comment  "A list of the available types of motor enclosure from which that required may be selected."@en ;
        rdfs:label    "MotorEnclosureType"@en .

PSD:DefrostTemperatureEffectiveness
        a             rdf:Property ;
        rdfs:comment  "Temperature heat transfer effectiveness when defrosting is active."@en ;
        rdfs:label    "DefrostTemperatureEffectiveness"@en .

PSD:LowerVaporResistanceFactor
        a             rdf:Property ;
        rdfs:comment  "The vapor permeability relationship of air/material (typically value > 1), measured in low relative humidity (typically in 0/50 % RH)."@en ;
        rdfs:label    "LowerVaporResistanceFactor"@en .

PSD:RadiatorType  a   rdf:Property ;
        rdfs:comment  "Indicates the type of radiator."@en ;
        rdfs:label    "RadiatorType"@en .

PSD:GlobalTradeItemNumber
        a             rdf:Property ;
        rdfs:comment  "The Global Trade Item Number (GTIN) is an identifier for trade items developed by GS1 (www.gs1.org)."@en ;
        rdfs:label    "GlobalTradeItemNumber"@en .

PSD:ColumnShoeBasePlateWidth
        a             rdf:Property ;
        rdfs:comment  "The width of the column shoe base plate."@en ;
        rdfs:label    "ColumnShoeBasePlateWidth"@en .

PSD:RangeAngle  a     rdf:Property ;
        rdfs:comment  "Indicates the maximum rotation the actuator must traverse."@en ;
        rdfs:label    "Range angle"@en .

PSD:CoolingWetBulb  a  rdf:Property ;
        rdfs:comment  "Outside wet bulb temperature for cooling design."@en ;
        rdfs:label    "CoolingWetBulb"@en .

PSD:OccupancyTimePerDay
        a             rdf:Property ;
        rdfs:comment  "The amount of time during the day that the activity is required within this space."@en ;
        rdfs:label    "OccupancyTimePerDay"@en .

PSD:IsentropicEfficiency
        a             rdf:Property ;
        rdfs:comment  "Ratio of the work required for isentropic compression of the gas to work input to the compressor shaft."@en ;
        rdfs:label    "IsentropicEfficiency"@en .

PSD:User  a           rdf:Property ;
        rdfs:comment  "Indicates acknowledging user over time by identification corresponding to IfcPerson.Identification on an IfcActor."@en ;
        rdfs:label    "User"@en .

PSD:OutsideAirPerPerson
        a             rdf:Property ;
        rdfs:comment  "Design quantity of outside air to be provided per person in the space."@en ;
        rdfs:label    "OutsideAirPerPerson"@en .

PSD:WaterSumpTemperature
        a             rdf:Property ;
        rdfs:comment  "Water sump temperature."@en ;
        rdfs:label    "WaterSumpTemperature"@en .

PSD:CenterlineAirVelocity
        a             rdf:Property ;
        rdfs:comment  "Centerline air velocity versus distance from the diffuser and temperature differential; a function of distance from diffuser and temperature difference between supply air and room air."@en ;
        rdfs:label    "CenterlineAirVelocity"@en .

PSD:RealPower  a      rdf:Property ;
        rdfs:comment  "Real power."@en ;
        rdfs:label    "RealPower"@en .

PSD:LeakageFullyClosed
        a             rdf:Property ;
        rdfs:comment  "Leakage when fully closed."@en ;
        rdfs:label    "LeakageFullyClosed"@en .

PSD:RequestSourceLabel
        a             rdf:Property ;
        rdfs:comment  "A specific name or label that further qualifies the identity of a request source. In the event of an email, this may be the email address."@en ;
        rdfs:label    "Resource source label"@en .

PSD:KeyOffset  a      rdf:Property ;
        rdfs:comment  "Key offset of the profile."@en ;
        rdfs:label    "KeyOffset"@en .

PSD:TotalSensibleLoad
        a             rdf:Property ;
        rdfs:comment  "Total energy added or removed from air that affects its temperature.  If a value is less than zero (negative), then the thermal load is lost from the space. If a value is greater than zero (positive), then the thermal load is a gain to the space."@en ;
        rdfs:label    "TotalSensibleLoad"@en .

PSD:Condition  a      rdf:Property ;
        rdfs:comment  "Indicates alarm condition over time.  The range of possible values and their meanings is defined by Pset_AlarmTypeCommon.Condition.  An empty value indicates no present alarm condition."@en ;
        rdfs:label    "Condition"@en .

PSD:ThermalTransmittanceSummer
        a           rdf:Property ;
        rdfs:label  "Thermal transmittance summer"@en .

PSD:HeatingWaterFlowRate
        a             rdf:Property ;
        rdfs:comment  "Water flow rate for heating."@en ;
        rdfs:label    "HeatingWaterFlowRate"@en .

PSD:IsSkilledOperator
        a             rdf:Property ;
        rdfs:comment  "Identifies if the current instance requires a skilled person or instructed person to perform operations on the distribution board (= TRUE) or whether operations may be performed by a person without appropriate skills or instruction (= FALSE)."@en ;
        rdfs:label    "IsSkilledOperator"@en .

PSD:BottomCover  a    rdf:Property ;
        rdfs:comment  "Bottom cover of the profile."@en ;
        rdfs:label    "BottomCover"@en .

PSD:MoistureCapacityThermalGradient
        a             rdf:Property ;
        rdfs:comment  "Thermal gradient coefficient for moisture capacity. Based on water vapor density."@en ;
        rdfs:label    "Moisture capacity thermal gradient"@en .

PSD:DistanceBetweenParallelCircuits
        a             rdf:Property ;
        rdfs:comment  "Distance measured between parallel circuits."@en ;
        rdfs:label    "DistanceBetweenParallelCircuits"@en .

PSD:StrengthClass  a  rdf:Property ;
        rdfs:label  "Strength class"@en .

PSD:EdgeDistanceToFirstAxis
        a           rdf:Property ;
        rdfs:label  "Edge distance to first axis"@en .

PSD:AirResistanceCurve
        a             rdf:Property ;
        rdfs:comment  "Air resistance curve (w/ fan only); Pressure = f ( flow rate)."@en ;
        rdfs:label    "AirResistanceCurve"@en .

PSD:TotalHeatingLoad  a  rdf:Property ;
        rdfs:comment  "The peak total heating load for the building, zone or space."@en ;
        rdfs:label    "TotalHeatingLoad"@en .

PSD:MarketSubCategoriesAvailableNow
        a             rdf:Property ;
        rdfs:comment  "A list of the sub categories of property that are currently available expressed in terms of IfcLabel."@en ;
        rdfs:label    "Market sub categories available now"@en .

PSD:NumberOfSockets  a  rdf:Property ;
        rdfs:comment  "The number of sockets that may be connected. In case of inconsistency, sockets defined on ports take precedence."@en ;
        rdfs:label    "Number of sockets"@en .

PSD:TotalPrimaryEnergyConsumptionPerUnit
        a           rdf:Property ;
        rdfs:label  "Total primary energy consumption per unit"@en .

PSD:CondenserLeavingTemperature
        a             rdf:Property ;
        rdfs:comment  "Termperature of fluid leaving condenser."@en ;
        rdfs:label    "CondenserLeavingTemperature"@en .

PSD:HasAntiStaticSurface
        a             rdf:Property ;
        rdfs:comment  "Indication whether the surface finish is designed to prevent electrostatic charge (TRUE) or not (FALSE)."@en ;
        rdfs:label    "HasAntiStaticSurface"@en .

PSD:InsideDiameter  a  rdf:Property ;
        rdfs:comment  "Actual inner diameter of the tube in the tube bundle."@en ;
        rdfs:label    "InsideDiameter"@en .

PSD:NominalDepth  a   rdf:Property ;
        rdfs:comment  "Nominal or quoted depth of the object. The size information is provided in addition to the shape representation and the geometric parameters used within. In cases of inconsistency between the geometric parameters and the size properties, provided in the attached property set, the geometric parameters take precedence."@en , "Nominal or quoted depth of the object measured from the inlet drain connection to the base of the unit."@en ;
        rdfs:label    "Nominal depth"@en , "NominalDepth"@en .

PSD:AspectRatio  a    rdf:Property ;
        rdfs:comment  "The default aspect ratio."@en ;
        rdfs:label    "AspectRatio"@en .

PSD:LadderTrussLength
        a             rdf:Property ;
        rdfs:comment  "The overall length of the truss connector."@en ;
        rdfs:label    "LadderTrussLength"@en .

PSD:ActivationTemperature
        a             rdf:Property ;
        rdfs:comment  "The temperature at which the object is designed to activate."@en ;
        rdfs:label    "ActivationTemperature"@en .

PSD:PHLevel  a        rdf:Property ;
        rdfs:comment  "Maximum water PH in a range from 0-14."@en ;
        rdfs:label    "PHLevel"@en .

PSD:FlangeTopFillet  a  rdf:Property ;
        rdfs:comment  "Flange top fillet of the profile."@en ;
        rdfs:label    "FlangeTopFillet"@en .

PSD:BarCode  a        rdf:Property ;
        rdfs:comment  "The identity of the bar code given to an occurrence of the product."@en ;
        rdfs:label    "BarCode"@en .

PSD:FlangeTable  a    rdf:Property ;
        rdfs:comment  "Designation of the standard table to which the flange conforms."@en ;
        rdfs:label    "FlangeTable"@en .

PSD:TubingLength  a   rdf:Property ;
        rdfs:comment  "Water tube length inside the component."@en ;
        rdfs:label    "TubingLength"@en .

PSD:Sound  a          rdf:Property ;
        rdfs:comment  "Sound performance."@en ;
        rdfs:label    "Sound"@en .

PSD:SurfaceTemperature
        a             rdf:Property ;
        rdfs:comment  "Average surface temperature of the component."@en ;
        rdfs:label    "SurfaceTemperature"@en .

PSD:TotalPrimaryEnergyConsumption
        a           rdf:Property ;
        rdfs:label  "Total primary energy consumption"@en .

PSD:MarketCategory  a  rdf:Property ;
        rdfs:comment  "Category of use e.g. residential, commercial, recreation etc."@en ;
        rdfs:label    "Market category"@en , "MarketCategory"@en .

PSD:HasThermalInsulation
        a             rdf:Property ;
        rdfs:comment  "If TRUE, the air terminal has thermal insulation."@en ;
        rdfs:label    "Has thermal insulation"@en .

PSD:ProcessName  a    rdf:Property ;
        rdfs:comment  "Name of the welding process.  Alternative to the numeric Process property."@en ;
        rdfs:label    "ProcessName"@en .

PSD:nameAlias  a      owl:DatatypeProperty ;
        rdfs:comment  "Name alias in local language."@en ;
        rdfs:domain   PSD:PropertyDef ;
        rdfs:label    "Name alias"@en ;
        rdfs:range    xsd:string .

PSD:ScheduleWork  a   rdf:Property ;
        rdfs:comment  "The scheduled work on behalf of the resource allocation."@en ;
        rdfs:label    "ScheduleWork"@en .

PSD:XDirectionTieHoopCount
        a             rdf:Property ;
        rdfs:comment  "The number of bars with X direction tie hoop bars."@en ;
        rdfs:label    "XDirectionTieHoopCount"@en .

PSD:l   a             rdf:Property ;
        rdfs:comment  "Measure l according to ISO 2553"@en ;
        rdfs:label    "l"@en .

PSD:MassFlowRate  a   rdf:Property ;
        rdfs:comment  "The mass flow rate of the fluid."@en ;
        rdfs:label    "MassFlowRate"@en .

PSD:FlowRateRange  a  rdf:Property ;
        rdfs:comment  "Allowable range of volume of fluid being pumped against the resistance specified."@en , "Possible range of fluid flowrate that can be delivered."@en ;
        rdfs:label    "FlowRateRange"@en , "Flow rate range"@en .

PSD:TotalCoolingLoad  a  rdf:Property ;
        rdfs:comment  "The peak total cooling load for the building, zone or space."@en ;
        rdfs:label    "TotalCoolingLoad"@en .

PSD:NominalBodyLength
        a             rdf:Property ;
        rdfs:comment  "Nominal or quoted length measured along the x-axis in the local coordinate system or the radius (in the case of a circular shape in plan) of the drain."@en , "Nominal or quoted length, measured along the x-axis of the local coordinate system of the object, of the body of the object."@en , "Nominal or quoted length measured along the x-axis in the local coordinate system or the radius (in the case of a circular shape in plan) of the waste."@en ;
        rdfs:label    "NominalBodyLength"@en .

PSD:IsOneWay  a       rdf:Property ;
        rdfs:comment  "Indicates whether the parking aisle is designed for oneway traffic (TRUE) or twoway traffic (FALSE). Should only be provided if the property IsAisle is set to TRUE."@en ;
        rdfs:label    "IsOneWay"@en .

PSD:NumberOfCompartments
        a             rdf:Property ;
        rdfs:comment  "The number of separate internal compartments within the trunking."@en ;
        rdfs:label    "NumberOfCompartments"@en .

PSD:SelfClosing  a  rdf:Property ;
        rdfs:label  "Self closing"@en .

PSD:Combustible  a  rdf:Property ;
        rdfs:label  "Combustible"@en .

PSD:BladeAction  a    rdf:Property ;
        rdfs:comment  "Blade action."@en ;
        rdfs:label    "BladeAction"@en .

PSD:DataReceived  a   rdf:Property ;
        rdfs:comment  "For data ports, captures log of data received.  The LIST at IfcTimeSeriesValue.Values may split out data according to Pset_DistributionPortTypeCable.Protocols."@en ;
        rdfs:label    "DataReceived"@en .

PSD:WetBulbTemperature
        a             rdf:Property ;
        rdfs:comment  "Wet bulb temperature of the fluid; only applicable if the fluid is air."@en ;
        rdfs:label    "WetBulbTemperature"@en .

PSD:LampCompensationType
        a             rdf:Property ;
        rdfs:comment  "Identifies the form of compensation used for power factor correction and radio suppression."@en ;
        rdfs:label    "Lamp compensation type"@en .

PSD:SlotLength  a     rdf:Property ;
        rdfs:comment  "Slot length."@en ;
        rdfs:label    "Slot length"@en .

PSD:UltimateStress  a  rdf:Property ;
        rdfs:comment  "A measure of the ultimate stress of the material."@en ;
        rdfs:label    "Ultimate stress"@en .

PSD:VerticalBarPitch  a  rdf:Property ;
        rdfs:comment  "The pitch length of the vertical bar."@en ;
        rdfs:label    "VerticalBarPitch"@en .

PSD:FinCorrugatedType
        a             rdf:Property ;
        rdfs:comment  "Description of a fin corrugated type."@en ;
        rdfs:label    "FinCorrugatedType"@en .

PSD:IsPermanentID  a  rdf:Property ;
        rdfs:comment  "Indicates whether the identity assigned to a land parcel is permanent (= TRUE) or temporary (=FALSE)."@en ;
        rdfs:label    "IsPermanentID"@en , "Is permanent ID"@en .

PSD:SpaceAirTemperature
        a             rdf:Property ;
        rdfs:comment  "Dry bulb temperature in the space."@en ;
        rdfs:label    "SpaceAirTemperature"@en .

PSD:LossCoefficentCurve
        a             rdf:Property ;
        rdfs:comment  "Loss coefficient  blade position angle curve; ratio of pressure drop to velocity pressure versus blade angle; C = f (blade angle position)."@en ;
        rdfs:label    "LossCoefficentCurve"@en .

PSD:JunctionRightRadius
        a             rdf:Property ;
        rdfs:comment  "The radius of bending for the right junction where 0 indicates sharp bend."@en ;
        rdfs:label    "JunctionRightRadius"@en .

PSD:BladeShape  a     rdf:Property ;
        rdfs:comment  "Blade shape. Flat means triple V-groove."@en ;
        rdfs:label    "BladeShape"@en .

PSD:WasherShape  a    rdf:Property ;
        rdfs:comment  "Shape of the washers, e.g. 'Standard', 'Square'"@en ;
        rdfs:label    "WasherShape"@en .

PSD:DisplaySize  a    rdf:Property ;
        rdfs:comment  "The physical size of the display. In the case of a stem thermometer, this will be the length of the stem. For a dial thermometer, it will be the diameter of the dial."@en , "The physical size of the display. For a dial pressure gauge it will be the diameter of the dial."@en ;
        rdfs:label    "DisplaySize"@en .

PSD:VersionDate  a    rdf:Property ;
        rdfs:comment  "The date on which the version of the agreement became applicable."@en ;
        rdfs:label    "VersionDate"@en .

PSD:Heat  a           rdf:Property ;
        rdfs:comment  "The amount of heat energy consumed during the period specified in the time series."@en ;
        rdfs:label    "Heat"@en .

PSD:CamberAtMidspan  a  rdf:Property ;
        rdfs:label  "Camber at midspan"@en .

PSD:ReliefValveSetting
        a             rdf:Property ;
        rdfs:comment  "Pressure at which the relief valve activates."@en ;
        rdfs:label    "ReliefValveSetting"@en .

PSD:InnerDiameter  a  rdf:Property ;
        rdfs:comment  "The actual inner diameter of the pipe."@en ;
        rdfs:label    "InnerDiameter"@en .

PSD:TemperatureEffectiveness
        a             rdf:Property ;
        rdfs:comment  "Temperature heat transfer effectiveness: The ratio of primary airflow temperature changes to maximum possible temperature changes."@en ;
        rdfs:label    "TemperatureEffectiveness"@en .

PSD:ParticleMassHolding
        a             rdf:Property ;
        rdfs:comment  "Mass of particle holding in the filter."@en ;
        rdfs:label    "ParticleMassHolding"@en .

PSD:CompressorTotalHeatGain
        a             rdf:Property ;
        rdfs:comment  "Compressor total heat gain."@en ;
        rdfs:label    "CompressorTotalHeatGain"@en .

PSD:CoreSpacing  a    rdf:Property ;
        rdfs:comment  "Core spacing of the profile."@en ;
        rdfs:label    "CoreSpacing"@en .

PSD:TotalSensibleHeatGain
        a             rdf:Property ;
        rdfs:comment  "The total sensible heat or energy gained by the space during the peak cooling conditions."@en ;
        rdfs:label    "TotalSensibleHeatGain"@en .

PSD:NumberOfRiser  a  rdf:Property ;
        rdfs:label  "Number of riser"@en .

PSD:NominalSize  a    rdf:Property ;
        rdfs:comment  "Indicates the diagonal screen size."@en ;
        rdfs:label    "NominalSize"@en .

PSD:ShortCircuit2PoleMinimumState
        a             rdf:Property ;
        rdfs:comment  "Minimum 2 pole short circuit current provided at the point of supply."@en ;
        rdfs:label    "ShortCircuit2PoleMinimumState"@en .

PSD:WalkingLineOffset
        a           rdf:Property ;
        rdfs:label  "Walking line offset"@en .

PSD:WaterTightnessRating
        a           rdf:Property ;
        rdfs:label  "Water tightness rating"@en .

PSD:ResourceDepletion
        a           rdf:Property ;
        rdfs:label  "Resource depletion"@en .

PSD:NonRenewableEnergyConsumptionPerUnit
        a           rdf:Property ;
        rdfs:label  "Non renewable energy consumption per unit"@en .

PSD:MainColor  a      rdf:Property ;
        rdfs:comment  "The main color of the furniture of this type."@en ;
        rdfs:label    "Main color"@en .

PSD:FlowPattern  a    rdf:Property ;
        rdfs:comment  "Flow pattern."@en ;
        rdfs:label    "Flow pattern"@en .

PSD:RenewableEnergyConsumption
        a           rdf:Property ;
        rdfs:label  "Renewable energy consumption"@en .

PSD:Thickness  a      rdf:Property ;
        rdfs:comment  "Thickness of the fin."@en ;
        rdfs:label    "Thickness"@en .

PSD:IsPotable  a      rdf:Property ;
        rdfs:comment  "If TRUE, then the water is considered potable."@en ;
        rdfs:label    "IsPotable"@en .

PSD:ProtectivePoreRatio
        a           rdf:Property ;
        rdfs:label  "Protective pore ratio"@en .

PSD:FailPosition  a   rdf:Property ;
        rdfs:comment  "Specifies the required fail-safe position of the actuator."@en ;
        rdfs:label    "Fail position"@en .

PSD:OccupancyNumber  a  rdf:Property ;
        rdfs:comment  "Number of people required for the activity assigned to this space."@en ;
        rdfs:label    "OccupancyNumber"@en .

PSD:Sensitivity  a    rdf:Property ;
        rdfs:comment  "Current leakage to an unwanted leading path during normal operation (IEC 151-14-49)."@en ;
        rdfs:label    "Sensitivity"@en .

PSD:NominalPressureDrop
        a             rdf:Property ;
        rdfs:comment  "Total pressure drop across the filter."@en ;
        rdfs:label    "Nominal pressure drop"@en .

PSD:WorkingPressure  a  rdf:Property ;
        rdfs:comment  "Working pressure."@en , "Pressure classification as defined by the authority having jurisdiction (e.g., SMACNA, etc.)."@en ;
        rdfs:label    "WorkingPressure"@en .

PSD:FaceType  a       rdf:Property ;
        rdfs:comment  "Identifies how the terminal face of an AirTerminal is constructed."@en ;
        rdfs:label    "Face type"@en .

PSD:Thickness2  a     rdf:Property ;
        rdfs:comment  "Second thickness parameter of a surface member with varying thickness"@en ;
        rdfs:label    "Thickness2"@en .

PSD:InitialTension  a  rdf:Property ;
        rdfs:label  "Initial tension"@en .

PSD:HeadShape  a      rdf:Property ;
        rdfs:comment  "Shape of the bolt's head, e.g. 'Hexagon', 'Countersunk', 'Cheese'"@en ;
        rdfs:label    "HeadShape"@en .

PSD:CurrentTolerance2
        a             rdf:Property ;
        rdfs:comment  "The tolerance for the current of time/current-curve in [%] valid for times above CurrentTolereanceLimit1."@en ;
        rdfs:label    "CurrentTolerance2"@en .

PSD:TotalHeatLoss  a  rdf:Property ;
        rdfs:comment  "The total amount of heat or energy lost by the space at the time of the space's peak heating conditions."@en ;
        rdfs:label    "TotalHeatLoss"@en .

PSD:SheathColors  a   rdf:Property ;
        rdfs:comment  "Colour of the core (derived from IEC 60757). Note that the combined color 'GreenAndYellow' shall be used only as Protective Earth (PE) conductors according to the requirements of IEC 60446."@en ;
        rdfs:label    "SheathColors"@en .

PSD:Name  a           rdf:Property ;
        rdfs:comment  "The name of the air side system."@en ;
        rdfs:label    "Name"@en .

PSD:NominalCurrent  a  rdf:Property ;
        rdfs:comment  "The nominal current that is designed to be measured."@en ;
        rdfs:label    "NominalCurrent"@en .

PSD:BoundaryAreaHeatLoss
        a             rdf:Property ;
        rdfs:comment  "Heat loss per unit area for the boundary object. This is a design input value for use in the absence of calculated load data."@en ;
        rdfs:label    "BoundaryAreaHeatLoss"@en .

PSD:HeatRejectionRate
        a             rdf:Property ;
        rdfs:comment  "Sum of the refrigeration effect and the heat equivalent of the power input to the compressor."@en ;
        rdfs:label    "HeatRejectionRate"@en .

PSD:HasBuiltInAlarm  a  rdf:Property ;
        rdfs:comment  "Indicates whether the smoke sensor is included as an element within a smoke alarm/sensor unit (TRUE) or not (FALSE)."@en ;
        rdfs:label    "HasBuiltInAlarm"@en .

PSD:ThermalConductivityTemperatureDerivative
        a             rdf:Property ;
        rdfs:comment  "Thermal conductivity temperature derivative."@en ;
        rdfs:label    "Thermal conductivity temperature derivative"@en .

PSD:ShaftPowerRate  a  rdf:Property ;
        rdfs:comment  "Fan shaft power."@en ;
        rdfs:label    "ShaftPowerRate"@en .

PSD:DataTransmitted  a  rdf:Property ;
        rdfs:comment  "For data ports, captures log of data transmitted.  The LIST at IfcTimeSeriesValue.Values may split out data according to Pset_DistributionPortTypeCable.Protocols."@en ;
        rdfs:label    "DataTransmitted"@en .

PSD:WaterInletTemperatureRange
        a             rdf:Property ;
        rdfs:comment  "Allowable water inlet temperature range."@en ;
        rdfs:label    "Water inlet temperature range"@en .

PSD:FlangeDraft  a    rdf:Property ;
        rdfs:comment  "Flange draft of the profile."@en ;
        rdfs:label    "FlangeDraft"@en .

PSD:requiredProp  a  owl:ObjectProperty ;
        rdfs:domain  PSD:RequiredPset ;
        rdfs:range   PSD:PropertyDef .

PSD:DrainSize  a      rdf:Property ;
        rdfs:comment  "The size of the drain outlet connection from the object."@en ;
        rdfs:label    "DrainSize"@en .

PSD:GlassLayers  a  rdf:Property ;
        rdfs:label  "Glass layers"@en .

PSD:LatentHeatTransferRate
        a             rdf:Property ;
        rdfs:comment  "Latent heat transfer rate."@en , "Latent heat transfer rate to primary air flow."@en ;
        rdfs:label    "LatentHeatTransferRate"@en .

PSD:ScheduleCompletion
        a             rdf:Property ;
        rdfs:comment  "The scheduled completion percentage of the allocation."@en ;
        rdfs:label    "ScheduleCompletion"@en .

PSD:VisibleReflectanceFront
        a             rdf:Property ;
        rdfs:comment  "Reflectance at normal incidence (visible): front side. Defines the fraction of the solar ray in the visible spectrum that is reflected and not transmitted when the ray passes from one medium into another, at the 'front' side of the other material, perpendicular to the surface. Dependent on material and surface characteristics."@en ;
        rdfs:label    "VisibleReflectanceFront"@en .

PSD:HoseLength  a     rdf:Property ;
        rdfs:comment  "Notional length of the hose fitted to the hose reel when fully extended."@en ;
        rdfs:label    "HoseLength"@en .

PSD:OperationPressureMax
        a             rdf:Property ;
        rdfs:comment  "Maximum pressure under normal operating conditions."@en ;
        rdfs:label    "OperationPressureMax"@en .

PSD:HasCaps  a        rdf:Property ;
        rdfs:comment  "Does the inlet connection have protective caps."@en ;
        rdfs:label    "HasCaps"@en .

PSD:IsWaterStorageHeater
        a             rdf:Property ;
        rdfs:comment  "This is used to identify if the boiler has storage capacity (TRUE). If FALSE, then there is no storage capacity built into the boiler, such as an instantaneous hot water heater."@en ;
        rdfs:label    "Is water storage heater"@en .

PSD:CenterCoreBaseHeight
        a             rdf:Property ;
        rdfs:comment  "Center core base height of the profile."@en ;
        rdfs:label    "CenterCoreBaseHeight"@en .

PSD:NumberOfStoreys  a  rdf:Property ;
        rdfs:label  "Number of storeys"@en .

PSD:ActualErectionDate
        a             rdf:Property ;
        rdfs:comment  "Date erected."@en ;
        rdfs:label    "ActualErectionDate"@en .

PSD:OverallWidth  a   rdf:Property ;
        rdfs:comment  "Overall width of the profile."@en ;
        rdfs:label    "OverallWidth"@en .

PSD:TypeDesignator  a  rdf:Property ;
        rdfs:comment  "Type designator for the precast concrete element. The content depends on local standards. For instance in Finland it usually a one-letter acronym, e.g. P=Column, K=reinforced concrete beam,etc."@en ;
        rdfs:label    "Type designator"@en , "TypeDesignator"@en .

PSD:NumberOfGangs  a  rdf:Property ;
        rdfs:comment  "Number of slots available for switches/outlets (most commonly 1, 2, 3, or 4)."@en ;
        rdfs:label    "NumberOfGangs"@en .

PSD:Exponent  a       rdf:Property ;
        rdfs:comment  "Characteristic exponent, slope of log(heat output) vs log (surface temperature minus environmental temperature)."@en ;
        rdfs:label    "Exponent"@en .

PSD:Reinforcement  a  rdf:Property ;
        rdfs:comment  "The type of reinforcement, if any, used for the duct segment."@en ;
        rdfs:label    "Reinforcement"@en .

PSD:ReturnWaterTemperatureCooling
        a             rdf:Property ;
        rdfs:comment  "Return water temperature in cooling mode."@en ;
        rdfs:label    "ReturnWaterTemperatureCooling"@en .

PSD:MixerControl  a   rdf:Property ;
        rdfs:comment  "Defines the form of control of the mixing valve."@en ;
        rdfs:label    "MixerControl"@en .

PSD:FlammabilityRating
        a           rdf:Property ;
        rdfs:label  "Flammability rating"@en .

PSD:HeatOutputRate  a  rdf:Property ;
        rdfs:comment  "Overall heat transfer rate."@en ;
        rdfs:label    "HeatOutputRate"@en .

PSD:TunerChannel  a   rdf:Property ;
        rdfs:comment  "Indicates the tuner channels, if applicable."@en ;
        rdfs:label    "TunerChannel"@en .

PSD:NominalTotalPressure
        a             rdf:Property ;
        rdfs:comment  "Nominal total pressure rise across the fan."@en ;
        rdfs:label    "Nominal total pressure"@en .

PSD:VolumetricEfficiency
        a             rdf:Property ;
        rdfs:comment  "Ratio of the actual volume of gas entering the compressor to the theoretical displacement of the compressor."@en ;
        rdfs:label    "VolumetricEfficiency"@en .

PSD:MultipleTarriff  a  rdf:Property ;
        rdfs:comment  "Indicates whether meter has built-in support for multiple tarriffs (variable energy cost rates)."@en ;
        rdfs:label    "MultipleTarriff"@en .

PSD:LogarithmicMeanTemperatureDifference
        a             rdf:Property ;
        rdfs:comment  "Logarithmic mean temperature difference between refrigerant and water or air."@en ;
        rdfs:label    "LogarithmicMeanTemperatureDifference"@en .

PSD:CompressiveStrength
        a           rdf:Property ;
        rdfs:label  "Compressive strength"@en .
